@prefix : <https://w3id.org/fmo#> .
@prefix dot: <https://w3id.org/dot#> .
@prefix fmo: <https://w3id.org/fmo#> .
@prefix hmo: <https://w3id.org/hmo#> .
@prefix owl: <http://www.w3.org/2002/07/owl#> .
@prefix rdf: <http://www.w3.org/1999/02/22-rdf-syntax-ns#> .
@prefix xml: <http://www.w3.org/XML/1998/namespace> .
@prefix xsd: <http://www.w3.org/2001/XMLSchema#> .
@prefix rdfs: <http://www.w3.org/2000/01/rdf-schema#> .
@prefix swrl: <http://www.w3.org/2003/11/swrl#> .
@prefix swrla: <http://swrl.stanford.edu/ontologies/3.3/swrla.owl#> .
@prefix swrlb: <http://www.w3.org/2003/11/swrlb#> .
@prefix terms: <http://purl.org/dc/terms/> .
@base <https://w3id.org/fmo#> .

<https://w3id.org/fmo> rdf:type owl:Ontology ;
                        terms:creator "Maria Laura Leonardi, Stefano Cursi, Elena Gigliarelli, José Granja, Daniel Oliveira, Miguel Azenha." ;
                        terms:description "An ontology to represent the failure mechanism of unreinforced masonry structures" ;
                        terms:issued "2024-04-29" ;
                        terms:license "https://creativecommons.org/licenses/by/1.0" ;
                        terms:modified "2024-04-29" ;
                        terms:title "Failure Mechanism Ontology"@en ;
                        rdfs:comment "Version 0.1" ;
                        owl:versionInfo 0.1 ;
                        fmo:preferredNamespacePrexif "fmo" ;
                        fmo:preferredNamespaceUri "https://w3id.org/fmo#" .

#################################################################
#    Annotation properties
#################################################################

###  http://purl.org/dc/terms/creator
terms:creator rdf:type owl:AnnotationProperty .


###  http://purl.org/dc/terms/description
terms:description rdf:type owl:AnnotationProperty .


###  http://purl.org/dc/terms/issued
terms:issued rdf:type owl:AnnotationProperty .


###  http://purl.org/dc/terms/license
terms:license rdf:type owl:AnnotationProperty .


###  http://purl.org/dc/terms/modified
terms:modified rdf:type owl:AnnotationProperty .


###  http://purl.org/dc/terms/title
terms:title rdf:type owl:AnnotationProperty .


###  http://swrl.stanford.edu/ontologies/3.3/swrla.owl#isRuleEnabled
swrla:isRuleEnabled rdf:type owl:AnnotationProperty .


###  https://w3id.org/fmo#preferredNamespacePrexif
fmo:preferredNamespacePrexif rdf:type owl:AnnotationProperty .


###  https://w3id.org/fmo#preferredNamespaceUri
fmo:preferredNamespaceUri rdf:type owl:AnnotationProperty .


#################################################################
#    Object Properties
#################################################################

###  https://w3id.org/dot#hasCausation
dot:hasCausation rdf:type owl:ObjectProperty ;
                 rdfs:domain dot:StructuralDamage ;
                 rdfs:range fmo:FailureMechanism ;
                 rdfs:comment "It indicates the relationship between a damage and the failure mechanism that causes it." ;
                 rdfs:label "Has causation" .


###  https://w3id.org/dot#hasDamage
dot:hasDamage rdf:type owl:ObjectProperty ;
              rdfs:domain <https://pi.pauwel.be/voc/buildingelement#Wall> ,
                          hmo:MasonryWall ;
              rdfs:range dot:StructuralDamage ;
              rdfs:comment "imported from https://w3id.org/dot ; used to describe damage hmo:MasonryWall, and understand its corration with possible ongoing mechanisms" ;
              rdfs:label "Has damage" .


###  https://w3id.org/fmo#FacilitatedBy
fmo:FacilitatedBy rdf:type owl:ObjectProperty ;
                  rdfs:domain fmo:FailureMechanism ;
                  rdfs:range fmo:Vulnerability ;
                  rdfs:comment "Indicates the relationship between a failure mechanism and the vulnerability that facilitates it." ;
                  rdfs:label "Facilitated by" .


###  https://w3id.org/fmo#FacilitatesMechanism
fmo:FacilitatesMechanism rdf:type owl:ObjectProperty ;
                         rdfs:domain fmo:Vulnerability ;
                         rdfs:range fmo:FailureMechanism ;
                         rdfs:comment "A relationship between a vulneability and the specific mechanism that it facilitates." ;
                         rdfs:label "Facilitates" .


###  https://w3id.org/fmo#hasBehaviour
fmo:hasBehaviour rdf:type owl:ObjectProperty ;
                 rdfs:domain <https://pi.pauwel.be/voc/buildingelement#Wall> ,
                             hmo:MasonryWall ;
                 rdfs:range fmo:WallBehaviour ;
                 rdfs:comment "Indicates the relationship between the masonry wall and its load response behaviour."@en ;
                 rdfs:label "Has behaviour" .


###  https://w3id.org/fmo#hasOccurringMechanism
fmo:hasOccurringMechanism rdf:type owl:ObjectProperty ;
                          rdfs:domain <https://pi.pauwel.be/voc/buildingelement#Wall> ,
                                      hmo:MasonryWall ;
                          rdfs:range fmo:FailureMechanism ;
                          rdfs:comment "It relates the masonry wall with the inferred occurred mechanism." ;
                          rdfs:label "Has occurring mechanism" .


###  https://w3id.org/fmo#hasVulnerability
fmo:hasVulnerability rdf:type owl:ObjectProperty ;
                     rdfs:domain <https://pi.pauwel.be/voc/buildingelement#Wall> ,
                                 hmo:MasonryWall ;
                     rdfs:range fmo:Vulnerability ;
                     rdfs:comment "Relates the masonry wall to the vulnerability that characterised them." ;
                     rdfs:label "Has Vulnerability"@en .


###  https://w3id.org/hmo#hasMasonryQualityIndex
hmo:hasMasonryQualityIndex rdf:type owl:ObjectProperty ;
                           rdfs:domain <https://pi.pauwel.be/voc/buildingelement#Wall> ,
                                       hmo:MasonryWall ;
                           rdfs:range hmo:MasonryQualityIndex ;
                           rdfs:comment "Imported from the https://w3id.org/hmo ontology, it relates a masonry wall to the value of the masonry quality index." ;
                           rdfs:label "Has Masonry Quality Index" .


#################################################################
#    Data properties
#################################################################

###  https://w3id.org/hmo#MQITotalInPlane
hmo:MQITotalInPlane rdf:type owl:DatatypeProperty ;
                    rdfs:domain hmo:MasonryQualityIndex ;
                    rdfs:range xsd:float ;
                    rdfs:comment "Defines the total value of MQI for in plane loads. Imported from https://w3id.org/hmo." ;
                    rdfs:label "Masonry Quality Index total value for in plane loads" .


###  https://w3id.org/hmo#MQITotalOutOfPlane
hmo:MQITotalOutOfPlane rdf:type owl:DatatypeProperty ;
                       rdfs:domain hmo:MasonryQualityIndex ;
                       rdfs:range xsd:float ;
                       rdfs:comment "Defines the total value of MQI for out of plane loads. Imported from https://w3id.org/hmo." ;
                       rdfs:label "Masonry Quality Index total value for out of plane loads" .


###  https://w3id.org/hmo#MQITotalVertical
hmo:MQITotalVertical rdf:type owl:DatatypeProperty ;
                     rdfs:domain hmo:MasonryQualityIndex ;
                     rdfs:range xsd:float ;
                     rdfs:comment "Defines the total value of MQI for vertical loads. Imported from https://w3id.org/hmo." ;
                     rdfs:label "Masonry Quality Index total value for vertical loads" .


#################################################################
#    Classes
#################################################################

###  https://pi.pauwel.be/voc/buildingelement#Wall
<https://pi.pauwel.be/voc/buildingelement#Wall> rdf:type owl:Class ;
                                                rdfs:comment "Class imported from https://pi.pauwel.be/voc/buildingelement ontology, to map an IFC wall with a masonry wall, in the ontology-BIM model." ;
                                                rdfs:label "Wall" .


###  https://w3id.org/dot#StructuralDamage
dot:StructuralDamage rdf:type owl:Class ;
                     rdfs:comment "Imported from https://w3id.org/dot.Indicates damage in a hmo:MasonryWall. In the context of failure mechanisms, it helps to understand when a mechanism is present in a wall."@en ;
                     rdfs:label "Structural Damage"@en .


###  https://w3id.org/fmo#Crack
fmo:Crack rdf:type owl:Class ;
          rdfs:subClassOf dot:StructuralDamage ;
          rdfs:comment "A type of damage, which is modelled as a specific subclass of https://w3id.org/dot#StructuralDamage. It may indicate the presence of an ongoing mechanism."@en ;
          rdfs:label "Crack" .


###  https://w3id.org/fmo#FailureMechanism
fmo:FailureMechanism rdf:type owl:Class ;
                     owl:disjointWith fmo:Vulnerability ,
                                      fmo:WallBehaviour ;
                     rdfs:comment "Indicates the collapse mechanism expected from a specific hmo:MasonryWall." ;
                     rdfs:label "Failure Mechanism"@en .


###  https://w3id.org/fmo#InPlaneBehaviour
fmo:InPlaneBehaviour rdf:type owl:Class ;
                     rdfs:subClassOf fmo:WallBehaviour ;
                     rdfs:comment "Indicates the behaviour of a wall subjected to a in plane load."@en ;
                     rdfs:label "In Plane Behaviour."@en .


###  https://w3id.org/fmo#OutOfPlaneBehaviour
fmo:OutOfPlaneBehaviour rdf:type owl:Class ;
                        rdfs:subClassOf fmo:WallBehaviour ;
                        rdfs:comment "Indicates the behaviour of a wall subjected to an out of plane load."@en ;
                        rdfs:label "Out Of Plane Behaviour"@en .


###  https://w3id.org/fmo#VerticalBehaviour
fmo:VerticalBehaviour rdf:type owl:Class ;
                      rdfs:subClassOf fmo:WallBehaviour ;
                      rdfs:comment "Indicates the behaviour of a wall subjected to a specific vertical load."@en ;
                      rdfs:label "Vertical Behaviour"@en .


###  https://w3id.org/fmo#Vulnerability
fmo:Vulnerability rdf:type owl:Class ;
                  rdfs:comment "It indicates a feature of the wall that can facilitate the occurrence of a mechanism."@en ;
                  rdfs:label "Vulnerability"@en .


###  https://w3id.org/fmo#WallBehaviour
fmo:WallBehaviour rdf:type owl:Class ;
                  rdfs:comment "Indicates the behaviour of a wall subjected to a specific load."@en ;
                  rdfs:label "Wall Behaviour"@en .


###  https://w3id.org/hmo#MasonryQualityIndex
hmo:MasonryQualityIndex rdf:type owl:Class ;
                        rdfs:comment "Class imported from the https://w3id.org/hmo# ontology, to define vertical, in plane and out of plane behaviour of the assessed wall." ;
                        rdfs:label "Masonry Quality Index"@en .


###  https://w3id.org/hmo#MasonryWall
hmo:MasonryWall rdf:type owl:Class ;
                rdfs:subClassOf <https://pi.pauwel.be/voc/buildingelement#Wall> ;
                rdfs:comment "imported from https://w3id.org/hmo, to apply the vulnerability - behaviour - failure mechanism to a hmo:MasonryWall"@en ;
                rdfs:label "Masonry Wall"@en .


#################################################################
#    Individuals
#################################################################

###  https://w3id.org/fmo#AbsenceOfIntermediateChains
fmo:AbsenceOfIntermediateChains rdf:type owl:NamedIndividual ,
                                         fmo:Vulnerability ;
                                rdfs:comment "A vulnerability that consists in the absence of chains in the intermediate floors of the slabs supported by the wall."@en ;
                                rdfs:label "Absence of intermediate chains"@en .


###  https://w3id.org/fmo#AbsenceOfIntermediateCurbstone
fmo:AbsenceOfIntermediateCurbstone rdf:type owl:NamedIndividual ,
                                            fmo:Vulnerability ;
                                   rdfs:comment "A vulnerability that consists in the absence of curbstones in the intermediate floors of the slabs supported by the wall."@en ;
                                   rdfs:label "Absence of intermediate curbstone" .


###  https://w3id.org/fmo#AbsenceOfTopChains
fmo:AbsenceOfTopChains rdf:type owl:NamedIndividual ,
                                fmo:Vulnerability ;
                       rdfs:comment "A vulnerability that consists in the absence of chains in the roof supported by the wall."@en ;
                       rdfs:label "Absence of Top Chains"@en .


###  https://w3id.org/fmo#AbsenceOfTopCurbstone
fmo:AbsenceOfTopCurbstone rdf:type owl:NamedIndividual ,
                                   fmo:Vulnerability ;
                          rdfs:comment "A vulnerability that consists in the absence of curbstone in the roof supported by the wall." ;
                          rdfs:label "Absence of Top Curbstone" .


###  https://w3id.org/fmo#AverageInPlaneBehaviour
fmo:AverageInPlaneBehaviour rdf:type owl:NamedIndividual ,
                                     fmo:InPlaneBehaviour ,
                                     fmo:WallBehaviour ;
                            rdfs:comment "It indicates a type of behaviour that is within the average range of how masonry walls behave when subjected to in plane load."@en ;
                            rdfs:label "Average in plane behaviour"@en .


###  https://w3id.org/fmo#AverageOutOfPlaneBehaviour
fmo:AverageOutOfPlaneBehaviour rdf:type owl:NamedIndividual ,
                                        fmo:OutOfPlaneBehaviour ,
                                        fmo:WallBehaviour ;
                               rdfs:comment "It indicates a type of behaviour (based on the values of https://w3id.org/hmo#MasonryQualityIndex) that is within the average range of how masonry walls behave when subjected to a out of plane load."@en ;
                               rdfs:label "Average out of plane behaviour"@en .


###  https://w3id.org/fmo#AverageVerticalBehaviour
fmo:AverageVerticalBehaviour rdf:type owl:NamedIndividual ,
                                      fmo:VerticalBehaviour ,
                                      fmo:WallBehaviour ;
                             rdfs:comment "It indicates a type of behaviour that is within the average range (based on the values assigned to https://w3id.org/hmo#MasonryQualityIndex) of how masonry walls behave when subjected to a vertical load."@en ;
                             rdfs:label "Average Vertical Behaviour"@en .


###  https://w3id.org/fmo#DeformableFloors
fmo:DeformableFloors rdf:type owl:NamedIndividual ,
                              fmo:Vulnerability ;
                     rdfs:comment "A vulnerability consisting of the presence of deformable slabs supported by the wall." ;
                     rdfs:label "Deformable Floors"@en .


###  https://w3id.org/fmo#DiagonalAndVerticalCracks
fmo:DiagonalAndVerticalCracks rdf:type owl:NamedIndividual ,
                                       dot:StructuralDamage ,
                                       fmo:Crack ;
                              dot:hasCausation fmo:HorizontalBending ;
                              rdfs:comment "Diagonal and vertical cracks in the same wall." ;
                              rdfs:label "Diagonal and vertical cracks" .


###  https://w3id.org/fmo#DiagonalCrack
fmo:DiagonalCrack rdf:type owl:NamedIndividual ,
                           dot:StructuralDamage ,
                           fmo:Crack ;
                  dot:hasCausation fmo:InPlaneFailure ;
                  rdfs:comment "Crack with diagonal progression."@en ;
                  rdfs:label "Diagonal crack" .


###  https://w3id.org/fmo#ExcessiveSlenderness
fmo:ExcessiveSlenderness rdf:type owl:NamedIndividual ,
                                  fmo:Vulnerability ;
                         rdfs:label "A specific vulnerability consisting of excessive slenderness of the wall."@en ,
                                    "Excessive slenderness"@en .


###  https://w3id.org/fmo#GoodInPlaneBehaviour
fmo:GoodInPlaneBehaviour rdf:type owl:NamedIndividual ,
                                  fmo:InPlaneBehaviour ,
                                  fmo:WallBehaviour ;
                         rdfs:comment "A type of (in plane) wall behaviour that is considered good based on the values assigned to https://w3id.org/hmo#MasonryQualityIndex."@en ;
                         rdfs:label "Good in plane behaviour"@en .


###  https://w3id.org/fmo#GoodOutOfPlaneBehaviour
fmo:GoodOutOfPlaneBehaviour rdf:type owl:NamedIndividual ,
                                     fmo:OutOfPlaneBehaviour ,
                                     fmo:WallBehaviour ;
                            rdfs:comment "A type of (out of plane) wall behaviour that is considered good based on the values assigned to https://w3id.org/hmo#MasonryQualityIndex."@en ;
                            rdfs:label "Good Out Of Plane Behaviour"@en .


###  https://w3id.org/fmo#GoodVerticalBehaviour
fmo:GoodVerticalBehaviour rdf:type owl:NamedIndividual ,
                                   fmo:VerticalBehaviour ,
                                   fmo:WallBehaviour ;
                          rdfs:comment "The vertical wall behaviour that is considered good based on the values assigned to https://w3id.org/hmo#MasonryQualityIndex."@en ;
                          rdfs:label "Good vertical behaviour"@en .


###  https://w3id.org/fmo#HorizontalAndVerticalCracks
fmo:HorizontalAndVerticalCracks rdf:type owl:NamedIndividual ,
                                         dot:StructuralDamage ,
                                         fmo:Crack ;
                                dot:hasCausation fmo:VerticalBending ;
                                rdfs:comment "Vertical and horizontal cracks in the same wall." ;
                                rdfs:label "Horizontal and vertical cracks" .


###  https://w3id.org/fmo#HorizontalBending
fmo:HorizontalBending rdf:type owl:NamedIndividual ,
                               fmo:FailureMechanism ;
                      rdfs:comment """A specific mechanism manifested by the expulsion of material from the top zone of the wall and the detachment of wedge-shaped bodies 
accompanied by the formation of oblique and vertical cylindrical hinges due to out-of-plane actions."""@en ;
                      rdfs:label "Horizontal Bending"@en .


###  https://w3id.org/fmo#InPlaneFailure
fmo:InPlaneFailure rdf:type owl:NamedIndividual ,
                            fmo:FailureMechanism ;
                   rdfs:comment "A specific mechanism that do not involve out of plane overturning, but in plane craking/failure."@en ;
                   rdfs:label "In Plane Failure"@en .


###  https://w3id.org/fmo#InadequateInPlaneBehaviour
fmo:InadequateInPlaneBehaviour rdf:type owl:NamedIndividual ,
                                        fmo:InPlaneBehaviour ,
                                        fmo:Vulnerability ,
                                        fmo:WallBehaviour ;
                               rdfs:comment "A type of (in plane) wall behaviour that is considered inadequate based on the values assigned to https://w3id.org/hmo#MasonryQualityIndex."@en ;
                               rdfs:label "Inadequate in plane behaviour"@en .


###  https://w3id.org/fmo#InadequateOutOfPlaneBehaviour
fmo:InadequateOutOfPlaneBehaviour rdf:type owl:NamedIndividual ,
                                           fmo:OutOfPlaneBehaviour ,
                                           fmo:Vulnerability ,
                                           fmo:WallBehaviour ;
                                  rdfs:comment "A type of (out of plane) wall behaviour that is considered inadequate based on the values assigned to https://w3id.org/hmo#MasonryQualityIndex."@en ;
                                  rdfs:label "Inadequate out of plane behaviour"@en .


###  https://w3id.org/fmo#InadequateVerticalBehaviour
fmo:InadequateVerticalBehaviour rdf:type owl:NamedIndividual ,
                                         fmo:VerticalBehaviour ,
                                         fmo:Vulnerability ,
                                         fmo:WallBehaviour ;
                                rdfs:comment "A type of (vertical) wall behaviour that is considered inadequate based on the values assigned to https://w3id.org/hmo#MasonryQualityIndex."@en ;
                                rdfs:label "Inadequate Vertical Behaviour"@en .


###  https://w3id.org/fmo#MQIWallFacadeA417_a
fmo:MQIWallFacadeA417_a rdf:type owl:NamedIndividual ,
                                 hmo:MasonryQualityIndex ;
                        hmo:MQITotalInPlane 4.55 ,
                                            4.90 ;
                        hmo:MQITotalOutOfPlane 3.15 .


###  https://w3id.org/fmo#OpeningsNearIntersections
fmo:OpeningsNearIntersections rdf:type owl:NamedIndividual ,
                                       fmo:Vulnerability ;
                              rdfs:label "Openings near intersections"@en .


###  https://w3id.org/fmo#PartialOverturn
fmo:PartialOverturn rdf:type owl:NamedIndividual ,
                             fmo:FailureMechanism ;
                    rdfs:comment "A specific mechanism consisting of the total rotation of part of a wall out of the plane."@en ;
                    rdfs:label "Partial Overturn"@en .


###  https://w3id.org/fmo#PresenceOfHorizontalThrust
fmo:PresenceOfHorizontalThrust rdf:type owl:NamedIndividual ,
                                        fmo:Vulnerability ;
                               rdfs:comment "A specific vulnerability in the wall consists in the presence of thrusting elements, which facilitate out-of-plane movement."@en ;
                               rdfs:label "Presence of horizontal thrust"@en .


###  https://w3id.org/fmo#TotalOverturn
fmo:TotalOverturn rdf:type owl:NamedIndividual ,
                           fmo:FailureMechanism ;
                  rdfs:comment "A specific mechanism consisting of the total rotation of the entire wall out of the plane."@en ;
                  rdfs:label "Total Overturn"@en .


###  https://w3id.org/fmo#VerticalBending
fmo:VerticalBending rdf:type owl:NamedIndividual ,
                             fmo:FailureMechanism ;
                    rdfs:comment "A specific mechanism manifested with the formation a horizontal cylindrical hinge that divides the wall into two blocks and is described by the mutual rotation of the same around this axis by out-of-plane actions."@en ;
                    rdfs:label "Vertical Bending"@en .


###  https://w3id.org/fmo#VerticalCrackEntireWallAtIntersection
fmo:VerticalCrackEntireWallAtIntersection rdf:type owl:NamedIndividual ,
                                                   dot:StructuralDamage ,
                                                   fmo:Crack ;
                                          dot:hasCausation fmo:TotalOverturn ;
                                          rdfs:comment "A vertical crack occurring at the intersection between walls."@en ;
                                          rdfs:label "Vertical crack near intersection" .


###  https://w3id.org/fmo#WallFacadeA417_a
fmo:WallFacadeA417_a rdf:type owl:NamedIndividual ,
                              <https://pi.pauwel.be/voc/buildingelement#Wall> ,
                              hmo:MasonryWall ;
                     dot:hasDamage fmo:VerticalCrackEntireWallAtIntersection ;
                     fmo:hasBehaviour fmo:AverageInPlaneBehaviour ,
                                      fmo:InadequateOutOfPlaneBehaviour ;
                     fmo:hasOccurringMechanism fmo:TotalOverturn ;
                     fmo:hasVulnerability fmo:InadequateOutOfPlaneBehaviour ;
                     hmo:hasMasonryQualityIndex fmo:MQIWallFacadeA417_a ;
                     rdfs:comment "Wall of the facade in the isolate A, units 417, side a. Castelnuovo di Porto"@en ;
                     rdfs:label "Wall Facade A417_a"@en .


#################################################################
#    Rules
#################################################################

fmo:wl rdf:type swrl:Variable .

fmo:MQI rdf:type swrl:Variable .

fmo:MQIv rdf:type swrl:Variable .

fmo:dmg rdf:type swrl:Variable .

fmo:mcn rdf:type swrl:Variable .

[ swrla:isRuleEnabled "true"^^xsd:boolean ;
   rdfs:comment "If a Masonry Wall has a Masonry Quality Index, which has a Masonry Quality Index Total In Plane Value less or equal than 5  and greater than 3, than the Masonry Wall has an average in Plane behaviour" ;
   rdfs:label "Average in plane behaviour" ;
   rdf:type swrl:Imp ;
   swrl:body [ rdf:type swrl:AtomList ;
               rdf:first [ rdf:type swrl:ClassAtom ;
                           swrl:classPredicate hmo:MasonryWall ;
                           swrl:argument1 fmo:wl
                         ] ;
               rdf:rest [ rdf:type swrl:AtomList ;
                          rdf:first [ rdf:type swrl:IndividualPropertyAtom ;
                                      swrl:propertyPredicate hmo:hasMasonryQualityIndex ;
                                      swrl:argument1 fmo:wl ;
                                      swrl:argument2 fmo:MQI
                                    ] ;
                          rdf:rest [ rdf:type swrl:AtomList ;
                                     rdf:first [ rdf:type swrl:DatavaluedPropertyAtom ;
                                                 swrl:propertyPredicate hmo:MQITotalInPlane ;
                                                 swrl:argument1 fmo:MQI ;
                                                 swrl:argument2 fmo:MQIv
                                               ] ;
                                     rdf:rest [ rdf:type swrl:AtomList ;
                                                rdf:first [ rdf:type swrl:BuiltinAtom ;
                                                            swrl:builtin swrlb:lessThanOrEqual ;
                                                            swrl:arguments [ rdf:type rdf:List ;
                                                                             rdf:first fmo:MQIv ;
                                                                             rdf:rest [ rdf:type rdf:List ;
                                                                                        rdf:first 5 ;
                                                                                        rdf:rest rdf:nil
                                                                                      ]
                                                                           ]
                                                          ] ;
                                                rdf:rest [ rdf:type swrl:AtomList ;
                                                           rdf:first [ rdf:type swrl:BuiltinAtom ;
                                                                       swrl:builtin swrlb:greaterThan ;
                                                                       swrl:arguments [ rdf:type rdf:List ;
                                                                                        rdf:first fmo:MQIv ;
                                                                                        rdf:rest [ rdf:type rdf:List ;
                                                                                                   rdf:first 3 ;
                                                                                                   rdf:rest rdf:nil
                                                                                                 ]
                                                                                      ]
                                                                     ] ;
                                                           rdf:rest rdf:nil
                                                         ]
                                              ]
                                   ]
                        ]
             ] ;
   swrl:head [ rdf:type swrl:AtomList ;
               rdf:first [ rdf:type swrl:IndividualPropertyAtom ;
                           swrl:propertyPredicate fmo:hasBehaviour ;
                           swrl:argument1 fmo:wl ;
                           swrl:argument2 fmo:AverageInPlaneBehaviour
                         ] ;
               rdf:rest rdf:nil
             ]
 ] .

[ swrla:isRuleEnabled "true"^^xsd:boolean ;
   rdfs:comment "If a Masonry Wall has a Masonry Quality Index, which has a Masonry Quality Index Total vertical value less or equal than 10 and greater than 5, than the Masonry Wall has a good vertical behaviour" ;
   rdfs:label "Good vertical behaviour" ;
   rdf:type swrl:Imp ;
   swrl:body [ rdf:type swrl:AtomList ;
               rdf:first [ rdf:type swrl:ClassAtom ;
                           swrl:classPredicate hmo:MasonryWall ;
                           swrl:argument1 fmo:wl
                         ] ;
               rdf:rest [ rdf:type swrl:AtomList ;
                          rdf:first [ rdf:type swrl:IndividualPropertyAtom ;
                                      swrl:propertyPredicate hmo:hasMasonryQualityIndex ;
                                      swrl:argument1 fmo:wl ;
                                      swrl:argument2 fmo:MQI
                                    ] ;
                          rdf:rest [ rdf:type swrl:AtomList ;
                                     rdf:first [ rdf:type swrl:DatavaluedPropertyAtom ;
                                                 swrl:propertyPredicate hmo:MQITotalVertical ;
                                                 swrl:argument1 fmo:MQI ;
                                                 swrl:argument2 fmo:MQIv
                                               ] ;
                                     rdf:rest [ rdf:type swrl:AtomList ;
                                                rdf:first [ rdf:type swrl:BuiltinAtom ;
                                                            swrl:builtin swrlb:lessThanOrEqual ;
                                                            swrl:arguments [ rdf:type rdf:List ;
                                                                             rdf:first fmo:MQIv ;
                                                                             rdf:rest [ rdf:type rdf:List ;
                                                                                        rdf:first 10 ;
                                                                                        rdf:rest rdf:nil
                                                                                      ]
                                                                           ]
                                                          ] ;
                                                rdf:rest [ rdf:type swrl:AtomList ;
                                                           rdf:first [ rdf:type swrl:BuiltinAtom ;
                                                                       swrl:builtin swrlb:greaterThan ;
                                                                       swrl:arguments [ rdf:type rdf:List ;
                                                                                        rdf:first fmo:MQIv ;
                                                                                        rdf:rest [ rdf:type rdf:List ;
                                                                                                   rdf:first 5 ;
                                                                                                   rdf:rest rdf:nil
                                                                                                 ]
                                                                                      ]
                                                                     ] ;
                                                           rdf:rest rdf:nil
                                                         ]
                                              ]
                                   ]
                        ]
             ] ;
   swrl:head [ rdf:type swrl:AtomList ;
               rdf:first [ rdf:type swrl:IndividualPropertyAtom ;
                           swrl:propertyPredicate fmo:hasBehaviour ;
                           swrl:argument1 fmo:wl ;
                           swrl:argument2 fmo:GoodVerticalBehaviour
                         ] ;
               rdf:rest rdf:nil
             ]
 ] .

[ swrla:isRuleEnabled "true"^^xsd:boolean ;
   rdfs:comment "If a Masonry Wall has a Masonry Quality Index, which has a Masonry Quality Index Total vertical value less or equal than 2.5 and greater or equal than 0, than the Masonry Wall has an inadequate vertical behaviour" ;
   rdfs:label "Inadequate vertical behaviour" ;
   rdf:type swrl:Imp ;
   swrl:body [ rdf:type swrl:AtomList ;
               rdf:first [ rdf:type swrl:ClassAtom ;
                           swrl:classPredicate hmo:MasonryWall ;
                           swrl:argument1 fmo:wl
                         ] ;
               rdf:rest [ rdf:type swrl:AtomList ;
                          rdf:first [ rdf:type swrl:IndividualPropertyAtom ;
                                      swrl:propertyPredicate hmo:hasMasonryQualityIndex ;
                                      swrl:argument1 fmo:wl ;
                                      swrl:argument2 fmo:MQI
                                    ] ;
                          rdf:rest [ rdf:type swrl:AtomList ;
                                     rdf:first [ rdf:type swrl:DatavaluedPropertyAtom ;
                                                 swrl:propertyPredicate hmo:MQITotalVertical ;
                                                 swrl:argument1 fmo:MQI ;
                                                 swrl:argument2 fmo:MQIv
                                               ] ;
                                     rdf:rest [ rdf:type swrl:AtomList ;
                                                rdf:first [ rdf:type swrl:BuiltinAtom ;
                                                            swrl:builtin swrlb:lessThanOrEqual ;
                                                            swrl:arguments [ rdf:type rdf:List ;
                                                                             rdf:first fmo:MQIv ;
                                                                             rdf:rest [ rdf:type rdf:List ;
                                                                                        rdf:first "2.5" ;
                                                                                        rdf:rest rdf:nil
                                                                                      ]
                                                                           ]
                                                          ] ;
                                                rdf:rest [ rdf:type swrl:AtomList ;
                                                           rdf:first [ rdf:type swrl:BuiltinAtom ;
                                                                       swrl:builtin swrlb:greaterThanOrEqual ;
                                                                       swrl:arguments [ rdf:type rdf:List ;
                                                                                        rdf:first fmo:MQIv ;
                                                                                        rdf:rest [ rdf:type rdf:List ;
                                                                                                   rdf:first "0" ;
                                                                                                   rdf:rest rdf:nil
                                                                                                 ]
                                                                                      ]
                                                                     ] ;
                                                           rdf:rest rdf:nil
                                                         ]
                                              ]
                                   ]
                        ]
             ] ;
   swrl:head [ rdf:type swrl:AtomList ;
               rdf:first [ rdf:type swrl:IndividualPropertyAtom ;
                           swrl:propertyPredicate fmo:hasBehaviour ;
                           swrl:argument1 fmo:wl ;
                           swrl:argument2 fmo:InadequateVerticalBehaviour
                         ] ;
               rdf:rest rdf:nil
             ]
 ] .

[ swrla:isRuleEnabled "true"^^xsd:boolean ;
   rdfs:comment "If a Masonry Wall has a Masonry Quality Index, which has a Masonry Quality Index Total Vertical value less or equal than 5 and greater than 2.5, than the Masonry Wall has an average vertical behaviour" ;
   rdfs:label "Average vertical Behaviour" ;
   rdf:type swrl:Imp ;
   swrl:body [ rdf:type swrl:AtomList ;
               rdf:first [ rdf:type swrl:ClassAtom ;
                           swrl:classPredicate hmo:MasonryWall ;
                           swrl:argument1 fmo:wl
                         ] ;
               rdf:rest [ rdf:type swrl:AtomList ;
                          rdf:first [ rdf:type swrl:IndividualPropertyAtom ;
                                      swrl:propertyPredicate hmo:hasMasonryQualityIndex ;
                                      swrl:argument1 fmo:wl ;
                                      swrl:argument2 fmo:MQI
                                    ] ;
                          rdf:rest [ rdf:type swrl:AtomList ;
                                     rdf:first [ rdf:type swrl:DatavaluedPropertyAtom ;
                                                 swrl:propertyPredicate hmo:MQITotalVertical ;
                                                 swrl:argument1 fmo:MQI ;
                                                 swrl:argument2 fmo:MQIv
                                               ] ;
                                     rdf:rest [ rdf:type swrl:AtomList ;
                                                rdf:first [ rdf:type swrl:BuiltinAtom ;
                                                            swrl:builtin swrlb:lessThanOrEqual ;
                                                            swrl:arguments [ rdf:type rdf:List ;
                                                                             rdf:first fmo:MQIv ;
                                                                             rdf:rest [ rdf:type rdf:List ;
                                                                                        rdf:first 5 ;
                                                                                        rdf:rest rdf:nil
                                                                                      ]
                                                                           ]
                                                          ] ;
                                                rdf:rest [ rdf:type swrl:AtomList ;
                                                           rdf:first [ rdf:type swrl:BuiltinAtom ;
                                                                       swrl:builtin swrlb:greaterThanOrEqual ;
                                                                       swrl:arguments [ rdf:type rdf:List ;
                                                                                        rdf:first fmo:MQIv ;
                                                                                        rdf:rest [ rdf:type rdf:List ;
                                                                                                   rdf:first 2.5 ;
                                                                                                   rdf:rest rdf:nil
                                                                                                 ]
                                                                                      ]
                                                                     ] ;
                                                           rdf:rest rdf:nil
                                                         ]
                                              ]
                                   ]
                        ]
             ] ;
   swrl:head [ rdf:type swrl:AtomList ;
               rdf:first [ rdf:type swrl:IndividualPropertyAtom ;
                           swrl:propertyPredicate fmo:hasBehaviour ;
                           swrl:argument1 fmo:wl ;
                           swrl:argument2 fmo:AverageVerticalBehaviour
                         ] ;
               rdf:rest rdf:nil
             ]
 ] .

[ swrla:isRuleEnabled "true"^^xsd:boolean ;
   rdfs:comment "If a wall has a damage, and the damage is caused by a specific mechanism, than the wall has a ongoing mechanism" ;
   rdfs:label "Mechanism and damage" ;
   rdf:type swrl:Imp ;
   swrl:body [ rdf:type swrl:AtomList ;
               rdf:first [ rdf:type swrl:IndividualPropertyAtom ;
                           swrl:propertyPredicate dot:hasDamage ;
                           swrl:argument1 fmo:wl ;
                           swrl:argument2 fmo:dmg
                         ] ;
               rdf:rest [ rdf:type swrl:AtomList ;
                          rdf:first [ rdf:type swrl:IndividualPropertyAtom ;
                                      swrl:propertyPredicate dot:hasCausation ;
                                      swrl:argument1 fmo:dmg ;
                                      swrl:argument2 fmo:mcn
                                    ] ;
                          rdf:rest rdf:nil
                        ]
             ] ;
   swrl:head [ rdf:type swrl:AtomList ;
               rdf:first [ rdf:type swrl:IndividualPropertyAtom ;
                           swrl:propertyPredicate fmo:hasOccurringMechanism ;
                           swrl:argument1 fmo:wl ;
                           swrl:argument2 fmo:mcn
                         ] ;
               rdf:rest rdf:nil
             ]
 ] .

[ swrla:isRuleEnabled "true"^^xsd:boolean ;
   rdfs:comment "If a masonry wall has a vulnerability that is ‘inadequate in plane behaviour’, then it has a vulnerability that is ‘inadequate in plane behaviour’." ;
   rdfs:label "Inadequate in plane behaviour vulnerability" ;
   rdf:type swrl:Imp ;
   swrl:body [ rdf:type swrl:AtomList ;
               rdf:first [ rdf:type swrl:IndividualPropertyAtom ;
                           swrl:propertyPredicate fmo:hasBehaviour ;
                           swrl:argument1 fmo:wl ;
                           swrl:argument2 fmo:InadequateInPlaneBehaviour
                         ] ;
               rdf:rest rdf:nil
             ] ;
   swrl:head [ rdf:type swrl:AtomList ;
               rdf:first [ rdf:type swrl:IndividualPropertyAtom ;
                           swrl:propertyPredicate fmo:hasVulnerability ;
                           swrl:argument1 fmo:wl ;
                           swrl:argument2 fmo:InadequateInPlaneBehaviour
                         ] ;
               rdf:rest rdf:nil
             ]
 ] .

[ swrla:isRuleEnabled "true"^^xsd:boolean ;
   rdfs:comment "If a masonry wall has a vulnerability that is ‘inadequate out of plane behaviour’, then it has an occurring mechanism that is ‘out of plane failure’." ;
   rdfs:label "Inadequate Out Of Plane Behaviour Vulnerability" ;
   rdf:type swrl:Imp ;
   swrl:body [ rdf:type swrl:AtomList ;
               rdf:first [ rdf:type swrl:IndividualPropertyAtom ;
                           swrl:propertyPredicate fmo:hasBehaviour ;
                           swrl:argument1 fmo:wl ;
                           swrl:argument2 fmo:InadequateOutOfPlaneBehaviour
                         ] ;
               rdf:rest rdf:nil
             ] ;
   swrl:head [ rdf:type swrl:AtomList ;
               rdf:first [ rdf:type swrl:IndividualPropertyAtom ;
                           swrl:propertyPredicate fmo:hasVulnerability ;
                           swrl:argument1 fmo:wl ;
                           swrl:argument2 fmo:InadequateOutOfPlaneBehaviour
                         ] ;
               rdf:rest rdf:nil
             ]
 ] .

[ swrla:isRuleEnabled "true"^^xsd:boolean ;
   rdfs:comment "If a masonry wall has a vulnerability that is ‘excessive slenderness’ and a vulnerability that is ‘absence of top chains’ and a vulnerability that is ‘presence of horizontal thrusts’ and a behaviour that is ‘inadequate out of plane behaviour’, then it has an occurring mechanism that is ‘horizontal bending’." ;
   rdfs:label "Horizontal bending - absence of top chains" ;
   rdf:type swrl:Imp ;
   swrl:body [ rdf:type swrl:AtomList ;
               rdf:first [ rdf:type swrl:IndividualPropertyAtom ;
                           swrl:propertyPredicate fmo:hasVulnerability ;
                           swrl:argument1 fmo:wl ;
                           swrl:argument2 fmo:ExcessiveSlenderness
                         ] ;
               rdf:rest [ rdf:type swrl:AtomList ;
                          rdf:first [ rdf:type swrl:IndividualPropertyAtom ;
                                      swrl:propertyPredicate fmo:hasVulnerability ;
                                      swrl:argument1 fmo:wl ;
                                      swrl:argument2 fmo:AbsenceOfTopChains
                                    ] ;
                          rdf:rest [ rdf:type swrl:AtomList ;
                                     rdf:first [ rdf:type swrl:IndividualPropertyAtom ;
                                                 swrl:propertyPredicate fmo:hasVulnerability ;
                                                 swrl:argument1 fmo:wl ;
                                                 swrl:argument2 fmo:PresenceOfHorizontalThrust
                                               ] ;
                                     rdf:rest [ rdf:type swrl:AtomList ;
                                                rdf:first [ rdf:type swrl:IndividualPropertyAtom ;
                                                            swrl:propertyPredicate fmo:hasBehaviour ;
                                                            swrl:argument1 fmo:wl ;
                                                            swrl:argument2 fmo:InadequateOutOfPlaneBehaviour
                                                          ] ;
                                                rdf:rest rdf:nil
                                              ]
                                   ]
                        ]
             ] ;
   swrl:head [ rdf:type swrl:AtomList ;
               rdf:first [ rdf:type swrl:IndividualPropertyAtom ;
                           swrl:propertyPredicate fmo:hasOccurringMechanism ;
                           swrl:argument1 fmo:wl ;
                           swrl:argument2 fmo:HorizontalBending
                         ] ;
               rdf:rest rdf:nil
             ]
 ] .

[ swrla:isRuleEnabled "true"^^xsd:boolean ;
   rdfs:comment "If a Masonry Wall has a Masonry Quality Index, which has a Masonry Quality Index Total In Plane Value less or equal than 10 and greater than 5, than the Masonry Wall has an good in plane behaviour" ;
   rdfs:label "Good in plane behaviour" ;
   rdf:type swrl:Imp ;
   swrl:body [ rdf:type swrl:AtomList ;
               rdf:first [ rdf:type swrl:ClassAtom ;
                           swrl:classPredicate hmo:MasonryWall ;
                           swrl:argument1 fmo:wl
                         ] ;
               rdf:rest [ rdf:type swrl:AtomList ;
                          rdf:first [ rdf:type swrl:IndividualPropertyAtom ;
                                      swrl:propertyPredicate hmo:hasMasonryQualityIndex ;
                                      swrl:argument1 fmo:wl ;
                                      swrl:argument2 fmo:MQI
                                    ] ;
                          rdf:rest [ rdf:type swrl:AtomList ;
                                     rdf:first [ rdf:type swrl:DatavaluedPropertyAtom ;
                                                 swrl:propertyPredicate hmo:MQITotalInPlane ;
                                                 swrl:argument1 fmo:MQI ;
                                                 swrl:argument2 fmo:MQIv
                                               ] ;
                                     rdf:rest [ rdf:type swrl:AtomList ;
                                                rdf:first [ rdf:type swrl:BuiltinAtom ;
                                                            swrl:builtin swrlb:lessThanOrEqual ;
                                                            swrl:arguments [ rdf:type rdf:List ;
                                                                             rdf:first fmo:MQIv ;
                                                                             rdf:rest [ rdf:type rdf:List ;
                                                                                        rdf:first 10 ;
                                                                                        rdf:rest rdf:nil
                                                                                      ]
                                                                           ]
                                                          ] ;
                                                rdf:rest [ rdf:type swrl:AtomList ;
                                                           rdf:first [ rdf:type swrl:BuiltinAtom ;
                                                                       swrl:builtin swrlb:greaterThan ;
                                                                       swrl:arguments [ rdf:type rdf:List ;
                                                                                        rdf:first fmo:MQIv ;
                                                                                        rdf:rest [ rdf:type rdf:List ;
                                                                                                   rdf:first 5 ;
                                                                                                   rdf:rest rdf:nil
                                                                                                 ]
                                                                                      ]
                                                                     ] ;
                                                           rdf:rest rdf:nil
                                                         ]
                                              ]
                                   ]
                        ]
             ] ;
   swrl:head [ rdf:type swrl:AtomList ;
               rdf:first [ rdf:type swrl:IndividualPropertyAtom ;
                           swrl:propertyPredicate fmo:hasBehaviour ;
                           swrl:argument1 fmo:wl ;
                           swrl:argument2 fmo:GoodInPlaneBehaviour
                         ] ;
               rdf:rest rdf:nil
             ]
 ] .

[ swrla:isRuleEnabled "true"^^xsd:boolean ;
   rdfs:comment "If a masonry wall has a vulnerability that is ‘excessive slenderness’ and a vulnerability that is ‘absence of top curbstone’ and a vulnerability that is ‘presence of horizontal thrusts’ and a behaviour that is ‘inadequate out of plane behaviour’, then it has an occurring mechanism that is ‘horizontal bending’." ;
   rdfs:label "Horizontal bending - absence of top curbstone" ;
   rdf:type swrl:Imp ;
   swrl:body [ rdf:type swrl:AtomList ;
               rdf:first [ rdf:type swrl:IndividualPropertyAtom ;
                           swrl:propertyPredicate fmo:hasVulnerability ;
                           swrl:argument1 fmo:wl ;
                           swrl:argument2 fmo:ExcessiveSlenderness
                         ] ;
               rdf:rest [ rdf:type swrl:AtomList ;
                          rdf:first [ rdf:type swrl:IndividualPropertyAtom ;
                                      swrl:propertyPredicate fmo:hasVulnerability ;
                                      swrl:argument1 fmo:wl ;
                                      swrl:argument2 fmo:AbsenceOfTopCurbstone
                                    ] ;
                          rdf:rest [ rdf:type swrl:AtomList ;
                                     rdf:first [ rdf:type swrl:IndividualPropertyAtom ;
                                                 swrl:propertyPredicate fmo:hasVulnerability ;
                                                 swrl:argument1 fmo:wl ;
                                                 swrl:argument2 fmo:PresenceOfHorizontalThrust
                                               ] ;
                                     rdf:rest [ rdf:type swrl:AtomList ;
                                                rdf:first [ rdf:type swrl:IndividualPropertyAtom ;
                                                            swrl:propertyPredicate fmo:hasBehaviour ;
                                                            swrl:argument1 fmo:wl ;
                                                            swrl:argument2 fmo:InadequateOutOfPlaneBehaviour
                                                          ] ;
                                                rdf:rest rdf:nil
                                              ]
                                   ]
                        ]
             ] ;
   swrl:head [ rdf:type swrl:AtomList ;
               rdf:first [ rdf:type swrl:IndividualPropertyAtom ;
                           swrl:propertyPredicate fmo:hasOccurringMechanism ;
                           swrl:argument1 fmo:wl ;
                           swrl:argument2 fmo:HorizontalBending
                         ] ;
               rdf:rest rdf:nil
             ]
 ] .

[ swrla:isRuleEnabled "true"^^xsd:boolean ;
   rdfs:comment "If a masonry wall has a vulnerability that is ‘excessive slenderness’  and has a vulnerability that is ‘presence of horizontal thrusts’, and has a vulnerability that is ‘deformable floor, and it has a behaviour that is ‘inadequate out of plane behaviour’, then it has an occurring mechanism that is ‘vertical bending’." ;
   rdfs:label "Vertical bending" ;
   rdf:type swrl:Imp ;
   swrl:body [ rdf:type swrl:AtomList ;
               rdf:first [ rdf:type swrl:IndividualPropertyAtom ;
                           swrl:propertyPredicate fmo:hasVulnerability ;
                           swrl:argument1 fmo:wl ;
                           swrl:argument2 fmo:ExcessiveSlenderness
                         ] ;
               rdf:rest [ rdf:type swrl:AtomList ;
                          rdf:first [ rdf:type swrl:IndividualPropertyAtom ;
                                      swrl:propertyPredicate fmo:hasVulnerability ;
                                      swrl:argument1 fmo:wl ;
                                      swrl:argument2 fmo:PresenceOfHorizontalThrust
                                    ] ;
                          rdf:rest [ rdf:type swrl:AtomList ;
                                     rdf:first [ rdf:type swrl:IndividualPropertyAtom ;
                                                 swrl:propertyPredicate fmo:hasVulnerability ;
                                                 swrl:argument1 fmo:wl ;
                                                 swrl:argument2 fmo:DeformableFloors
                                               ] ;
                                     rdf:rest [ rdf:type swrl:AtomList ;
                                                rdf:first [ rdf:type swrl:IndividualPropertyAtom ;
                                                            swrl:propertyPredicate fmo:hasBehaviour ;
                                                            swrl:argument1 fmo:wl ;
                                                            swrl:argument2 fmo:InadequateOutOfPlaneBehaviour
                                                          ] ;
                                                rdf:rest rdf:nil
                                              ]
                                   ]
                        ]
             ] ;
   swrl:head [ rdf:type swrl:AtomList ;
               rdf:first [ rdf:type swrl:IndividualPropertyAtom ;
                           swrl:propertyPredicate fmo:hasOccurringMechanism ;
                           swrl:argument1 fmo:wl ;
                           swrl:argument2 fmo:VerticalBending
                         ] ;
               rdf:rest rdf:nil
             ]
 ] .

[ swrla:isRuleEnabled "true"^^xsd:boolean ;
   rdfs:comment "If a masonry wall has a behaviour that is ‘inadequate vertical behaviour’, then it has a vulnerability that is ‘inadequate vertical behaviour’." ;
   rdfs:label "Inadequate Vertical Behaviour Vulnerability" ;
   rdf:type swrl:Imp ;
   swrl:body [ rdf:type swrl:AtomList ;
               rdf:first [ rdf:type swrl:IndividualPropertyAtom ;
                           swrl:propertyPredicate fmo:hasBehaviour ;
                           swrl:argument1 fmo:wl ;
                           swrl:argument2 fmo:InadequateVerticalBehaviour
                         ] ;
               rdf:rest rdf:nil
             ] ;
   swrl:head [ rdf:type swrl:AtomList ;
               rdf:first [ rdf:type swrl:IndividualPropertyAtom ;
                           swrl:propertyPredicate fmo:hasVulnerability ;
                           swrl:argument1 fmo:wl ;
                           swrl:argument2 fmo:InadequateVerticalBehaviour
                         ] ;
               rdf:rest rdf:nil
             ]
 ] .

[ swrla:isRuleEnabled "true"^^xsd:boolean ;
   rdfs:comment "If a masonry wall has a vulnerability that is ‘absence of intermediate chains’ and has a vulnerability that is ‘absence of top chains’, then it has an occurring mechanism that is ‘total overturn'." ;
   rdfs:label "Total overtun - chains" ;
   rdf:type swrl:Imp ;
   swrl:body [ rdf:type swrl:AtomList ;
               rdf:first [ rdf:type swrl:IndividualPropertyAtom ;
                           swrl:propertyPredicate fmo:hasVulnerability ;
                           swrl:argument1 fmo:wl ;
                           swrl:argument2 fmo:AbsenceOfIntermediateChains
                         ] ;
               rdf:rest [ rdf:type swrl:AtomList ;
                          rdf:first [ rdf:type swrl:IndividualPropertyAtom ;
                                      swrl:propertyPredicate fmo:hasVulnerability ;
                                      swrl:argument1 fmo:wl ;
                                      swrl:argument2 fmo:AbsenceOfTopChains
                                    ] ;
                          rdf:rest rdf:nil
                        ]
             ] ;
   swrl:head [ rdf:type swrl:AtomList ;
               rdf:first [ rdf:type swrl:IndividualPropertyAtom ;
                           swrl:propertyPredicate fmo:hasOccurringMechanism ;
                           swrl:argument1 fmo:wl ;
                           swrl:argument2 fmo:TotalOverturn
                         ] ;
               rdf:rest rdf:nil
             ]
 ] .

[ swrla:isRuleEnabled "true"^^xsd:boolean ;
   rdfs:comment "If a masonry wall has a vulnerability that is ‘absence of intermediate chains' and has a vulnerability that is ‘absence of top curbstone', then it has an occurring mechanism that is ‘total overturn." ;
   rdfs:label "Total overturn chain - curbston" ;
   rdf:type swrl:Imp ;
   swrl:body [ rdf:type swrl:AtomList ;
               rdf:first [ rdf:type swrl:IndividualPropertyAtom ;
                           swrl:propertyPredicate fmo:hasVulnerability ;
                           swrl:argument1 fmo:wl ;
                           swrl:argument2 fmo:AbsenceOfIntermediateChains
                         ] ;
               rdf:rest [ rdf:type swrl:AtomList ;
                          rdf:first [ rdf:type swrl:IndividualPropertyAtom ;
                                      swrl:propertyPredicate fmo:hasVulnerability ;
                                      swrl:argument1 fmo:wl ;
                                      swrl:argument2 fmo:AbsenceOfTopCurbstone
                                    ] ;
                          rdf:rest rdf:nil
                        ]
             ] ;
   swrl:head [ rdf:type swrl:AtomList ;
               rdf:first [ rdf:type swrl:IndividualPropertyAtom ;
                           swrl:propertyPredicate fmo:hasOccurringMechanism ;
                           swrl:argument1 fmo:wl ;
                           swrl:argument2 fmo:TotalOverturn
                         ] ;
               rdf:rest rdf:nil
             ]
 ] .

[ swrla:isRuleEnabled "true"^^xsd:boolean ;
   rdfs:comment "If a masonry wall has a vulnerability that is ‘absence of intermediate curbstone’ and has a vulnerability that is ‘absence of top chains', then it has an occurring mechanism that is ‘total overturn." ;
   rdfs:label "Total overturn - curstone -chain" ;
   rdf:type swrl:Imp ;
   swrl:body [ rdf:type swrl:AtomList ;
               rdf:first [ rdf:type swrl:IndividualPropertyAtom ;
                           swrl:propertyPredicate fmo:hasVulnerability ;
                           swrl:argument1 fmo:wl ;
                           swrl:argument2 fmo:AbsenceOfIntermediateCurbstone
                         ] ;
               rdf:rest [ rdf:type swrl:AtomList ;
                          rdf:first [ rdf:type swrl:IndividualPropertyAtom ;
                                      swrl:propertyPredicate fmo:hasVulnerability ;
                                      swrl:argument1 fmo:wl ;
                                      swrl:argument2 fmo:AbsenceOfTopChains
                                    ] ;
                          rdf:rest rdf:nil
                        ]
             ] ;
   swrl:head [ rdf:type swrl:AtomList ;
               rdf:first [ rdf:type swrl:IndividualPropertyAtom ;
                           swrl:propertyPredicate fmo:hasOccurringMechanism ;
                           swrl:argument1 fmo:wl ;
                           swrl:argument2 fmo:TotalOverturn
                         ] ;
               rdf:rest rdf:nil
             ]
 ] .

[ swrla:isRuleEnabled "true"^^xsd:boolean ;
   rdfs:comment "If a masonry wall has a vulnerability that is ‘absence of intermediate curbstone’ and has a vulnerability that is ‘absence of top curbstone’, then it has an occurring mechanism that is ‘total overturn." ;
   rdfs:label "Total overturn - curbstone" ;
   rdf:type swrl:Imp ;
   swrl:body [ rdf:type swrl:AtomList ;
               rdf:first [ rdf:type swrl:IndividualPropertyAtom ;
                           swrl:propertyPredicate fmo:hasVulnerability ;
                           swrl:argument1 fmo:wl ;
                           swrl:argument2 fmo:AbsenceOfIntermediateCurbstone
                         ] ;
               rdf:rest [ rdf:type swrl:AtomList ;
                          rdf:first [ rdf:type swrl:IndividualPropertyAtom ;
                                      swrl:propertyPredicate fmo:hasVulnerability ;
                                      swrl:argument1 fmo:wl ;
                                      swrl:argument2 fmo:AbsenceOfTopCurbstone
                                    ] ;
                          rdf:rest rdf:nil
                        ]
             ] ;
   swrl:head [ rdf:type swrl:AtomList ;
               rdf:first [ rdf:type swrl:IndividualPropertyAtom ;
                           swrl:propertyPredicate fmo:hasOccurringMechanism ;
                           swrl:argument1 fmo:wl ;
                           swrl:argument2 fmo:TotalOverturn
                         ] ;
               rdf:rest rdf:nil
             ]
 ] .

[ swrla:isRuleEnabled "true"^^xsd:boolean ;
   rdfs:comment "If a masonry wall has a vulnerability that is ‘absence of top chains’, then it has an occurring mechanism that is ‘partial overturn." ;
   rdfs:label "Partial overturn - chains" ;
   rdf:type swrl:Imp ;
   swrl:body [ rdf:type swrl:AtomList ;
               rdf:first [ rdf:type swrl:IndividualPropertyAtom ;
                           swrl:propertyPredicate fmo:hasVulnerability ;
                           swrl:argument1 fmo:wl ;
                           swrl:argument2 fmo:AbsenceOfTopChains
                         ] ;
               rdf:rest rdf:nil
             ] ;
   swrl:head [ rdf:type swrl:AtomList ;
               rdf:first [ rdf:type swrl:IndividualPropertyAtom ;
                           swrl:propertyPredicate fmo:hasOccurringMechanism ;
                           swrl:argument1 fmo:wl ;
                           swrl:argument2 fmo:PartialOverturn
                         ] ;
               rdf:rest rdf:nil
             ]
 ] .

[ swrla:isRuleEnabled "true"^^xsd:boolean ;
   rdfs:comment "If a masonry wall has a vulnerability that is ‘absence of top curbstone, then it has an occurring mechanism that is ‘partial overturn." ;
   rdfs:label "Partial overturn - curbstone" ;
   rdf:type swrl:Imp ;
   swrl:body [ rdf:type swrl:AtomList ;
               rdf:first [ rdf:type swrl:IndividualPropertyAtom ;
                           swrl:propertyPredicate fmo:hasVulnerability ;
                           swrl:argument1 fmo:wl ;
                           swrl:argument2 fmo:AbsenceOfTopCurbstone
                         ] ;
               rdf:rest rdf:nil
             ] ;
   swrl:head [ rdf:type swrl:AtomList ;
               rdf:first [ rdf:type swrl:IndividualPropertyAtom ;
                           swrl:propertyPredicate fmo:hasOccurringMechanism ;
                           swrl:argument1 fmo:wl ;
                           swrl:argument2 fmo:PartialOverturn
                         ] ;
               rdf:rest rdf:nil
             ]
 ] .

[ swrla:isRuleEnabled "true"^^xsd:boolean ;
   rdfs:comment "If a masonry wall has a vulnerability that is ‘inadequate in plane behaviour’, than it has an occurring mechanism that is ‘in plane failure’." ;
   rdfs:label "In plane failure" ;
   rdf:type swrl:Imp ;
   swrl:body [ rdf:type swrl:AtomList ;
               rdf:first [ rdf:type swrl:IndividualPropertyAtom ;
                           swrl:propertyPredicate fmo:hasVulnerability ;
                           swrl:argument1 fmo:wl ;
                           swrl:argument2 fmo:InadequateInPlaneBehaviour
                         ] ;
               rdf:rest rdf:nil
             ] ;
   swrl:head [ rdf:type swrl:AtomList ;
               rdf:first [ rdf:type swrl:IndividualPropertyAtom ;
                           swrl:propertyPredicate fmo:hasOccurringMechanism ;
                           swrl:argument1 fmo:wl ;
                           swrl:argument2 fmo:InPlaneFailure
                         ] ;
               rdf:rest rdf:nil
             ]
 ] .

[ swrla:isRuleEnabled "true"^^xsd:boolean ;
   rdfs:comment "If a Masonry Wall has a Masonry Quality Index, which has a Masonry Quality Index Total in plane value less or equal than 3 and greater or equal than 0, than the Masonry Wall has an inadequate In plane behaviour" ;
   rdfs:label "Inadequate in plane behavior" ;
   rdf:type swrl:Imp ;
   swrl:body [ rdf:type swrl:AtomList ;
               rdf:first [ rdf:type swrl:ClassAtom ;
                           swrl:classPredicate hmo:MasonryWall ;
                           swrl:argument1 fmo:wl
                         ] ;
               rdf:rest [ rdf:type swrl:AtomList ;
                          rdf:first [ rdf:type swrl:IndividualPropertyAtom ;
                                      swrl:propertyPredicate hmo:hasMasonryQualityIndex ;
                                      swrl:argument1 fmo:wl ;
                                      swrl:argument2 fmo:MQI
                                    ] ;
                          rdf:rest [ rdf:type swrl:AtomList ;
                                     rdf:first [ rdf:type swrl:DatavaluedPropertyAtom ;
                                                 swrl:propertyPredicate hmo:MQITotalInPlane ;
                                                 swrl:argument1 fmo:MQI ;
                                                 swrl:argument2 fmo:MQIv
                                               ] ;
                                     rdf:rest [ rdf:type swrl:AtomList ;
                                                rdf:first [ rdf:type swrl:BuiltinAtom ;
                                                            swrl:builtin swrlb:lessThanOrEqual ;
                                                            swrl:arguments [ rdf:type rdf:List ;
                                                                             rdf:first fmo:MQIv ;
                                                                             rdf:rest [ rdf:type rdf:List ;
                                                                                        rdf:first 3 ;
                                                                                        rdf:rest rdf:nil
                                                                                      ]
                                                                           ]
                                                          ] ;
                                                rdf:rest [ rdf:type swrl:AtomList ;
                                                           rdf:first [ rdf:type swrl:BuiltinAtom ;
                                                                       swrl:builtin swrlb:greaterThanOrEqual ;
                                                                       swrl:arguments [ rdf:type rdf:List ;
                                                                                        rdf:first fmo:MQIv ;
                                                                                        rdf:rest [ rdf:type rdf:List ;
                                                                                                   rdf:first 0 ;
                                                                                                   rdf:rest rdf:nil
                                                                                                 ]
                                                                                      ]
                                                                     ] ;
                                                           rdf:rest rdf:nil
                                                         ]
                                              ]
                                   ]
                        ]
             ] ;
   swrl:head [ rdf:type swrl:AtomList ;
               rdf:first [ rdf:type swrl:IndividualPropertyAtom ;
                           swrl:propertyPredicate fmo:hasBehaviour ;
                           swrl:argument1 fmo:wl ;
                           swrl:argument2 fmo:InadequateInPlaneBehaviour
                         ] ;
               rdf:rest rdf:nil
             ]
 ] .

[ swrla:isRuleEnabled "true"^^xsd:boolean ;
   rdfs:comment "If a Masonry Wall has a Masonry Quality Index, which has a Masonry Quality Index Total Out Of Plane Value less or equal than 7 and greater than 4, than the Masonry Wall has an average out of Plane behaviour" ;
   rdfs:label "Average out of plane behaviour" ;
   rdf:type swrl:Imp ;
   swrl:body [ rdf:type swrl:AtomList ;
               rdf:first [ rdf:type swrl:ClassAtom ;
                           swrl:classPredicate hmo:MasonryWall ;
                           swrl:argument1 fmo:wl
                         ] ;
               rdf:rest [ rdf:type swrl:AtomList ;
                          rdf:first [ rdf:type swrl:IndividualPropertyAtom ;
                                      swrl:propertyPredicate hmo:hasMasonryQualityIndex ;
                                      swrl:argument1 fmo:wl ;
                                      swrl:argument2 fmo:MQI
                                    ] ;
                          rdf:rest [ rdf:type swrl:AtomList ;
                                     rdf:first [ rdf:type swrl:DatavaluedPropertyAtom ;
                                                 swrl:propertyPredicate hmo:MQITotalOutOfPlane ;
                                                 swrl:argument1 fmo:MQI ;
                                                 swrl:argument2 fmo:MQIv
                                               ] ;
                                     rdf:rest [ rdf:type swrl:AtomList ;
                                                rdf:first [ rdf:type swrl:BuiltinAtom ;
                                                            swrl:builtin swrlb:lessThanOrEqual ;
                                                            swrl:arguments [ rdf:type rdf:List ;
                                                                             rdf:first fmo:MQIv ;
                                                                             rdf:rest [ rdf:type rdf:List ;
                                                                                        rdf:first 7 ;
                                                                                        rdf:rest rdf:nil
                                                                                      ]
                                                                           ]
                                                          ] ;
                                                rdf:rest [ rdf:type swrl:AtomList ;
                                                           rdf:first [ rdf:type swrl:BuiltinAtom ;
                                                                       swrl:builtin swrlb:greaterThan ;
                                                                       swrl:arguments [ rdf:type rdf:List ;
                                                                                        rdf:first fmo:MQIv ;
                                                                                        rdf:rest [ rdf:type rdf:List ;
                                                                                                   rdf:first 4 ;
                                                                                                   rdf:rest rdf:nil
                                                                                                 ]
                                                                                      ]
                                                                     ] ;
                                                           rdf:rest rdf:nil
                                                         ]
                                              ]
                                   ]
                        ]
             ] ;
   swrl:head [ rdf:type swrl:AtomList ;
               rdf:first [ rdf:type swrl:IndividualPropertyAtom ;
                           swrl:propertyPredicate fmo:hasBehaviour ;
                           swrl:argument1 fmo:wl ;
                           swrl:argument2 fmo:AverageOutOfPlaneBehaviour
                         ] ;
               rdf:rest rdf:nil
             ]
 ] .

[ swrla:isRuleEnabled "true"^^xsd:boolean ;
   rdfs:comment "If a Masonry Wall has a Masonry Quality Index, which has a Masonry Quality Index Total out of plane value less or equal than 10 and greater than 7, than the Masonry Wall has an good out of plane behaviour" ;
   rdfs:label "Good out of plane behaviour" ;
   rdf:type swrl:Imp ;
   swrl:body [ rdf:type swrl:AtomList ;
               rdf:first [ rdf:type swrl:ClassAtom ;
                           swrl:classPredicate hmo:MasonryWall ;
                           swrl:argument1 fmo:wl
                         ] ;
               rdf:rest [ rdf:type swrl:AtomList ;
                          rdf:first [ rdf:type swrl:IndividualPropertyAtom ;
                                      swrl:propertyPredicate hmo:hasMasonryQualityIndex ;
                                      swrl:argument1 fmo:wl ;
                                      swrl:argument2 fmo:MQI
                                    ] ;
                          rdf:rest [ rdf:type swrl:AtomList ;
                                     rdf:first [ rdf:type swrl:DatavaluedPropertyAtom ;
                                                 swrl:propertyPredicate hmo:MQITotalOutOfPlane ;
                                                 swrl:argument1 fmo:MQI ;
                                                 swrl:argument2 fmo:MQIv
                                               ] ;
                                     rdf:rest [ rdf:type swrl:AtomList ;
                                                rdf:first [ rdf:type swrl:BuiltinAtom ;
                                                            swrl:builtin swrlb:lessThanOrEqual ;
                                                            swrl:arguments [ rdf:type rdf:List ;
                                                                             rdf:first fmo:MQIv ;
                                                                             rdf:rest [ rdf:type rdf:List ;
                                                                                        rdf:first 10 ;
                                                                                        rdf:rest rdf:nil
                                                                                      ]
                                                                           ]
                                                          ] ;
                                                rdf:rest [ rdf:type swrl:AtomList ;
                                                           rdf:first [ rdf:type swrl:BuiltinAtom ;
                                                                       swrl:builtin swrlb:greaterThan ;
                                                                       swrl:arguments [ rdf:type rdf:List ;
                                                                                        rdf:first fmo:MQIv ;
                                                                                        rdf:rest [ rdf:type rdf:List ;
                                                                                                   rdf:first 7 ;
                                                                                                   rdf:rest rdf:nil
                                                                                                 ]
                                                                                      ]
                                                                     ] ;
                                                           rdf:rest rdf:nil
                                                         ]
                                              ]
                                   ]
                        ]
             ] ;
   swrl:head [ rdf:type swrl:AtomList ;
               rdf:first [ rdf:type swrl:IndividualPropertyAtom ;
                           swrl:propertyPredicate fmo:hasBehaviour ;
                           swrl:argument1 fmo:wl ;
                           swrl:argument2 fmo:GoodOutOfPlaneBehaviour
                         ] ;
               rdf:rest rdf:nil
             ]
 ] .

[ swrla:isRuleEnabled "true"^^xsd:boolean ;
   rdfs:comment "If a Masonry Wall has a Masonry Quality Index, which has a Masonry Quality Index Total out of plane value less or equal than 4 and greater or equal than 0, than the Masonry Wall has an inadequate out of plane behaviour" ;
   rdfs:label "Inadequate out of plane behaviour" ;
   rdf:type swrl:Imp ;
   swrl:body [ rdf:type swrl:AtomList ;
               rdf:first [ rdf:type swrl:ClassAtom ;
                           swrl:classPredicate hmo:MasonryWall ;
                           swrl:argument1 fmo:wl
                         ] ;
               rdf:rest [ rdf:type swrl:AtomList ;
                          rdf:first [ rdf:type swrl:IndividualPropertyAtom ;
                                      swrl:propertyPredicate hmo:hasMasonryQualityIndex ;
                                      swrl:argument1 fmo:wl ;
                                      swrl:argument2 fmo:MQI
                                    ] ;
                          rdf:rest [ rdf:type swrl:AtomList ;
                                     rdf:first [ rdf:type swrl:DatavaluedPropertyAtom ;
                                                 swrl:propertyPredicate hmo:MQITotalOutOfPlane ;
                                                 swrl:argument1 fmo:MQI ;
                                                 swrl:argument2 fmo:MQIv
                                               ] ;
                                     rdf:rest [ rdf:type swrl:AtomList ;
                                                rdf:first [ rdf:type swrl:BuiltinAtom ;
                                                            swrl:builtin swrlb:lessThanOrEqual ;
                                                            swrl:arguments [ rdf:type rdf:List ;
                                                                             rdf:first fmo:MQIv ;
                                                                             rdf:rest [ rdf:type rdf:List ;
                                                                                        rdf:first 4 ;
                                                                                        rdf:rest rdf:nil
                                                                                      ]
                                                                           ]
                                                          ] ;
                                                rdf:rest [ rdf:type swrl:AtomList ;
                                                           rdf:first [ rdf:type swrl:BuiltinAtom ;
                                                                       swrl:builtin swrlb:greaterThanOrEqual ;
                                                                       swrl:arguments [ rdf:type rdf:List ;
                                                                                        rdf:first fmo:MQIv ;
                                                                                        rdf:rest [ rdf:type rdf:List ;
                                                                                                   rdf:first 0 ;
                                                                                                   rdf:rest rdf:nil
                                                                                                 ]
                                                                                      ]
                                                                     ] ;
                                                           rdf:rest rdf:nil
                                                         ]
                                              ]
                                   ]
                        ]
             ] ;
   swrl:head [ rdf:type swrl:AtomList ;
               rdf:first [ rdf:type swrl:IndividualPropertyAtom ;
                           swrl:propertyPredicate fmo:hasBehaviour ;
                           swrl:argument1 fmo:wl ;
                           swrl:argument2 fmo:InadequateOutOfPlaneBehaviour
                         ] ;
               rdf:rest rdf:nil
             ]
 ] .

###  Generated by the OWL API (version 4.5.29.2024-05-13T12:11:03Z) https://github.com/owlcs/owlapi
