@prefix rdf: <http://www.w3.org/1999/02/22-rdf-syntax-ns#> .
@prefix rdfs: <http://www.w3.org/2000/01/rdf-schema#> .
@prefix xsd: <http://www.w3.org/2001/XMLSchema#> .
@prefix owl: <http://www.w3.org/2002/07/owl#> .
@prefix ph: <https://project-haystack.org/def/ph/4.0.0#> .
@prefix phIct: <https://project-haystack.org/def/phIct/4.0.0#> .
@prefix phScience: <https://project-haystack.org/def/phScience/4.0.0#> .
@prefix phIoT: <https://project-haystack.org/def/phIoT/4.0.0#> .

ph:hasTag a owl:ObjectProperty ;
    rdfs:range ph:marker .

phIoT:absorption a owl:Class ;
    rdfs:subClassOf ph:marker ;
    rdfs:label "absorption" ;
    rdfs:comment "Cooling process using energy from heat source such as hot water" ;
    ph:is ph:marker ;
    ph:lib phIoT:lib:phIoT ;
    ph:wikipedia "https://en.wikipedia.org/wiki/Absorption_refrigerator"^^xsd:anyURI .

phIoT:ac a owl:Class ;
    rdfs:subClassOf ph:marker ;
    rdfs:label "ac" ;
    rdfs:comment "Relating to alternating current (AC) electricity" ;
    ph:is ph:marker ;
    ph:lib phIoT:lib:phIoT .

phIoT:ac-elec a owl:Class ;
    rdfs:subClassOf phScience:elec ;
    rdfs:label "ac-elec" ;
    rdfs:comment "Alternating current electricity" ;
    ph:is phScience:elec ;
    ph:lib phIoT:lib:phIoT ;
    ph:wikipedia "https://en.wikipedia.org/wiki/Alternating_current"^^xsd:anyURI .

phIoT:ac-elec-meter a owl:Class ;
    rdfs:subClassOf phIoT:elec-meter ;
    rdfs:label "ac-elec-meter" ;
    ph:children _:0b2cb027-c6fa-9440-0d10-f23c91a70cca,
        _:0b2cb027-c6fa-9441-0d11-f23c91a70cca,
        _:0b2cb027-c6fa-9442-0d12-f23c91a70cca,
        _:0b2cb027-c6fa-9443-0d13-f23c91a70cca,
        _:0b2cb027-c6fa-9444-0d14-f23c91a70cca,
        _:0b2cb027-c6fa-9445-0d15-f23c91a70cca,
        _:0b2cb027-c6fa-9446-0d16-f23c91a70cca,
        _:0b2cb027-c6fa-9447-0d17-f23c91a70cca,
        _:0b2cb027-c6fa-9448-0d18-f23c91a70cca,
        _:0b2cb027-c709-d680-0d19-f23c91a70cca,
        _:0b2cb027-c709-d681-0d1a-f23c91a70cca,
        _:0b2cb027-c709-d682-0d1b-f23c91a70cca,
        _:0b2cb027-c709-d683-0d1c-f23c91a70cca,
        _:0b2cb027-c709-d684-0d1d-f23c91a70cca,
        _:0b2cb027-c709-d685-0d1e-f23c91a70cca,
        _:0b2cb027-c709-d686-0d1f-f23c91a70cca,
        _:0b2cb027-c709-d687-0d20-f23c91a70cca,
        _:0b2cb027-c709-d688-0d21-f23c91a70cca,
        _:0b2cb027-c709-d689-0d22-f23c91a70cca,
        _:0b2cb027-c709-d68a-0d23-f23c91a70cca,
        _:0b2cb027-c709-d68b-0d24-f23c91a70cca,
        _:0b2cb027-c709-d68c-0d25-f23c91a70cca,
        _:0b2cb027-c709-d68d-0d26-f23c91a70cca,
        _:0b2cb027-c709-d68e-0d27-f23c91a70cca,
        _:0b2cb027-c709-d68f-0d28-f23c91a70cca,
        _:0b2cb027-c709-d690-0d29-f23c91a70cca,
        _:0b2cb027-c709-d691-0d2a-f23c91a70cca,
        _:0b2cb027-c709-d692-0d2b-f23c91a70cca,
        _:0b2cb027-c709-d693-0d2c-f23c91a70cca,
        _:0b2cb027-c709-d694-0d2d-f23c91a70cca,
        _:0b2cb027-c709-d695-0d2e-f23c91a70cca ;
    rdfs:comment "AC Electricity meter.\nSee `docHaystack::Meters` chapter." ;
    ph:is phIoT:elec-meter ;
    ph:lib phIoT:lib:phIoT .

_:0b2cb027-c6fa-9440-0d10-f23c91a70cca a phIoT:point ;
    ph:hasTag phScience:avg,
        phIoT:ac,
        phScience:elec,
        phScience:current,
        phScience:angle,
        phIoT:sensor,
        phIoT:point ;
    rdfs:label "{avg, ac, elec, current, angle, sensor, point}" .

_:0b2cb027-c6fa-9441-0d11-f23c91a70cca a phIoT:point ;
    ph:hasTag phScience:avg,
        phIoT:ac,
        phScience:elec,
        phScience:current,
        phIoT:imbalance,
        phIoT:sensor,
        phIoT:point ;
    rdfs:label "{avg, ac, elec, current, imbalance, sensor, point}" .

_:0b2cb027-c6fa-9442-0d12-f23c91a70cca a phIoT:point ;
    ph:hasTag phScience:avg,
        phIoT:ac,
        phScience:elec,
        phScience:current,
        phScience:magnitude,
        phIoT:sensor,
        phIoT:point ;
    rdfs:label "{avg, ac, elec, current, magnitude, sensor, point}" .

_:0b2cb027-c6fa-9443-0d13-f23c91a70cca a phIoT:point ;
    ph:hasTag phScience:avg,
        phIoT:ac,
        phScience:elec,
        phScience:current,
        phIoT:thd,
        phIoT:sensor,
        phIoT:point ;
    rdfs:label "{avg, ac, elec, current, thd, sensor, point}" .

_:0b2cb027-c6fa-9444-0d14-f23c91a70cca a phIoT:point ;
    ph:hasTag phScience:avg,
        phIoT:ac,
        phScience:elec,
        phIoT:pf,
        phIoT:sensor,
        phIoT:point ;
    rdfs:label "{avg, ac, elec, pf, sensor, point}" .

_:0b2cb027-c6fa-9445-0d15-f23c91a70cca a phIoT:point ;
    ph:hasTag phScience:avg,
        phIoT:ac,
        phScience:elec,
        phScience:volt,
        phScience:angle,
        phIoT:sensor,
        phIoT:point ;
    rdfs:label "{avg, ac, elec, volt, angle, sensor, point}" .

_:0b2cb027-c6fa-9446-0d16-f23c91a70cca a phIoT:point ;
    ph:hasTag phScience:avg,
        phIoT:ac,
        phScience:elec,
        phScience:volt,
        phIoT:imbalance,
        phIoT:sensor,
        phIoT:point ;
    rdfs:label "{avg, ac, elec, volt, imbalance, sensor, point}" .

_:0b2cb027-c6fa-9447-0d17-f23c91a70cca a phIoT:point ;
    ph:hasTag phScience:avg,
        phIoT:ac,
        phScience:elec,
        phScience:volt,
        phScience:magnitude,
        phIoT:sensor,
        phIoT:point ;
    rdfs:label "{avg, ac, elec, volt, magnitude, sensor, point}" .

_:0b2cb027-c6fa-9448-0d18-f23c91a70cca a phIoT:point ;
    ph:hasTag phScience:avg,
        phIoT:ac,
        phScience:elec,
        phScience:volt,
        phIoT:thd,
        phIoT:sensor,
        phIoT:point ;
    rdfs:label "{avg, ac, elec, volt, thd, sensor, point}" .

_:0b2cb027-c709-d680-0d19-f23c91a70cca a phIoT:equip ;
    ph:hasTag phIoT:equip ;
    rdfs:label "{equip}" .

_:0b2cb027-c709-d681-0d1a-f23c91a70cca a phIoT:point ;
    ph:hasTag phIoT:ac,
        phScience:elec,
        phScience:current,
        phScience:angle,
        phIoT:sensor,
        phIoT:point ;
    rdfs:label "{phase:A, ac, elec, current, angle, sensor, point}" ;
    phIoT:phase "A" .

_:0b2cb027-c709-d682-0d1b-f23c91a70cca a phIoT:point ;
    ph:hasTag phIoT:ac,
        phScience:elec,
        phScience:current,
        phIoT:imbalance,
        phIoT:sensor,
        phIoT:point ;
    rdfs:label "{phase:A, ac, elec, current, imbalance, sensor, point}" ;
    phIoT:phase "A" .

_:0b2cb027-c709-d683-0d1c-f23c91a70cca a phIoT:point ;
    ph:hasTag phIoT:ac,
        phScience:elec,
        phScience:current,
        phScience:magnitude,
        phIoT:sensor,
        phIoT:point ;
    rdfs:label "{phase:A, ac, elec, current, magnitude, sensor, point}" ;
    phIoT:phase "A" .

_:0b2cb027-c709-d684-0d1d-f23c91a70cca a phIoT:point ;
    ph:hasTag phIoT:ac,
        phScience:elec,
        phScience:current,
        phIoT:thd,
        phIoT:sensor,
        phIoT:point ;
    rdfs:label "{phase:A, ac, elec, current, thd, sensor, point}" ;
    phIoT:phase "A" .

_:0b2cb027-c709-d685-0d1e-f23c91a70cca a phIoT:point ;
    ph:hasTag phIoT:ac,
        phScience:elec,
        phIoT:pf,
        phIoT:sensor,
        phIoT:point ;
    rdfs:label "{phase:A, ac, elec, pf, sensor, point}" ;
    phIoT:phase "A" .

_:0b2cb027-c709-d686-0d1f-f23c91a70cca a phIoT:point ;
    ph:hasTag phIoT:ac,
        phScience:elec,
        phScience:volt,
        phScience:angle,
        phIoT:sensor,
        phIoT:point ;
    rdfs:label "{phase:A, ac, elec, volt, angle, sensor, point}" ;
    phIoT:phase "A" .

_:0b2cb027-c709-d687-0d20-f23c91a70cca a phIoT:point ;
    ph:hasTag phIoT:ac,
        phScience:elec,
        phScience:volt,
        phIoT:imbalance,
        phIoT:sensor,
        phIoT:point ;
    rdfs:label "{phase:A, ac, elec, volt, imbalance, sensor, point}" ;
    phIoT:phase "A" .

_:0b2cb027-c709-d688-0d21-f23c91a70cca a phIoT:point ;
    ph:hasTag phIoT:ac,
        phScience:elec,
        phScience:volt,
        phScience:magnitude,
        phIoT:sensor,
        phIoT:point ;
    rdfs:label "{phase:A, ac, elec, volt, magnitude, sensor, point}" ;
    phIoT:phase "A" .

_:0b2cb027-c709-d689-0d22-f23c91a70cca a phIoT:point ;
    ph:hasTag phIoT:ac,
        phScience:elec,
        phScience:volt,
        phIoT:thd,
        phIoT:sensor,
        phIoT:point ;
    rdfs:label "{phase:A, ac, elec, volt, thd, sensor, point}" ;
    phIoT:phase "A" .

_:0b2cb027-c709-d68a-0d23-f23c91a70cca a phIoT:point ;
    ph:hasTag phIoT:active,
        phIoT:ac,
        phScience:elec,
        phScience:power,
        phIoT:sensor,
        phIoT:point ;
    rdfs:label "{phase:A, active, ac, elec, power, sensor, point}" ;
    phIoT:phase "A" .

_:0b2cb027-c709-d68b-0d24-f23c91a70cca a phIoT:point ;
    ph:hasTag phScience:apparent,
        phIoT:ac,
        phScience:elec,
        phScience:power,
        phIoT:sensor,
        phIoT:point ;
    rdfs:label "{phase:A, apparent, ac, elec, power, sensor, point}" ;
    phIoT:phase "A" .

_:0b2cb027-c709-d68c-0d25-f23c91a70cca a phIoT:point ;
    ph:hasTag phIoT:net,
        phIoT:ac,
        phScience:elec,
        phIoT:active,
        phScience:energy,
        phIoT:sensor,
        phIoT:point ;
    rdfs:label "{phase:A, net, ac, elec, active, energy, sensor, point}" ;
    phIoT:phase "A" .

_:0b2cb027-c709-d68d-0d26-f23c91a70cca a phIoT:point ;
    ph:hasTag phIoT:reactive,
        phIoT:ac,
        phScience:elec,
        phScience:power,
        phIoT:sensor,
        phIoT:point ;
    rdfs:label "{phase:A, reactive, ac, elec, power, sensor, point}" ;
    phIoT:phase "A" .

_:0b2cb027-c709-d68e-0d27-f23c91a70cca a phIoT:point ;
    ph:hasTag phIoT:point ;
    rdfs:label "{point}" .

_:0b2cb027-c709-d68f-0d28-f23c91a70cca a phIoT:point ;
    ph:hasTag phScience:total,
        phIoT:ac,
        phScience:elec,
        phIoT:demand,
        phIoT:sensor,
        phIoT:point ;
    rdfs:label "{total, ac, elec, demand, sensor, point}" .

_:0b2cb027-c709-d690-0d29-f23c91a70cca a phIoT:point ;
    ph:hasTag phScience:total,
        phIoT:active,
        phIoT:ac,
        phScience:elec,
        phScience:power,
        phIoT:sensor,
        phIoT:point ;
    rdfs:label "{total, active, ac, elec, power, sensor, point}" .

_:0b2cb027-c709-d691-0d2a-f23c91a70cca a phIoT:point ;
    ph:hasTag phScience:total,
        phScience:apparent,
        phIoT:ac,
        phScience:elec,
        phScience:power,
        phIoT:sensor,
        phIoT:point ;
    rdfs:label "{total, apparent, ac, elec, power, sensor, point}" .

_:0b2cb027-c709-d692-0d2b-f23c91a70cca a phIoT:point ;
    ph:hasTag phScience:total,
        phIoT:export,
        phIoT:ac,
        phScience:elec,
        phIoT:active,
        phScience:energy,
        phIoT:sensor,
        phIoT:point ;
    rdfs:label "{total, export, ac, elec, active, energy, sensor, point}" .

_:0b2cb027-c709-d693-0d2c-f23c91a70cca a phIoT:point ;
    ph:hasTag phScience:total,
        phIoT:import,
        phIoT:ac,
        phScience:elec,
        phIoT:active,
        phScience:energy,
        phIoT:sensor,
        phIoT:point ;
    rdfs:label "{total, import, ac, elec, active, energy, sensor, point}" .

_:0b2cb027-c709-d694-0d2d-f23c91a70cca a phIoT:point ;
    ph:hasTag phScience:total,
        phIoT:net,
        phIoT:ac,
        phScience:elec,
        phIoT:active,
        phScience:energy,
        phIoT:sensor,
        phIoT:point ;
    rdfs:label "{total, net, ac, elec, active, energy, sensor, point}" .

_:0b2cb027-c709-d695-0d2e-f23c91a70cca a phIoT:point ;
    ph:hasTag phScience:total,
        phIoT:reactive,
        phIoT:ac,
        phScience:elec,
        phScience:power,
        phIoT:sensor,
        phIoT:point ;
    rdfs:label "{total, reactive, ac, elec, power, sensor, point}" .

phIoT:ac-evse-port a owl:Class ;
    rdfs:subClassOf phIoT:evse-port ;
    rdfs:label "ac-evse-port" ;
    ph:children _:0b2cb027-c81c-7f00-0d2f-f23c91a70cca,
        _:0b2cb027-c81c-7f01-0d30-f23c91a70cca,
        _:0b2cb027-c81c-7f02-0d31-f23c91a70cca,
        _:0b2cb027-c81c-7f03-0d32-f23c91a70cca,
        _:0b2cb027-c81c-7f04-0d33-f23c91a70cca,
        _:0b2cb027-c81c-7f05-0d34-f23c91a70cca,
        _:0b2cb027-c81c-7f06-0d35-f23c91a70cca,
        _:0b2cb027-c81c-7f07-0d36-f23c91a70cca,
        _:0b2cb027-c81c-7f08-0d37-f23c91a70cca,
        _:0b2cb027-c81c-7f09-0d38-f23c91a70cca,
        _:0b2cb027-c81c-7f0a-0d39-f23c91a70cca,
        _:0b2cb027-c81c-7f0b-0d3a-f23c91a70cca ;
    rdfs:comment "An AC EVSE port delivers `ac` electricity to a single EV charging inlet\nat a time.  See `docHaystack::EVSE#port` chapter.\n\nTypically a max current or max power setpoint should reference an AC\nEVSE port, but not both.  Usually it is preferred to control an AC EVSE\nport using a max current setpoint.\n\nIt is recommended to include electrical location related tags on\nelectrical points that reference an AC EVSE port.  See\n`docHaystack::Meters#elecMeters` chapter for more details." ;
    ph:is phIoT:evse-port ;
    ph:lib phIoT:lib:phIoT ;
    ph:wikipedia "https://en.wikipedia.org/wiki/Charging_station"^^xsd:anyURI .

_:0b2cb027-c81c-7f00-0d2f-f23c91a70cca a phIoT:point ;
    ph:hasTag phIoT:dc,
        phScience:elec,
        phIoT:stateOfCharge,
        phIoT:sensor,
        phIoT:point ;
    rdfs:label "{dc, elec, stateOfCharge, sensor, point}" .

_:0b2cb027-c81c-7f01-0d30-f23c91a70cca a phIoT:equip ;
    ph:hasTag phIoT:equip ;
    rdfs:label "{equip}" .

_:0b2cb027-c81c-7f02-0d31-f23c91a70cca a phIoT:cable,
        phIoT:evse-cable ;
    ph:hasTag phIoT:evse,
        phIoT:cable,
        phIoT:equip ;
    rdfs:label "{evse, cable, equip}" .

_:0b2cb027-c81c-7f03-0d32-f23c91a70cca a phIoT:point ;
    ph:hasTag phIoT:evse,
        phIoT:evseStatus,
        phIoT:sensor,
        phIoT:point ;
    rdfs:label "{evse, evseStatus, sensor, point}" .

_:0b2cb027-c81c-7f04-0d33-f23c91a70cca a phIoT:point ;
    ph:hasTag phIoT:import,
        phIoT:ac,
        phScience:elec,
        phIoT:active,
        phScience:energy,
        phIoT:hisTotalized,
        phIoT:sensor,
        phIoT:point ;
    rdfs:label "{import, ac, elec, active, energy, hisTotalized, sensor, point}" .

_:0b2cb027-c81c-7f05-0d34-f23c91a70cca a phIoT:point ;
    ph:hasTag phIoT:import,
        phIoT:ac,
        phScience:elec,
        phIoT:active,
        phScience:power,
        ph:max,
        phIoT:sp,
        phIoT:point ;
    rdfs:label "{import, ac, elec, active, power, max, sp, point}" .

_:0b2cb027-c81c-7f06-0d35-f23c91a70cca a phIoT:point ;
    ph:hasTag phIoT:import,
        phIoT:ac,
        phScience:elec,
        phIoT:active,
        phScience:power,
        phIoT:sensor,
        phIoT:point ;
    rdfs:label "{import, ac, elec, active, power, sensor, point}" .

_:0b2cb027-c81c-7f07-0d36-f23c91a70cca a phIoT:point ;
    ph:hasTag phIoT:import,
        phIoT:ac,
        phScience:elec,
        phScience:magnitude,
        phScience:current,
        ph:max,
        phIoT:sp,
        phIoT:point ;
    rdfs:label "{import, ac, elec, magnitude, current, max, sp, point}" .

_:0b2cb027-c81c-7f08-0d37-f23c91a70cca a phIoT:point ;
    ph:hasTag phIoT:import,
        phIoT:ac,
        phScience:elec,
        phScience:magnitude,
        phScience:current,
        phIoT:sensor,
        phIoT:point ;
    rdfs:label "{import, ac, elec, magnitude, current, sensor, point}" .

_:0b2cb027-c81c-7f09-0d38-f23c91a70cca a phIoT:point ;
    ph:hasTag phIoT:import,
        phIoT:ac,
        phScience:elec,
        phScience:magnitude,
        phScience:volt,
        phIoT:sensor,
        phIoT:point ;
    rdfs:label "{import, ac, elec, magnitude, volt, sensor, point}" .

_:0b2cb027-c81c-7f0a-0d39-f23c91a70cca a phIoT:point ;
    ph:hasTag phIoT:import,
        phIoT:ac,
        phScience:elec,
        phIoT:pfScope,
        phIoT:pf,
        phIoT:sensor,
        phIoT:point ;
    rdfs:label "{import, ac, elec, pfScope, pf, sensor, point}" .

_:0b2cb027-c81c-7f0b-0d3a-f23c91a70cca a phIoT:point ;
    ph:hasTag phIoT:point ;
    rdfs:label "{point}" .

phIoT:ac-freq a owl:Class ;
    rdfs:subClassOf phScience:freq ;
    rdfs:label "ac-freq" ;
    rdfs:comment "Frequency of an alternating current waveform" ;
    ph:is phScience:freq ;
    ph:lib phIoT:lib:phIoT ;
    phScience:prefUnit "Hz" ;
    phScience:quantityOf phIoT:ac-elec .

ph:accumulate a owl:Class ;
    rdfs:subClassOf ph:marker ;
    rdfs:label "accumulate" ;
    rdfs:comment "Accumulate the tag's value during [inheritance]`docHaystack::Normalization#inherit`\nand [defx]`docHaystack::Normalization#defx`.  Tags marked as accumulate\nare aggregated together during normalization and deduplicated.  This\nmarker must only be used on tags which expect a list value." ;
    ph:is ph:marker ;
    ph:lib ph:lib:ph .

phIoT:active a owl:Class ;
    rdfs:subClassOf ph:marker ;
    rdfs:label "active" ;
    rdfs:comment "Working, operative, effective" ;
    ph:is ph:marker ;
    ph:lib phIoT:lib:phIoT .

phIoT:active-energy a owl:Class ;
    rdfs:subClassOf phScience:elec-energy ;
    rdfs:label "active-energy" ;
    rdfs:comment "Active energy in an AC eletrical power system. Integral of\n`active-power` over time." ;
    ph:is phScience:elec-energy ;
    ph:lib phIoT:lib:phIoT ;
    phScience:prefUnit "kWh" ;
    phScience:quantityOf phIoT:ac-elec ;
    ph:wikipedia "https://en.wikipedia.org/wiki/Electrical_energy"^^xsd:anyURI .

phIoT:active-power a owl:Class ;
    rdfs:subClassOf phScience:elec-power ;
    rdfs:label "active-power" ;
    rdfs:comment "Active power or real power; represents energy transfer that contributes\nuseful work." ;
    ph:is phScience:elec-power ;
    ph:lib phIoT:lib:phIoT ;
    phScience:prefUnit "kW" ;
    phScience:quantityOf phIoT:ac-elec ;
    ph:wikipedia "https://en.wikipedia.org/wiki/Electric_power"^^xsd:anyURI .

phIoT:actuator a owl:Class ;
    rdfs:subClassOf phIoT:equip,
        phIoT:elec-input ;
    rdfs:label "actuator" ;
    ph:children _:0b2cb027-c8a5-d340-0d3b-f23c91a70cca,
        _:0b2cb027-c8a5-d341-0d3c-f23c91a70cca ;
    rdfs:comment "Equipment to move or control a mechanism.  Actuators may be manually\noperated or automated via a control system to convert an energy source\ninto mechanical energy.  Typically the energy source is electricity,\nhydraulics, or pneumatics." ;
    ph:is phIoT:equip,
        phIoT:elec-input ;
    ph:lib phIoT:lib:phIoT ;
    ph:wikipedia "https://en.wikipedia.org/wiki/Actuator"^^xsd:anyURI .

_:0b2cb027-c8a5-d340-0d3b-f23c91a70cca a phIoT:equip ;
    ph:hasTag phIoT:equip ;
    rdfs:label "{equip}" .

_:0b2cb027-c8a5-d341-0d3c-f23c91a70cca a phIoT:point ;
    ph:hasTag phIoT:point ;
    rdfs:label "{point}" .

phIoT:ahu a owl:Class ;
    rdfs:subClassOf phIoT:airHandlingEquip ;
    rdfs:label "ahu" ;
    ph:children _:0b2cb027-c8a5-d342-0d3d-f23c91a70cca,
        _:0b2cb027-c8a5-d343-0d3e-f23c91a70cca,
        _:0b2cb027-c8a5-d344-0d3f-f23c91a70cca,
        _:0b2cb027-c8a5-d345-0d40-f23c91a70cca,
        _:0b2cb027-c8a5-d346-0d41-f23c91a70cca,
        _:0b2cb027-c8a5-d347-0d42-f23c91a70cca,
        _:0b2cb027-c8a5-d348-0d43-f23c91a70cca,
        _:0b2cb027-c8a5-d349-0d44-f23c91a70cca,
        _:0b2cb027-c8a5-d34a-0d45-f23c91a70cca,
        _:0b2cb027-c8a5-d34b-0d46-f23c91a70cca,
        _:0b2cb027-c8a5-d34c-0d47-f23c91a70cca,
        _:0b2cb027-c8a5-d34d-0d48-f23c91a70cca,
        _:0b2cb027-c8a5-d34e-0d49-f23c91a70cca,
        _:0b2cb027-c8b5-1580-0d4a-f23c91a70cca,
        _:0b2cb027-c8b5-1581-0d4b-f23c91a70cca,
        _:0b2cb027-c8b5-1582-0d4c-f23c91a70cca,
        _:0b2cb027-c8b5-1583-0d4d-f23c91a70cca,
        _:0b2cb027-c8b5-1584-0d4e-f23c91a70cca,
        _:0b2cb027-c8b5-1585-0d4f-f23c91a70cca,
        _:0b2cb027-c8b5-1586-0d50-f23c91a70cca,
        _:0b2cb027-c8b5-1587-0d51-f23c91a70cca ;
    rdfs:comment "Air Handling Unit: An enclosure with a fan that delivers air to a space\nvia ductwork and performs one or more of the functions of cleaning,\nheating, cooling, humidifying, dehumidifying, ventilating or circulating\nthe air.  See `docHaystack::AHUs` chapter." ;
    ph:is phIoT:airHandlingEquip ;
    ph:lib phIoT:lib:phIoT ;
    ph:mandatory ph:marker ;
    ph:wikipedia "https://en.wikipedia.org/wiki/Air_handler"^^xsd:anyURI .

_:0b2cb027-c8a5-d342-0d3d-f23c91a70cca a phIoT:point ;
    ph:hasTag phIoT:bypass,
        phIoT:damper,
        phIoT:cmd,
        phIoT:point ;
    rdfs:label "{bypass, damper, cmd, point}" .

_:0b2cb027-c8a5-d343-0d3e-f23c91a70cca a phIoT:point ;
    ph:hasTag phIoT:cool,
        phIoT:cmd,
        phIoT:point ;
    rdfs:label "{cool, cmd, point}" .

_:0b2cb027-c8a5-d344-0d3f-f23c91a70cca a phIoT:point ;
    ph:hasTag phIoT:dessicantDehumidifier,
        phIoT:cmd,
        phIoT:point ;
    rdfs:label "{dessicantDehumidifier, cmd, point}" .

_:0b2cb027-c8a5-d345-0d40-f23c91a70cca a phIoT:duct ;
    ph:hasTag phIoT:discharge,
        phIoT:duct,
        phIoT:equip ;
    rdfs:label "{discharge, duct, equip}" .

_:0b2cb027-c8a5-d346-0d41-f23c91a70cca a phIoT:duct ;
    ph:hasTag phIoT:economizer,
        phIoT:duct,
        phIoT:equip ;
    rdfs:label "{economizer, duct, equip}" .

_:0b2cb027-c8a5-d347-0d42-f23c91a70cca a phIoT:point ;
    ph:hasTag phIoT:economizing,
        phIoT:cmd,
        phIoT:point ;
    rdfs:label "{economizing, cmd, point}" .

_:0b2cb027-c8a5-d348-0d43-f23c91a70cca a phIoT:equip ;
    ph:hasTag phIoT:equip ;
    rdfs:label "{equip}" .

_:0b2cb027-c8a5-d349-0d44-f23c91a70cca a phIoT:duct ;
    ph:hasTag phIoT:exhaust,
        phIoT:duct,
        phIoT:equip ;
    rdfs:label "{exhaust, duct, equip}" .

_:0b2cb027-c8a5-d34a-0d45-f23c91a70cca a phIoT:point ;
    ph:hasTag phIoT:faceBypass,
        phIoT:cmd,
        phIoT:point ;
    rdfs:label "{faceBypass, cmd, point}" .

_:0b2cb027-c8a5-d34b-0d46-f23c91a70cca a phIoT:point ;
    ph:hasTag phIoT:filter,
        phIoT:sensor,
        phIoT:point ;
    rdfs:label "{filter, sensor, point}" .

_:0b2cb027-c8a5-d34c-0d47-f23c91a70cca a phIoT:point ;
    ph:hasTag phIoT:freezeStat,
        phIoT:sensor,
        phIoT:point ;
    rdfs:label "{freezeStat, sensor, point}" .

_:0b2cb027-c8a5-d34d-0d48-f23c91a70cca a phIoT:point ;
    ph:hasTag phIoT:heat,
        phIoT:cmd,
        phIoT:point ;
    rdfs:label "{heat, cmd, point}" .

_:0b2cb027-c8a5-d34e-0d49-f23c91a70cca a phIoT:point ;
    ph:hasTag phIoT:heatWheel,
        phIoT:cmd,
        phIoT:point ;
    rdfs:label "{heatWheel, cmd, point}" .

_:0b2cb027-c8b5-1580-0d4a-f23c91a70cca a phIoT:humidifier-equip ;
    ph:hasTag phIoT:humidifier,
        phIoT:equip ;
    rdfs:label "{humidifier, equip}" .

_:0b2cb027-c8b5-1581-0d4b-f23c91a70cca a phIoT:point ;
    ph:hasTag phIoT:hvacMode,
        phIoT:sp,
        phIoT:point ;
    rdfs:label "{hvacMode, sp, point}" .

_:0b2cb027-c8b5-1582-0d4c-f23c91a70cca a phIoT:duct ;
    ph:hasTag phIoT:mixed,
        phIoT:duct,
        phIoT:equip ;
    rdfs:label "{mixed, duct, equip}" .

_:0b2cb027-c8b5-1583-0d4d-f23c91a70cca a phIoT:duct ;
    ph:hasTag phIoT:outside,
        phIoT:duct,
        phIoT:equip ;
    rdfs:label "{outside, duct, equip}" .

_:0b2cb027-c8b5-1584-0d4e-f23c91a70cca a phIoT:point ;
    ph:hasTag phIoT:point ;
    rdfs:label "{point}" .

_:0b2cb027-c8b5-1585-0d4f-f23c91a70cca a phIoT:duct ;
    ph:hasTag phIoT:return,
        phIoT:duct,
        phIoT:equip ;
    rdfs:label "{return, duct, equip}" .

_:0b2cb027-c8b5-1586-0d50-f23c91a70cca a phIoT:thermostat ;
    ph:hasTag phIoT:thermostat,
        phIoT:equip ;
    rdfs:label "{thermostat, equip}" .

_:0b2cb027-c8b5-1587-0d51-f23c91a70cca a phIoT:duct ;
    ph:hasTag phIoT:ventilation,
        phIoT:duct,
        phIoT:equip ;
    rdfs:label "{ventilation, duct, equip}" .

phIoT:ahuZoneDelivery a owl:Class ;
    rdfs:subClassOf ph:choice ;
    rdfs:label "ahuZoneDelivery" ;
    rdfs:comment "AHU delivery method of conditioned air to the zone" ;
    ph:is ph:choice ;
    ph:lib phIoT:lib:phIoT ;
    ph:tagOn phIoT:airHandlingEquip .

phScience:air a owl:Class ;
    rdfs:subClassOf phScience:gas ;
    rdfs:label "air" ;
    rdfs:comment "The mixture of gases which surrounds the earth" ;
    ph:is phScience:gas ;
    ph:lib phScience:lib:phScience ;
    ph:wikipedia "https://en.wikipedia.org/wiki/Atmosphere_of_Earth"^^xsd:anyURI .

phIoT:air-conditioning-system a owl:Class ;
    rdfs:subClassOf phIoT:air-system ;
    rdfs:label "air-conditioning-system" ;
    ph:children _:0b2cb027-c92f-2780-0d52-f23c91a70cca,
        _:0b2cb027-c92f-2781-0d53-f23c91a70cca ;
    rdfs:comment "System for air treatment to control its temperature, humidity, cleanliness,\nand distribution to meet the requirements of a conditioned space." ;
    ph:is phIoT:air-system ;
    ph:lib phIoT:lib:phIoT .

_:0b2cb027-c92f-2780-0d52-f23c91a70cca a phIoT:equip ;
    ph:hasTag phIoT:equip ;
    rdfs:label "{equip}" .

_:0b2cb027-c92f-2781-0d53-f23c91a70cca a phIoT:point ;
    ph:hasTag phIoT:point ;
    rdfs:label "{point}" .

phIoT:air-exhaust-system a owl:Class ;
    rdfs:subClassOf phIoT:air-system ;
    rdfs:label "air-exhaust-system" ;
    ph:children _:0b2cb027-c92f-2782-0d54-f23c91a70cca,
        _:0b2cb027-c92f-2783-0d55-f23c91a70cca ;
    rdfs:comment "System consisting of one or more fans that remove air from the building.\nExhaust systems allow outdoor air to enter by ventilation inlets or normal\nleakage paths sthrough the building envelope." ;
    ph:is phIoT:air-system ;
    ph:lib phIoT:lib:phIoT .

_:0b2cb027-c92f-2782-0d54-f23c91a70cca a phIoT:equip ;
    ph:hasTag phIoT:equip ;
    rdfs:label "{equip}" .

_:0b2cb027-c92f-2783-0d55-f23c91a70cca a phIoT:point ;
    ph:hasTag phIoT:point ;
    rdfs:label "{point}" .

phIoT:air-input a owl:Class ;
    rdfs:subClassOf ph:input ;
    rdfs:label "air-input" ;
    rdfs:comment "Entity inputs air which flows from another entity" ;
    ph:is ph:input ;
    ph:lib phIoT:lib:phIoT .

phIoT:air-output a owl:Class ;
    rdfs:subClassOf ph:output ;
    rdfs:label "air-output" ;
    rdfs:comment "Entity outputs air to other entities" ;
    ph:is ph:output ;
    ph:lib phIoT:lib:phIoT .

phIoT:air-system a owl:Class ;
    rdfs:subClassOf phIoT:system ;
    rdfs:label "air-system" ;
    ph:children _:0b2cb027-c92f-2784-0d56-f23c91a70cca,
        _:0b2cb027-c92f-2785-0d57-f23c91a70cca ;
    rdfs:comment "System for moving air to maintain indoor thermal comfort and/or air quality." ;
    ph:is phIoT:system ;
    ph:lib phIoT:lib:phIoT .

_:0b2cb027-c92f-2784-0d56-f23c91a70cca a phIoT:equip ;
    ph:hasTag phIoT:equip ;
    rdfs:label "{equip}" .

_:0b2cb027-c92f-2785-0d57-f23c91a70cca a phIoT:point ;
    ph:hasTag phIoT:point ;
    rdfs:label "{point}" .

phScience:air-temp a owl:Class ;
    rdfs:subClassOf phScience:temp ;
    rdfs:label "air-temp" ;
    rdfs:comment "Dry bulb temperature" ;
    ph:is phScience:temp ;
    ph:lib phScience:lib:phScience ;
    phScience:prefUnit "\u00b0C",
        "\u00b0F" ;
    phScience:quantityOf phScience:air ;
    ph:wikipedia "https://en.wikipedia.org/wiki/Temperature"^^xsd:anyURI .

phScience:air-velocity a owl:Class ;
    rdfs:subClassOf phScience:quantity ;
    rdfs:label "air-velocity" ;
    rdfs:comment "Rate of air movement as distance over time" ;
    ph:is phScience:quantity ;
    ph:lib phScience:lib:phScience ;
    phScience:prefUnit "m/sec",
        "ft/min" ;
    phScience:quantityOf phScience:air .

phIoT:air-ventilation-system a owl:Class ;
    rdfs:subClassOf phIoT:air-system ;
    rdfs:label "air-ventilation-system" ;
    ph:children _:0b2cb027-c93e-69c0-0d58-f23c91a70cca,
        _:0b2cb027-c93e-69c1-0d59-f23c91a70cca ;
    rdfs:comment "System that supplies or removes air by natural or mechanical means to or\nfrom any space in order to provide outdoor air to the space. Such air may or\nmay not have been conditioned." ;
    ph:is phIoT:air-system ;
    ph:lib phIoT:lib:phIoT .

_:0b2cb027-c93e-69c0-0d58-f23c91a70cca a phIoT:equip ;
    ph:hasTag phIoT:equip ;
    rdfs:label "{equip}" .

_:0b2cb027-c93e-69c1-0d59-f23c91a70cca a phIoT:point ;
    ph:hasTag phIoT:point ;
    rdfs:label "{point}" .

phIoT:airCooling a owl:Class ;
    rdfs:subClassOf phIoT:coolingProcess,
        phIoT:air-input ;
    rdfs:label "airCooling" ;
    rdfs:comment "Cooling by dissipating heat into the surrounding air" ;
    ph:is phIoT:coolingProcess,
        phIoT:air-input ;
    ph:lib phIoT:lib:phIoT ;
    ph:wikipedia "https://en.wikipedia.org/wiki/Air_cooling"^^xsd:anyURI .

phIoT:airHandlingEquip a owl:Class ;
    rdfs:subClassOf phIoT:equip,
        phIoT:air-output,
        phIoT:elec-input ;
    rdfs:label "airHandlingEquip" ;
    ph:children _:0b2cb027-c93e-69c2-0d5a-f23c91a70cca,
        _:0b2cb027-c93e-69c3-0d5b-f23c91a70cca,
        _:0b2cb027-c93e-69c4-0d5c-f23c91a70cca,
        _:0b2cb027-c93e-69c5-0d5d-f23c91a70cca,
        _:0b2cb027-c93e-69c6-0d5e-f23c91a70cca,
        _:0b2cb027-c93e-69c7-0d5f-f23c91a70cca,
        _:0b2cb027-c93e-69c8-0d60-f23c91a70cca,
        _:0b2cb027-c93e-69c9-0d61-f23c91a70cca,
        _:0b2cb027-c93e-69ca-0d62-f23c91a70cca,
        _:0b2cb027-c93e-69cb-0d63-f23c91a70cca,
        _:0b2cb027-c93e-69cc-0d64-f23c91a70cca,
        _:0b2cb027-c93e-69cd-0d65-f23c91a70cca,
        _:0b2cb027-c93e-69ce-0d66-f23c91a70cca,
        _:0b2cb027-c93e-69cf-0d67-f23c91a70cca,
        _:0b2cb027-c93e-69d0-0d68-f23c91a70cca,
        _:0b2cb027-c93e-69d1-0d69-f23c91a70cca,
        _:0b2cb027-c93e-69d2-0d6a-f23c91a70cca,
        _:0b2cb027-c93e-69d3-0d6b-f23c91a70cca,
        _:0b2cb027-c93e-69d4-0d6c-f23c91a70cca,
        _:0b2cb027-c93e-69d5-0d6d-f23c91a70cca,
        _:0b2cb027-c93e-69d6-0d6e-f23c91a70cca ;
    rdfs:comment "HVAC equipment that conditions and delivers air via one or more fans.\nConditioning of air includes heating, cooling, humidification,\ndehumidification, and ventilation. See `docHaystack::AHUs` chapter." ;
    ph:is phIoT:equip,
        phIoT:air-output,
        phIoT:elec-input ;
    ph:lib phIoT:lib:phIoT ;
    ph:wikipedia "https://en.wikipedia.org/wiki/Air_handler"^^xsd:anyURI .

_:0b2cb027-c93e-69c2-0d5a-f23c91a70cca a phIoT:point ;
    ph:hasTag phIoT:bypass,
        phIoT:damper,
        phIoT:cmd,
        phIoT:point ;
    rdfs:label "{bypass, damper, cmd, point}" .

_:0b2cb027-c93e-69c3-0d5b-f23c91a70cca a phIoT:point ;
    ph:hasTag phIoT:cool,
        phIoT:cmd,
        phIoT:point ;
    rdfs:label "{cool, cmd, point}" .

_:0b2cb027-c93e-69c4-0d5c-f23c91a70cca a phIoT:point ;
    ph:hasTag phIoT:dessicantDehumidifier,
        phIoT:cmd,
        phIoT:point ;
    rdfs:label "{dessicantDehumidifier, cmd, point}" .

_:0b2cb027-c93e-69c5-0d5d-f23c91a70cca a phIoT:duct ;
    ph:hasTag phIoT:discharge,
        phIoT:duct,
        phIoT:equip ;
    rdfs:label "{discharge, duct, equip}" .

_:0b2cb027-c93e-69c6-0d5e-f23c91a70cca a phIoT:duct ;
    ph:hasTag phIoT:economizer,
        phIoT:duct,
        phIoT:equip ;
    rdfs:label "{economizer, duct, equip}" .

_:0b2cb027-c93e-69c7-0d5f-f23c91a70cca a phIoT:point ;
    ph:hasTag phIoT:economizing,
        phIoT:cmd,
        phIoT:point ;
    rdfs:label "{economizing, cmd, point}" .

_:0b2cb027-c93e-69c8-0d60-f23c91a70cca a phIoT:equip ;
    ph:hasTag phIoT:equip ;
    rdfs:label "{equip}" .

_:0b2cb027-c93e-69c9-0d61-f23c91a70cca a phIoT:duct ;
    ph:hasTag phIoT:exhaust,
        phIoT:duct,
        phIoT:equip ;
    rdfs:label "{exhaust, duct, equip}" .

_:0b2cb027-c93e-69ca-0d62-f23c91a70cca a phIoT:point ;
    ph:hasTag phIoT:faceBypass,
        phIoT:cmd,
        phIoT:point ;
    rdfs:label "{faceBypass, cmd, point}" .

_:0b2cb027-c93e-69cb-0d63-f23c91a70cca a phIoT:point ;
    ph:hasTag phIoT:filter,
        phIoT:sensor,
        phIoT:point ;
    rdfs:label "{filter, sensor, point}" .

_:0b2cb027-c93e-69cc-0d64-f23c91a70cca a phIoT:point ;
    ph:hasTag phIoT:freezeStat,
        phIoT:sensor,
        phIoT:point ;
    rdfs:label "{freezeStat, sensor, point}" .

_:0b2cb027-c93e-69cd-0d65-f23c91a70cca a phIoT:point ;
    ph:hasTag phIoT:heat,
        phIoT:cmd,
        phIoT:point ;
    rdfs:label "{heat, cmd, point}" .

_:0b2cb027-c93e-69ce-0d66-f23c91a70cca a phIoT:point ;
    ph:hasTag phIoT:heatWheel,
        phIoT:cmd,
        phIoT:point ;
    rdfs:label "{heatWheel, cmd, point}" .

_:0b2cb027-c93e-69cf-0d67-f23c91a70cca a phIoT:humidifier-equip ;
    ph:hasTag phIoT:humidifier,
        phIoT:equip ;
    rdfs:label "{humidifier, equip}" .

_:0b2cb027-c93e-69d0-0d68-f23c91a70cca a phIoT:point ;
    ph:hasTag phIoT:hvacMode,
        phIoT:sp,
        phIoT:point ;
    rdfs:label "{hvacMode, sp, point}" .

_:0b2cb027-c93e-69d1-0d69-f23c91a70cca a phIoT:duct ;
    ph:hasTag phIoT:mixed,
        phIoT:duct,
        phIoT:equip ;
    rdfs:label "{mixed, duct, equip}" .

_:0b2cb027-c93e-69d2-0d6a-f23c91a70cca a phIoT:duct ;
    ph:hasTag phIoT:outside,
        phIoT:duct,
        phIoT:equip ;
    rdfs:label "{outside, duct, equip}" .

_:0b2cb027-c93e-69d3-0d6b-f23c91a70cca a phIoT:point ;
    ph:hasTag phIoT:point ;
    rdfs:label "{point}" .

_:0b2cb027-c93e-69d4-0d6c-f23c91a70cca a phIoT:duct ;
    ph:hasTag phIoT:return,
        phIoT:duct,
        phIoT:equip ;
    rdfs:label "{return, duct, equip}" .

_:0b2cb027-c93e-69d5-0d6d-f23c91a70cca a phIoT:thermostat ;
    ph:hasTag phIoT:thermostat,
        phIoT:equip ;
    rdfs:label "{thermostat, equip}" .

_:0b2cb027-c93e-69d6-0d6e-f23c91a70cca a phIoT:duct ;
    ph:hasTag phIoT:ventilation,
        phIoT:duct,
        phIoT:equip ;
    rdfs:label "{ventilation, duct, equip}" .

phScience:airQuality a owl:Class ;
    rdfs:subClassOf phScience:concentration ;
    rdfs:label "airQuality" ;
    rdfs:comment "Concentration of contaminants in the air" ;
    ph:is phScience:concentration ;
    ph:lib phScience:lib:phScience ;
    phScience:quantityOf phScience:air ;
    ph:wikipedia "https://en.wikipedia.org/wiki/Concentration"^^xsd:anyURI .

phIoT:airQualityZonePoints a owl:Class ;
    rdfs:subClassOf phIoT:pointGroup ;
    rdfs:label "airQualityZonePoints" ;
    ph:children _:0b2cb027-c94d-ac00-0d6f-f23c91a70cca,
        _:0b2cb027-c94d-ac01-0d70-f23c91a70cca,
        _:0b2cb027-c94d-ac02-0d71-f23c91a70cca,
        _:0b2cb027-c94d-ac03-0d72-f23c91a70cca,
        _:0b2cb027-c94d-ac04-0d73-f23c91a70cca,
        _:0b2cb027-c94d-ac05-0d74-f23c91a70cca,
        _:0b2cb027-c94d-ac06-0d75-f23c91a70cca,
        _:0b2cb027-c94d-ac07-0d76-f23c91a70cca,
        _:0b2cb027-c94d-ac08-0d77-f23c91a70cca,
        _:0b2cb027-c94d-ac09-0d78-f23c91a70cca,
        _:0b2cb027-c94d-ac0a-0d79-f23c91a70cca ;
    rdfs:comment "Entity with logical grouping of zone air quality points.\nSee `docHaystack::Zones#airQuality` chapter." ;
    ph:is phIoT:pointGroup ;
    ph:lib phIoT:lib:phIoT .

_:0b2cb027-c94d-ac00-0d6f-f23c91a70cca a phIoT:point ;
    ph:hasTag phIoT:zone,
        phScience:air,
        phScience:ch2o,
        phScience:concentration,
        phIoT:sensor,
        phIoT:point ;
    rdfs:label "{zone, air, ch2o, concentration, sensor, point}" .

_:0b2cb027-c94d-ac01-0d70-f23c91a70cca a phIoT:point ;
    ph:hasTag phIoT:zone,
        phScience:air,
        phScience:co,
        phScience:concentration,
        phIoT:sensor,
        phIoT:point ;
    rdfs:label "{zone, air, co, concentration, sensor, point}" .

_:0b2cb027-c94d-ac02-0d71-f23c91a70cca a phIoT:point ;
    ph:hasTag phIoT:zone,
        phScience:air,
        phScience:co2,
        phScience:concentration,
        phIoT:sensor,
        phIoT:point ;
    rdfs:label "{zone, air, co2, concentration, sensor, point}" .

_:0b2cb027-c94d-ac03-0d72-f23c91a70cca a phIoT:point ;
    ph:hasTag phIoT:zone,
        phScience:air,
        phScience:co2,
        phScience:concentration,
        phIoT:sp,
        phIoT:point ;
    rdfs:label "{zone, air, co2, concentration, sp, point}" .

_:0b2cb027-c94d-ac04-0d73-f23c91a70cca a phIoT:point ;
    ph:hasTag phIoT:zone,
        phScience:air,
        phScience:nh3,
        phScience:concentration,
        phIoT:sensor,
        phIoT:point ;
    rdfs:label "{zone, air, nh3, concentration, sensor, point}" .

_:0b2cb027-c94d-ac05-0d74-f23c91a70cca a phIoT:point ;
    ph:hasTag phIoT:zone,
        phScience:air,
        phScience:no2,
        phScience:concentration,
        phIoT:sensor,
        phIoT:point ;
    rdfs:label "{zone, air, no2, concentration, sensor, point}" .

_:0b2cb027-c94d-ac06-0d75-f23c91a70cca a phIoT:point ;
    ph:hasTag phIoT:zone,
        phScience:air,
        phScience:o3,
        phScience:concentration,
        phIoT:sensor,
        phIoT:point ;
    rdfs:label "{zone, air, o3, concentration, sensor, point}" .

_:0b2cb027-c94d-ac07-0d76-f23c91a70cca a phIoT:point ;
    ph:hasTag phIoT:zone,
        phScience:air,
        phScience:pm01,
        phScience:concentration,
        phIoT:sensor,
        phIoT:point ;
    rdfs:label "{zone, air, pm01, concentration, sensor, point}" .

_:0b2cb027-c94d-ac08-0d77-f23c91a70cca a phIoT:point ;
    ph:hasTag phIoT:zone,
        phScience:air,
        phScience:pm10,
        phScience:concentration,
        phIoT:sensor,
        phIoT:point ;
    rdfs:label "{zone, air, pm10, concentration, sensor, point}" .

_:0b2cb027-c94d-ac09-0d78-f23c91a70cca a phIoT:point ;
    ph:hasTag phIoT:zone,
        phScience:air,
        phScience:pm25,
        phScience:concentration,
        phIoT:sensor,
        phIoT:point ;
    rdfs:label "{zone, air, pm25, concentration, sensor, point}" .

_:0b2cb027-c94d-ac0a-0d79-f23c91a70cca a phIoT:point ;
    ph:hasTag phIoT:zone,
        phScience:air,
        phScience:tvoc,
        phScience:concentration,
        phIoT:sensor,
        phIoT:point ;
    rdfs:label "{zone, air, tvoc, concentration, sensor, point}" .

phIoT:airRef a owl:ObjectProperty ;
    rdfs:domain phIoT:air-input ;
    rdfs:range phIoT:air-output ;
    rdfs:label "airRef" ;
    rdfs:comment "Air flows from the referent to this entity" ;
    ph:inputs phScience:air ;
    ph:is ph:ref ;
    ph:lib phIoT:lib:phIoT ;
    ph:of phIoT:air-output ;
    ph:tagOn phIoT:air-input .

phIoT:airTerminalUnit a owl:Class ;
    rdfs:subClassOf phIoT:equip,
        phIoT:air-input,
        phIoT:air-output,
        phIoT:elec-input ;
    rdfs:label "airTerminalUnit" ;
    ph:children _:0b2cb027-c9c7-be00-0d7a-f23c91a70cca,
        _:0b2cb027-c9c7-be01-0d7b-f23c91a70cca,
        _:0b2cb027-c9c7-be02-0d7c-f23c91a70cca,
        _:0b2cb027-c9c7-be03-0d7d-f23c91a70cca,
        _:0b2cb027-c9c7-be04-0d7e-f23c91a70cca ;
    rdfs:comment "Equipment in air distribution systems which terminate at the space.\nTerminal units receive air from `airHandlingEquip` which have the\nprimarily responsibility to condition air.  Terminal units are primarily\nresponsible for delivery of air to the space and tempering the temperature." ;
    ph:is phIoT:equip,
        phIoT:air-input,
        phIoT:air-output,
        phIoT:elec-input ;
    ph:lib phIoT:lib:phIoT .

_:0b2cb027-c9c7-be00-0d7a-f23c91a70cca a phIoT:duct ;
    ph:hasTag phIoT:discharge,
        phIoT:duct,
        phIoT:equip ;
    rdfs:label "{discharge, duct, equip}" .

_:0b2cb027-c9c7-be01-0d7b-f23c91a70cca a phIoT:equip ;
    ph:hasTag phIoT:equip ;
    rdfs:label "{equip}" .

_:0b2cb027-c9c7-be02-0d7c-f23c91a70cca a phIoT:duct ;
    ph:hasTag phIoT:inlet,
        phIoT:duct,
        phIoT:equip ;
    rdfs:label "{inlet, duct, equip}" .

_:0b2cb027-c9c7-be03-0d7d-f23c91a70cca a phIoT:point ;
    ph:hasTag phIoT:point ;
    rdfs:label "{point}" .

_:0b2cb027-c9c7-be04-0d7e-f23c91a70cca a phIoT:thermostat ;
    ph:hasTag phIoT:thermostat,
        phIoT:equip ;
    rdfs:label "{thermostat, equip}" .

phIoT:airVolumeAdjustability a owl:Class ;
    rdfs:subClassOf ph:choice ;
    rdfs:label "airVolumeAdjustability" ;
    rdfs:comment "Ability of air handling equip to adjust volume of air flow" ;
    ph:is ph:choice ;
    ph:lib phIoT:lib:phIoT ;
    ph:tagOn phIoT:airHandlingEquip .

phIoT:alarm a owl:Class ;
    rdfs:subClassOf ph:marker ;
    rdfs:label "alarm" ;
    rdfs:comment "Notification of a condition which requires attention" ;
    ph:is ph:marker ;
    ph:lib phIoT:lib:phIoT .

phScience:angle a owl:Class ;
    rdfs:subClassOf ph:marker ;
    rdfs:label "angle" ;
    rdfs:comment "Measurement of the relative difference in direction between two vectors or phasors" ;
    ph:is ph:marker ;
    ph:lib phScience:lib:phScience .

phScience:apparent a owl:Class ;
    rdfs:subClassOf ph:marker ;
    rdfs:label "apparent" ;
    rdfs:comment "Perceived quantity" ;
    ph:is ph:marker ;
    ph:lib phScience:lib:phScience .

phIoT:apparent-energy a owl:Class ;
    rdfs:subClassOf phScience:quantity ;
    rdfs:label "apparent-energy" ;
    rdfs:comment "Apparent energy in an AC eletrical power system. Integral of\n`apparent-power` over time." ;
    ph:is phScience:quantity ;
    ph:lib phIoT:lib:phIoT ;
    phScience:quantityOf phIoT:ac-elec .

phIoT:apparent-power a owl:Class ;
    rdfs:subClassOf phScience:quantity ;
    rdfs:label "apparent-power" ;
    rdfs:comment "Apparent power; the perceived magnitude of electric power transfer in an\nAC electric system due to the combination of active and reactive power." ;
    ph:is phScience:quantity ;
    ph:lib phIoT:lib:phIoT ;
    phScience:prefUnit "kVA" ;
    phScience:quantityOf phIoT:ac-elec .

phIoT:area a owl:DatatypeProperty ;
    rdfs:domain phIoT:site,
        phIoT:space ;
    rdfs:range ph:number ;
    rdfs:label "area" ;
    rdfs:comment "Area of a shape or floor space" ;
    ph:is ph:number ;
    ph:lib phIoT:lib:phIoT ;
    phScience:prefUnit "ft\u00b2",
        "m\u00b2" ;
    ph:tagOn phIoT:site,
        phIoT:space .

ph:association a owl:DatatypeProperty ;
    rdfs:range ph:list ;
    rdfs:label "association" ;
    rdfs:comment "Associations model ontological relationships between definitions.\nSee [Associations]`docHaystack::Associations` chapter." ;
    ph:docTaxonomy ph:marker ;
    ph:is ph:list ;
    ph:lib ph:lib:ph ;
    ph:of ph:symbol .

phIoT:ates a owl:Class ;
    rdfs:subClassOf phIoT:equip ;
    rdfs:label "ates" ;
    ph:children _:0b2cb027-c9d7-0040-0d7f-f23c91a70cca,
        _:0b2cb027-c9d7-0041-0d80-f23c91a70cca,
        _:0b2cb027-c9d7-0042-0d81-f23c91a70cca,
        _:0b2cb027-c9d7-0043-0d82-f23c91a70cca,
        _:0b2cb027-c9d7-0044-0d83-f23c91a70cca,
        _:0b2cb027-c9d7-0045-0d84-f23c91a70cca,
        _:0b2cb027-c9d7-0046-0d85-f23c91a70cca,
        _:0b2cb027-c9d7-0047-0d86-f23c91a70cca,
        _:0b2cb027-c9d7-0048-0d87-f23c91a70cca,
        _:0b2cb027-c9d7-0049-0d88-f23c91a70cca,
        _:0b2cb027-c9d7-004a-0d89-f23c91a70cca,
        _:0b2cb027-c9d7-004b-0d8a-f23c91a70cca,
        _:0b2cb027-c9d7-004c-0d8b-f23c91a70cca,
        _:0b2cb027-c9d7-004d-0d8c-f23c91a70cca,
        _:0b2cb027-c9d7-004e-0d8d-f23c91a70cca ;
    rdfs:comment "Aquifer Thermal Energy Storage system.\nSee `docHaystack::ATES` chapter." ;
    ph:is phIoT:equip ;
    ph:lib phIoT:lib:phIoT ;
    ph:wikipedia "https://en.wikipedia.org/wiki/Aquifer_thermal_energy_storage"^^xsd:anyURI .

_:0b2cb027-c9d7-0040-0d7f-f23c91a70cca a phIoT:flow-meter ;
    ph:hasTag phIoT:cool,
        phScience:water,
        phScience:flow,
        phIoT:thermal,
        phIoT:meter,
        phIoT:equip ;
    rdfs:label "{cool, water, flow, thermal, meter, equip}" .

_:0b2cb027-c9d7-0041-0d80-f23c91a70cca a phIoT:well ;
    ph:hasTag phIoT:cool,
        phIoT:well,
        phIoT:equip ;
    rdfs:label "{cool, well, equip}" .

_:0b2cb027-c9d7-0042-0d81-f23c91a70cca a phIoT:equip ;
    ph:hasTag phIoT:equip ;
    rdfs:label "{equip}" .

_:0b2cb027-c9d7-0043-0d82-f23c91a70cca a phIoT:well ;
    ph:hasTag phIoT:extraction,
        phIoT:well,
        phIoT:equip ;
    rdfs:label "{extraction, well, equip}" .

_:0b2cb027-c9d7-0044-0d83-f23c91a70cca a phIoT:flowInverter ;
    ph:hasTag phIoT:flowInverter,
        phIoT:equip ;
    rdfs:label "{flowInverter, equip}" .

_:0b2cb027-c9d7-0045-0d84-f23c91a70cca a phIoT:point ;
    ph:hasTag phIoT:ground,
        phScience:water,
        phScience:flow,
        phIoT:sensor,
        phIoT:point ;
    rdfs:label "{ground, water, flow, sensor, point}" .

_:0b2cb027-c9d7-0046-0d85-f23c91a70cca a phIoT:point ;
    ph:hasTag phIoT:ground,
        phScience:water,
        phScience:pressure,
        phIoT:sensor,
        phIoT:point ;
    rdfs:label "{ground, water, pressure, sensor, point}" .

_:0b2cb027-c9d7-0047-0d86-f23c91a70cca a phIoT:point ;
    ph:hasTag phIoT:ground,
        phScience:water,
        phScience:volume,
        phIoT:sensor,
        phIoT:point ;
    rdfs:label "{ground, water, volume, sensor, point}" .

_:0b2cb027-c9d7-0048-0d87-f23c91a70cca a phIoT:heatExchanger ;
    ph:hasTag phIoT:heatExchanger,
        phIoT:equip ;
    rdfs:label "{heatExchanger, equip}" .

_:0b2cb027-c9d7-0049-0d88-f23c91a70cca a phIoT:well ;
    ph:hasTag phIoT:infiltration,
        phIoT:well,
        phIoT:equip ;
    rdfs:label "{infiltration, well, equip}" .

_:0b2cb027-c9d7-004a-0d89-f23c91a70cca a phIoT:point ;
    ph:hasTag phIoT:point ;
    rdfs:label "{point}" .

_:0b2cb027-c9d7-004b-0d8a-f23c91a70cca a phIoT:point ;
    ph:hasTag phIoT:purge,
        phScience:water,
        phScience:flow,
        phIoT:sensor,
        phIoT:point ;
    rdfs:label "{purge, water, flow, sensor, point}" .

_:0b2cb027-c9d7-004c-0d8b-f23c91a70cca a phIoT:point ;
    ph:hasTag phIoT:purge,
        phScience:water,
        phScience:volume,
        phIoT:sensor,
        phIoT:point ;
    rdfs:label "{purge, water, volume, sensor, point}" .

_:0b2cb027-c9d7-004d-0d8c-f23c91a70cca a phIoT:flow-meter ;
    ph:hasTag phIoT:warm,
        phScience:water,
        phScience:flow,
        phIoT:thermal,
        phIoT:meter,
        phIoT:equip ;
    rdfs:label "{warm, water, flow, thermal, meter, equip}" .

_:0b2cb027-c9d7-004e-0d8d-f23c91a70cca a phIoT:well ;
    ph:hasTag phIoT:warm,
        phIoT:well,
        phIoT:equip ;
    rdfs:label "{warm, well, equip}" .

phIoT:atesClosedLoop a owl:Class ;
    rdfs:subClassOf phIoT:atesDesign ;
    rdfs:label "atesClosedLoop" ;
    rdfs:comment "The ATES uses closed piping to transport a water/glycol mixture\nthrough the ground. The system works like a heat exchanger; there\nis no ground water transported." ;
    ph:is phIoT:atesDesign ;
    ph:lib phIoT:lib:phIoT .

phIoT:atesDesign a owl:Class ;
    rdfs:subClassOf ph:choice ;
    rdfs:label "atesDesign" ;
    rdfs:comment "Design type of the ATES underground system." ;
    ph:is ph:choice ;
    ph:lib phIoT:lib:phIoT ;
    ph:tagOn phIoT:ates .

phIoT:atesDoublet a owl:Class ;
    rdfs:subClassOf phIoT:atesDesign ;
    rdfs:label "atesDoublet" ;
    rdfs:comment "The ATES has one or more pairs of a separate warm and cool well." ;
    ph:is phIoT:atesDesign ;
    ph:lib phIoT:lib:phIoT .

phIoT:atesDoubletPaired a owl:Class ;
    rdfs:subClassOf phIoT:atesDesign ;
    rdfs:label "atesDoubletPaired" ;
    rdfs:comment "The ATES is as a doublet, but with specific warm and cool wells linked together.\nThese linked wells do not exchange water with other wells." ;
    ph:is phIoT:atesDesign ;
    ph:lib phIoT:lib:phIoT .

phIoT:atesMono a owl:Class ;
    rdfs:subClassOf phIoT:atesDesign ;
    rdfs:label "atesMono" ;
    rdfs:comment "The ATES has only one physical well.  This well is deep enough\nto penetrate two layers of groundwater." ;
    ph:is phIoT:atesDesign ;
    ph:lib phIoT:lib:phIoT .

phIoT:atesUnidirectional a owl:Class ;
    rdfs:subClassOf phIoT:atesDesign ;
    rdfs:label "atesUnidirectional" ;
    rdfs:comment "Similar to a doublet, but water always flows in the same direction from\nthe extraction to the infiltration well." ;
    ph:is phIoT:atesDesign ;
    ph:lib phIoT:lib:phIoT .

phScience:atmospheric a owl:Class ;
    rdfs:subClassOf ph:marker ;
    rdfs:label "atmospheric" ;
    rdfs:comment "Related to the atmosphere of the earth" ;
    ph:is ph:marker ;
    ph:lib phScience:lib:phScience .

phScience:atmospheric-pressure a owl:Class ;
    rdfs:subClassOf phScience:pressure ;
    rdfs:label "atmospheric-pressure" ;
    rdfs:comment "Barometric pressure exerted by the weight of the atmosphere" ;
    ph:is phScience:pressure ;
    ph:lib phScience:lib:phScience ;
    phScience:prefUnit "millibar",
        "inHg" ;
    phScience:quantityOf phScience:weather ;
    ph:wikipedia "https://en.wikipedia.org/wiki/Pressure"^^xsd:anyURI .

phScience:avg a owl:Class ;
    rdfs:subClassOf ph:marker ;
    rdfs:label "avg" ;
    rdfs:comment "Average; central or typical value; median" ;
    ph:is ph:marker ;
    ph:lib phScience:lib:phScience .

phIct:bacnet a owl:Class ;
    rdfs:subClassOf phIct:protocol ;
    rdfs:label "bacnet" ;
    rdfs:comment "ASHRAE building automation and control protocol" ;
    ph:is phIct:protocol ;
    ph:lib phIct:lib:phIct ;
    ph:wikipedia "https://en.wikipedia.org/wiki/BACnet"^^xsd:anyURI .

phIoT:barometric a owl:Class ;
    rdfs:subClassOf ph:marker ;
    rdfs:label "barometric" ;
    rdfs:comment "Relating atmospheric pressure" ;
    ph:is ph:marker ;
    ph:lib phIoT:lib:phIoT .

ph:baseUri a owl:DatatypeProperty ;
    rdfs:domain ph:lib ;
    rdfs:range ph:uri ;
    rdfs:label "baseUri" ;
    rdfs:comment "Base URI for normalizing relative URIs" ;
    ph:is ph:uri ;
    ph:lib ph:lib:ph ;
    ph:tagOn ph:lib .

phIoT:battery a owl:Class ;
    rdfs:subClassOf phIoT:equip,
        phIoT:elec-output ;
    rdfs:label "battery" ;
    ph:children _:0b2cb027-c9e6-4280-0d8e-f23c91a70cca,
        _:0b2cb027-c9e6-4281-0d8f-f23c91a70cca ;
    rdfs:comment "Equipment used to store electric energy" ;
    ph:is phIoT:equip,
        phIoT:elec-output ;
    ph:lib phIoT:lib:phIoT ;
    ph:wikipedia "https://en.wikipedia.org/wiki/Electric_battery"^^xsd:anyURI .

_:0b2cb027-c9e6-4280-0d8e-f23c91a70cca a phIoT:equip ;
    ph:hasTag phIoT:equip ;
    rdfs:label "{equip}" .

_:0b2cb027-c9e6-4281-0d8f-f23c91a70cca a phIoT:point ;
    ph:hasTag phIoT:point ;
    rdfs:label "{point}" .

phIoT:biomass a owl:Class ;
    rdfs:subClassOf phScience:substance ;
    rdfs:label "biomass" ;
    rdfs:comment "Plant or animal material used as fuel to produce electricity or heat" ;
    ph:is phScience:substance ;
    ph:lib phIoT:lib:phIoT ;
    ph:wikipedia "https://en.wikipedia.org/wiki/Biomass"^^xsd:anyURI .

phIoT:biomassHeating a owl:Class ;
    rdfs:subClassOf phIoT:heatingProcess ;
    rdfs:label "biomassHeating" ;
    rdfs:comment "Heating by the combustion of biomass" ;
    ph:is phIoT:heatingProcess ;
    ph:lib phIoT:lib:phIoT .

phIoT:blowdown a owl:Class ;
    rdfs:subClassOf ph:marker ;
    rdfs:label "blowdown" ;
    rdfs:comment "Removal from container or pipe" ;
    ph:is ph:marker ;
    ph:lib phIoT:lib:phIoT .

phIoT:blowdown-water a owl:Class ;
    rdfs:subClassOf phScience:water ;
    rdfs:label "blowdown-water" ;
    rdfs:comment "Water expelled from a system to remove mineral build up" ;
    ph:is phScience:water ;
    ph:lib phIoT:lib:phIoT ;
    ph:wikipedia "https://en.wikipedia.org/wiki/Water"^^xsd:anyURI .

phIoT:blowdown-water-input a owl:Class ;
    rdfs:subClassOf ph:input ;
    rdfs:label "blowdown-water-input" ;
    rdfs:comment "Entity inputs blowdown water which flows from another entity" ;
    ph:is ph:input ;
    ph:lib phIoT:lib:phIoT .

phIoT:blowdown-water-output a owl:Class ;
    rdfs:subClassOf ph:output ;
    rdfs:label "blowdown-water-output" ;
    rdfs:comment "Entity outputs blowdown water to other entities" ;
    ph:is ph:output ;
    ph:lib phIoT:lib:phIoT .

phIoT:blowdownWaterRef a owl:ObjectProperty ;
    rdfs:domain phIoT:blowdown-water-input ;
    rdfs:range phIoT:blowdown-water-output ;
    rdfs:label "blowdownWaterRef" ;
    rdfs:comment "Blowdown water flows from the referent to this entity" ;
    ph:inputs phIoT:blowdown-water ;
    ph:is ph:ref ;
    ph:lib phIoT:lib:phIoT ;
    ph:of phIoT:blowdown-water-output ;
    ph:tagOn phIoT:blowdown-water-input .

phIct:bluetooth a owl:Class ;
    rdfs:subClassOf phIct:protocol ;
    rdfs:label "bluetooth" ;
    rdfs:comment "Short range wireless communication protocol" ;
    ph:is phIct:protocol ;
    ph:lib phIct:lib:phIct ;
    ph:wikipedia "https://en.wikipedia.org/wiki/Bluetooth"^^xsd:anyURI .

phIoT:boiler a owl:Class ;
    rdfs:subClassOf phIoT:equip,
        phIoT:elec-input ;
    rdfs:label "boiler" ;
    ph:children _:0b2cb027-d210-b6c0-0d90-f23c91a70cca,
        _:0b2cb027-d210-b6c1-0d91-f23c91a70cca,
        _:0b2cb027-d210-b6c2-0d92-f23c91a70cca ;
    rdfs:comment "Equipment to generate hot water or steam for heating" ;
    ph:is phIoT:equip,
        phIoT:elec-input ;
    ph:lib phIoT:lib:phIoT ;
    ph:wikipedia "https://en.wikipedia.org/wiki/Boiler"^^xsd:anyURI .

_:0b2cb027-d210-b6c0-0d90-f23c91a70cca a phIoT:point ;
    ph:hasTag phIoT:alarm,
        phIoT:sensor,
        phIoT:point ;
    rdfs:label "{alarm, sensor, point}" .

_:0b2cb027-d210-b6c1-0d91-f23c91a70cca a phIoT:equip ;
    ph:hasTag phIoT:equip ;
    rdfs:label "{equip}" .

_:0b2cb027-d210-b6c2-0d92-f23c91a70cca a phIoT:point ;
    ph:hasTag phIoT:point ;
    rdfs:label "{point}" .

ph:bool a owl:DatatypeProperty ;
    rdfs:subClassOf xsd:boolean ;
    rdfs:label "bool" ;
    rdfs:comment "Boolean value 'true' or 'false'.\nSee [Kinds chapter]`docHaystack::Kinds#bool`." ;
    ph:is ph:scalar ;
    ph:lib ph:lib:ph .

phIoT:branchSelector a owl:Class ;
    rdfs:subClassOf phIoT:vrf-equip,
        phIoT:refrig-input ;
    rdfs:label "branchSelector" ;
    ph:children _:0b2cb027-d21f-f900-0d93-f23c91a70cca,
        _:0b2cb027-d21f-f901-0d94-f23c91a70cca ;
    rdfs:comment "Branch selector used for heat recovery in a VRF system.  These are\ncontrol devices directing the liquid refrigerant or gas refrigerant\nto zones requiring cooling or heating. See `docHaystack::VRF#branchSelector`\nchapter." ;
    ph:is phIoT:vrf-equip,
        phIoT:refrig-input ;
    ph:lib phIoT:lib:phIoT .

_:0b2cb027-d21f-f900-0d93-f23c91a70cca a phIoT:equip ;
    ph:hasTag phIoT:equip ;
    rdfs:label "{equip}" .

_:0b2cb027-d21f-f901-0d94-f23c91a70cca a phIoT:point ;
    ph:hasTag phIoT:point ;
    rdfs:label "{point}" .

phIoT:bypass a owl:Class ;
    rdfs:subClassOf phIoT:pipeSection ;
    rdfs:label "bypass" ;
    rdfs:comment "Pipe used to bypass an equipment" ;
    ph:is phIoT:pipeSection ;
    ph:lib phIoT:lib:phIoT .

phIoT:cable a owl:Class ;
    rdfs:subClassOf phIoT:equip ;
    rdfs:label "cable" ;
    ph:children _:0b2cb027-d21f-f902-0d95-f23c91a70cca,
        _:0b2cb027-d21f-f903-0d96-f23c91a70cca ;
    rdfs:comment "An assembly of one or more insulated conductors." ;
    ph:is phIoT:equip ;
    ph:lib phIoT:lib:phIoT .

_:0b2cb027-d21f-f902-0d95-f23c91a70cca a phIoT:equip ;
    ph:hasTag phIoT:equip ;
    rdfs:label "{equip}" .

_:0b2cb027-d21f-f903-0d96-f23c91a70cca a phIoT:point ;
    ph:hasTag phIoT:point ;
    rdfs:label "{point}" .

phIoT:cav a owl:Class ;
    rdfs:subClassOf phIoT:airTerminalUnit ;
    rdfs:label "cav" ;
    ph:children _:0b2cb027-d21f-f904-0d97-f23c91a70cca,
        _:0b2cb027-d21f-f905-0d98-f23c91a70cca,
        _:0b2cb027-d21f-f906-0d99-f23c91a70cca,
        _:0b2cb027-d21f-f907-0d9a-f23c91a70cca,
        _:0b2cb027-d21f-f908-0d9b-f23c91a70cca ;
    rdfs:comment "Constant air volume terminal unit.  CAV systems use a constant\nair flow rate with a variable air temperature." ;
    ph:is phIoT:airTerminalUnit ;
    ph:lib phIoT:lib:phIoT ;
    ph:wikipedia "https://en.wikipedia.org/wiki/Constant_air_volume"^^xsd:anyURI .

_:0b2cb027-d21f-f904-0d97-f23c91a70cca a phIoT:duct ;
    ph:hasTag phIoT:discharge,
        phIoT:duct,
        phIoT:equip ;
    rdfs:label "{discharge, duct, equip}" .

_:0b2cb027-d21f-f905-0d98-f23c91a70cca a phIoT:equip ;
    ph:hasTag phIoT:equip ;
    rdfs:label "{equip}" .

_:0b2cb027-d21f-f906-0d99-f23c91a70cca a phIoT:duct ;
    ph:hasTag phIoT:inlet,
        phIoT:duct,
        phIoT:equip ;
    rdfs:label "{inlet, duct, equip}" .

_:0b2cb027-d21f-f907-0d9a-f23c91a70cca a phIoT:point ;
    ph:hasTag phIoT:point ;
    rdfs:label "{point}" .

_:0b2cb027-d21f-f908-0d9b-f23c91a70cca a phIoT:thermostat ;
    ph:hasTag phIoT:thermostat,
        phIoT:equip ;
    rdfs:label "{thermostat, equip}" .

phIoT:centrifugal a owl:Class ;
    rdfs:subClassOf ph:marker ;
    rdfs:label "centrifugal" ;
    rdfs:comment "Compression via a continuous flow of fluid through an impeller" ;
    ph:is ph:marker ;
    ph:lib phIoT:lib:phIoT ;
    ph:wikipedia "https://en.wikipedia.org/wiki/Centrifugal_compressor"^^xsd:anyURI .

phScience:ch2o a owl:Class ;
    rdfs:subClassOf phScience:gas ;
    rdfs:label "ch2o" ;
    rdfs:comment "Formaldehyde (CH\u2082O)" ;
    ph:is phScience:gas ;
    ph:lib phScience:lib:phScience ;
    ph:wikipedia "https://en.wikipedia.org/wiki/Formaldehyde"^^xsd:anyURI .

phScience:ch2o-concentration a owl:Class ;
    rdfs:subClassOf phScience:airQuality ;
    rdfs:label "ch2o-concentration" ;
    rdfs:comment "Concentration of formaldehyde (CH\u2082O) in the air." ;
    ph:is phScience:airQuality ;
    ph:lib phScience:lib:phScience ;
    phScience:prefUnit "\u00b5g/m\u00b3",
        "ppb" ;
    phScience:quantityOf phScience:air ;
    ph:wikipedia "https://en.wikipedia.org/wiki/Concentration"^^xsd:anyURI .

phScience:ch4 a owl:Class ;
    rdfs:subClassOf phScience:gas ;
    rdfs:label "ch4" ;
    rdfs:comment "Methane (CH\u2084)" ;
    ph:is phScience:gas ;
    ph:lib phScience:lib:phScience ;
    ph:wikipedia "https://en.wikipedia.org/wiki/Methane"^^xsd:anyURI .

phScience:ch4-emission a owl:Class ;
    rdfs:subClassOf phScience:emission ;
    rdfs:label "ch4-emission" ;
    rdfs:comment "Greenhouse gas emission of methane (CH\u2084) into the air." ;
    ph:is phScience:emission ;
    ph:lib phScience:lib:phScience ;
    phScience:prefUnit "kg",
        "ton",
        "lb" ;
    phScience:quantityOf phScience:air .

ph:children a owl:DatatypeProperty ;
    rdfs:range ph:list ;
    rdfs:label "children" ;
    ph:accumulate ph:marker ;
    rdfs:comment "List of prototypes contained by this entity.\nSee [Protos chapter]`docHaystack::Protos` for more details." ;
    ph:is ph:list ;
    ph:lib ph:lib:ph ;
    ph:of ph:dict .

ph:childrenFlatten a owl:DatatypeProperty ;
    rdfs:range ph:list ;
    rdfs:label "childrenFlatten" ;
    rdfs:comment "List of aspects to flatten into children prototypes.\nSee [Protos chapter]`docHaystack::Protos` for more details." ;
    ph:is ph:list ;
    ph:lib ph:lib:ph ;
    ph:of ph:symbol .

phIoT:chilled a owl:Class ;
    rdfs:subClassOf ph:marker ;
    rdfs:label "chilled" ;
    rdfs:comment "Substance is cooled using cooling process" ;
    ph:is ph:marker ;
    ph:lib phIoT:lib:phIoT .

phIoT:chilled-water a owl:Class ;
    rdfs:subClassOf phScience:water ;
    rdfs:label "chilled-water" ;
    rdfs:comment "Water cooled for use in HVAC and industrial processes" ;
    ph:is phScience:water ;
    ph:lib phIoT:lib:phIoT ;
    ph:wikipedia "https://en.wikipedia.org/wiki/Chilled_water"^^xsd:anyURI .

phIoT:chilled-water-input a owl:Class ;
    rdfs:subClassOf ph:input ;
    rdfs:label "chilled-water-input" ;
    rdfs:comment "Entity inputs chilled water which flows from another entity" ;
    ph:is ph:input ;
    ph:lib phIoT:lib:phIoT .

phIoT:chilled-water-output a owl:Class ;
    rdfs:subClassOf ph:output ;
    rdfs:label "chilled-water-output" ;
    rdfs:comment "Entity outputs chilled water to other entities" ;
    ph:is ph:output ;
    ph:lib phIoT:lib:phIoT .

phIoT:chilled-water-plant a owl:Class ;
    rdfs:subClassOf phIoT:plant,
        phIoT:chilled-water-output ;
    rdfs:label "chilled-water-plant" ;
    ph:children _:0b2cb027-d22f-3b40-0d9c-f23c91a70cca,
        _:0b2cb027-d22f-3b41-0d9d-f23c91a70cca,
        _:0b2cb027-d22f-3b42-0d9e-f23c91a70cca,
        _:0b2cb027-d22f-3b43-0d9f-f23c91a70cca,
        _:0b2cb027-d22f-3b44-0da0-f23c91a70cca,
        _:0b2cb027-d22f-3b45-0da1-f23c91a70cca,
        _:0b2cb027-d22f-3b46-0da2-f23c91a70cca,
        _:0b2cb027-d22f-3b47-0da3-f23c91a70cca,
        _:0b2cb027-d22f-3b48-0da4-f23c91a70cca,
        _:0b2cb027-d22f-3b49-0da5-f23c91a70cca,
        _:0b2cb027-d22f-3b4a-0da6-f23c91a70cca,
        _:0b2cb027-d22f-3b4b-0da7-f23c91a70cca,
        _:0b2cb027-d22f-3b4c-0da8-f23c91a70cca,
        _:0b2cb027-d22f-3b4d-0da9-f23c91a70cca,
        _:0b2cb027-d22f-3b4e-0daa-f23c91a70cca,
        _:0b2cb027-d22f-3b4f-0dab-f23c91a70cca,
        _:0b2cb027-d22f-3b50-0dac-f23c91a70cca,
        _:0b2cb027-d22f-3b51-0dad-f23c91a70cca ;
    rdfs:comment "Plant used to generate chilled water for cooling.\nSee `docHaystack::Plants`." ;
    ph:is phIoT:plant,
        phIoT:chilled-water-output ;
    ph:lib phIoT:lib:phIoT .

_:0b2cb027-d22f-3b40-0d9c-f23c91a70cca a phIoT:pipe ;
    ph:hasTag phIoT:chilled,
        phScience:water,
        phIoT:bypass,
        phIoT:pipe,
        phIoT:equip ;
    rdfs:label "{chilled, water, bypass, pipe, equip}" .

_:0b2cb027-d22f-3b41-0d9d-f23c91a70cca a phIoT:point ;
    ph:hasTag phIoT:chilled,
        phScience:water,
        phIoT:delta,
        phScience:flow,
        phIoT:point ;
    rdfs:label "{chilled, water, delta, flow, point}" .

_:0b2cb027-d22f-3b42-0d9e-f23c91a70cca a phIoT:point ;
    ph:hasTag phIoT:chilled,
        phScience:water,
        phIoT:delta,
        phScience:pressure,
        phIoT:point ;
    rdfs:label "{chilled, water, delta, pressure, point}" .

_:0b2cb027-d22f-3b43-0d9f-f23c91a70cca a phIoT:point ;
    ph:hasTag phIoT:chilled,
        phScience:water,
        phIoT:delta,
        phScience:temp,
        phIoT:point ;
    rdfs:label "{chilled, water, delta, temp, point}" .

_:0b2cb027-d22f-3b44-0da0-f23c91a70cca a phIoT:pipe ;
    ph:hasTag phIoT:chilled,
        phScience:water,
        phIoT:entering,
        phIoT:pipe,
        phIoT:equip ;
    rdfs:label "{chilled, water, entering, pipe, equip}" .

_:0b2cb027-d22f-3b45-0da1-f23c91a70cca a phIoT:pipe ;
    ph:hasTag phIoT:chilled,
        phScience:water,
        phIoT:header,
        phIoT:pipe,
        phIoT:equip ;
    rdfs:label "{chilled, water, header, pipe, equip}" .

_:0b2cb027-d22f-3b46-0da2-f23c91a70cca a phIoT:heatExchanger ;
    ph:hasTag phIoT:chilled,
        phScience:water,
        phIoT:heatExchanger,
        phIoT:equip ;
    rdfs:label "{chilled, water, heatExchanger, equip}" .

_:0b2cb027-d22f-3b47-0da3-f23c91a70cca a phIoT:pipe ;
    ph:hasTag phIoT:chilled,
        phScience:water,
        phIoT:leaving,
        phIoT:pipe,
        phIoT:equip ;
    rdfs:label "{chilled, water, leaving, pipe, equip}" .

_:0b2cb027-d22f-3b48-0da4-f23c91a70cca a phIoT:point ;
    ph:hasTag phIoT:chilled,
        phScience:water,
        phIoT:mixing,
        phIoT:valve,
        phIoT:cmd,
        phIoT:point ;
    rdfs:label "{chilled, water, mixing, valve, cmd, point}" .

_:0b2cb027-d22f-3b49-0da5-f23c91a70cca a phIoT:chiller ;
    ph:hasTag phIoT:chiller,
        phIoT:equip ;
    rdfs:label "{chiller, equip}" .

_:0b2cb027-d22f-3b4a-0da6-f23c91a70cca a phIoT:pipe ;
    ph:hasTag phIoT:condenser,
        phScience:water,
        phIoT:bypass,
        phIoT:pipe,
        phIoT:equip ;
    rdfs:label "{condenser, water, bypass, pipe, equip}" .

_:0b2cb027-d22f-3b4b-0da7-f23c91a70cca a phIoT:point ;
    ph:hasTag phIoT:condenser,
        phScience:water,
        phIoT:delta,
        phScience:flow,
        phIoT:sensor,
        phIoT:point ;
    rdfs:label "{condenser, water, delta, flow, sensor, point}" .

_:0b2cb027-d22f-3b4c-0da8-f23c91a70cca a phIoT:point ;
    ph:hasTag phIoT:condenser,
        phScience:water,
        phIoT:delta,
        phScience:pressure,
        phIoT:sensor,
        phIoT:point ;
    rdfs:label "{condenser, water, delta, pressure, sensor, point}" .

_:0b2cb027-d22f-3b4d-0da9-f23c91a70cca a phIoT:point ;
    ph:hasTag phIoT:condenser,
        phScience:water,
        phIoT:delta,
        phScience:temp,
        phIoT:sensor,
        phIoT:point ;
    rdfs:label "{condenser, water, delta, temp, sensor, point}" .

_:0b2cb027-d22f-3b4e-0daa-f23c91a70cca a phIoT:coolingTower ;
    ph:hasTag phIoT:coolingTower,
        phIoT:equip ;
    rdfs:label "{coolingTower, equip}" .

_:0b2cb027-d22f-3b4f-0dab-f23c91a70cca a phIoT:point ;
    ph:hasTag phIoT:enable,
        phIoT:cmd,
        phIoT:point ;
    rdfs:label "{enable, cmd, point}" .

_:0b2cb027-d22f-3b50-0dac-f23c91a70cca a phIoT:equip ;
    ph:hasTag phIoT:equip ;
    rdfs:label "{equip}" .

_:0b2cb027-d22f-3b51-0dad-f23c91a70cca a phIoT:point ;
    ph:hasTag phIoT:point ;
    rdfs:label "{point}" .

phIoT:chilled-water-system a owl:Class ;
    rdfs:subClassOf phIoT:water-system ;
    rdfs:label "chilled-water-system" ;
    ph:children _:0b2cb027-d2a9-4d40-0dae-f23c91a70cca,
        _:0b2cb027-d2a9-4d41-0daf-f23c91a70cca ;
    rdfs:comment "System that circulates water in its liquid state below ambient temperature\nfor cooling a space or process." ;
    ph:is phIoT:water-system ;
    ph:lib phIoT:lib:phIoT .

_:0b2cb027-d2a9-4d40-0dae-f23c91a70cca a phIoT:equip ;
    ph:hasTag phIoT:equip ;
    rdfs:label "{equip}" .

_:0b2cb027-d2a9-4d41-0daf-f23c91a70cca a phIoT:point ;
    ph:hasTag phIoT:point ;
    rdfs:label "{point}" .

phIoT:chilledBeam a owl:Class ;
    rdfs:subClassOf phIoT:radiantEquip ;
    rdfs:label "chilledBeam" ;
    ph:children _:0b2cb027-d2b8-8f80-0db0-f23c91a70cca,
        _:0b2cb027-d2b8-8f81-0db1-f23c91a70cca ;
    rdfs:comment "Conditions a space using a heat exchanger integrated into the ceiling" ;
    ph:is phIoT:radiantEquip ;
    ph:lib phIoT:lib:phIoT ;
    ph:wikipedia "https://en.wikipedia.org/wiki/Chilled_beam"^^xsd:anyURI .

_:0b2cb027-d2b8-8f80-0db0-f23c91a70cca a phIoT:equip ;
    ph:hasTag phIoT:equip ;
    rdfs:label "{equip}" .

_:0b2cb027-d2b8-8f81-0db1-f23c91a70cca a phIoT:point ;
    ph:hasTag phIoT:point ;
    rdfs:label "{point}" .

phIoT:chilledBeamZone a owl:Class ;
    rdfs:subClassOf phIoT:ahuZoneDelivery ;
    rdfs:label "chilledBeamZone" ;
    rdfs:comment "AHU supplies air to chilled beam terminal units" ;
    ph:is phIoT:ahuZoneDelivery ;
    ph:lib phIoT:lib:phIoT .

phIoT:chilledWaterCooling a owl:Class ;
    rdfs:subClassOf phIoT:coolingProcess,
        phIoT:chilled-water-input ;
    rdfs:label "chilledWaterCooling" ;
    rdfs:comment "Cooling using transfer of heat to chilled water" ;
    ph:is phIoT:coolingProcess,
        phIoT:chilled-water-input ;
    ph:lib phIoT:lib:phIoT .

phIoT:chilledWaterRef a owl:ObjectProperty ;
    rdfs:domain phIoT:chilled-water-input ;
    rdfs:range phIoT:chilled-water-output ;
    rdfs:label "chilledWaterRef" ;
    rdfs:comment "Chilled water flows from the referent to this entity" ;
    ph:inputs phIoT:chilled-water ;
    ph:is ph:ref ;
    ph:lib phIoT:lib:phIoT ;
    ph:of phIoT:chilled-water-output ;
    ph:tagOn phIoT:chilled-water-input .

phIoT:chiller a owl:Class ;
    rdfs:subClassOf phIoT:equip,
        phIoT:elec-input ;
    rdfs:label "chiller" ;
    ph:children _:0b2cb027-d2b8-8f82-0db2-f23c91a70cca,
        _:0b2cb027-d2b8-8f83-0db3-f23c91a70cca,
        _:0b2cb027-d2b8-8f84-0db4-f23c91a70cca,
        _:0b2cb027-d2b8-8f85-0db5-f23c91a70cca,
        _:0b2cb027-d2b8-8f86-0db6-f23c91a70cca,
        _:0b2cb027-d2b8-8f87-0db7-f23c91a70cca,
        _:0b2cb027-d2b8-8f88-0db8-f23c91a70cca,
        _:0b2cb027-d2b8-8f89-0db9-f23c91a70cca,
        _:0b2cb027-d2b8-8f8a-0dba-f23c91a70cca,
        _:0b2cb027-d2b8-8f8b-0dbb-f23c91a70cca,
        _:0b2cb027-d2b8-8f8c-0dbc-f23c91a70cca,
        _:0b2cb027-d2b8-8f8d-0dbd-f23c91a70cca,
        _:0b2cb027-d2b8-8f8e-0dbe-f23c91a70cca,
        _:0b2cb027-d2b8-8f8f-0dbf-f23c91a70cca,
        _:0b2cb027-d2b8-8f90-0dc0-f23c91a70cca,
        _:0b2cb027-d2b8-8f91-0dc1-f23c91a70cca,
        _:0b2cb027-d2b8-8f92-0dc2-f23c91a70cca,
        _:0b2cb027-d2b8-8f93-0dc3-f23c91a70cca,
        _:0b2cb027-d2b8-8f94-0dc4-f23c91a70cca,
        _:0b2cb027-d2b8-8f95-0dc5-f23c91a70cca,
        _:0b2cb027-d2b8-8f96-0dc6-f23c91a70cca,
        _:0b2cb027-d2b8-8f97-0dc7-f23c91a70cca,
        _:0b2cb027-d2b8-8f98-0dc8-f23c91a70cca,
        _:0b2cb027-d2b8-8f99-0dc9-f23c91a70cca ;
    rdfs:comment "Equipment to remove heat from a liquid.  Chillers typically use a vapor\ncompression or an absorption refrigeration cycle." ;
    ph:is phIoT:equip,
        phIoT:elec-input ;
    ph:lib phIoT:lib:phIoT ;
    ph:wikipedia "https://en.wikipedia.org/wiki/Chiller"^^xsd:anyURI .

_:0b2cb027-d2b8-8f82-0db2-f23c91a70cca a phIoT:point ;
    ph:hasTag phIoT:alarm,
        phIoT:sensor,
        phIoT:point ;
    rdfs:label "{alarm, sensor, point}" .

_:0b2cb027-d2b8-8f83-0db3-f23c91a70cca a phIoT:point ;
    ph:hasTag phIoT:chilled,
        phScience:water,
        phIoT:delta,
        phScience:flow,
        phIoT:sensor,
        phIoT:point ;
    rdfs:label "{chilled, water, delta, flow, sensor, point}" .

_:0b2cb027-d2b8-8f84-0db4-f23c91a70cca a phIoT:point ;
    ph:hasTag phIoT:chilled,
        phScience:water,
        phIoT:delta,
        phScience:temp,
        phIoT:sensor,
        phIoT:point ;
    rdfs:label "{chilled, water, delta, temp, sensor, point}" .

_:0b2cb027-d2b8-8f85-0db5-f23c91a70cca a phIoT:pipe ;
    ph:hasTag phIoT:chilled,
        phScience:water,
        phIoT:entering,
        phIoT:pipe,
        phIoT:equip ;
    rdfs:label "{chilled, water, entering, pipe, equip}" .

_:0b2cb027-d2b8-8f86-0db6-f23c91a70cca a phIoT:pipe ;
    ph:hasTag phIoT:chilled,
        phScience:water,
        phIoT:leaving,
        phIoT:pipe,
        phIoT:equip ;
    rdfs:label "{chilled, water, leaving, pipe, equip}" .

_:0b2cb027-d2b8-8f87-0db7-f23c91a70cca a phIoT:point ;
    ph:hasTag phIoT:chilled,
        phScience:water,
        phIoT:valve,
        phIoT:isolation,
        phIoT:cmd,
        phIoT:point ;
    rdfs:label "{chilled, water, valve, isolation, cmd, point}" .

_:0b2cb027-d2b8-8f88-0db8-f23c91a70cca a phIoT:point ;
    ph:hasTag phIoT:condenser,
        phIoT:refrig,
        phScience:pressure,
        phIoT:sensor,
        phIoT:point ;
    rdfs:label "{condenser, refrig, pressure, sensor, point}" .

_:0b2cb027-d2b8-8f89-0db9-f23c91a70cca a phIoT:point ;
    ph:hasTag phIoT:condenser,
        phIoT:refrig,
        phScience:temp,
        phIoT:sensor,
        phIoT:point ;
    rdfs:label "{condenser, refrig, temp, sensor, point}" .

_:0b2cb027-d2b8-8f8a-0dba-f23c91a70cca a phIoT:point ;
    ph:hasTag phIoT:condenser,
        phIoT:run,
        phIoT:cmd,
        phIoT:point ;
    rdfs:label "{condenser, run, cmd, point}" .

_:0b2cb027-d2b8-8f8b-0dbb-f23c91a70cca a phIoT:point ;
    ph:hasTag phIoT:condenser,
        phIoT:run,
        phIoT:sensor,
        phIoT:point ;
    rdfs:label "{condenser, run, sensor, point}" .

_:0b2cb027-d2b8-8f8c-0dbc-f23c91a70cca a phIoT:pipe ;
    ph:hasTag phIoT:condenser,
        phScience:water,
        phIoT:entering,
        phIoT:pipe,
        phIoT:equip ;
    rdfs:label "{condenser, water, entering, pipe, equip}" .

_:0b2cb027-d2b8-8f8d-0dbd-f23c91a70cca a phIoT:pipe ;
    ph:hasTag phIoT:condenser,
        phScience:water,
        phIoT:leaving,
        phIoT:pipe,
        phIoT:equip ;
    rdfs:label "{condenser, water, leaving, pipe, equip}" .

_:0b2cb027-d2b8-8f8e-0dbe-f23c91a70cca a phIoT:point ;
    ph:hasTag phIoT:condenser,
        phScience:water,
        phIoT:valve,
        phIoT:isolation,
        phIoT:cmd,
        phIoT:point ;
    rdfs:label "{condenser, water, valve, isolation, cmd, point}" .

_:0b2cb027-d2b8-8f8f-0dbf-f23c91a70cca a phIoT:point ;
    ph:hasTag phIoT:efficiency,
        phIoT:sensor,
        phIoT:point ;
    rdfs:label "{efficiency, sensor, point}" .

_:0b2cb027-d2b8-8f90-0dc0-f23c91a70cca a phIoT:point ;
    ph:hasTag phIoT:enable,
        phIoT:cmd,
        phIoT:point ;
    rdfs:label "{enable, cmd, point}" .

_:0b2cb027-d2b8-8f91-0dc1-f23c91a70cca a phIoT:point ;
    ph:hasTag phIoT:enable,
        phIoT:sensor,
        phIoT:point ;
    rdfs:label "{enable, sensor, point}" .

_:0b2cb027-d2b8-8f92-0dc2-f23c91a70cca a phIoT:equip ;
    ph:hasTag phIoT:equip ;
    rdfs:label "{equip}" .

_:0b2cb027-d2b8-8f93-0dc3-f23c91a70cca a phIoT:point ;
    ph:hasTag phIoT:evaporator,
        phIoT:refrig,
        phScience:pressure,
        phIoT:sensor,
        phIoT:point ;
    rdfs:label "{evaporator, refrig, pressure, sensor, point}" .

_:0b2cb027-d2b8-8f94-0dc4-f23c91a70cca a phIoT:point ;
    ph:hasTag phIoT:evaporator,
        phIoT:refrig,
        phScience:temp,
        phIoT:sensor,
        phIoT:point ;
    rdfs:label "{evaporator, refrig, temp, sensor, point}" .

_:0b2cb027-d2b8-8f95-0dc5-f23c91a70cca a phIoT:point ;
    ph:hasTag phIoT:load,
        phIoT:cmd,
        phIoT:point ;
    rdfs:label "{load, cmd, point}" .

_:0b2cb027-d2b8-8f96-0dc6-f23c91a70cca a phIoT:point ;
    ph:hasTag phIoT:load,
        phIoT:sensor,
        phIoT:point ;
    rdfs:label "{load, sensor, point}" .

_:0b2cb027-d2b8-8f97-0dc7-f23c91a70cca a phIoT:point ;
    ph:hasTag phIoT:point ;
    rdfs:label "{point}" .

_:0b2cb027-d2b8-8f98-0dc8-f23c91a70cca a phIoT:point ;
    ph:hasTag phIoT:run,
        phIoT:cmd,
        phIoT:point ;
    rdfs:label "{run, cmd, point}" .

_:0b2cb027-d2b8-8f99-0dc9-f23c91a70cca a phIoT:point ;
    ph:hasTag phIoT:run,
        phIoT:sensor,
        phIoT:point ;
    rdfs:label "{run, sensor, point}" .

phIoT:chiller-absorption a owl:Class ;
    rdfs:subClassOf phIoT:absorption,
        phIoT:chillerMechanism ;
    rdfs:label "chiller-absorption" ;
    rdfs:comment "Cooling process using energy from heat source such as hot water" ;
    ph:is phIoT:absorption,
        phIoT:chillerMechanism ;
    ph:lib phIoT:lib:phIoT ;
    ph:wikipedia "https://en.wikipedia.org/wiki/Absorption_refrigerator"^^xsd:anyURI .

phIoT:chiller-centrifugal a owl:Class ;
    rdfs:subClassOf phIoT:centrifugal,
        phIoT:chillerMechanism ;
    rdfs:label "chiller-centrifugal" ;
    rdfs:comment "Compression via a continuous flow of fluid through an impeller" ;
    ph:is phIoT:centrifugal,
        phIoT:chillerMechanism ;
    ph:lib phIoT:lib:phIoT ;
    ph:wikipedia "https://en.wikipedia.org/wiki/Centrifugal_compressor"^^xsd:anyURI .

phIoT:chiller-reciprocal a owl:Class ;
    rdfs:subClassOf phIoT:reciprocal,
        phIoT:chillerMechanism ;
    rdfs:label "chiller-reciprocal" ;
    rdfs:comment "Piston compressor driven by a crankshaft" ;
    ph:is phIoT:reciprocal,
        phIoT:chillerMechanism ;
    ph:lib phIoT:lib:phIoT ;
    ph:wikipedia "https://en.wikipedia.org/wiki/Reciprocating_compressor"^^xsd:anyURI .

phIoT:chiller-rotaryScrew a owl:Class ;
    rdfs:subClassOf phIoT:rotaryScrew,
        phIoT:chillerMechanism ;
    rdfs:label "chiller-rotaryScrew" ;
    rdfs:comment "Rotary screw compression" ;
    ph:is phIoT:rotaryScrew,
        phIoT:chillerMechanism ;
    ph:lib phIoT:lib:phIoT ;
    ph:wikipedia "https://en.wikipedia.org/wiki/Rotary-screw_compressor"^^xsd:anyURI .

phIoT:chillerMechanism a owl:Class ;
    rdfs:subClassOf ph:choice ;
    rdfs:label "chillerMechanism" ;
    rdfs:comment "Primary mechanism of chiller" ;
    ph:is ph:choice ;
    ph:lib phIoT:lib:phIoT ;
    ph:tagOn phIoT:chiller .

ph:choice a owl:Class ;
    rdfs:subClassOf ph:marker ;
    rdfs:label "choice" ;
    rdfs:comment "Choice specifies an exclusive marker selection.\nSee [Choices]`docHaystack::Choices` chapter." ;
    ph:docTaxonomy ph:marker ;
    ph:is ph:marker ;
    ph:lib ph:lib:ph .

phIoT:circ a owl:Class ;
    rdfs:subClassOf phIoT:pipeSection ;
    rdfs:label "circ" ;
    rdfs:comment "Pipe used to circulate fluid through an equipment or system" ;
    ph:is phIoT:pipeSection ;
    ph:lib phIoT:lib:phIoT .

phIoT:circuit a owl:Class ;
    rdfs:subClassOf phIoT:equip,
        phIoT:elec-input,
        phIoT:elec-output ;
    rdfs:label "circuit" ;
    ph:children _:0b2cb027-d2c7-d1c0-0dca-f23c91a70cca,
        _:0b2cb027-d2c7-d1c1-0dcb-f23c91a70cca ;
    rdfs:comment "Electrical circuit and its associated components such as breakers.\nSee `docHaystack::ElecPanels#circuits` chapter." ;
    ph:is phIoT:equip,
        phIoT:elec-input,
        phIoT:elec-output ;
    ph:lib phIoT:lib:phIoT ;
    ph:wikipedia "https://en.wikipedia.org/wiki/Electrical_network"^^xsd:anyURI .

_:0b2cb027-d2c7-d1c0-0dca-f23c91a70cca a phIoT:equip ;
    ph:hasTag phIoT:equip ;
    rdfs:label "{equip}" .

_:0b2cb027-d2c7-d1c1-0dcb-f23c91a70cca a phIoT:point ;
    ph:hasTag phIoT:point ;
    rdfs:label "{point}" .

phScience:cloudage a owl:Class ;
    rdfs:subClassOf phScience:quantity ;
    rdfs:label "cloudage" ;
    rdfs:comment "Percentage of sky obscured by clouds. This is also known as cloudiness, or cloud amount." ;
    ph:is phScience:quantity ;
    ph:lib phScience:lib:phScience ;
    phScience:prefUnit "%" ;
    phScience:quantityOf phScience:weather .

phIoT:cmd a owl:Class ;
    rdfs:subClassOf phIoT:pointFunction ;
    rdfs:label "cmd" ;
    rdfs:comment "Point is a command, actuator, AO/BO.\nSee `docHaystack::Points#function` chapter." ;
    ph:is phIoT:pointFunction ;
    ph:lib phIoT:lib:phIoT .

phScience:co a owl:Class ;
    rdfs:subClassOf phScience:gas ;
    rdfs:label "co" ;
    rdfs:comment "Carbon monoxide (CO)" ;
    ph:is phScience:gas ;
    ph:lib phScience:lib:phScience ;
    ph:wikipedia "https://en.wikipedia.org/wiki/Carbon_monoxide"^^xsd:anyURI .

phScience:co-concentration a owl:Class ;
    rdfs:subClassOf phScience:airQuality ;
    rdfs:label "co-concentration" ;
    rdfs:comment "Concentration of carbon monoxide (CO) in the air." ;
    ph:is phScience:airQuality ;
    ph:lib phScience:lib:phScience ;
    phScience:prefUnit "ppm" ;
    phScience:quantityOf phScience:air ;
    ph:wikipedia "https://en.wikipedia.org/wiki/Concentration"^^xsd:anyURI .

phScience:co2 a owl:Class ;
    rdfs:subClassOf phScience:gas ;
    rdfs:label "co2" ;
    rdfs:comment "Carbon dioxide (CO\u2082)" ;
    ph:is phScience:gas ;
    ph:lib phScience:lib:phScience ;
    ph:wikipedia "https://en.wikipedia.org/wiki/Carbon_dioxide"^^xsd:anyURI .

phScience:co2-concentration a owl:Class ;
    rdfs:subClassOf phScience:airQuality ;
    rdfs:label "co2-concentration" ;
    rdfs:comment "Concentration of carbon dioxide (CO\u2082) in the air." ;
    ph:is phScience:airQuality ;
    ph:lib phScience:lib:phScience ;
    phScience:prefUnit "ppm" ;
    phScience:quantityOf phScience:air ;
    ph:wikipedia "https://en.wikipedia.org/wiki/Concentration"^^xsd:anyURI .

phScience:co2-emission a owl:Class ;
    rdfs:subClassOf phScience:emission ;
    rdfs:label "co2-emission" ;
    rdfs:comment "Greenhouse gas emission of carbon dioxide (CO\u2082) into the air." ;
    ph:is phScience:emission ;
    ph:lib phScience:lib:phScience ;
    phScience:prefUnit "kg",
        "ton",
        "lb" ;
    phScience:quantityOf phScience:air .

phScience:co2e a owl:Class ;
    rdfs:subClassOf ph:marker ;
    rdfs:label "co2e" ;
    rdfs:comment "Carbon dioxide equivalent" ;
    ph:is ph:marker ;
    ph:lib phScience:lib:phScience ;
    ph:wikipedia "https://en.wikipedia.org/wiki/Global_warming_potential"^^xsd:anyURI .

phIoT:coal a owl:Class ;
    rdfs:subClassOf phScience:solid ;
    rdfs:label "coal" ;
    rdfs:comment "Combustible sedimentary rock" ;
    ph:is phScience:solid ;
    ph:lib phIoT:lib:phIoT ;
    ph:wikipedia "https://en.wikipedia.org/wiki/Coal"^^xsd:anyURI .

phIoT:coalHeating a owl:Class ;
    rdfs:subClassOf phIoT:heatingProcess ;
    rdfs:label "coalHeating" ;
    rdfs:comment "Heating by the combustion of coal" ;
    ph:is phIoT:heatingProcess ;
    ph:lib phIoT:lib:phIoT .

phIct:coap a owl:Class ;
    rdfs:subClassOf phIct:protocol ;
    rdfs:label "coap" ;
    rdfs:comment "Constrained Application Protocol" ;
    ph:is phIct:protocol ;
    ph:lib phIct:lib:phIct ;
    ph:wikipedia "https://en.wikipedia.org/wiki/Constrained_Application_Protocol"^^xsd:anyURI .

phIoT:coil a owl:Class ;
    rdfs:subClassOf phIoT:heatExchanger ;
    rdfs:label "coil" ;
    ph:children _:0b2cb027-d2d7-1400-0dcc-f23c91a70cca,
        _:0b2cb027-d2d7-1401-0dcd-f23c91a70cca ;
    rdfs:comment "Heat exchanger used to heat or cool air.  Coils are sub-components\nof HVAC equipment such as `airHandlingEquip`." ;
    ph:is phIoT:heatExchanger ;
    ph:lib phIoT:lib:phIoT ;
    ph:wikipedia "https://en.wikipedia.org/wiki/Heat_exchanger#HVAC_air_coils"^^xsd:anyURI .

_:0b2cb027-d2d7-1400-0dcc-f23c91a70cca a phIoT:equip ;
    ph:hasTag phIoT:equip ;
    rdfs:label "{equip}" .

_:0b2cb027-d2d7-1401-0dcd-f23c91a70cca a phIoT:point ;
    ph:hasTag phIoT:point ;
    rdfs:label "{point}" .

phIoT:cold a owl:Class ;
    rdfs:subClassOf ph:marker ;
    rdfs:label "cold" ;
    rdfs:comment "Having low degree of heat" ;
    ph:is ph:marker ;
    ph:lib phIoT:lib:phIoT .

phIoT:cold-water a owl:Class ;
    rdfs:subClassOf phScience:water ;
    rdfs:label "cold-water" ;
    rdfs:comment "Water supplied to cold taps" ;
    ph:is phScience:water ;
    ph:lib phIoT:lib:phIoT ;
    ph:wikipedia "https://en.wikipedia.org/wiki/Water"^^xsd:anyURI .

phIoT:coldDeck a owl:Class ;
    rdfs:subClassOf phIoT:ductDeck ;
    rdfs:label "coldDeck" ;
    rdfs:comment "Duct carries air for cooling" ;
    ph:is phIoT:ductDeck ;
    ph:lib phIoT:lib:phIoT .

phIoT:compressor a owl:Class ;
    rdfs:subClassOf ph:marker ;
    rdfs:label "compressor" ;
    rdfs:comment "Device for mechanically increasing the pressure of a gas or refrigerant\nvapor by reducing its volume." ;
    ph:is ph:marker ;
    ph:lib phIoT:lib:phIoT .

phIoT:computed a owl:Class ;
    rdfs:subClassOf phIoT:synthetic ;
    rdfs:label "computed" ;
    rdfs:comment "Computed point. See `docHaystack::Synthetics` chapter." ;
    ph:is phIoT:synthetic ;
    ph:lib phIoT:lib:phIoT .

phIoT:computed-point a owl:Class ;
    rdfs:subClassOf phIoT:synthetic-point ;
    rdfs:label "computed-point" ;
    rdfs:comment "See `docHaystack::Synthetics` chapter." ;
    ph:is phIoT:synthetic-point ;
    ph:lib phIoT:lib:phIoT .

ph:computedFromReciprocal a owl:Class ;
    rdfs:subClassOf ph:marker ;
    rdfs:label "computedFromReciprocal" ;
    rdfs:comment "Indicates a relationship that is computed from its reciprocal.\nComputed defs cannot be used as tags themselves." ;
    ph:is ph:marker ;
    ph:lib ph:lib:ph .

phIoT:computedModel a owl:Class ;
    rdfs:subClassOf phIoT:syntheticModel ;
    rdfs:label "computedModel" ;
    rdfs:comment "See `docHaystack::Synthetics` chapter." ;
    ph:is phIoT:syntheticModel ;
    ph:lib phIoT:lib:phIoT .

phIct:computer a owl:Class ;
    rdfs:subClassOf phIct:device ;
    rdfs:label "computer" ;
    rdfs:comment "General purpose computer." ;
    ph:is phIct:device ;
    ph:lib phIct:lib:phIct ;
    ph:wikipedia "https://en.wikipedia.org/wiki/Computer"^^xsd:anyURI .

phScience:concentration a owl:Class ;
    rdfs:subClassOf phScience:quantity ;
    rdfs:label "concentration" ;
    rdfs:comment "Abundance of substance in the total volume of a mixture." ;
    ph:is phScience:quantity ;
    ph:lib phScience:lib:phScience ;
    phScience:quantityOf phScience:substance ;
    ph:wikipedia "https://en.wikipedia.org/wiki/Concentration"^^xsd:anyURI .

phIoT:condensate a owl:Class ;
    rdfs:subClassOf phScience:liquid ;
    rdfs:label "condensate" ;
    rdfs:comment "Liquid phase produced by the condensation of steam or other gas" ;
    ph:is phScience:liquid ;
    ph:lib phIoT:lib:phIoT ;
    ph:wikipedia "https://en.wikipedia.org/wiki/Liquid"^^xsd:anyURI .

phIoT:condensate-input a owl:Class ;
    rdfs:subClassOf ph:input ;
    rdfs:label "condensate-input" ;
    rdfs:comment "Entity inputs condensate which flows from another entity" ;
    ph:is ph:input ;
    ph:lib phIoT:lib:phIoT .

phIoT:condensate-output a owl:Class ;
    rdfs:subClassOf ph:output ;
    rdfs:label "condensate-output" ;
    rdfs:comment "Entity outputs condensate to other entities" ;
    ph:is ph:output ;
    ph:lib phIoT:lib:phIoT .

phIoT:condensateRef a owl:ObjectProperty ;
    rdfs:domain phIoT:condensate-input ;
    rdfs:range phIoT:condensate-output ;
    rdfs:label "condensateRef" ;
    rdfs:comment "Condensate flows from the referent to this entity" ;
    ph:inputs phIoT:condensate ;
    ph:is ph:ref ;
    ph:lib phIoT:lib:phIoT ;
    ph:of phIoT:condensate-output ;
    ph:tagOn phIoT:condensate-input .

phIoT:condenser a owl:Class ;
    rdfs:subClassOf ph:marker ;
    rdfs:label "condenser" ;
    rdfs:comment "Device or related to process of condensation" ;
    ph:is ph:marker ;
    ph:lib phIoT:lib:phIoT .

phIoT:condenser-water a owl:Class ;
    rdfs:subClassOf phScience:water ;
    rdfs:label "condenser-water" ;
    rdfs:comment "Water used used to remove heat through condensation" ;
    ph:is phScience:water ;
    ph:lib phIoT:lib:phIoT ;
    ph:wikipedia "https://en.wikipedia.org/wiki/Water"^^xsd:anyURI .

phIoT:condenser-water-input a owl:Class ;
    rdfs:subClassOf ph:input ;
    rdfs:label "condenser-water-input" ;
    rdfs:comment "Entity inputs condenser water which flows from another entity" ;
    ph:is ph:input ;
    ph:lib phIoT:lib:phIoT .

phIoT:condenser-water-output a owl:Class ;
    rdfs:subClassOf ph:output ;
    rdfs:label "condenser-water-output" ;
    rdfs:comment "Entity outputs condenser water to other entities" ;
    ph:is ph:output ;
    ph:lib phIoT:lib:phIoT .

phIoT:condenser-water-system a owl:Class ;
    rdfs:subClassOf phIoT:water-system ;
    rdfs:label "condenser-water-system" ;
    ph:children _:0b2cb027-d2d7-1402-0dce-f23c91a70cca,
        _:0b2cb027-d2d7-1403-0dcf-f23c91a70cca ;
    rdfs:comment "System that circulates water in its liquid state for rejecting heat\nfrom a space or process." ;
    ph:is phIoT:water-system ;
    ph:lib phIoT:lib:phIoT .

_:0b2cb027-d2d7-1402-0dce-f23c91a70cca a phIoT:equip ;
    ph:hasTag phIoT:equip ;
    rdfs:label "{equip}" .

_:0b2cb027-d2d7-1403-0dcf-f23c91a70cca a phIoT:point ;
    ph:hasTag phIoT:point ;
    rdfs:label "{point}" .

phIoT:condenserClosedLoop a owl:Class ;
    rdfs:subClassOf phIoT:condenserLoop ;
    rdfs:label "condenserClosedLoop" ;
    rdfs:comment "Working fluid is kept separate from fluid used for heat transfer into the atmosphere" ;
    ph:is phIoT:condenserLoop ;
    ph:lib phIoT:lib:phIoT .

phIoT:condenserCooling a owl:Class ;
    rdfs:subClassOf phIoT:coolingProcess ;
    rdfs:label "condenserCooling" ;
    rdfs:comment "Removal of heat through the process of water condensation" ;
    ph:is phIoT:coolingProcess ;
    ph:lib phIoT:lib:phIoT .

phIoT:condenserLoop a owl:Class ;
    rdfs:subClassOf ph:choice ;
    rdfs:label "condenserLoop" ;
    rdfs:comment "Open or closed loop for condenser working fluid" ;
    ph:is ph:choice ;
    ph:lib phIoT:lib:phIoT ;
    ph:tagOn phIoT:chilled-water-plant .

phIoT:condenserOpenLoop a owl:Class ;
    rdfs:subClassOf phIoT:condenserLoop ;
    rdfs:label "condenserOpenLoop" ;
    rdfs:comment "Uses working fluid itself for evaporation into the atmosphere" ;
    ph:is phIoT:condenserLoop ;
    ph:lib phIoT:lib:phIoT .

phIoT:condenserWaterRef a owl:ObjectProperty ;
    rdfs:domain phIoT:condenser-water-input ;
    rdfs:range phIoT:condenser-water-output ;
    rdfs:label "condenserWaterRef" ;
    rdfs:comment "Condenser water flows from the referent to this entity" ;
    ph:inputs phIoT:condenser-water ;
    ph:is ph:ref ;
    ph:lib phIoT:lib:phIoT ;
    ph:of phIoT:condenser-water-output ;
    ph:tagOn phIoT:condenser-water-input .

phIoT:conditioning a owl:Class ;
    rdfs:subClassOf ph:marker ;
    rdfs:label "conditioning" ;
    rdfs:comment "Related to cleaning, heating, cooling, humidifying, dehumidifying,\nventilating or circulating \u00a0air.\u00a0" ;
    ph:is ph:marker ;
    ph:lib phIoT:lib:phIoT .

phIoT:conduit a owl:Class ;
    rdfs:subClassOf phIoT:equip ;
    rdfs:label "conduit" ;
    ph:children _:0b2cb027-d314-1d00-0dd0-f23c91a70cca,
        _:0b2cb027-d314-1d01-0dd1-f23c91a70cca ;
    rdfs:comment "Duct, pipe, or cable to convey a substance or phenomenon" ;
    ph:is phIoT:equip ;
    ph:lib phIoT:lib:phIoT .

_:0b2cb027-d314-1d00-0dd0-f23c91a70cca a phIoT:equip ;
    ph:hasTag phIoT:equip ;
    rdfs:label "{equip}" .

_:0b2cb027-d314-1d01-0dd1-f23c91a70cca a phIoT:point ;
    ph:hasTag phIoT:point ;
    rdfs:label "{point}" .

phIoT:constantAirVolume a owl:Class ;
    rdfs:subClassOf phIoT:airVolumeAdjustability ;
    rdfs:label "constantAirVolume" ;
    rdfs:comment "Delivers a constant volume of air flow.  Typically this means\nequipment with a single speed fan." ;
    ph:is phIoT:airVolumeAdjustability ;
    ph:lib phIoT:lib:phIoT .

ph:containedBy a owl:DatatypeProperty ;
    rdfs:range ph:symbol ;
    rdfs:label "containedBy" ;
    rdfs:comment "The entity is logically contained by the referent." ;
    ph:is ph:relationship ;
    ph:lib ph:lib:ph ;
    ph:reciprocalOf ph:contains ;
    ph:transitive ph:marker .

ph:contains a owl:DatatypeProperty ;
    rdfs:range ph:symbol ;
    rdfs:label "contains" ;
    ph:computedFromReciprocal ph:marker ;
    rdfs:comment "Entities logically contained by this entity" ;
    ph:is ph:relationship ;
    ph:lib ph:lib:ph ;
    ph:reciprocalOf ph:containedBy ;
    ph:transitive ph:marker .

phIct:controller a owl:Class ;
    rdfs:subClassOf phIct:device ;
    rdfs:label "controller" ;
    rdfs:comment "Microprocessor based device used in a control system.  Controllers\ninteract with the physical world through direct I/O to sensors and\nactuators or via network [protocols]`protocol`." ;
    ph:is phIct:device ;
    ph:lib phIct:lib:phIct .

phIoT:controls a owl:Class ;
    rdfs:subClassOf ph:marker ;
    rdfs:label "controls" ;
    rdfs:comment "Associated with the control system for an industrial process" ;
    ph:is ph:marker ;
    ph:lib phIoT:lib:phIoT ;
    ph:wikipedia "https://en.wikipedia.org/wiki/Control_system"^^xsd:anyURI .

phIct:controls-panel a owl:Class ;
    rdfs:subClassOf phIoT:panel ;
    rdfs:label "controls-panel" ;
    ph:children _:0b2cb027-d323-5f40-0dd2-f23c91a70cca,
        _:0b2cb027-d323-5f41-0dd3-f23c91a70cca,
        _:0b2cb027-d323-5f42-0dd4-f23c91a70cca,
        _:0b2cb027-d323-5f43-0dd5-f23c91a70cca ;
    rdfs:comment "Panel housing controllers and networking gear" ;
    ph:is phIoT:panel ;
    ph:lib phIct:lib:phIct .

_:0b2cb027-d323-5f40-0dd2-f23c91a70cca a phIct:controller ;
    ph:hasTag phIct:controller,
        phIct:device ;
    rdfs:label "{controller, device}" .

_:0b2cb027-d323-5f41-0dd3-f23c91a70cca a phIoT:equip ;
    ph:hasTag phIoT:equip ;
    rdfs:label "{equip}" .

_:0b2cb027-d323-5f42-0dd4-f23c91a70cca a phIct:networking-device ;
    ph:hasTag phIct:networking,
        phIct:device ;
    rdfs:label "{networking, device}" .

_:0b2cb027-d323-5f43-0dd5-f23c91a70cca a phIoT:point ;
    ph:hasTag phIoT:point ;
    rdfs:label "{point}" .

phIoT:cool a owl:Class ;
    rdfs:subClassOf ph:marker ;
    rdfs:label "cool" ;
    rdfs:comment "Associted with low temperature or cooling processes.  When used on a point,\nthis tag is associated with the control of cooling.  When paired with a\nsubstance, this tag indicates the substance is relatively cool in comparison\nto another substance, without being actively cooled by e.g. a chiller." ;
    ph:is ph:marker ;
    ph:lib phIoT:lib:phIoT .

phIoT:cool-water a owl:Class ;
    rdfs:subClassOf phScience:water ;
    rdfs:label "cool-water" ;
    rdfs:comment "Relatively cool water without active chilling" ;
    ph:is phScience:water ;
    ph:lib phIoT:lib:phIoT ;
    ph:wikipedia "https://en.wikipedia.org/wiki/Water"^^xsd:anyURI .

phIoT:cooling a owl:Class ;
    rdfs:subClassOf ph:marker ;
    rdfs:label "cooling" ;
    rdfs:comment "Cooling mode or process" ;
    ph:is ph:marker ;
    ph:lib phIoT:lib:phIoT .

phIoT:coolingCapacity a owl:DatatypeProperty ;
    rdfs:domain phIoT:chiller ;
    rdfs:range ph:number ;
    rdfs:label "coolingCapacity" ;
    rdfs:comment "Measurement of a chiller ability to remove heat measured" ;
    ph:is ph:number ;
    ph:lib phIoT:lib:phIoT ;
    phScience:prefUnit "tonref",
        "BTU/h",
        "kW" ;
    ph:tagOn phIoT:chiller .

phIoT:coolingCoil a owl:Class ;
    rdfs:subClassOf phIoT:coil ;
    rdfs:label "coolingCoil" ;
    ph:children _:0b2cb027-d323-5f44-0dd6-f23c91a70cca,
        _:0b2cb027-d323-5f45-0dd7-f23c91a70cca,
        _:0b2cb027-d323-5f46-0dd8-f23c91a70cca,
        _:0b2cb027-d323-5f47-0dd9-f23c91a70cca ;
    ph:childrenFlatten phIoT:ductDeck,
        phIoT:ductSection ;
    rdfs:comment "Coil used to cool air." ;
    ph:is phIoT:coil ;
    ph:lib phIoT:lib:phIoT ;
    ph:wikipedia "https://en.wikipedia.org/wiki/Heat_exchanger#HVAC_air_coils"^^xsd:anyURI .

_:0b2cb027-d323-5f44-0dd6-f23c91a70cca a phIoT:point ;
    ph:hasTag phIoT:chilled,
        phScience:water,
        phIoT:cool,
        phIoT:valve,
        phIoT:cmd,
        phIoT:point ;
    rdfs:label "{chilled, water, cool, valve, cmd, point}" .

_:0b2cb027-d323-5f45-0dd7-f23c91a70cca a phIoT:equip ;
    ph:hasTag phIoT:equip ;
    rdfs:label "{equip}" .

_:0b2cb027-d323-5f46-0dd8-f23c91a70cca a phIoT:point ;
    ph:hasTag phIoT:point ;
    rdfs:label "{point}" .

_:0b2cb027-d323-5f47-0dd9-f23c91a70cca a phIoT:point ;
    ph:hasTag phIoT:cool,
        phIoT:run,
        phIoT:cmd,
        phIoT:point ;
    rdfs:label "{stage:1, cool, run, cmd, point}" ;
    phIoT:stage 1 .

phIoT:coolingOnly a owl:Class ;
    rdfs:subClassOf ph:marker ;
    rdfs:label "coolingOnly" ;
    rdfs:comment "Equipment without heating" ;
    ph:is ph:marker ;
    ph:lib phIoT:lib:phIoT .

phIoT:coolingProcess a owl:Class ;
    rdfs:subClassOf ph:choice ;
    rdfs:label "coolingProcess" ;
    rdfs:comment "Processed used to cool a substance" ;
    ph:is ph:choice ;
    ph:lib phIoT:lib:phIoT ;
    ph:tagOn phIoT:airHandlingEquip,
        phIoT:chilledBeam,
        phIoT:coolingCoil .

phIoT:coolingTower a owl:Class ;
    rdfs:subClassOf phIoT:equip,
        phIoT:elec-input ;
    rdfs:label "coolingTower" ;
    ph:children _:0b2cb027-d323-5f48-0dda-f23c91a70cca,
        _:0b2cb027-d323-5f49-0ddb-f23c91a70cca,
        _:0b2cb027-d323-5f4a-0ddc-f23c91a70cca,
        _:0b2cb027-d323-5f4b-0ddd-f23c91a70cca,
        _:0b2cb027-d323-5f4c-0dde-f23c91a70cca ;
    rdfs:comment "Equipment to transfer waste heat into the atmosphere" ;
    ph:is phIoT:equip,
        phIoT:elec-input ;
    ph:lib phIoT:lib:phIoT ;
    ph:wikipedia "https://en.wikipedia.org/wiki/Cooling_tower"^^xsd:anyURI .

_:0b2cb027-d323-5f48-0dda-f23c91a70cca a phIoT:pipe ;
    ph:hasTag phIoT:condenser,
        phScience:water,
        phIoT:entering,
        phIoT:pipe,
        phIoT:equip ;
    rdfs:label "{condenser, water, entering, pipe, equip}" .

_:0b2cb027-d323-5f49-0ddb-f23c91a70cca a phIoT:pipe ;
    ph:hasTag phIoT:condenser,
        phScience:water,
        phIoT:leaving,
        phIoT:pipe,
        phIoT:equip ;
    rdfs:label "{condenser, water, leaving, pipe, equip}" .

_:0b2cb027-d323-5f4a-0ddc-f23c91a70cca a phIoT:equip ;
    ph:hasTag phIoT:equip ;
    rdfs:label "{equip}" .

_:0b2cb027-d323-5f4b-0ddd-f23c91a70cca a phIoT:fan-motor ;
    ph:hasTag phIoT:fan,
        phIoT:motor,
        phIoT:equip ;
    rdfs:label "{fan, motor, equip}" .

_:0b2cb027-d323-5f4c-0dde-f23c91a70cca a phIoT:point ;
    ph:hasTag phIoT:point ;
    rdfs:label "{point}" .

ph:coord a owl:DatatypeProperty ;
    rdfs:subClassOf xsd:string ;
    rdfs:label "coord" ;
    rdfs:comment "Geographic coordinate in latitude/longitude in decimal degrees.\nSee [Kinds chapter]`docHaystack::Kinds#coord`." ;
    ph:is ph:scalar ;
    ph:lib ph:lib:ph .

phIoT:crac a owl:Class ;
    rdfs:subClassOf phIoT:fcu ;
    rdfs:label "crac" ;
    ph:children _:0b2cb027-d332-a180-0ddf-f23c91a70cca,
        _:0b2cb027-d332-a181-0de0-f23c91a70cca,
        _:0b2cb027-d332-a182-0de1-f23c91a70cca,
        _:0b2cb027-d332-a183-0de2-f23c91a70cca,
        _:0b2cb027-d332-a184-0de3-f23c91a70cca,
        _:0b2cb027-d332-a185-0de4-f23c91a70cca,
        _:0b2cb027-d332-a186-0de5-f23c91a70cca,
        _:0b2cb027-d332-a187-0de6-f23c91a70cca,
        _:0b2cb027-d332-a188-0de7-f23c91a70cca,
        _:0b2cb027-d332-a189-0de8-f23c91a70cca,
        _:0b2cb027-d332-a18a-0de9-f23c91a70cca,
        _:0b2cb027-d332-a18b-0dea-f23c91a70cca,
        _:0b2cb027-d332-a18c-0deb-f23c91a70cca,
        _:0b2cb027-d332-a18d-0dec-f23c91a70cca,
        _:0b2cb027-d332-a18e-0ded-f23c91a70cca,
        _:0b2cb027-d332-a18f-0dee-f23c91a70cca,
        _:0b2cb027-d332-a190-0def-f23c91a70cca,
        _:0b2cb027-d332-a191-0df0-f23c91a70cca,
        _:0b2cb027-d332-a192-0df1-f23c91a70cca,
        _:0b2cb027-d332-a193-0df2-f23c91a70cca,
        _:0b2cb027-d332-a194-0df3-f23c91a70cca ;
    rdfs:comment "Computer Room Air Conditioner: An FCU designed to condition a computer\nroom.  See `docHaystack::AHUs` and `docHaystack::DataCenters` chapters." ;
    ph:is phIoT:fcu ;
    ph:lib phIoT:lib:phIoT ;
    ph:wikipedia "https://en.wikipedia.org/wiki/Fan_coil_unit"^^xsd:anyURI .

_:0b2cb027-d332-a180-0ddf-f23c91a70cca a phIoT:point ;
    ph:hasTag phIoT:bypass,
        phIoT:damper,
        phIoT:cmd,
        phIoT:point ;
    rdfs:label "{bypass, damper, cmd, point}" .

_:0b2cb027-d332-a181-0de0-f23c91a70cca a phIoT:point ;
    ph:hasTag phIoT:cool,
        phIoT:cmd,
        phIoT:point ;
    rdfs:label "{cool, cmd, point}" .

_:0b2cb027-d332-a182-0de1-f23c91a70cca a phIoT:point ;
    ph:hasTag phIoT:dessicantDehumidifier,
        phIoT:cmd,
        phIoT:point ;
    rdfs:label "{dessicantDehumidifier, cmd, point}" .

_:0b2cb027-d332-a183-0de2-f23c91a70cca a phIoT:duct ;
    ph:hasTag phIoT:discharge,
        phIoT:duct,
        phIoT:equip ;
    rdfs:label "{discharge, duct, equip}" .

_:0b2cb027-d332-a184-0de3-f23c91a70cca a phIoT:duct ;
    ph:hasTag phIoT:economizer,
        phIoT:duct,
        phIoT:equip ;
    rdfs:label "{economizer, duct, equip}" .

_:0b2cb027-d332-a185-0de4-f23c91a70cca a phIoT:point ;
    ph:hasTag phIoT:economizing,
        phIoT:cmd,
        phIoT:point ;
    rdfs:label "{economizing, cmd, point}" .

_:0b2cb027-d332-a186-0de5-f23c91a70cca a phIoT:equip ;
    ph:hasTag phIoT:equip ;
    rdfs:label "{equip}" .

_:0b2cb027-d332-a187-0de6-f23c91a70cca a phIoT:duct ;
    ph:hasTag phIoT:exhaust,
        phIoT:duct,
        phIoT:equip ;
    rdfs:label "{exhaust, duct, equip}" .

_:0b2cb027-d332-a188-0de7-f23c91a70cca a phIoT:point ;
    ph:hasTag phIoT:faceBypass,
        phIoT:cmd,
        phIoT:point ;
    rdfs:label "{faceBypass, cmd, point}" .

_:0b2cb027-d332-a189-0de8-f23c91a70cca a phIoT:point ;
    ph:hasTag phIoT:filter,
        phIoT:sensor,
        phIoT:point ;
    rdfs:label "{filter, sensor, point}" .

_:0b2cb027-d332-a18a-0de9-f23c91a70cca a phIoT:point ;
    ph:hasTag phIoT:freezeStat,
        phIoT:sensor,
        phIoT:point ;
    rdfs:label "{freezeStat, sensor, point}" .

_:0b2cb027-d332-a18b-0dea-f23c91a70cca a phIoT:point ;
    ph:hasTag phIoT:heat,
        phIoT:cmd,
        phIoT:point ;
    rdfs:label "{heat, cmd, point}" .

_:0b2cb027-d332-a18c-0deb-f23c91a70cca a phIoT:point ;
    ph:hasTag phIoT:heatWheel,
        phIoT:cmd,
        phIoT:point ;
    rdfs:label "{heatWheel, cmd, point}" .

_:0b2cb027-d332-a18d-0dec-f23c91a70cca a phIoT:humidifier-equip ;
    ph:hasTag phIoT:humidifier,
        phIoT:equip ;
    rdfs:label "{humidifier, equip}" .

_:0b2cb027-d332-a18e-0ded-f23c91a70cca a phIoT:point ;
    ph:hasTag phIoT:hvacMode,
        phIoT:sp,
        phIoT:point ;
    rdfs:label "{hvacMode, sp, point}" .

_:0b2cb027-d332-a18f-0dee-f23c91a70cca a phIoT:duct ;
    ph:hasTag phIoT:mixed,
        phIoT:duct,
        phIoT:equip ;
    rdfs:label "{mixed, duct, equip}" .

_:0b2cb027-d332-a190-0def-f23c91a70cca a phIoT:duct ;
    ph:hasTag phIoT:outside,
        phIoT:duct,
        phIoT:equip ;
    rdfs:label "{outside, duct, equip}" .

_:0b2cb027-d332-a191-0df0-f23c91a70cca a phIoT:point ;
    ph:hasTag phIoT:point ;
    rdfs:label "{point}" .

_:0b2cb027-d332-a192-0df1-f23c91a70cca a phIoT:duct ;
    ph:hasTag phIoT:return,
        phIoT:duct,
        phIoT:equip ;
    rdfs:label "{return, duct, equip}" .

_:0b2cb027-d332-a193-0df2-f23c91a70cca a phIoT:thermostat ;
    ph:hasTag phIoT:thermostat,
        phIoT:equip ;
    rdfs:label "{thermostat, equip}" .

_:0b2cb027-d332-a194-0df3-f23c91a70cca a phIoT:duct ;
    ph:hasTag phIoT:ventilation,
        phIoT:duct,
        phIoT:equip ;
    rdfs:label "{ventilation, duct, equip}" .

phIoT:cur a owl:Class ;
    rdfs:subClassOf ph:marker ;
    rdfs:label "cur" ;
    rdfs:comment "Supports current value" ;
    ph:is ph:marker ;
    ph:lib phIoT:lib:phIoT ;
    ph:tagOn phIoT:point .

phIoT:cur-point a owl:Class ;
    rdfs:subClassOf phIoT:point ;
    rdfs:label "cur-point" ;
    rdfs:comment "Point with support to report a \"real-time\" current value.  By real-time\nwe typically mean freshness within the order of a few seconds or at\nmost a few minutes.  For systems with direct I/O the current value is\ntypically driven by the I/O scan rate. For overlay systems which acquire\ndata via a protocol such as BACnet or Modbus then the current value\nis typically refreshed using polling or subscription over a network.\nAlso see `docHaystack::Points#cur` chapter." ;
    ph:is phIoT:point ;
    ph:lib phIoT:lib:phIoT .

phIoT:curErr a owl:DatatypeProperty ;
    rdfs:domain phIoT:cur-point ;
    rdfs:range ph:str ;
    rdfs:label "curErr" ;
    rdfs:comment "Error description when `curStatus` indicates error condition" ;
    ph:is ph:str ;
    ph:lib phIoT:lib:phIoT ;
    ph:tagOn phIoT:cur-point ;
    ph:transient ph:marker .

phIoT:curStatus a owl:DatatypeProperty ;
    rdfs:domain phIoT:cur-point ;
    rdfs:range ph:str ;
    rdfs:label "curStatus" ;
    rdfs:comment "Status of point's current value reading.  The `curVal` is only available\nwhen curStatus is \"ok\" or \"stale\".  However a \"stale\" value should\nbe used with caution since the local system does not have a fresh value.\nIt is recommended that the `curVal` tag is removed from a point\nwhen the curStatus is not \"ok\" nor \"stale\"." ;
    ph:enum "- ok: all is okay\n- stale: the point's curVal is not fresh data\n- fault: a configuration or hardware problem - see `curErr`\n- down: a communication or network problem - see `curErr`\n- disabled: manual disable of the point or connector\n- unknown: we don't know anything (usually boot state)\n- remoteFault: point in remote system is fault\n- remoteDown: point in remote system is down\n- remoteDisabled: point in remote system is disabled\n- remoteUnknown: point in remote system is unknown" ;
    ph:is ph:str ;
    ph:lib phIoT:lib:phIoT ;
    ph:tagOn phIoT:cur-point ;
    ph:transient ph:marker .

phIoT:curVal a owl:DatatypeProperty ;
    rdfs:subClassOf rdfs:Literal ;
    rdfs:label "curVal" ;
    rdfs:comment "Current value of a point.  The current value is only available when\nthe `curStatus` is \"ok\" or \"stale\"." ;
    ph:is ph:scalar ;
    ph:lib phIoT:lib:phIoT ;
    ph:tagOn phIoT:cur-point ;
    ph:transient ph:marker .

phScience:current a owl:Class ;
    rdfs:subClassOf ph:marker ;
    rdfs:label "current" ;
    rdfs:comment "Movement of fluid or electricity" ;
    ph:is ph:marker ;
    ph:lib phScience:lib:phScience .

phIoT:current-angle a owl:Class ;
    rdfs:subClassOf phScience:quantity ;
    rdfs:label "current-angle" ;
    rdfs:comment "AC current phase angle" ;
    ph:is phScience:quantity ;
    ph:lib phIoT:lib:phIoT ;
    phScience:prefUnit "deg" ;
    phScience:quantityOf phIoT:ac-elec .

phIoT:current-imbalance a owl:Class ;
    rdfs:subClassOf phScience:quantity ;
    rdfs:label "current-imbalance" ;
    rdfs:comment "AC current phase imbalance. Also referred to as current unbalance." ;
    ph:is phScience:quantity ;
    ph:lib phIoT:lib:phIoT ;
    phScience:prefUnit "%" ;
    phScience:quantityOf phIoT:ac-elec .

phIoT:current-magnitude a owl:Class ;
    rdfs:subClassOf phScience:elec-current ;
    rdfs:label "current-magnitude" ;
    rdfs:comment "Root-mean-square (RMS) magnitude of AC electrical current" ;
    ph:is phScience:elec-current ;
    ph:lib phIoT:lib:phIoT ;
    phScience:prefUnit "A" ;
    phScience:quantityOf phIoT:ac-elec .

phIoT:current-thd a owl:Class ;
    rdfs:subClassOf phScience:quantity ;
    rdfs:label "current-thd" ;
    rdfs:comment "Total harmonic distortion (THD) of AC current" ;
    ph:is phScience:quantity ;
    ph:lib phIoT:lib:phIoT ;
    phScience:prefUnit "%" ;
    phScience:quantityOf phIoT:ac-elec .

phIct:dali a owl:Class ;
    rdfs:subClassOf phIct:protocol ;
    rdfs:label "dali" ;
    rdfs:comment "Digital Addressable Lighting Interface protocol for lighting" ;
    ph:is phIct:protocol ;
    ph:lib phIct:lib:phIct ;
    ph:wikipedia "https://en.wikipedia.org/wiki/Digital_Addressable_Lighting_Interface"^^xsd:anyURI .

phIoT:damper a owl:Class ;
    rdfs:subClassOf ph:marker ;
    rdfs:label "damper" ;
    rdfs:comment "Damper equipment or control point." ;
    ph:is ph:marker ;
    ph:lib phIoT:lib:phIoT ;
    ph:wikipedia "https://en.wikipedia.org/wiki/Damper_(flow)"^^xsd:anyURI .

phIoT:damper-actuator a owl:Class ;
    rdfs:subClassOf phIoT:actuator ;
    rdfs:label "damper-actuator" ;
    ph:children _:0b2cb027-d351-2600-0df4-f23c91a70cca,
        _:0b2cb027-d351-2601-0df5-f23c91a70cca,
        _:0b2cb027-d351-2602-0df6-f23c91a70cca,
        _:0b2cb027-d351-2603-0df7-f23c91a70cca ;
    ph:childrenFlatten phIoT:ductSection ;
    rdfs:comment "Actuator to regulate the flow of air." ;
    ph:is phIoT:actuator ;
    ph:lib phIoT:lib:phIoT ;
    ph:wikipedia "https://en.wikipedia.org/wiki/Damper_(flow)"^^xsd:anyURI .

_:0b2cb027-d351-2600-0df4-f23c91a70cca a phIoT:point ;
    ph:hasTag phIoT:damper,
        phIoT:cmd,
        phIoT:point ;
    rdfs:label "{damper, cmd, point}" .

_:0b2cb027-d351-2601-0df5-f23c91a70cca a phIoT:point ;
    ph:hasTag phIoT:damper,
        phIoT:sensor,
        phIoT:point ;
    rdfs:label "{damper, sensor, point}" .

_:0b2cb027-d351-2602-0df6-f23c91a70cca a phIoT:equip ;
    ph:hasTag phIoT:equip ;
    rdfs:label "{equip}" .

_:0b2cb027-d351-2603-0df7-f23c91a70cca a phIoT:point ;
    ph:hasTag phIoT:point ;
    rdfs:label "{point}" .

phIct:dataCenter a owl:Class ;
    rdfs:subClassOf phIoT:space ;
    rdfs:label "dataCenter" ;
    ph:children _:0b2cb027-d360-6840-0df8-f23c91a70cca,
        _:0b2cb027-d360-6841-0df9-f23c91a70cca,
        _:0b2cb027-d360-6842-0dfa-f23c91a70cca,
        _:0b2cb027-d360-6843-0dfb-f23c91a70cca,
        _:0b2cb027-d360-6844-0dfc-f23c91a70cca ;
    rdfs:comment "Space used to house computer and networking gear.\nSee `docHaystack::DataCenters` chapter." ;
    ph:is phIoT:space ;
    ph:lib phIct:lib:phIct ;
    ph:wikipedia "https://en.wikipedia.org/wiki/Data_center"^^xsd:anyURI .

_:0b2cb027-d360-6840-0df8-f23c91a70cca a phIoT:crac ;
    ph:hasTag phIoT:crac,
        phIoT:fcu,
        phIoT:equip ;
    rdfs:label "{crac, fcu, equip}" .

_:0b2cb027-d360-6841-0df9-f23c91a70cca a phIoT:equip ;
    ph:hasTag phIoT:equip ;
    rdfs:label "{equip}" .

_:0b2cb027-d360-6842-0dfa-f23c91a70cca a phIoT:point ;
    ph:hasTag phIoT:point ;
    rdfs:label "{point}" .

_:0b2cb027-d360-6843-0dfb-f23c91a70cca a phIct:rack ;
    ph:hasTag phIct:rack,
        phIoT:equip ;
    rdfs:label "{rack, equip}" .

_:0b2cb027-d360-6844-0dfc-f23c91a70cca a phIoT:space ;
    ph:hasTag phIoT:space ;
    rdfs:label "{space}" .

ph:date a owl:DatatypeProperty ;
    rdfs:subClassOf xsd:date ;
    rdfs:label "date" ;
    rdfs:comment "ISO 8601 date as year, month, day: '2011-06-07'.\nSee [Kinds chapter]`docHaystack::Kinds#date`." ;
    ph:is ph:scalar ;
    ph:lib ph:lib:ph .

ph:dateTime a owl:DatatypeProperty ;
    rdfs:subClassOf xsd:dateTime ;
    rdfs:label "dateTime" ;
    rdfs:comment "ISO 8601 timestamp followed by timezone identifier.\nSee [Kinds chapter]`docHaystack::Kinds#dateTime`." ;
    ph:is ph:scalar ;
    ph:lib ph:lib:ph .

phScience:daytime a owl:Class ;
    rdfs:subClassOf phScience:quantity ;
    rdfs:label "daytime" ;
    rdfs:comment "Time between sunrise and sunset" ;
    ph:enum "- nighttime: false indicates sun is below horizon\n- daytime: true indicates sun is above horizon" ;
    ph:is phScience:quantity ;
    ph:lib phScience:lib:phScience ;
    phScience:quantityOf phScience:weather .

phIoT:dc a owl:Class ;
    rdfs:subClassOf ph:marker ;
    rdfs:label "dc" ;
    rdfs:comment "Relating to direct current (DC) electricity" ;
    ph:is ph:marker ;
    ph:lib phIoT:lib:phIoT .

phIoT:dc-elec a owl:Class ;
    rdfs:subClassOf phScience:elec ;
    rdfs:label "dc-elec" ;
    rdfs:comment "Direct current electricity" ;
    ph:is phScience:elec ;
    ph:lib phIoT:lib:phIoT ;
    ph:wikipedia "https://en.wikipedia.org/wiki/Direct_current"^^xsd:anyURI .

phIoT:dc-elec-meter a owl:Class ;
    rdfs:subClassOf phIoT:elec-meter ;
    rdfs:label "dc-elec-meter" ;
    ph:children _:0b2cb027-d360-6845-0dfd-f23c91a70cca,
        _:0b2cb027-d360-6846-0dfe-f23c91a70cca ;
    rdfs:comment "DC Electricity meter.\nSee `docHaystack::Meters` chapter." ;
    ph:is phIoT:elec-meter ;
    ph:lib phIoT:lib:phIoT .

_:0b2cb027-d360-6845-0dfd-f23c91a70cca a phIoT:equip ;
    ph:hasTag phIoT:equip ;
    rdfs:label "{equip}" .

_:0b2cb027-d360-6846-0dfe-f23c91a70cca a phIoT:point ;
    ph:hasTag phIoT:point ;
    rdfs:label "{point}" .

phIoT:dc-evse-port a owl:Class ;
    rdfs:subClassOf phIoT:evse-port ;
    rdfs:label "dc-evse-port" ;
    ph:children _:0b2cb027-d360-6847-0dff-f23c91a70cca,
        _:0b2cb027-d360-6848-0e00-f23c91a70cca,
        _:0b2cb027-d360-6849-0e01-f23c91a70cca,
        _:0b2cb027-d360-684a-0e02-f23c91a70cca,
        _:0b2cb027-d360-684b-0e03-f23c91a70cca,
        _:0b2cb027-d360-684c-0e04-f23c91a70cca,
        _:0b2cb027-d360-684d-0e05-f23c91a70cca,
        _:0b2cb027-d360-684e-0e06-f23c91a70cca,
        _:0b2cb027-d360-684f-0e07-f23c91a70cca,
        _:0b2cb027-d360-6850-0e08-f23c91a70cca,
        _:0b2cb027-d360-6851-0e09-f23c91a70cca ;
    rdfs:comment "A DC EVSE port delivers `dc` electricity to a single EV charging inlet\nat a time.  See `docHaystack::EVSE#port` chapter.\n\nTypically a max current or max power setpoint should reference a DC\nEVSE port, but not both.  Usually it is preferred to control a DC EVSE\nport using a max power setpoint." ;
    ph:is phIoT:evse-port ;
    ph:lib phIoT:lib:phIoT ;
    ph:wikipedia "https://en.wikipedia.org/wiki/Charging_station"^^xsd:anyURI .

_:0b2cb027-d360-6847-0dff-f23c91a70cca a phIoT:point ;
    ph:hasTag phIoT:dc,
        phScience:elec,
        phIoT:stateOfCharge,
        phIoT:sensor,
        phIoT:point ;
    rdfs:label "{dc, elec, stateOfCharge, sensor, point}" .

_:0b2cb027-d360-6848-0e00-f23c91a70cca a phIoT:equip ;
    ph:hasTag phIoT:equip ;
    rdfs:label "{equip}" .

_:0b2cb027-d360-6849-0e01-f23c91a70cca a phIoT:cable,
        phIoT:evse-cable ;
    ph:hasTag phIoT:evse,
        phIoT:cable,
        phIoT:equip ;
    rdfs:label "{evse, cable, equip}" .

_:0b2cb027-d360-684a-0e02-f23c91a70cca a phIoT:point ;
    ph:hasTag phIoT:evse,
        phIoT:evseStatus,
        phIoT:sensor,
        phIoT:point ;
    rdfs:label "{evse, evseStatus, sensor, point}" .

_:0b2cb027-d360-684b-0e03-f23c91a70cca a phIoT:point ;
    ph:hasTag phIoT:import,
        phIoT:dc,
        phScience:elec,
        phScience:current,
        ph:max,
        phIoT:sp,
        phIoT:point ;
    rdfs:label "{import, dc, elec, current, max, sp, point}" .

_:0b2cb027-d360-684c-0e04-f23c91a70cca a phIoT:point ;
    ph:hasTag phIoT:import,
        phIoT:dc,
        phScience:elec,
        phScience:current,
        phIoT:sensor,
        phIoT:point ;
    rdfs:label "{import, dc, elec, current, sensor, point}" .

_:0b2cb027-d360-684d-0e05-f23c91a70cca a phIoT:point ;
    ph:hasTag phIoT:import,
        phIoT:dc,
        phScience:elec,
        phScience:energy,
        phIoT:hisTotalized,
        phIoT:sensor,
        phIoT:point ;
    rdfs:label "{import, dc, elec, energy, hisTotalized, sensor, point}" .

_:0b2cb027-d360-684e-0e06-f23c91a70cca a phIoT:point ;
    ph:hasTag phIoT:import,
        phIoT:dc,
        phScience:elec,
        phScience:power,
        ph:max,
        phIoT:sp,
        phIoT:point ;
    rdfs:label "{import, dc, elec, power, max, sp, point}" .

_:0b2cb027-d360-684f-0e07-f23c91a70cca a phIoT:point ;
    ph:hasTag phIoT:import,
        phIoT:dc,
        phScience:elec,
        phScience:power,
        phIoT:sensor,
        phIoT:point ;
    rdfs:label "{import, dc, elec, power, sensor, point}" .

_:0b2cb027-d360-6850-0e08-f23c91a70cca a phIoT:point ;
    ph:hasTag phIoT:import,
        phIoT:dc,
        phScience:elec,
        phScience:volt,
        phIoT:sensor,
        phIoT:point ;
    rdfs:label "{import, dc, elec, volt, sensor, point}" .

_:0b2cb027-d360-6851-0e09-f23c91a70cca a phIoT:point ;
    ph:hasTag phIoT:point ;
    rdfs:label "{point}" .

phIoT:deadband a owl:Class ;
    rdfs:subClassOf ph:marker ;
    rdfs:label "deadband" ;
    rdfs:comment "The range in a process where no changes to output are made.\nMay also indicate the difference between a base setpoint and effective\nsetpoint." ;
    ph:is ph:marker ;
    ph:lib phIoT:lib:phIoT .

ph:def a owl:DatatypeProperty ;
    rdfs:range ph:symbol ;
    rdfs:label "def" ;
    rdfs:comment "Create a new definition bound to the given symbol.\nSee [Defs chapter]`docHaystack::Defs`." ;
    ph:is ph:symbol ;
    ph:lib ph:lib:ph .

ph:defx a owl:DatatypeProperty ;
    rdfs:range ph:symbol ;
    rdfs:label "defx" ;
    rdfs:comment "Extends the given definition with additional meta tags.\nSee [Normalization]`docHaystack::Normalization#defx`." ;
    ph:is ph:symbol ;
    ph:lib ph:lib:ph .

phIoT:delta a owl:Class ;
    rdfs:subClassOf ph:marker ;
    rdfs:label "delta" ;
    rdfs:comment "Differential of fluid between entering and leaving sensors." ;
    ph:is ph:marker ;
    ph:lib phIoT:lib:phIoT .

phIoT:demand a owl:Class ;
    rdfs:subClassOf ph:marker ;
    rdfs:label "demand" ;
    rdfs:comment "Rate required for a process." ;
    ph:is ph:marker ;
    ph:lib phIoT:lib:phIoT .

ph:depends a owl:DatatypeProperty ;
    rdfs:domain ph:lib ;
    rdfs:range ph:list ;
    rdfs:label "depends" ;
    rdfs:comment "List of this library's dependencies.  The dependent libs define the\n[lib namespace]`docHaystack::Namespaces#lib`. Also see\n[Normalization]`docHaystack::Normalization#resolve`." ;
    ph:is ph:list ;
    ph:lib ph:lib:ph ;
    ph:of ph:ref ;
    ph:tagOn ph:lib .

ph:deprecated a owl:Class ;
    rdfs:subClassOf ph:marker ;
    rdfs:label "deprecated" ;
    rdfs:comment "Obsoleted" ;
    ph:is ph:marker ;
    ph:lib ph:lib:ph .

phIoT:design a owl:Class ;
    rdfs:subClassOf ph:marker ;
    rdfs:label "design" ;
    rdfs:comment "Data related to intended design and operating conditions.  This\nincludes sizing and other data specified by design engineers and\nengineered drawings.  Also see `rated`." ;
    ph:is ph:marker ;
    ph:lib phIoT:lib:phIoT .

phIoT:dessicantDehumidifier a owl:Class ;
    rdfs:subClassOf ph:marker ;
    rdfs:label "dessicantDehumidifier" ;
    rdfs:comment "Decreases humidity from air using a substance which absorbs moisture." ;
    ph:is ph:marker ;
    ph:lib phIoT:lib:phIoT .

phIct:device a owl:Class ;
    rdfs:subClassOf ph:entity ;
    rdfs:label "device" ;
    rdfs:comment "Microprocessor based hardware device.  This is the general term for\nall computers, mobile phones, controllers, and I/O modules.\nSee `docHaystack::Devices#networks` chapter." ;
    ph:docTaxonomy ph:marker ;
    ph:is ph:entity ;
    ph:lib phIct:lib:phIct ;
    ph:mandatory ph:marker .

phIct:deviceRef a owl:ObjectProperty ;
    rdfs:range phIct:device ;
    rdfs:label "deviceRef" ;
    rdfs:comment "Device which controls a monitors this entity" ;
    ph:is ph:ref ;
    ph:lib phIct:lib:phIct ;
    ph:of phIct:device .

phScience:dewPoint a owl:Class ;
    rdfs:subClassOf phScience:quantity ;
    rdfs:label "dewPoint" ;
    rdfs:comment "Dew point temperature at which water vapor will form dew" ;
    ph:is phScience:quantity ;
    ph:lib phScience:lib:phScience ;
    phScience:prefUnit "\u00b0C",
        "\u00b0F" ;
    phScience:quantityOf phScience:air .

ph:dict a owl:DatatypeProperty ;
    rdfs:range ph:dict ;
    rdfs:label "dict" ;
    rdfs:comment "Map of name/value tag pairs.\nSee [Kinds chapter]`docHaystack::Kinds#dict`." ;
    ph:is ph:val ;
    ph:lib ph:lib:ph .

phIoT:diesel a owl:Class ;
    rdfs:subClassOf phScience:liquid ;
    rdfs:label "diesel" ;
    rdfs:comment "Liquid fuel specifically designed for use in diesel engines" ;
    ph:is phScience:liquid ;
    ph:lib phIoT:lib:phIoT ;
    ph:wikipedia "https://en.wikipedia.org/wiki/Diesel_fuel"^^xsd:anyURI .

phIoT:directZone a owl:Class ;
    rdfs:subClassOf phIoT:ahuZoneDelivery ;
    rdfs:label "directZone" ;
    rdfs:comment "AHU supplies air directly to the zone" ;
    ph:is phIoT:ahuZoneDelivery ;
    ph:lib phIoT:lib:phIoT .

phScience:direction a owl:Class ;
    rdfs:subClassOf phScience:quantity ;
    rdfs:label "direction" ;
    rdfs:comment "Compass direction measured in degrees: North: 0\u00b0 = 360\u00b0, East: 90\u00b0, South: 180\u00b0, West: 270\u00b0" ;
    ph:is phScience:quantity ;
    ph:lib phScience:lib:phScience ;
    phScience:prefUnit "deg" .

ph:dis a owl:DatatypeProperty ;
    rdfs:domain ph:entity ;
    rdfs:range ph:str ;
    rdfs:label "dis" ;
    rdfs:comment "Display name for an entity.\nSee `docHaystack::Ontology#entities` chapter." ;
    ph:is ph:str ;
    ph:lib ph:lib:ph ;
    ph:tagOn ph:entity .

phIoT:discharge a owl:Class ;
    rdfs:subClassOf phIoT:ductSection ;
    rdfs:label "discharge" ;
    rdfs:comment "Duct for air leaving an equipment" ;
    ph:is phIoT:ductSection ;
    ph:lib phIoT:lib:phIoT .

phIoT:dispenser a owl:Class ;
    rdfs:subClassOf ph:marker ;
    rdfs:label "dispenser" ;
    rdfs:comment "Equipment that releases a specific amount of a substance." ;
    ph:is ph:marker ;
    ph:lib phIoT:lib:phIoT .

phIoT:diverting a owl:Class ;
    rdfs:subClassOf ph:marker ;
    rdfs:label "diverting" ;
    rdfs:comment "Three way valve which inputs one pipe and diverts between two output pipes." ;
    ph:is ph:marker ;
    ph:lib phIoT:lib:phIoT .

phIoT:doas a owl:Class ;
    rdfs:subClassOf phIoT:ahu ;
    rdfs:label "doas" ;
    ph:children _:0b2cb027-d36f-aa80-0e0a-f23c91a70cca,
        _:0b2cb027-d36f-aa81-0e0b-f23c91a70cca,
        _:0b2cb027-d36f-aa82-0e0c-f23c91a70cca,
        _:0b2cb027-d36f-aa83-0e0d-f23c91a70cca,
        _:0b2cb027-d36f-aa84-0e0e-f23c91a70cca,
        _:0b2cb027-d36f-aa85-0e0f-f23c91a70cca,
        _:0b2cb027-d36f-aa86-0e10-f23c91a70cca,
        _:0b2cb027-d36f-aa87-0e11-f23c91a70cca,
        _:0b2cb027-d36f-aa88-0e12-f23c91a70cca,
        _:0b2cb027-d36f-aa89-0e13-f23c91a70cca,
        _:0b2cb027-d36f-aa8a-0e14-f23c91a70cca,
        _:0b2cb027-d36f-aa8b-0e15-f23c91a70cca,
        _:0b2cb027-d36f-aa8c-0e16-f23c91a70cca,
        _:0b2cb027-d36f-aa8d-0e17-f23c91a70cca,
        _:0b2cb027-d36f-aa8e-0e18-f23c91a70cca,
        _:0b2cb027-d36f-aa8f-0e19-f23c91a70cca,
        _:0b2cb027-d36f-aa90-0e1a-f23c91a70cca,
        _:0b2cb027-d36f-aa91-0e1b-f23c91a70cca,
        _:0b2cb027-d36f-aa92-0e1c-f23c91a70cca,
        _:0b2cb027-d36f-aa93-0e1d-f23c91a70cca,
        _:0b2cb027-d36f-aa94-0e1e-f23c91a70cca ;
    rdfs:comment "Dedicated Outside Air System: An AHU that brings in 100% outside air and\nno recirculated air in order to provide ventilation to spaces.\nSee `docHaystack::AHUs` chapter." ;
    ph:is phIoT:ahu ;
    ph:lib phIoT:lib:phIoT ;
    ph:wikipedia "https://en.wikipedia.org/wiki/Air_handler"^^xsd:anyURI .

_:0b2cb027-d36f-aa80-0e0a-f23c91a70cca a phIoT:point ;
    ph:hasTag phIoT:bypass,
        phIoT:damper,
        phIoT:cmd,
        phIoT:point ;
    rdfs:label "{bypass, damper, cmd, point}" .

_:0b2cb027-d36f-aa81-0e0b-f23c91a70cca a phIoT:point ;
    ph:hasTag phIoT:cool,
        phIoT:cmd,
        phIoT:point ;
    rdfs:label "{cool, cmd, point}" .

_:0b2cb027-d36f-aa82-0e0c-f23c91a70cca a phIoT:point ;
    ph:hasTag phIoT:dessicantDehumidifier,
        phIoT:cmd,
        phIoT:point ;
    rdfs:label "{dessicantDehumidifier, cmd, point}" .

_:0b2cb027-d36f-aa83-0e0d-f23c91a70cca a phIoT:duct ;
    ph:hasTag phIoT:discharge,
        phIoT:duct,
        phIoT:equip ;
    rdfs:label "{discharge, duct, equip}" .

_:0b2cb027-d36f-aa84-0e0e-f23c91a70cca a phIoT:duct ;
    ph:hasTag phIoT:economizer,
        phIoT:duct,
        phIoT:equip ;
    rdfs:label "{economizer, duct, equip}" .

_:0b2cb027-d36f-aa85-0e0f-f23c91a70cca a phIoT:point ;
    ph:hasTag phIoT:economizing,
        phIoT:cmd,
        phIoT:point ;
    rdfs:label "{economizing, cmd, point}" .

_:0b2cb027-d36f-aa86-0e10-f23c91a70cca a phIoT:equip ;
    ph:hasTag phIoT:equip ;
    rdfs:label "{equip}" .

_:0b2cb027-d36f-aa87-0e11-f23c91a70cca a phIoT:duct ;
    ph:hasTag phIoT:exhaust,
        phIoT:duct,
        phIoT:equip ;
    rdfs:label "{exhaust, duct, equip}" .

_:0b2cb027-d36f-aa88-0e12-f23c91a70cca a phIoT:point ;
    ph:hasTag phIoT:faceBypass,
        phIoT:cmd,
        phIoT:point ;
    rdfs:label "{faceBypass, cmd, point}" .

_:0b2cb027-d36f-aa89-0e13-f23c91a70cca a phIoT:point ;
    ph:hasTag phIoT:filter,
        phIoT:sensor,
        phIoT:point ;
    rdfs:label "{filter, sensor, point}" .

_:0b2cb027-d36f-aa8a-0e14-f23c91a70cca a phIoT:point ;
    ph:hasTag phIoT:freezeStat,
        phIoT:sensor,
        phIoT:point ;
    rdfs:label "{freezeStat, sensor, point}" .

_:0b2cb027-d36f-aa8b-0e15-f23c91a70cca a phIoT:point ;
    ph:hasTag phIoT:heat,
        phIoT:cmd,
        phIoT:point ;
    rdfs:label "{heat, cmd, point}" .

_:0b2cb027-d36f-aa8c-0e16-f23c91a70cca a phIoT:point ;
    ph:hasTag phIoT:heatWheel,
        phIoT:cmd,
        phIoT:point ;
    rdfs:label "{heatWheel, cmd, point}" .

_:0b2cb027-d36f-aa8d-0e17-f23c91a70cca a phIoT:humidifier-equip ;
    ph:hasTag phIoT:humidifier,
        phIoT:equip ;
    rdfs:label "{humidifier, equip}" .

_:0b2cb027-d36f-aa8e-0e18-f23c91a70cca a phIoT:point ;
    ph:hasTag phIoT:hvacMode,
        phIoT:sp,
        phIoT:point ;
    rdfs:label "{hvacMode, sp, point}" .

_:0b2cb027-d36f-aa8f-0e19-f23c91a70cca a phIoT:duct ;
    ph:hasTag phIoT:mixed,
        phIoT:duct,
        phIoT:equip ;
    rdfs:label "{mixed, duct, equip}" .

_:0b2cb027-d36f-aa90-0e1a-f23c91a70cca a phIoT:duct ;
    ph:hasTag phIoT:outside,
        phIoT:duct,
        phIoT:equip ;
    rdfs:label "{outside, duct, equip}" .

_:0b2cb027-d36f-aa91-0e1b-f23c91a70cca a phIoT:point ;
    ph:hasTag phIoT:point ;
    rdfs:label "{point}" .

_:0b2cb027-d36f-aa92-0e1c-f23c91a70cca a phIoT:duct ;
    ph:hasTag phIoT:return,
        phIoT:duct,
        phIoT:equip ;
    rdfs:label "{return, duct, equip}" .

_:0b2cb027-d36f-aa93-0e1d-f23c91a70cca a phIoT:thermostat ;
    ph:hasTag phIoT:thermostat,
        phIoT:equip ;
    rdfs:label "{thermostat, equip}" .

_:0b2cb027-d36f-aa94-0e1e-f23c91a70cca a phIoT:duct ;
    ph:hasTag phIoT:ventilation,
        phIoT:duct,
        phIoT:equip ;
    rdfs:label "{ventilation, duct, equip}" .

ph:doc a owl:DatatypeProperty ;
    rdfs:domain ph:def ;
    rdfs:range ph:str ;
    rdfs:label "doc" ;
    rdfs:comment "Documentation in simplified flavor of markdown.  The first\nsentence up to the period is used as the summary.\n\nSpecific formatting options:\npre>\n// inline formatting\n*italic*           // italics font\n**bold**           // bold font\n'code'             // code or API term\n`point`            // hyperlink to def (code link)\n[text]`point`      // hyperlink with explicit link text\n![alt]`image.png`  // image\n\n// unordered list\n- one\n- two\n- three\n\n// ordered list; use numbers or letters\n1. one\n2. two\n3. three\n<pre\n\nThe main difference between markdown is that inline code uses single\nticks and hyperlinks are annotated using the backtick.  Links may be:\n  - absolute http/https URIs\n  - def symbol such as \"site\" or \"hot-water\"" ;
    ph:is ph:str ;
    ph:lib ph:lib:ph ;
    ph:tagOn ph:def .

ph:docAssociations a owl:Class ;
    rdfs:subClassOf ph:marker ;
    rdfs:label "docAssociations" ;
    rdfs:comment "Generate a section in the docs for this association." ;
    ph:is ph:marker ;
    ph:lib ph:lib:ph .

ph:docTaxonomy a owl:Class ;
    rdfs:subClassOf ph:marker ;
    rdfs:label "docTaxonomy" ;
    rdfs:comment "Generate a taxonomy tree for this term in the documentationindex.\nWhen applied to a def, then it will will be listed in the docs\nunder the [taxonomies]`docHaystack::Docs#taxonomies` section." ;
    ph:is ph:marker ;
    ph:lib ph:lib:ph ;
    ph:notInherited ph:marker .

phIoT:domestic a owl:Class ;
    rdfs:subClassOf ph:marker ;
    rdfs:label "domestic" ;
    rdfs:comment "For human use" ;
    ph:is ph:marker ;
    ph:lib phIoT:lib:phIoT .

phIoT:domestic-cold-water-system a owl:Class ;
    rdfs:subClassOf phIoT:domestic-water-system ;
    rdfs:label "domestic-cold-water-system" ;
    ph:children _:0b2cb027-d3e9-bc80-0e1f-f23c91a70cca,
        _:0b2cb027-d3e9-bc81-0e20-f23c91a70cca ;
    rdfs:comment "System that circulates potable cold water in its liquid state for purposes\nother than space cooling and process requirements." ;
    ph:is phIoT:domestic-water-system ;
    ph:lib phIoT:lib:phIoT .

_:0b2cb027-d3e9-bc80-0e1f-f23c91a70cca a phIoT:equip ;
    ph:hasTag phIoT:equip ;
    rdfs:label "{equip}" .

_:0b2cb027-d3e9-bc81-0e20-f23c91a70cca a phIoT:point ;
    ph:hasTag phIoT:point ;
    rdfs:label "{point}" .

phIoT:domestic-hot-water-system a owl:Class ;
    rdfs:subClassOf phIoT:domestic-water-system ;
    rdfs:label "domestic-hot-water-system" ;
    ph:children _:0b2cb027-d3e9-bc82-0e21-f23c91a70cca,
        _:0b2cb027-d3e9-bc83-0e22-f23c91a70cca ;
    rdfs:comment "System that circulates potable hot water in its liquid state for purposes\nother than space heating and process requirements." ;
    ph:is phIoT:domestic-water-system ;
    ph:lib phIoT:lib:phIoT .

_:0b2cb027-d3e9-bc82-0e21-f23c91a70cca a phIoT:equip ;
    ph:hasTag phIoT:equip ;
    rdfs:label "{equip}" .

_:0b2cb027-d3e9-bc83-0e22-f23c91a70cca a phIoT:point ;
    ph:hasTag phIoT:point ;
    rdfs:label "{point}" .

phIoT:domestic-water a owl:Class ;
    rdfs:subClassOf phScience:water ;
    rdfs:label "domestic-water" ;
    rdfs:comment "Tap water for drinking, washing, cooking, and flushing of toilets" ;
    ph:is phScience:water ;
    ph:lib phIoT:lib:phIoT ;
    ph:wikipedia "https://en.wikipedia.org/wiki/Water"^^xsd:anyURI .

phIoT:domestic-water-input a owl:Class ;
    rdfs:subClassOf ph:input ;
    rdfs:label "domestic-water-input" ;
    rdfs:comment "Entity inputs domestic water which flows from another entity" ;
    ph:is ph:input ;
    ph:lib phIoT:lib:phIoT .

phIoT:domestic-water-output a owl:Class ;
    rdfs:subClassOf ph:output ;
    rdfs:label "domestic-water-output" ;
    rdfs:comment "Entity outputs domestic water to other entities" ;
    ph:is ph:output ;
    ph:lib phIoT:lib:phIoT .

phIoT:domestic-water-system a owl:Class ;
    rdfs:subClassOf phIoT:water-system ;
    rdfs:label "domestic-water-system" ;
    ph:children _:0b2cb027-d3e9-bc84-0e23-f23c91a70cca,
        _:0b2cb027-d3e9-bc85-0e24-f23c91a70cca ;
    rdfs:comment "System that circulates potable water in its liquid state for purposes\nother than space conditioning and process requirements." ;
    ph:is phIoT:water-system ;
    ph:lib phIoT:lib:phIoT .

_:0b2cb027-d3e9-bc84-0e23-f23c91a70cca a phIoT:equip ;
    ph:hasTag phIoT:equip ;
    rdfs:label "{equip}" .

_:0b2cb027-d3e9-bc85-0e24-f23c91a70cca a phIoT:point ;
    ph:hasTag phIoT:point ;
    rdfs:label "{point}" .

phIoT:domesticWaterRef a owl:ObjectProperty ;
    rdfs:domain phIoT:domestic-water-input ;
    rdfs:range phIoT:domestic-water-output ;
    rdfs:label "domesticWaterRef" ;
    rdfs:comment "Domestic water flows from the referent to this entity" ;
    ph:inputs phIoT:domestic-water ;
    ph:is ph:ref ;
    ph:lib phIoT:lib:phIoT ;
    ph:of phIoT:domestic-water-output ;
    ph:tagOn phIoT:domestic-water-input .

phIoT:dualDuct a owl:Class ;
    rdfs:subClassOf phIoT:ductConfig ;
    rdfs:label "dualDuct" ;
    rdfs:comment "Two ducts: combination of hotDeck, coldDeck, or neutralDeck" ;
    ph:is phIoT:ductConfig ;
    ph:lib phIoT:lib:phIoT .

phIoT:duct a owl:Class ;
    rdfs:subClassOf phIoT:conduit ;
    rdfs:label "duct" ;
    ph:children _:0b2cb027-d3e9-bc86-0e25-f23c91a70cca,
        _:0b2cb027-d3e9-bc87-0e26-f23c91a70cca,
        _:0b2cb027-d3e9-bc88-0e27-f23c91a70cca,
        _:0b2cb027-d3e9-bc89-0e28-f23c91a70cca,
        _:0b2cb027-d3e9-bc8a-0e29-f23c91a70cca,
        _:0b2cb027-d3e9-bc8b-0e2a-f23c91a70cca,
        _:0b2cb027-d3e9-bc8c-0e2b-f23c91a70cca,
        _:0b2cb027-d3e9-bc8d-0e2c-f23c91a70cca,
        _:0b2cb027-d3e9-bc8e-0e2d-f23c91a70cca,
        _:0b2cb027-d3e9-bc8f-0e2e-f23c91a70cca,
        _:0b2cb027-d3e9-bc90-0e2f-f23c91a70cca,
        _:0b2cb027-d3e9-bc91-0e30-f23c91a70cca,
        _:0b2cb027-d3e9-bc92-0e31-f23c91a70cca,
        _:0b2cb027-d3e9-bc93-0e32-f23c91a70cca,
        _:0b2cb027-d3e9-bc94-0e33-f23c91a70cca,
        _:0b2cb027-d3e9-bc95-0e34-f23c91a70cca,
        _:0b2cb027-d3e9-bc96-0e35-f23c91a70cca,
        _:0b2cb027-d3e9-bc97-0e36-f23c91a70cca,
        _:0b2cb027-d3e9-bc98-0e37-f23c91a70cca,
        _:0b2cb027-d3e9-bc99-0e38-f23c91a70cca ;
    ph:childrenFlatten phIoT:ductDeck,
        phIoT:ductSection ;
    rdfs:comment "Conduit used to convey air for HVAC" ;
    ph:is phIoT:conduit ;
    ph:lib phIoT:lib:phIoT ;
    ph:wikipedia "https://en.wikipedia.org/wiki/Duct_(flow)"^^xsd:anyURI .

_:0b2cb027-d3e9-bc86-0e25-f23c91a70cca a phIoT:point ;
    ph:hasTag phScience:air,
        phScience:co2,
        phScience:concentration,
        phIoT:sensor,
        phIoT:point ;
    rdfs:label "{air, co2, concentration, sensor, point}" .

_:0b2cb027-d3e9-bc87-0e26-f23c91a70cca a phIoT:point ;
    ph:hasTag phScience:air,
        phScience:co2,
        phScience:concentration,
        phIoT:sp,
        phIoT:point ;
    rdfs:label "{air, co2, concentration, sp, point}" .

_:0b2cb027-d3e9-bc88-0e27-f23c91a70cca a phIoT:point ;
    ph:hasTag phScience:air,
        phScience:dewPoint,
        phIoT:sensor,
        phIoT:point ;
    rdfs:label "{air, dewPoint, sensor, point}" .

_:0b2cb027-d3e9-bc89-0e28-f23c91a70cca a phIoT:point ;
    ph:hasTag phScience:air,
        phScience:dewPoint,
        phIoT:sp,
        phIoT:point ;
    rdfs:label "{air, dewPoint, sp, point}" .

_:0b2cb027-d3e9-bc8a-0e29-f23c91a70cca a phIoT:point ;
    ph:hasTag phScience:air,
        phScience:enthalpy,
        phIoT:sensor,
        phIoT:point ;
    rdfs:label "{air, enthalpy, sensor, point}" .

_:0b2cb027-d3e9-bc8b-0e2a-f23c91a70cca a phIoT:point ;
    ph:hasTag phScience:air,
        phScience:enthalpy,
        phIoT:sp,
        phIoT:point ;
    rdfs:label "{air, enthalpy, sp, point}" .

_:0b2cb027-d3e9-bc8c-0e2b-f23c91a70cca a phIoT:point ;
    ph:hasTag phScience:air,
        phScience:flow,
        phIoT:sensor,
        phIoT:point ;
    rdfs:label "{air, flow, sensor, point}" .

_:0b2cb027-d3e9-bc8d-0e2c-f23c91a70cca a phIoT:point ;
    ph:hasTag phScience:air,
        phScience:flow,
        phIoT:sp,
        phIoT:point ;
    rdfs:label "{air, flow, sp, point}" .

_:0b2cb027-d3e9-bc8e-0e2d-f23c91a70cca a phIoT:point ;
    ph:hasTag phScience:air,
        phScience:humidity,
        phIoT:sensor,
        phIoT:point ;
    rdfs:label "{air, humidity, sensor, point}" .

_:0b2cb027-d3e9-bc8f-0e2e-f23c91a70cca a phIoT:point ;
    ph:hasTag phScience:air,
        phScience:humidity,
        phIoT:sp,
        phIoT:point ;
    rdfs:label "{air, humidity, sp, point}" .

_:0b2cb027-d3e9-bc90-0e2f-f23c91a70cca a phIoT:point ;
    ph:hasTag phScience:air,
        phScience:pressure,
        phIoT:sensor,
        phIoT:point ;
    rdfs:label "{air, pressure, sensor, point}" .

_:0b2cb027-d3e9-bc91-0e30-f23c91a70cca a phIoT:point ;
    ph:hasTag phScience:air,
        phScience:pressure,
        phIoT:sp,
        phIoT:point ;
    rdfs:label "{air, pressure, sp, point}" .

_:0b2cb027-d3e9-bc92-0e31-f23c91a70cca a phIoT:point ;
    ph:hasTag phScience:air,
        phScience:temp,
        phIoT:sensor,
        phIoT:point ;
    rdfs:label "{air, temp, sensor, point}" .

_:0b2cb027-d3e9-bc93-0e32-f23c91a70cca a phIoT:point ;
    ph:hasTag phScience:air,
        phScience:temp,
        phIoT:sp,
        phIoT:point ;
    rdfs:label "{air, temp, sp, point}" .

_:0b2cb027-d3e9-bc94-0e33-f23c91a70cca a phIoT:coolingCoil ;
    ph:hasTag phIoT:coolingCoil,
        phIoT:equip ;
    rdfs:label "{coolingCoil, equip}" .

_:0b2cb027-d3e9-bc95-0e34-f23c91a70cca a phIoT:damper-actuator ;
    ph:hasTag phIoT:damper,
        phIoT:actuator,
        phIoT:equip ;
    rdfs:label "{damper, actuator, equip}" .

_:0b2cb027-d3e9-bc96-0e35-f23c91a70cca a phIoT:equip ;
    ph:hasTag phIoT:equip ;
    rdfs:label "{equip}" .

_:0b2cb027-d3e9-bc97-0e36-f23c91a70cca a phIoT:fan-motor ;
    ph:hasTag phIoT:fan,
        phIoT:motor,
        phIoT:equip ;
    rdfs:label "{fan, motor, equip}" .

_:0b2cb027-d3e9-bc98-0e37-f23c91a70cca a phIoT:heatingCoil ;
    ph:hasTag phIoT:heatingCoil,
        phIoT:equip ;
    rdfs:label "{heatingCoil, equip}" .

_:0b2cb027-d3e9-bc99-0e38-f23c91a70cca a phIoT:point ;
    ph:hasTag phIoT:point ;
    rdfs:label "{point}" .

phIoT:ductArea a owl:Class ;
    rdfs:subClassOf ph:marker ;
    rdfs:label "ductArea" ;
    rdfs:comment "Config point on a `vav` for duct area measured in ft\u00b2 or m\u00b2" ;
    ph:is ph:marker ;
    ph:lib phIoT:lib:phIoT .

phIoT:ductConfig a owl:Class ;
    rdfs:subClassOf ph:choice ;
    rdfs:label "ductConfig" ;
    rdfs:comment "Ductwork configuration" ;
    ph:is ph:choice ;
    ph:lib phIoT:lib:phIoT ;
    ph:tagOn phIoT:airHandlingEquip,
        phIoT:airTerminalUnit .

phIoT:ductDeck a owl:Class ;
    rdfs:subClassOf ph:choice ;
    rdfs:label "ductDeck" ;
    rdfs:comment "Cold, hot, or neutral deck. Can be applied to 'ahu' equip if the AHU\nis part of a 'dualDuct' or 'tripleDuct' system but only serves a single\ndeck type." ;
    ph:is ph:choice ;
    ph:lib phIoT:lib:phIoT ;
    ph:tagOn phIoT:duct,
        phIoT:airHandlingEquip .

phIoT:ductSection a owl:Class ;
    rdfs:subClassOf ph:choice ;
    rdfs:label "ductSection" ;
    rdfs:comment "Equipment section of ductwork" ;
    ph:is ph:choice ;
    ph:lib phIoT:lib:phIoT ;
    ph:tagOn phIoT:duct,
        phIoT:damper-actuator,
        phIoT:fan-motor .

ph:duration a owl:DatatypeProperty ;
    rdfs:range ph:number ;
    rdfs:label "duration" ;
    rdfs:comment "Number with a unit of time" ;
    ph:is ph:number ;
    ph:lib ph:lib:ph .

phIoT:dxCooling a owl:Class ;
    rdfs:subClassOf phIoT:coolingProcess ;
    rdfs:label "dxCooling" ;
    rdfs:comment "Cooling using direct expansion of a refrigerant vapor.\nAlso see `dxHeating` and `heatPump`." ;
    ph:is phIoT:coolingProcess ;
    ph:lib phIoT:lib:phIoT .

phIoT:dxHeating a owl:Class ;
    rdfs:subClassOf phIoT:heatingProcess ;
    rdfs:label "dxHeating" ;
    rdfs:comment "Heating using direct expansion of a refrigerant vapor.\nAlso see `dxCooling` and `heatPump`." ;
    ph:is phIoT:heatingProcess ;
    ph:lib phIoT:lib:phIoT .

phIoT:economizer a owl:Class ;
    rdfs:subClassOf phIoT:ductSection ;
    rdfs:label "economizer" ;
    rdfs:comment "Duct to access fresh outside air only for economizing, not ventilation" ;
    ph:is phIoT:ductSection ;
    ph:lib phIoT:lib:phIoT .

phIoT:economizing a owl:Class ;
    rdfs:subClassOf ph:marker ;
    rdfs:label "economizing" ;
    rdfs:comment "Energy reduction mode which augments heating/cooling with outside air." ;
    ph:is ph:marker ;
    ph:lib phIoT:lib:phIoT .

phIoT:effective a owl:Class ;
    rdfs:subClassOf ph:marker ;
    rdfs:label "effective" ;
    rdfs:comment "Current control setpoint in effect taking into account other factors" ;
    ph:is ph:marker ;
    ph:lib phIoT:lib:phIoT .

phIoT:efficiency a owl:Class ;
    rdfs:subClassOf ph:marker ;
    rdfs:label "efficiency" ;
    rdfs:comment "Efficiency point of a chiller measured in \"COP\" or \"kW/ton\"." ;
    ph:is ph:marker ;
    ph:lib phIoT:lib:phIoT .

phScience:elec a owl:Class ;
    rdfs:subClassOf phScience:phenomenon ;
    rdfs:label "elec" ;
    rdfs:comment "Associated with electricity or with electrical force, power, or energy.\nThis is often opposed to `mech` mechanical energy." ;
    ph:is phScience:phenomenon ;
    ph:lib phScience:lib:phScience ;
    ph:wikipedia "https://en.wikipedia.org/wiki/Electricity"^^xsd:anyURI .

phScience:elec-current a owl:Class ;
    rdfs:subClassOf phScience:quantity ;
    rdfs:label "elec-current" ;
    rdfs:comment "Electrical current" ;
    ph:is phScience:quantity ;
    ph:lib phScience:lib:phScience ;
    phScience:quantityOf phScience:elec .

phIoT:elec-demand a owl:Class ;
    rdfs:subClassOf phIoT:active-power ;
    rdfs:label "elec-demand" ;
    rdfs:comment "Active power averaged over a regular interval.  For utility meters\nthe demand interval is based on the billing period." ;
    ph:is phIoT:active-power ;
    ph:lib phIoT:lib:phIoT ;
    phScience:prefUnit "kW" ;
    phScience:quantityOf phIoT:ac-elec ;
    ph:wikipedia "https://en.wikipedia.org/wiki/Electric_power"^^xsd:anyURI .

phScience:elec-energy a owl:Class ;
    rdfs:subClassOf phScience:energy ;
    rdfs:label "elec-energy" ;
    rdfs:comment "Electrical energy; integral of electric power" ;
    ph:is phScience:energy ;
    ph:lib phScience:lib:phScience ;
    phScience:prefUnit "kWh" ;
    phScience:quantityOf phScience:elec ;
    ph:wikipedia "https://en.wikipedia.org/wiki/Electrical_energy"^^xsd:anyURI .

phIoT:elec-input a owl:Class ;
    rdfs:subClassOf ph:input ;
    rdfs:label "elec-input" ;
    rdfs:comment "Entity inputs electricity which flows from another entity" ;
    ph:is ph:input ;
    ph:lib phIoT:lib:phIoT .

phIoT:elec-meter a owl:Class ;
    rdfs:subClassOf phIoT:meter,
        phIoT:elec-input,
        phIoT:elec-output ;
    rdfs:label "elec-meter" ;
    ph:children _:0b2cb027-d408-4100-0e39-f23c91a70cca,
        _:0b2cb027-d408-4101-0e3a-f23c91a70cca ;
    rdfs:comment "Electricity meter" ;
    ph:is phIoT:meter,
        phIoT:elec-input,
        phIoT:elec-output ;
    ph:lib phIoT:lib:phIoT .

_:0b2cb027-d408-4100-0e39-f23c91a70cca a phIoT:equip ;
    ph:hasTag phIoT:equip ;
    rdfs:label "{equip}" .

_:0b2cb027-d408-4101-0e3a-f23c91a70cca a phIoT:point ;
    ph:hasTag phIoT:point ;
    rdfs:label "{point}" .

phIoT:elec-output a owl:Class ;
    rdfs:subClassOf ph:output ;
    rdfs:label "elec-output" ;
    rdfs:comment "Entity outputs electricity to other entities" ;
    ph:is ph:output ;
    ph:lib phIoT:lib:phIoT .

phIoT:elec-panel a owl:Class ;
    rdfs:subClassOf phIoT:panel,
        phIoT:elec-input,
        phIoT:elec-output ;
    rdfs:label "elec-panel" ;
    ph:children _:0b2cb027-d408-4102-0e3b-f23c91a70cca,
        _:0b2cb027-d408-4103-0e3c-f23c91a70cca ;
    rdfs:comment "Physical housing for electrical circuits, fuses, and breakers.\nSee `docHaystack::ElecPanels#panels` chapter." ;
    ph:is phIoT:panel,
        phIoT:elec-input,
        phIoT:elec-output ;
    ph:lib phIoT:lib:phIoT ;
    ph:wikipedia "https://en.wikipedia.org/wiki/Distribution_board"^^xsd:anyURI .

_:0b2cb027-d408-4102-0e3b-f23c91a70cca a phIoT:equip ;
    ph:hasTag phIoT:equip ;
    rdfs:label "{equip}" .

_:0b2cb027-d408-4103-0e3c-f23c91a70cca a phIoT:point ;
    ph:hasTag phIoT:point ;
    rdfs:label "{point}" .

phScience:elec-power a owl:Class ;
    rdfs:subClassOf phScience:power ;
    rdfs:label "elec-power" ;
    rdfs:comment "Rate of electrical energy transfer; energy transfer per unit time" ;
    ph:is phScience:power ;
    ph:lib phScience:lib:phScience ;
    phScience:prefUnit "kW" ;
    phScience:quantityOf phScience:elec ;
    ph:wikipedia "https://en.wikipedia.org/wiki/Electric_power"^^xsd:anyURI .

phIoT:elec-system a owl:Class ;
    rdfs:subClassOf phIoT:system ;
    rdfs:label "elec-system" ;
    ph:children _:0b2cb027-d408-4104-0e3d-f23c91a70cca,
        _:0b2cb027-d408-4105-0e3e-f23c91a70cca ;
    rdfs:comment "System that generates, converts, distributes, and/or stores electricity." ;
    ph:is phIoT:system ;
    ph:lib phIoT:lib:phIoT .

_:0b2cb027-d408-4104-0e3d-f23c91a70cca a phIoT:equip ;
    ph:hasTag phIoT:equip ;
    rdfs:label "{equip}" .

_:0b2cb027-d408-4105-0e3e-f23c91a70cca a phIoT:point ;
    ph:hasTag phIoT:point ;
    rdfs:label "{point}" .

phScience:elec-volt a owl:Class ;
    rdfs:subClassOf phScience:quantity ;
    rdfs:label "elec-volt" ;
    rdfs:comment "Electrical voltage, potential difference" ;
    ph:is phScience:quantity ;
    ph:lib phScience:lib:phScience ;
    phScience:quantityOf phScience:elec .

phIoT:elecHeating a owl:Class ;
    rdfs:subClassOf phIoT:heatingProcess,
        phIoT:elec-input ;
    rdfs:label "elecHeating" ;
    rdfs:comment "Heating by the conversion of electrical energy" ;
    ph:is phIoT:heatingProcess,
        phIoT:elec-input ;
    ph:lib phIoT:lib:phIoT ;
    ph:wikipedia "https://en.wikipedia.org/wiki/Electric_heating"^^xsd:anyURI .

phIoT:elecLine a owl:DatatypeProperty ;
    rdfs:range ph:str ;
    rdfs:label "elecLine" ;
    rdfs:comment "Single-phase line measurement of an electric quantity in a multi-phase\nAC electric power system." ;
    ph:enum "- L1: line 1 measurement\n- L2: line 2 measurement\n- L3: line 3 measurement" ;
    ph:is ph:str ;
    ph:lib phIoT:lib:phIoT .

phIoT:elecLineToLine a owl:DatatypeProperty ;
    rdfs:range ph:str ;
    rdfs:label "elecLineToLine" ;
    rdfs:comment "Single-phase electric quantity measured line-to-line in a multi-phase AC\nelectric power system." ;
    ph:enum "- L1-L2: line 1 to line 2 measurement\n- L2-L3: line 2 to line 3 measurement\n- L3-L1: line 3 to line 1 measurement" ;
    ph:is ph:str ;
    ph:lib phIoT:lib:phIoT .

phIoT:elecLineToNeutral a owl:DatatypeProperty ;
    rdfs:range ph:str ;
    rdfs:label "elecLineToNeutral" ;
    rdfs:comment "Single-phase electric quantity measured line-to-neutral in a multi-phase\nAC electric power system." ;
    ph:enum "- L1-N: line 1 to neutral measurement\n- L2-N: line 2 to neutral measurement\n- L3-N: line 3 to neutral measurement" ;
    ph:is ph:str ;
    ph:lib phIoT:lib:phIoT .

phIoT:elecRef a owl:ObjectProperty ;
    rdfs:domain phIoT:elec-input ;
    rdfs:range phIoT:elec-output ;
    rdfs:label "elecRef" ;
    rdfs:comment "Electricity flows from the referent to this entity" ;
    ph:inputs phScience:elec ;
    ph:is ph:ref ;
    ph:lib phIoT:lib:phIoT ;
    ph:of phIoT:elec-output ;
    ph:tagOn phIoT:elec-input .

phIoT:elevator a owl:Class ;
    rdfs:subClassOf phIoT:verticalTransport,
        phIoT:elec-input ;
    rdfs:label "elevator" ;
    ph:children _:0b2cb027-d408-4106-0e3f-f23c91a70cca,
        _:0b2cb027-d408-4107-0e40-f23c91a70cca ;
    rdfs:comment "Enclosure used to move people between floors." ;
    ph:is phIoT:verticalTransport,
        phIoT:elec-input ;
    ph:lib phIoT:lib:phIoT ;
    ph:wikipedia "https://en.wikipedia.org/wiki/Elevator"^^xsd:anyURI .

_:0b2cb027-d408-4106-0e3f-f23c91a70cca a phIoT:equip ;
    ph:hasTag phIoT:equip ;
    rdfs:label "{equip}" .

_:0b2cb027-d408-4107-0e40-f23c91a70cca a phIoT:point ;
    ph:hasTag phIoT:point ;
    rdfs:label "{point}" .

phScience:emission a owl:Class ;
    rdfs:subClassOf phScience:quantity ;
    rdfs:label "emission" ;
    rdfs:comment "Amount of a substance discharged into the air" ;
    ph:is phScience:quantity ;
    ph:lib phScience:lib:phScience ;
    phScience:quantityOf phScience:air .

phIoT:enable a owl:Class ;
    rdfs:subClassOf ph:marker ;
    rdfs:label "enable" ;
    rdfs:comment "Secondary on/off `point` of an `equip` especially used with a `vfd`.\nEnable is used with Bool points where true indicates on and false\nindicates off.  Equip with an enable should always also define a `run`\npoint which indicates the primary on/off state of the equipment." ;
    ph:is ph:marker ;
    ph:lib phIoT:lib:phIoT .

phScience:energy a owl:Class ;
    rdfs:subClassOf phScience:quantity ;
    rdfs:label "energy" ;
    rdfs:comment "Measure of ability to do work" ;
    ph:is phScience:quantity ;
    ph:lib phScience:lib:phScience .

phIoT:entering a owl:Class ;
    rdfs:subClassOf phIoT:pipeSection ;
    rdfs:label "entering" ;
    rdfs:comment "Pipe conveys fluid into an equipment" ;
    ph:is phIoT:pipeSection ;
    ph:lib phIoT:lib:phIoT .

phScience:enthalpy a owl:Class ;
    rdfs:subClassOf phScience:quantity ;
    rdfs:label "enthalpy" ;
    rdfs:comment "Total heat content of a system. It is defined as internal energy of the system plus the product of pressure and volume." ;
    ph:is phScience:quantity ;
    ph:lib phScience:lib:phScience ;
    phScience:prefUnit "kJ/kg",
        "BTU/lb" ;
    phScience:quantityOf phScience:air .

ph:entity a owl:Class ;
    rdfs:subClassOf ph:marker ;
    rdfs:label "entity" ;
    rdfs:comment "Top-level dicts with a unique identifier.\nSee `docHaystack::Ontology#entities` chapter." ;
    ph:is ph:marker ;
    ph:lib ph:lib:ph .

ph:enum a owl:DatatypeProperty ;
    rdfs:domain ph:def,
        phIoT:point ;
    rdfs:range ph:enum ;
    rdfs:label "enum" ;
    rdfs:comment "Defines an eumeration of string key names.  The range may also be applied\nto format a Bool ordered as \"false,true\".  The value of this tag may be\nformatted in one of five ways:\n - dict of dicts keyed by name and Dict values for meta such as 'doc' tag\n - comma separated names on one line\n - names separated by a \"\\n\" newline character\n - markdown unordered list formatted as a series of \"- name: description\\n\"\n - ref to a Xeto 'sys::Enum' spec\n\nEnum names *should* follow valid tag naming rules (start with lowercase\nASCII letter and contain only ASCII letters and numbers).  However in\ncases where mapping directly to external enumerations enum names can\ncontain arbitrary characters such as space." ;
    ph:is ph:val ;
    ph:lib ph:lib:ph ;
    ph:tagOn ph:def,
        phIoT:point .

phIoT:equip a owl:Class ;
    rdfs:subClassOf ph:entity ;
    rdfs:label "equip" ;
    ph:children _:0b2cb027-d408-4108-0e41-f23c91a70cca,
        _:0b2cb027-d408-4109-0e42-f23c91a70cca ;
    rdfs:comment "Equipment asset.\nSee `docHaystack::Equips` chapter." ;
    ph:docTaxonomy ph:marker ;
    ph:is ph:entity ;
    ph:lib phIoT:lib:phIoT ;
    ph:mandatory ph:marker .

_:0b2cb027-d408-4108-0e41-f23c91a70cca a phIoT:equip ;
    ph:hasTag phIoT:equip ;
    rdfs:label "{equip}" .

_:0b2cb027-d408-4109-0e42-f23c91a70cca a phIoT:point ;
    ph:hasTag phIoT:point ;
    rdfs:label "{point}" .

phIoT:equipRef a owl:ObjectProperty ;
    rdfs:domain phIct:controller,
        phIoT:equip,
        phIoT:point ;
    rdfs:range phIoT:equip ;
    rdfs:label "equipRef" ;
    ph:containedBy phIoT:equip ;
    rdfs:comment "Reference to equip which contains this entity" ;
    ph:is ph:ref ;
    ph:lib phIoT:lib:phIoT ;
    ph:of phIoT:equip ;
    ph:tagOn phIct:controller,
        phIoT:equip,
        phIoT:point .

phIoT:escalator a owl:Class ;
    rdfs:subClassOf phIoT:verticalTransport,
        phIoT:elec-input ;
    rdfs:label "escalator" ;
    ph:children _:0b2cb027-d445-4a00-0e43-f23c91a70cca,
        _:0b2cb027-d445-4a01-0e44-f23c91a70cca ;
    rdfs:comment "Moving staircase used to move people between floors." ;
    ph:is phIoT:verticalTransport,
        phIoT:elec-input ;
    ph:lib phIoT:lib:phIoT ;
    ph:wikipedia "https://en.wikipedia.org/wiki/Escalator"^^xsd:anyURI .

_:0b2cb027-d445-4a00-0e43-f23c91a70cca a phIoT:equip ;
    ph:hasTag phIoT:equip ;
    rdfs:label "{equip}" .

_:0b2cb027-d445-4a01-0e44-f23c91a70cca a phIoT:point ;
    ph:hasTag phIoT:point ;
    rdfs:label "{point}" .

phIoT:evaporator a owl:Class ;
    rdfs:subClassOf ph:marker ;
    rdfs:label "evaporator" ;
    rdfs:comment "Mechanism used to convert a refrigerant from its liquid to gaseous state." ;
    ph:is ph:marker ;
    ph:lib phIoT:lib:phIoT .

phIoT:evse a owl:Class ;
    rdfs:subClassOf ph:marker ;
    rdfs:label "evse" ;
    rdfs:comment "Electric Vehicle Supply Equipment.  See `docHaystack::EVSE` chapter." ;
    ph:is ph:marker ;
    ph:lib phIoT:lib:phIoT ;
    ph:wikipedia "https://en.wikipedia.org/wiki/Charging_station"^^xsd:anyURI .

phIoT:evse-cable a owl:Class ;
    rdfs:subClassOf phIoT:evse-equip ;
    rdfs:label "evse-cable" ;
    ph:children _:0b2cb027-d445-4a02-0e45-f23c91a70cca,
        _:0b2cb027-d445-4a03-0e46-f23c91a70cca ;
    rdfs:comment "The electrical cable between an `evse-port` and an EV charging inlet\non a vehicle. The `evseCableType` tag distinguishes the type of cable.\nSee `docHaystack::EVSE#cable` chapter." ;
    ph:is phIoT:evse-equip ;
    ph:lib phIoT:lib:phIoT ;
    ph:wikipedia "https://en.wikipedia.org/wiki/Charging_station"^^xsd:anyURI .

_:0b2cb027-d445-4a02-0e45-f23c91a70cca a phIoT:equip ;
    ph:hasTag phIoT:equip ;
    rdfs:label "{equip}" .

_:0b2cb027-d445-4a03-0e46-f23c91a70cca a phIoT:point ;
    ph:hasTag phIoT:point ;
    rdfs:label "{point}" .

phIoT:evse-dispenser a owl:Class ;
    rdfs:subClassOf phIoT:evse-equip ;
    rdfs:label "evse-dispenser" ;
    ph:children _:0b2cb027-d445-4a04-0e47-f23c91a70cca,
        _:0b2cb027-d445-4a05-0e48-f23c91a70cca,
        _:0b2cb027-d445-4a06-0e49-f23c91a70cca,
        _:0b2cb027-d445-4a07-0e4a-f23c91a70cca,
        _:0b2cb027-d445-4a08-0e4b-f23c91a70cca,
        _:0b2cb027-d445-4a09-0e4c-f23c91a70cca ;
    rdfs:comment "Equipment that dispenses electricity to an EV.  It consists of a\nphysical EVSE enclosure and its contents to which an `evse-cable`\nattaches.  An `evse-dispenser` can contain zero or more `evse-port`.\n\nChildren points are used to describe or control one or more `evse-port`\nwithin the EVSE manufacturer's package.\n\nSee `docHaystack::EVSE#dispenser` chapter." ;
    ph:is phIoT:evse-equip ;
    ph:lib phIoT:lib:phIoT ;
    ph:wikipedia "https://en.wikipedia.org/wiki/Charging_station"^^xsd:anyURI .

_:0b2cb027-d445-4a04-0e47-f23c91a70cca a phIoT:equip ;
    ph:hasTag phIoT:equip ;
    rdfs:label "{equip}" .

_:0b2cb027-d445-4a05-0e48-f23c91a70cca a phIoT:point ;
    ph:hasTag phIoT:evse,
        phIoT:evseStatus,
        phIoT:sensor,
        phIoT:point ;
    rdfs:label "{evse, evseStatus, sensor, point}" .

_:0b2cb027-d445-4a06-0e49-f23c91a70cca a phIoT:evse-port ;
    ph:hasTag phIoT:evse,
        phIoT:port,
        phIoT:equip ;
    rdfs:label "{evse, port, equip}" .

_:0b2cb027-d445-4a07-0e4a-f23c91a70cca a phIoT:point ;
    ph:hasTag phIoT:import,
        phIoT:ac,
        phScience:elec,
        phScience:magnitude,
        phScience:current,
        ph:max,
        phIoT:sp,
        phIoT:point ;
    rdfs:label "{import, ac, elec, magnitude, current, max, sp, point}" .

_:0b2cb027-d445-4a08-0e4b-f23c91a70cca a phIoT:point ;
    ph:hasTag phIoT:import,
        phIoT:dc,
        phScience:elec,
        phScience:power,
        ph:max,
        phIoT:sp,
        phIoT:point ;
    rdfs:label "{import, dc, elec, power, max, sp, point}" .

_:0b2cb027-d445-4a09-0e4c-f23c91a70cca a phIoT:point ;
    ph:hasTag phIoT:point ;
    rdfs:label "{point}" .

phIoT:evse-equip a owl:Class ;
    rdfs:subClassOf phIoT:equip,
        phIoT:elec-input,
        phIoT:elec-output ;
    rdfs:label "evse-equip" ;
    ph:children _:0b2cb027-d454-8c40-0e4d-f23c91a70cca,
        _:0b2cb027-d454-8c41-0e4e-f23c91a70cca ;
    rdfs:comment "Equipment that supports the delivery of electricity to charging inlets\nlocated on EVs.  See `docHaystack::EVSE` chapter." ;
    ph:is phIoT:equip,
        phIoT:elec-input,
        phIoT:elec-output ;
    ph:lib phIoT:lib:phIoT ;
    ph:wikipedia "https://en.wikipedia.org/wiki/Charging_station"^^xsd:anyURI .

_:0b2cb027-d454-8c40-0e4d-f23c91a70cca a phIoT:equip ;
    ph:hasTag phIoT:equip ;
    rdfs:label "{equip}" .

_:0b2cb027-d454-8c41-0e4e-f23c91a70cca a phIoT:point ;
    ph:hasTag phIoT:point ;
    rdfs:label "{point}" .

phIoT:evse-port a owl:Class ;
    rdfs:subClassOf phIoT:evse-equip,
        phIoT:elec-meter ;
    rdfs:label "evse-port" ;
    ph:children _:0b2cb027-d454-8c42-0e4f-f23c91a70cca,
        _:0b2cb027-d463-ce80-0e50-f23c91a70cca,
        _:0b2cb027-d463-ce81-0e51-f23c91a70cca,
        _:0b2cb027-d463-ce82-0e52-f23c91a70cca ;
    rdfs:comment "An EVSE port delivers electricity to a single EV charging inlet at a\ntime.  Comprised of a software-controlled electrical contactor or\ncircuit breaker.  Typically contained within an `evse-dispenser`, but\nmay be contained within an `evse-powerConverter`.  More than one\n`evse-cable` may be connected to a single `evse-port`, however, only one\nmay be energized at any given time.\n\nNote:  In the future we might add an entity that describes `evse-port`\ncontained in an AC distribution panel.  This scenario is not common.\n\nSee `docHaystack::EVSE#port` chapter." ;
    ph:is phIoT:evse-equip,
        phIoT:elec-meter ;
    ph:lib phIoT:lib:phIoT ;
    ph:wikipedia "https://en.wikipedia.org/wiki/Charging_station"^^xsd:anyURI .

_:0b2cb027-d454-8c42-0e4f-f23c91a70cca a phIoT:equip ;
    ph:hasTag phIoT:equip ;
    rdfs:label "{equip}" .

_:0b2cb027-d463-ce80-0e50-f23c91a70cca a phIoT:cable,
        phIoT:evse-cable ;
    ph:hasTag phIoT:evse,
        phIoT:cable,
        phIoT:equip ;
    rdfs:label "{evse, cable, equip}" .

_:0b2cb027-d463-ce81-0e51-f23c91a70cca a phIoT:point ;
    ph:hasTag phIoT:evse,
        phIoT:evseStatus,
        phIoT:sensor,
        phIoT:point ;
    rdfs:label "{evse, evseStatus, sensor, point}" .

_:0b2cb027-d463-ce82-0e52-f23c91a70cca a phIoT:point ;
    ph:hasTag phIoT:point ;
    rdfs:label "{point}" .

phIoT:evse-powerConverter a owl:Class ;
    rdfs:subClassOf phIoT:evse-equip ;
    rdfs:label "evse-powerConverter" ;
    ph:children _:0b2cb027-d463-ce83-0e53-f23c91a70cca,
        _:0b2cb027-d463-ce84-0e54-f23c91a70cca,
        _:0b2cb027-d463-ce85-0e55-f23c91a70cca,
        _:0b2cb027-d463-ce86-0e56-f23c91a70cca,
        _:0b2cb027-d463-ce87-0e57-f23c91a70cca ;
    rdfs:comment "A power converter that has a `dc` electrical output applied to a\n`dc-evse-port`.  May be contained within an `evse-dispenser` or in a\nseparate dedicated equipment enclosure.\n\nChildren points are used to describe or control one or more `evse-port`\nwithin the EVSE manufacturer's package.\n\nSee `docHaystack::EVSE#powerConverter` chapter." ;
    ph:is phIoT:evse-equip ;
    ph:lib phIoT:lib:phIoT ;
    ph:wikipedia "https://en.wikipedia.org/wiki/Charging_station"^^xsd:anyURI .

_:0b2cb027-d463-ce83-0e53-f23c91a70cca a phIoT:equip ;
    ph:hasTag phIoT:equip ;
    rdfs:label "{equip}" .

_:0b2cb027-d463-ce84-0e54-f23c91a70cca a phIoT:point ;
    ph:hasTag phIoT:evse,
        phIoT:evseStatus,
        phIoT:sensor,
        phIoT:point ;
    rdfs:label "{evse, evseStatus, sensor, point}" .

_:0b2cb027-d463-ce85-0e55-f23c91a70cca a phIoT:evse-port ;
    ph:hasTag phIoT:evse,
        phIoT:port,
        phIoT:equip ;
    rdfs:label "{evse, port, equip}" .

_:0b2cb027-d463-ce86-0e56-f23c91a70cca a phIoT:point ;
    ph:hasTag phIoT:import,
        phIoT:dc,
        phScience:elec,
        phScience:power,
        ph:max,
        phIoT:sp,
        phIoT:point ;
    rdfs:label "{import, dc, elec, power, max, sp, point}" .

_:0b2cb027-d463-ce87-0e57-f23c91a70cca a phIoT:point ;
    ph:hasTag phIoT:point ;
    rdfs:label "{point}" .

phIoT:evse-system a owl:Class ;
    rdfs:subClassOf phIoT:elec-system ;
    rdfs:label "evse-system" ;
    ph:children _:0b2cb027-d463-ce88-0e58-f23c91a70cca,
        _:0b2cb027-d463-ce89-0e59-f23c91a70cca ;
    rdfs:comment "A system that supplies electricity to EVSE assembly equipment and its\nauxiliary loads." ;
    ph:is phIoT:elec-system ;
    ph:lib phIoT:lib:phIoT .

_:0b2cb027-d463-ce88-0e58-f23c91a70cca a phIoT:equip ;
    ph:hasTag phIoT:equip ;
    rdfs:label "{equip}" .

_:0b2cb027-d463-ce89-0e59-f23c91a70cca a phIoT:point ;
    ph:hasTag phIoT:point ;
    rdfs:label "{point}" .

phIoT:evseCableType a owl:DatatypeProperty ;
    rdfs:domain phIoT:evse-cable ;
    rdfs:range ph:str ;
    rdfs:label "evseCableType" ;
    rdfs:comment "Physical type of `evse-cable`." ;
    ph:enum "- ccs1:  CCS1 charging cable\n- ccs2:  CCS2 charging cable\n- chademo:  CHAdeMO charging cable\n- saeJ3400:  SAE J3400 charging cable\n- saeJ1772:  SAE J1772 charging cable\n- saeJ3068:  SAE J3068 charging cable\n- iecType2:  IEC 62196 Type 2 charging cable\n- mcs:  Megawatt Charging System charging cable\n- gbt:  GB/T charging cable" ;
    ph:is ph:str ;
    ph:lib phIoT:lib:phIoT ;
    ph:tagOn phIoT:evse-cable .

phIoT:evseSession a owl:Class ;
    rdfs:subClassOf ph:entity ;
    rdfs:label "evseSession" ;
    rdfs:comment "Describes an event during which an `evse-port` can deliver power to an EV.\nThe EVSE may need to authorize a user to initiate an `evseSession`.\n\nAt minimum has the following data:\n - ts:  when the event was logged by the system of record\n - started:  when the event started\n - stopped:  when the event stopped\n - tx:  transaction ID for the event\n - targetRef:  reference to the `evse-port`\n - energyDelivered:  energy delivered during the `evseSession`\n - event:  marker tag\n - meterStart:  meter register's value at the beginning of the `evseSession`\n\nIn the future additional data might be included, such as the means of\nEV charging session authorization." ;
    ph:is ph:entity ;
    ph:lib phIoT:lib:phIoT ;
    ph:mandatory ph:marker .

phIoT:evseStatus a owl:DatatypeProperty ;
    rdfs:range ph:str ;
    rdfs:label "evseStatus" ;
    rdfs:comment "Status of one or more `evse-port` reported by an EVSE.\n\nWhen applied to an `evse-port`, indicates the status of an EVSE port.\n\nWhen applied to an `evse-dispenser` or `evse-powerConverter`, indicates\nthe status of one or more `evse-port` within an EVSE manufacturer's\npackage.  In this case only the enum values available, unavailable,\nand fault apply." ;
    ph:enum "- available:  When the point references an `evse-port`, indicates the\n  `evse-port` is available for recharging a vehicle.  During this\n  condition none of the `evse-cable` that reference the `evse-port` are\n  plugged into a vehicle charging inlet.  Also, a parked vehicle may\n  prohibit another vehicle from recharging.\n\n  When the point references `evse-dispenser` or `evse-powerConverter`,\n  indicates `evse-port` within the EVSE manufacturer's package are\n  available for an `evseSession` and may actively be in one.  Also, an\n  `evse-port` may have another `evseStatus` based on its condition.\n- preparing:  After an `evse-port` is no longer available and before an\n  `evseSession` begins.  Typically this condition applies during the\n  authorization of an `evseSession`.  This value is deprecated in favor\n  of the occupied value.\n- charging:  When there is an active `evseSession` and the contactor\n  for the `evse-port` is closed.  This value is deprecated in favor of\n  the occupied value.\n- suspendedEVSE:  When the `evse-port` is occupied and not within an\n  active `evseSession` due to inavailability of power to deliver to the\n  vehicle or an unsuccessful attempt to establish an `evseSession`.\n  This value is deprecated in favor of the occupied value.\n- suspendedEV:  When a vehicle does not accept power being offered by\n  the `evse-port` during an active `evseSession`.  This value is\n  deprecated in favor of the occupied value.\n- finishing:  After an `evseSession` when the `evse-port` is still\n  occupied.  This value is deprecated in favor of the occupied value.\n- occupied:  When an `evse-cable` that references the `evse-port` is\n  plugged into a vehicle's charging inlet.  During this condition the\n  `evse-port` may or may not be within an active `evseSession`.\n- reserved:  When the `evse-port` is dedicated to a specific user.\n  During this condition only the intended user can authorize an\n  `evseSession` with their vehicle.  An unauthorized user and their\n  parked vehicle may prohibit an authorized user from recharging.\n- unavailable:  When the EVSE prohibits EV charging on the `evse-port`\n  due to an applied software setting for the `evse-port` or EVSE\n  manufacturer's package.\n- fault:  When the EVSE prohibits EV charging on the `evse-port` due to\n  a fault condition within the `evse-port` or EVSE manufacturer's\n  package." ;
    ph:is ph:str ;
    ph:lib phIoT:lib:phIoT .

phIoT:exhaust a owl:Class ;
    rdfs:subClassOf phIoT:ductSection ;
    rdfs:label "exhaust" ;
    rdfs:comment "Duct used to expel air back outside" ;
    ph:is phIoT:ductSection ;
    ph:lib phIoT:lib:phIoT .

phIoT:export a owl:Class ;
    rdfs:subClassOf ph:marker ;
    rdfs:label "export" ;
    rdfs:comment "Supplied out of a system" ;
    ph:is ph:marker ;
    ph:lib phIoT:lib:phIoT .

phIoT:extraction a owl:Class ;
    rdfs:subClassOf ph:marker ;
    rdfs:label "extraction" ;
    rdfs:comment "Taking a substance out of another substance" ;
    ph:is ph:marker ;
    ph:lib phIoT:lib:phIoT .

phIoT:faceBypass a owl:Class ;
    rdfs:subClassOf ph:marker ;
    rdfs:label "faceBypass" ;
    rdfs:comment "Point of an ahu indicating air flow is by-passing the heating/cooling\ncoils. If a boolean point, then true indicates the unit is in by-pass\nmode and false indicates by-pass is disabled. If the point is an analog\npoint then 100% indicates full by-pass mode and 0% indicates by-pass is\ncompletely disabled." ;
    ph:is ph:marker ;
    ph:lib phIoT:lib:phIoT .

phIoT:fan a owl:Class ;
    rdfs:subClassOf ph:marker ;
    rdfs:label "fan" ;
    rdfs:comment "Fan equipment or control point" ;
    ph:is ph:marker ;
    ph:lib phIoT:lib:phIoT ;
    ph:wikipedia "https://en.wikipedia.org/wiki/Fan_(machine)"^^xsd:anyURI .

phIoT:fan-motor a owl:Class ;
    rdfs:subClassOf phIoT:motor ;
    rdfs:label "fan-motor" ;
    ph:children _:0b2cb027-d473-10c0-0e5a-f23c91a70cca,
        _:0b2cb027-d473-10c1-0e5b-f23c91a70cca,
        _:0b2cb027-d473-10c2-0e5c-f23c91a70cca,
        _:0b2cb027-d473-10c3-0e5d-f23c91a70cca,
        _:0b2cb027-d473-10c4-0e5e-f23c91a70cca,
        _:0b2cb027-d473-10c5-0e5f-f23c91a70cca,
        _:0b2cb027-d473-10c6-0e60-f23c91a70cca,
        _:0b2cb027-d473-10c7-0e61-f23c91a70cca,
        _:0b2cb027-d473-10c8-0e62-f23c91a70cca,
        _:0b2cb027-d473-10c9-0e63-f23c91a70cca,
        _:0b2cb027-d473-10ca-0e64-f23c91a70cca ;
    ph:childrenFlatten phIoT:ductSection,
        phIoT:fan ;
    rdfs:comment "Motor used with a fan to create air flow.\nSee `docHaystack::Motors` chapter." ;
    ph:is phIoT:motor ;
    ph:lib phIoT:lib:phIoT ;
    ph:wikipedia "https://en.wikipedia.org/wiki/Fan_(machine)"^^xsd:anyURI .

_:0b2cb027-d473-10c0-0e5a-f23c91a70cca a phIoT:point ;
    ph:hasTag phIoT:alarm,
        phIoT:sensor,
        phIoT:point ;
    rdfs:label "{alarm, sensor, point}" .

_:0b2cb027-d473-10c1-0e5b-f23c91a70cca a phIoT:point ;
    ph:hasTag phIoT:enable,
        phIoT:cmd,
        phIoT:point ;
    rdfs:label "{enable, cmd, point}" .

_:0b2cb027-d473-10c2-0e5c-f23c91a70cca a phIoT:point ;
    ph:hasTag phIoT:enable,
        phIoT:sensor,
        phIoT:point ;
    rdfs:label "{enable, sensor, point}" .

_:0b2cb027-d473-10c3-0e5d-f23c91a70cca a phIoT:equip ;
    ph:hasTag phIoT:equip ;
    rdfs:label "{equip}" .

_:0b2cb027-d473-10c4-0e5e-f23c91a70cca a phIoT:point ;
    ph:hasTag phIoT:point ;
    rdfs:label "{point}" .

_:0b2cb027-d473-10c5-0e5f-f23c91a70cca a phIoT:point ;
    ph:hasTag phIoT:run,
        phIoT:cmd,
        phIoT:point ;
    rdfs:label "{run, cmd, point}" .

_:0b2cb027-d473-10c6-0e60-f23c91a70cca a phIoT:point ;
    ph:hasTag phIoT:run,
        phIoT:sensor,
        phIoT:point ;
    rdfs:label "{run, sensor, point}" .

_:0b2cb027-d473-10c7-0e61-f23c91a70cca a phIoT:point ;
    ph:hasTag phIoT:vfd,
        phScience:freq,
        phIoT:cmd,
        phIoT:point ;
    rdfs:label "{vfd, freq, cmd, point}" .

_:0b2cb027-d473-10c8-0e62-f23c91a70cca a phIoT:point ;
    ph:hasTag phIoT:vfd,
        phScience:freq,
        phIoT:sensor,
        phIoT:point ;
    rdfs:label "{vfd, freq, sensor, point}" .

_:0b2cb027-d473-10c9-0e63-f23c91a70cca a phIoT:point ;
    ph:hasTag phIoT:vfd,
        phScience:speed,
        phIoT:cmd,
        phIoT:point ;
    rdfs:label "{vfd, speed, cmd, point}" .

_:0b2cb027-d473-10ca-0e64-f23c91a70cca a phIoT:point ;
    ph:hasTag phIoT:vfd,
        phScience:speed,
        phIoT:sensor,
        phIoT:point ;
    rdfs:label "{vfd, speed, sensor, point}" .

phIoT:fanPowered a owl:Class ;
    rdfs:subClassOf ph:marker ;
    rdfs:label "fanPowered" ;
    rdfs:comment "Device with a fan" ;
    ph:is ph:marker ;
    ph:lib phIoT:lib:phIoT .

phIoT:fcu a owl:Class ;
    rdfs:subClassOf phIoT:airHandlingEquip ;
    rdfs:label "fcu" ;
    ph:children _:0b2cb027-d473-10cb-0e65-f23c91a70cca,
        _:0b2cb027-d473-10cc-0e66-f23c91a70cca,
        _:0b2cb027-d473-10cd-0e67-f23c91a70cca,
        _:0b2cb027-d473-10ce-0e68-f23c91a70cca,
        _:0b2cb027-d473-10cf-0e69-f23c91a70cca,
        _:0b2cb027-d473-10d0-0e6a-f23c91a70cca,
        _:0b2cb027-d473-10d1-0e6b-f23c91a70cca,
        _:0b2cb027-d473-10d2-0e6c-f23c91a70cca,
        _:0b2cb027-d473-10d3-0e6d-f23c91a70cca,
        _:0b2cb027-d473-10d4-0e6e-f23c91a70cca,
        _:0b2cb027-d473-10d5-0e6f-f23c91a70cca,
        _:0b2cb027-d473-10d6-0e70-f23c91a70cca,
        _:0b2cb027-d473-10d7-0e71-f23c91a70cca,
        _:0b2cb027-d473-10d8-0e72-f23c91a70cca,
        _:0b2cb027-d473-10d9-0e73-f23c91a70cca,
        _:0b2cb027-d473-10da-0e74-f23c91a70cca,
        _:0b2cb027-d473-10db-0e75-f23c91a70cca,
        _:0b2cb027-d473-10dc-0e76-f23c91a70cca,
        _:0b2cb027-d473-10dd-0e77-f23c91a70cca,
        _:0b2cb027-d473-10de-0e78-f23c91a70cca,
        _:0b2cb027-d473-10df-0e79-f23c91a70cca ;
    rdfs:comment "Fan Coil Unit: A unitary, factory-made enclosure with a fan and coil\nthat recirculates air in a space and performs one or more of the\nfunctions of cleaning, heating, cooling, humidifying, dehumidifying,\nor ventilating the air. Unit heaters are examples of FCUs.\nSee `docHaystack::AHUs` chapter." ;
    ph:is phIoT:airHandlingEquip ;
    ph:lib phIoT:lib:phIoT ;
    ph:mandatory ph:marker ;
    ph:wikipedia "https://en.wikipedia.org/wiki/Fan_coil_unit"^^xsd:anyURI .

_:0b2cb027-d473-10cb-0e65-f23c91a70cca a phIoT:point ;
    ph:hasTag phIoT:bypass,
        phIoT:damper,
        phIoT:cmd,
        phIoT:point ;
    rdfs:label "{bypass, damper, cmd, point}" .

_:0b2cb027-d473-10cc-0e66-f23c91a70cca a phIoT:point ;
    ph:hasTag phIoT:cool,
        phIoT:cmd,
        phIoT:point ;
    rdfs:label "{cool, cmd, point}" .

_:0b2cb027-d473-10cd-0e67-f23c91a70cca a phIoT:point ;
    ph:hasTag phIoT:dessicantDehumidifier,
        phIoT:cmd,
        phIoT:point ;
    rdfs:label "{dessicantDehumidifier, cmd, point}" .

_:0b2cb027-d473-10ce-0e68-f23c91a70cca a phIoT:duct ;
    ph:hasTag phIoT:discharge,
        phIoT:duct,
        phIoT:equip ;
    rdfs:label "{discharge, duct, equip}" .

_:0b2cb027-d473-10cf-0e69-f23c91a70cca a phIoT:duct ;
    ph:hasTag phIoT:economizer,
        phIoT:duct,
        phIoT:equip ;
    rdfs:label "{economizer, duct, equip}" .

_:0b2cb027-d473-10d0-0e6a-f23c91a70cca a phIoT:point ;
    ph:hasTag phIoT:economizing,
        phIoT:cmd,
        phIoT:point ;
    rdfs:label "{economizing, cmd, point}" .

_:0b2cb027-d473-10d1-0e6b-f23c91a70cca a phIoT:equip ;
    ph:hasTag phIoT:equip ;
    rdfs:label "{equip}" .

_:0b2cb027-d473-10d2-0e6c-f23c91a70cca a phIoT:duct ;
    ph:hasTag phIoT:exhaust,
        phIoT:duct,
        phIoT:equip ;
    rdfs:label "{exhaust, duct, equip}" .

_:0b2cb027-d473-10d3-0e6d-f23c91a70cca a phIoT:point ;
    ph:hasTag phIoT:faceBypass,
        phIoT:cmd,
        phIoT:point ;
    rdfs:label "{faceBypass, cmd, point}" .

_:0b2cb027-d473-10d4-0e6e-f23c91a70cca a phIoT:point ;
    ph:hasTag phIoT:filter,
        phIoT:sensor,
        phIoT:point ;
    rdfs:label "{filter, sensor, point}" .

_:0b2cb027-d473-10d5-0e6f-f23c91a70cca a phIoT:point ;
    ph:hasTag phIoT:freezeStat,
        phIoT:sensor,
        phIoT:point ;
    rdfs:label "{freezeStat, sensor, point}" .

_:0b2cb027-d473-10d6-0e70-f23c91a70cca a phIoT:point ;
    ph:hasTag phIoT:heat,
        phIoT:cmd,
        phIoT:point ;
    rdfs:label "{heat, cmd, point}" .

_:0b2cb027-d473-10d7-0e71-f23c91a70cca a phIoT:point ;
    ph:hasTag phIoT:heatWheel,
        phIoT:cmd,
        phIoT:point ;
    rdfs:label "{heatWheel, cmd, point}" .

_:0b2cb027-d473-10d8-0e72-f23c91a70cca a phIoT:humidifier-equip ;
    ph:hasTag phIoT:humidifier,
        phIoT:equip ;
    rdfs:label "{humidifier, equip}" .

_:0b2cb027-d473-10d9-0e73-f23c91a70cca a phIoT:point ;
    ph:hasTag phIoT:hvacMode,
        phIoT:sp,
        phIoT:point ;
    rdfs:label "{hvacMode, sp, point}" .

_:0b2cb027-d473-10da-0e74-f23c91a70cca a phIoT:duct ;
    ph:hasTag phIoT:mixed,
        phIoT:duct,
        phIoT:equip ;
    rdfs:label "{mixed, duct, equip}" .

_:0b2cb027-d473-10db-0e75-f23c91a70cca a phIoT:duct ;
    ph:hasTag phIoT:outside,
        phIoT:duct,
        phIoT:equip ;
    rdfs:label "{outside, duct, equip}" .

_:0b2cb027-d473-10dc-0e76-f23c91a70cca a phIoT:point ;
    ph:hasTag phIoT:point ;
    rdfs:label "{point}" .

_:0b2cb027-d473-10dd-0e77-f23c91a70cca a phIoT:duct ;
    ph:hasTag phIoT:return,
        phIoT:duct,
        phIoT:equip ;
    rdfs:label "{return, duct, equip}" .

_:0b2cb027-d473-10de-0e78-f23c91a70cca a phIoT:thermostat ;
    ph:hasTag phIoT:thermostat,
        phIoT:equip ;
    rdfs:label "{thermostat, equip}" .

_:0b2cb027-d473-10df-0e79-f23c91a70cca a phIoT:duct ;
    ph:hasTag phIoT:ventilation,
        phIoT:duct,
        phIoT:equip ;
    rdfs:label "{ventilation, duct, equip}" .

ph:feature rdfs:label "feature" ;
    rdfs:comment "Feature namespace of definitions formatted as 'feature:name'" ;
    ph:docTaxonomy ph:marker ;
    ph:lib ph:lib:ph .

phScience:feelsLike a owl:Class ;
    rdfs:subClassOf phScience:quantity ;
    rdfs:label "feelsLike" ;
    rdfs:comment "Apparent temperature perceived when considering humidity, wind chill, and heat index" ;
    ph:is phScience:quantity ;
    ph:lib phScience:lib:phScience ;
    phScience:prefUnit "\u00b0C",
        "\u00b0F" ;
    phScience:quantityOf phScience:air .

ph:fileExt a owl:DatatypeProperty ;
    rdfs:domain ph:filetype ;
    rdfs:range ph:str ;
    rdfs:label "fileExt" ;
    rdfs:comment "Filename extension such as \"csv\"" ;
    ph:is ph:str ;
    ph:lib ph:lib:ph ;
    ph:tagOn ph:filetype .

ph:filetype rdfs:label "filetype" ;
    rdfs:comment "File format type definition" ;
    ph:is ph:feature ;
    ph:lib ph:lib:ph .

ph:filetype:csv rdfs:label "CSV" ;
    ph:dis "CSV" ;
    rdfs:comment "Comma Separated Values - see `docHaystack::Csv`" ;
    ph:fileExt "csv" ;
    ph:is ph:filetype ;
    ph:lib ph:lib:ph ;
    ph:mime "text/csv" ;
    ph:wikipedia "https://wikipedia.org/wiki/Comma-separated_values"^^xsd:anyURI .

ph:filetype:json rdfs:label "JSON" ;
    ph:dis "JSON" ;
    rdfs:comment "Haystack JavaScript Object Notation format - see `docHaystack::Json`" ;
    ph:fileExt "json" ;
    ph:is ph:filetype ;
    ph:lib ph:lib:ph ;
    ph:mime "application/json" ;
    ph:wikipedia "https://wikipedia.org/wiki/JSON"^^xsd:anyURI .

ph:filetype:jsonld rdfs:label "JSON-LD" ;
    ph:dis "JSON-LD" ;
    rdfs:comment "JavaScript Object Notation for Linked Data - see `docHaystack::Rdf`" ;
    ph:fileExt "jsonld" ;
    ph:is ph:filetype ;
    ph:lib ph:lib:ph ;
    ph:mime "application/ld+json" ;
    ph:wikipedia "https://wikipedia.org/wiki/JSON-LD"^^xsd:anyURI .

ph:filetype:trio rdfs:label "Trio" ;
    ph:dis "Trio" ;
    rdfs:comment "Haystack Tag Record Input Output - see `docHaystack::Trio`" ;
    ph:fileExt "trio" ;
    ph:is ph:filetype ;
    ph:lib ph:lib:ph ;
    ph:mime "text/trio" .

ph:filetype:turtle rdfs:label "Turtle" ;
    ph:dis "Turtle" ;
    rdfs:comment "RDF Turtle - see `docHaystack::Rdf`" ;
    ph:fileExt "ttl" ;
    ph:is ph:filetype ;
    ph:lib ph:lib:ph ;
    ph:mime "text/turtle" ;
    ph:wikipedia "https://wikipedia.org/wiki/Turtle_(syntax)"^^xsd:anyURI .

ph:filetype:zinc rdfs:label "Zinc" ;
    ph:dis "Zinc" ;
    rdfs:comment "Haystack typed CSV format - see `docHaystack::Zinc`" ;
    ph:fileExt "zinc" ;
    ph:is ph:filetype ;
    ph:lib ph:lib:ph ;
    ph:mime "text/zinc" .

phIoT:filter a owl:Class ;
    rdfs:subClassOf ph:marker ;
    rdfs:label "filter" ;
    rdfs:comment "Related to an air or fluid filter." ;
    ph:is ph:marker ;
    ph:lib phIoT:lib:phIoT .

ph:filterStr a owl:DatatypeProperty ;
    rdfs:range ph:str ;
    rdfs:label "filterStr" ;
    rdfs:comment "Haystack filter string.  See `docHaystack::Filters`" ;
    ph:is ph:str ;
    ph:lib ph:lib:ph .

phIoT:floor a owl:Class ;
    rdfs:subClassOf phIoT:space ;
    rdfs:label "floor" ;
    ph:children _:0b2cb027-d4bf-5c00-0e7a-f23c91a70cca,
        _:0b2cb027-d4bf-5c01-0e7b-f23c91a70cca,
        _:0b2cb027-d4bf-5c02-0e7c-f23c91a70cca ;
    rdfs:comment "Storey of a building.  See `docHaystack::Spaces#floors` chapter." ;
    ph:is phIoT:space ;
    ph:lib phIoT:lib:phIoT ;
    ph:wikipedia "https://en.wikipedia.org/wiki/Storey"^^xsd:anyURI .

_:0b2cb027-d4bf-5c00-0e7a-f23c91a70cca a phIoT:equip ;
    ph:hasTag phIoT:equip ;
    rdfs:label "{equip}" .

_:0b2cb027-d4bf-5c01-0e7b-f23c91a70cca a phIoT:point ;
    ph:hasTag phIoT:point ;
    rdfs:label "{point}" .

_:0b2cb027-d4bf-5c02-0e7c-f23c91a70cca a phIoT:space ;
    ph:hasTag phIoT:space ;
    rdfs:label "{space}" .

phIoT:floorNum a owl:DatatypeProperty ;
    rdfs:domain phIoT:floor ;
    rdfs:range ph:number ;
    rdfs:label "floorNum" ;
    rdfs:comment "Unitless integer indicating the floor's distance from ground level.  The\nground floor is always defined as zero.  Additional floors above ground are\nnumbered 1, 2, 3, etc.  Subterranean floors are numbered -1, -2, -3, etc.\nThis convention is consistent with how most European buildings number\nfloors.  In North America its common to label the ground floor\nas the first floor; however Haystack requires the ground level to be\nassigned a floorNum of 0." ;
    ph:is ph:int ;
    ph:lib phIoT:lib:phIoT ;
    ph:tagOn phIoT:floor .

phScience:flow a owl:Class ;
    rdfs:subClassOf phScience:quantity ;
    rdfs:label "flow" ;
    rdfs:comment "Measure of volumetric flow of fluid" ;
    ph:is phScience:quantity ;
    ph:lib phScience:lib:phScience ;
    phScience:prefUnit "m\u00b3/s",
        "gal/min" ;
    phScience:quantityOf phScience:fluid ;
    ph:wikipedia "https://en.wikipedia.org/wiki/Fluid_dynamics"^^xsd:anyURI .

phIoT:flow-meter a owl:Class ;
    rdfs:subClassOf phIoT:meter ;
    rdfs:label "flow-meter" ;
    ph:children _:0b2cb027-d4bf-5c03-0e7d-f23c91a70cca,
        _:0b2cb027-d4bf-5c04-0e7e-f23c91a70cca ;
    rdfs:comment "Meter to measure flow rate and total volume of fluid.\nSee `docHaystack::Meters` chapter." ;
    ph:is phIoT:meter ;
    ph:lib phIoT:lib:phIoT .

_:0b2cb027-d4bf-5c03-0e7d-f23c91a70cca a phIoT:equip ;
    ph:hasTag phIoT:equip ;
    rdfs:label "{equip}" .

_:0b2cb027-d4bf-5c04-0e7e-f23c91a70cca a phIoT:point ;
    ph:hasTag phIoT:point ;
    rdfs:label "{point}" .

phIoT:flowInverter a owl:Class ;
    rdfs:subClassOf phIoT:equip ;
    rdfs:label "flowInverter" ;
    ph:children _:0b2cb027-d4bf-5c05-0e7f-f23c91a70cca,
        _:0b2cb027-d4bf-5c06-0e80-f23c91a70cca ;
    rdfs:comment "System to change direction of substance flow " ;
    ph:is phIoT:equip ;
    ph:lib phIoT:lib:phIoT .

_:0b2cb027-d4bf-5c05-0e7f-f23c91a70cca a phIoT:equip ;
    ph:hasTag phIoT:equip ;
    rdfs:label "{equip}" .

_:0b2cb027-d4bf-5c06-0e80-f23c91a70cca a phIoT:point ;
    ph:hasTag phIoT:point ;
    rdfs:label "{point}" .

phIoT:flue a owl:Class ;
    rdfs:subClassOf phIoT:ductSection ;
    rdfs:label "flue" ;
    rdfs:comment "Duct for exhausting combustion" ;
    ph:is phIoT:ductSection ;
    ph:lib phIoT:lib:phIoT ;
    ph:wikipedia "https://en.wikipedia.org/wiki/Flue"^^xsd:anyURI .

phScience:fluid a owl:Class ;
    rdfs:subClassOf phScience:substance ;
    rdfs:label "fluid" ;
    rdfs:comment "Liquid or gas" ;
    ph:is phScience:substance ;
    ph:lib phScience:lib:phScience ;
    ph:wikipedia "https://en.wikipedia.org/wiki/Fluid"^^xsd:anyURI .

phScience:flux a owl:Class ;
    rdfs:subClassOf ph:marker ;
    rdfs:label "flux" ;
    rdfs:comment "Measurement through a given surface" ;
    ph:is ph:marker ;
    ph:lib phScience:lib:phScience .

phIoT:freezeStat a owl:Class ;
    rdfs:subClassOf ph:marker ;
    rdfs:label "freezeStat" ;
    rdfs:comment "A boolean point of an ahu indicating a freezing condition.  This\nmight require a control sequence to protect the equipment. If true\nthen a freeze condition is detected, or false if not." ;
    ph:is ph:marker ;
    ph:lib phIoT:lib:phIoT .

phScience:freq a owl:Class ;
    rdfs:subClassOf phScience:quantity ;
    rdfs:label "freq" ;
    rdfs:comment "Occurrences per unit time" ;
    ph:is phScience:quantity ;
    ph:lib phScience:lib:phScience ;
    phScience:prefUnit "Hz" .

phIct:ftp a owl:Class ;
    rdfs:subClassOf phIct:protocol ;
    rdfs:label "ftp" ;
    rdfs:comment "File Transfer Protocol" ;
    ph:is phIct:protocol ;
    ph:lib phIct:lib:phIct ;
    ph:wikipedia "https://en.wikipedia.org/wiki/File_Transfer_Protocol"^^xsd:anyURI .

phIoT:fuelOil a owl:Class ;
    rdfs:subClassOf phScience:liquid ;
    rdfs:label "fuelOil" ;
    rdfs:comment "Petroleum based oil burned for energy" ;
    ph:is phScience:liquid ;
    ph:lib phIoT:lib:phIoT ;
    ph:wikipedia "https://en.wikipedia.org/wiki/Fuel_oil"^^xsd:anyURI .

phIoT:fuelOil-input a owl:Class ;
    rdfs:subClassOf ph:input ;
    rdfs:label "fuelOil-input" ;
    rdfs:comment "Entity inputs fuel oil which flows from another entity" ;
    ph:is ph:input ;
    ph:lib phIoT:lib:phIoT .

phIoT:fuelOil-output a owl:Class ;
    rdfs:subClassOf ph:output ;
    rdfs:label "fuelOil-output" ;
    rdfs:comment "Entity outputs fuel oil to other entities" ;
    ph:is ph:output ;
    ph:lib phIoT:lib:phIoT .

phIoT:fuelOilHeating a owl:Class ;
    rdfs:subClassOf phIoT:heatingProcess,
        phIoT:fuelOil-input ;
    rdfs:label "fuelOilHeating" ;
    rdfs:comment "Heating by the combustion of fuel oil" ;
    ph:is phIoT:heatingProcess,
        phIoT:fuelOil-input ;
    ph:lib phIoT:lib:phIoT .

phIoT:fuelOilRef a owl:ObjectProperty ;
    rdfs:domain phIoT:fuelOil-input ;
    rdfs:range phIoT:fuelOil-output ;
    rdfs:label "fuelOilRef" ;
    rdfs:comment "Fuel oil flows from the referent to this entity" ;
    ph:inputs phIoT:fuelOil ;
    ph:is ph:ref ;
    ph:lib phIoT:lib:phIoT ;
    ph:of phIoT:fuelOil-output ;
    ph:tagOn phIoT:fuelOil-input .

phIoT:fumeHood a owl:Class ;
    rdfs:subClassOf phIoT:equip,
        phIoT:elec-input ;
    rdfs:label "fumeHood" ;
    ph:children _:0b2cb027-d4ce-9e40-0e81-f23c91a70cca,
        _:0b2cb027-d4ce-9e41-0e82-f23c91a70cca,
        _:0b2cb027-d4ce-9e42-0e83-f23c91a70cca,
        _:0b2cb027-d4ce-9e43-0e84-f23c91a70cca,
        _:0b2cb027-d4ce-9e44-0e85-f23c91a70cca,
        _:0b2cb027-d4ce-9e45-0e86-f23c91a70cca,
        _:0b2cb027-d4ce-9e46-0e87-f23c91a70cca ;
    rdfs:comment "Ventilation equipment to limit exposure to hazardous fumes." ;
    ph:is phIoT:equip,
        phIoT:elec-input ;
    ph:lib phIoT:lib:phIoT ;
    ph:wikipedia "https://en.wikipedia.org/wiki/Fume_hood"^^xsd:anyURI .

_:0b2cb027-d4ce-9e40-0e81-f23c91a70cca a phIoT:point ;
    ph:hasTag phScience:air,
        phScience:flow,
        phIoT:sensor,
        phIoT:point ;
    rdfs:label "{air, flow, sensor, point}" .

_:0b2cb027-d4ce-9e41-0e82-f23c91a70cca a phIoT:point ;
    ph:hasTag phScience:air,
        phScience:flow,
        phIoT:sp,
        phIoT:point ;
    rdfs:label "{air, flow, sp, point}" .

_:0b2cb027-d4ce-9e42-0e83-f23c91a70cca a phIoT:point ;
    ph:hasTag phScience:air,
        phScience:velocity,
        phIoT:sensor,
        phIoT:point ;
    rdfs:label "{air, velocity, sensor, point}" .

_:0b2cb027-d4ce-9e43-0e84-f23c91a70cca a phIoT:point ;
    ph:hasTag phScience:air,
        phScience:velocity,
        phIoT:sp,
        phIoT:point ;
    rdfs:label "{air, velocity, sp, point}" .

_:0b2cb027-d4ce-9e44-0e85-f23c91a70cca a phIoT:point ;
    ph:hasTag phIoT:alarm,
        phIoT:sensor,
        phIoT:point ;
    rdfs:label "{alarm, sensor, point}" .

_:0b2cb027-d4ce-9e45-0e86-f23c91a70cca a phIoT:equip ;
    ph:hasTag phIoT:equip ;
    rdfs:label "{equip}" .

_:0b2cb027-d4ce-9e46-0e87-f23c91a70cca a phIoT:point ;
    ph:hasTag phIoT:point ;
    rdfs:label "{point}" .

phScience:gas a owl:Class ;
    rdfs:subClassOf phScience:fluid ;
    rdfs:label "gas" ;
    rdfs:comment "Substance with neither definite volume nor shape" ;
    ph:is phScience:fluid ;
    ph:lib phScience:lib:phScience ;
    ph:wikipedia "https://en.wikipedia.org/wiki/Gas"^^xsd:anyURI .

phIoT:gasoline a owl:Class ;
    rdfs:subClassOf phScience:liquid ;
    rdfs:label "gasoline" ;
    rdfs:comment "Petroleum derived liquid used as a fuel source" ;
    ph:is phScience:liquid ;
    ph:lib phIoT:lib:phIoT ;
    ph:wikipedia "https://en.wikipedia.org/wiki/Gasoline"^^xsd:anyURI .

phIoT:gasoline-input a owl:Class ;
    rdfs:subClassOf ph:input ;
    rdfs:label "gasoline-input" ;
    rdfs:comment "Entity inputs gasoline which flows from another entity" ;
    ph:is ph:input ;
    ph:lib phIoT:lib:phIoT .

phIoT:gasoline-output a owl:Class ;
    rdfs:subClassOf ph:output ;
    rdfs:label "gasoline-output" ;
    rdfs:comment "Entity outputs gasoline to other entities" ;
    ph:is ph:output ;
    ph:lib phIoT:lib:phIoT .

phIoT:gasolineRef a owl:ObjectProperty ;
    rdfs:domain phIoT:gasoline-input ;
    rdfs:range phIoT:gasoline-output ;
    rdfs:label "gasolineRef" ;
    rdfs:comment "Gasoline flows from the referent to this entity" ;
    ph:inputs phIoT:gasoline ;
    ph:is ph:ref ;
    ph:lib phIoT:lib:phIoT ;
    ph:of phIoT:gasoline-output ;
    ph:tagOn phIoT:gasoline-input .

ph:geoAddr a owl:DatatypeProperty ;
    rdfs:domain ph:geoPlace ;
    rdfs:range ph:str ;
    rdfs:label "geoAddr" ;
    rdfs:comment "Free form street address.  Best practice is to follow local\nnorms for a postal address.  Typically this string includes\nthe `geoStreet`, `geoCity`, `geoState` (in US), and `geoPostalCode`:\n\nExamples:\n  \"1600 Pennsylvania Avenue NW, Washington, DC 20500\"\n\n  \"10 Downing St, Westminster, London SW1A 2AA, United Kingdom\"\n\n  \"Champ de Mars, 5 Avenue Anatole France, 75007 Paris, France\"" ;
    ph:is ph:str ;
    ph:lib ph:lib:ph ;
    ph:tagOn ph:geoPlace .

ph:geoCity a owl:DatatypeProperty ;
    rdfs:domain ph:geoPlace ;
    rdfs:range ph:str ;
    rdfs:label "geoCity" ;
    rdfs:comment "Geographic city or locality name" ;
    ph:is ph:str ;
    ph:lib ph:lib:ph ;
    ph:tagOn ph:geoPlace .

ph:geoCoord a owl:DatatypeProperty ;
    rdfs:domain ph:geoPlace ;
    rdfs:range ph:coord ;
    rdfs:label "geoCoord" ;
    rdfs:comment "Geographic coordinate as 'C(latitude,longitude)'" ;
    ph:is ph:coord ;
    ph:lib ph:lib:ph ;
    ph:tagOn ph:geoPlace .

ph:geoCountry a owl:DatatypeProperty ;
    rdfs:domain ph:geoPlace ;
    rdfs:range ph:str ;
    rdfs:label "geoCountry" ;
    rdfs:comment "Geographic country as [ISO 3166-1]`http://en.wikipedia.org/wiki/ISO_3166-1`\ntwo letter code" ;
    ph:enum "- AF: Afghanistan\n- AX: Aland Islands\n- AL: Albania\n- DZ: Algeria\n- AS: American Samoa\n- AD: Andorra\n- AO: Angola\n- AI: Anguilla\n- AQ: Antarctica\n- AG: Antigua and Barbuda\n- AR: Argentina\n- AM: Armenia\n- AW: Aruba\n- AU: Australia\n- AT: Austria\n- AZ: Azerbaijan\n- BS: Bahamas\n- BH: Bahrain\n- BD: Bangladesh\n- BB: Barbados\n- BY: Belarus\n- BE: Belgium\n- BZ: Belize\n- BJ: Benin\n- BM: Bermuda\n- BT: Bhutan\n- BO: Bolivia, Plurinational State of\n- BO: Bolivia\n- BA: Bosnia and Herzegovina\n- BA: Bosnia\n- BA: Herzegovina\n- BW: Botswana\n- BV: Bouvet Island\n- BR: Brazil\n- IO: British Indian Ocean Territory\n- BN: Brunei Darussalam\n- BG: Bulgaria\n- BF: Burkina Faso\n- BI: Burundi\n- KH: Cambodia\n- CM: Cameroon\n- CA: Canada\n- CV: Cape Verde\n- KY: Cayman Islands\n- CF: Central African Republic\n- TD: Chad\n- CL: Chile\n- CN: China\n- CX: Christmas Island\n- CC: Cocos (keeling) Islands\n- CC: Cocos\n- CO: Colombia\n- KM: Comoros\n- CG: Congo\n- CD: Congo, the Democratic Republic of the\n- CK: Cook Islands\n- CR: Costa Rica\n- CI: Cote D'ivoire\n- HR: Croatia\n- CU: Cuba\n- CY: Cyprus\n- CZ: Czech Republic\n- DK: Denmark\n- DJ: Djibouti\n- DM: Dominica\n- DO: Dominican Republic\n- EC: Ecuador\n- EG: Egypt\n- SV: El Salvador\n- GQ: Equatorial Guinea\n- ER: Eritrea\n- EE: Estonia\n- ET: Ethiopia\n- FK: Falkland Islands (malvinas)\n- FK: Falkland Islands\n- FO: Faroe Islands\n- FJ: Fiji\n- FI: Finland\n- FR: France\n- GF: French Guiana\n- PF: French Polynesia\n- TF: French Southern Territories\n- GA: Gabon\n- GM: Gambia\n- GE: Georgia\n- DE: Germany\n- GH: Ghana\n- GI: Gibraltar\n- GR: Greece\n- GL: Greenland\n- GD: Grenada\n- GP: Guadeloupe\n- GU: Guam\n- GT: Guatemala\n- GG: Guernsey\n- GN: Guinea\n- GW: Guinea-bissau\n- GY: Guyana\n- HT: Haiti\n- HM: Heard Island and Mcdonald Islands\n- VA: Holy See (vatican City State)\n- VA: Vatican\n- HN: Honduras\n- HK: Hong Kong\n- HU: Hungary\n- IS: Iceland\n- IN: India\n- ID: Indonesia\n- IR: Iran, Islamic Republic of\n- IR: Iran\n- IQ: Iraq\n- IE: Ireland\n- IM: Isle of Man\n- IL: Israel\n- IT: Italy\n- JM: Jamaica\n- JP: Japan\n- JE: Jersey\n- JO: Jordan\n- KZ: Kazakhstan\n- KE: Kenya\n- KI: Kiribati\n- KP: Korea, Democratic People's Republic of\n- KR: Korea, Republic of\n- KR: Korea\n- KW: Kuwait\n- KG: Kyrgyzstan\n- LA: Lao People's Democratic Republic\n- LA: Lao\n- LV: Latvia\n- LB: Lebanon\n- LS: Lesotho\n- LR: Liberia\n- LY: Libyan Arab Jamahiriya\n- LI: Liechtenstein\n- LT: Lithuania\n- LU: Luxembourg\n- MO: Macao\n- MK: Macedonia, the Former Yugoslav Republic of\n- MK: Macedonia\n- MG: Madagascar\n- MW: Malawi\n- MY: Malaysia\n- MV: Maldives\n- ML: Mali\n- MT: Malta\n- MH: Marshall Islands\n- MQ: Martinique\n- MR: Mauritania\n- MU: Mauritius\n- YT: Mayotte\n- MX: Mexico\n- FM: Micronesia, Federated States of\n- FM: Micronesia\n- MD: Moldova, Republic of\n- MD: Moldova\n- MC: Monaco\n- MN: Mongolia\n- ME: Montenegro\n- MS: Montserrat\n- MA: Morocco\n- MZ: Mozambique\n- MM: Myanmar\n- NA: Namibia\n- NR: Nauru\n- NP: Nepal\n- NL: Netherlands\n- AN: Netherlands Antilles\n- NC: New Caledonia\n- NZ: New Zealand\n- NI: Nicaragua\n- NE: Niger\n- NG: Nigeria\n- NU: Niue\n- NF: Norfolk Island\n- MP: Northern Mariana Islands\n- NO: Norway\n- OM: Oman\n- PK: Pakistan\n- PW: Palau\n- PS: Palestinian Territory, Occupied\n- PS: Palestine\n- PA: Panama\n- PG: Papua New Guinea\n- PY: Paraguay\n- PE: Peru\n- PH: Philippines\n- PN: Pitcairn\n- PL: Poland\n- PT: Portugal\n- PR: Puerto Rico\n- QA: Qatar\n- RE: Reunion\n- RO: Romania\n- RU: Russian Federation\n- RW: Rwanda\n- BL: Saint Barthelemy\n- SH: Saint Helena, Ascension and Tristan Da Cunha\n- SH: Saint Helena\n- KN: Saint Kitts and Nevis\n- LC: Saint Lucia\n- MF: Saint Martin\n- PM: Saint Pierre and Miquelon\n- VC: Saint Vincent and the Grenadines\n- WS: Samoa\n- SM: San Marino\n- ST: Sao Tome and Principe\n- SA: Saudi Arabia\n- SN: Senegal\n- RS: Serbia\n- SC: Seychelles\n- SL: Sierra Leone\n- SG: Singapore\n- SK: Slovakia\n- SI: Slovenia\n- SB: Solomon Islands\n- SO: Somalia\n- ZA: South Africa\n- GS: South Georgia and the South Sandwich Islands\n- ES: Spain\n- LK: Sri Lanka\n- SD: Sudan\n- SR: Suriname\n- SJ: Svalbard and Jan Mayen\n- SZ: Swaziland\n- SE: Sweden\n- CH: Switzerland\n- SY: Syrian Arab Republic\n- TW: Taiwan, Province of China\n- TW: Taiwan\n- TJ: Tajikistan\n- TZ: Tanzania, United Republic of\n- TZ: Tanzania\n- TH: Thailand\n- TL: Timor-leste\n- TG: Togo\n- TK: Tokelau\n- TO: Tonga\n- TT: Trinidad and Tobago\n- TN: Tunisia\n- TR: Turkey\n- TM: Turkmenistan\n- TC: Turks and Caicos Islands\n- TV: Tuvalu\n- UG: Uganda\n- UA: Ukraine\n- AE: United Arab Emirates\n- GB: United Kingdom\n- GB: England\n- GB: Britain\n- GB: Great Britain\n- US: United States\n- US: United States of America\n- US: USA\n- UM: United States Minor Outlying Islands\n- UY: Uruguay\n- UZ: Uzbekistan\n- VU: Vanuatu\n- EE: Vatican City State See Holy\n- VE: Venezuela, Bolivarian Republic of\n- VE: Venezuela\n- VN: Viet Nam\n- VG: Virgin Islands, British\n- VI: Virgin Islands, U.S.\n- WF: Wallis and Futuna\n- EH: Western Sahara\n- YE: Yemen\n- ZM: Zambia\n- ZW: Zimbabwe" ;
    ph:is ph:str ;
    ph:lib ph:lib:ph ;
    ph:tagOn ph:geoPlace .

ph:geoCounty a owl:DatatypeProperty ;
    rdfs:domain ph:geoPlace ;
    rdfs:range ph:str ;
    rdfs:label "geoCounty" ;
    rdfs:comment "Geographic subdivision of US state" ;
    ph:is ph:str ;
    ph:lib ph:lib:ph ;
    ph:tagOn ph:geoPlace .

ph:geoElevation a owl:DatatypeProperty ;
    rdfs:domain ph:geoPlace ;
    rdfs:range ph:number ;
    rdfs:label "geoElevation" ;
    rdfs:comment "Elevation above sea-level of the location" ;
    ph:is ph:number ;
    ph:lib ph:lib:ph ;
    ph:tagOn ph:geoPlace .

ph:geoPlace a owl:Class ;
    rdfs:subClassOf ph:marker ;
    rdfs:label "geoPlace" ;
    rdfs:comment "Geographic place" ;
    ph:is ph:marker ;
    ph:lib ph:lib:ph .

ph:geoPostalCode a owl:DatatypeProperty ;
    rdfs:domain ph:geoPlace ;
    rdfs:range ph:str ;
    rdfs:label "geoPostalCode" ;
    rdfs:comment "Geographic postal code; for US this is a five digit zip code" ;
    ph:is ph:str ;
    ph:lib ph:lib:ph ;
    ph:tagOn ph:geoPlace .

ph:geoState a owl:DatatypeProperty ;
    rdfs:domain ph:geoPlace ;
    rdfs:range ph:str ;
    rdfs:label "geoState" ;
    rdfs:comment "State or province name; for US this is two letter state code. May be\nused in other countries to model administrative area between the geoCity\nand geoCountry level." ;
    ph:enum "- AL: Alabama\n- AK: Alaska\n- AS: American Samoa\n- AZ: Arizona\n- AR: Arkansas\n- CA: California\n- CO: Colorado\n- CT: Connecticut\n- DE: Delaware\n- DC: District of Columbia\n- FM: Federated States of Micronesia\n- FL: Florida\n- GA: Georgia\n- GU: Guam\n- HI: Hawaii\n- ID: Idaho\n- IL: Illinois\n- IN: Indiana\n- IA: Iowa\n- KS: Kansas\n- KY: Kentucky\n- LA: Louisiana\n- ME: Maine\n- MH: Marshall Islands\n- MD: Maryland\n- MA: Massachusetts\n- MI: Michigan\n- MN: Minnesota\n- MS: Mississippi\n- MO: Missouri\n- MT: Montana\n- NE: Nebraska\n- NV: Nevada\n- NH: New Hampshire\n- NJ: New Jersey\n- NM: New Mexico\n- NY: New York\n- NC: North Carolina\n- ND: North Dakota\n- MP: Northern Mariana Islands\n- OH: Ohio\n- OK: Oklahoma\n- OR: Oregon\n- PW: Palau\n- PA: Pennsylvania\n- PR: Puerto Rico\n- RI: Rhode Island\n- SC: South Carolina\n- SD: South Dakota\n- TN: Tennessee\n- TX: Texas\n- UT: Utah\n- VA: Virginia\n- VI: Virgin Islands\n- VT: Vermont\n- WA: Washington\n- WV: West Virginia\n- WI: Wisconsin\n- WY: Wyoming" ;
    ph:is ph:str ;
    ph:lib ph:lib:ph ;
    ph:openEnum ph:marker ;
    ph:tagOn ph:geoPlace .

ph:geoStreet a owl:DatatypeProperty ;
    rdfs:domain ph:geoPlace ;
    rdfs:range ph:str ;
    rdfs:label "geoStreet" ;
    rdfs:comment "Geographic street address and name" ;
    ph:is ph:str ;
    ph:lib ph:lib:ph ;
    ph:tagOn ph:geoPlace .

ph:grid a owl:DatatypeProperty ;
    rdfs:range ph:grid ;
    rdfs:label "grid" ;
    rdfs:comment "Two dimension table of columns and rows.\nSee [Kinds chapter]`docHaystack::Kinds#grid`." ;
    ph:is ph:val ;
    ph:lib ph:lib:ph .

phIoT:ground a owl:Class ;
    rdfs:subClassOf ph:marker ;
    rdfs:label "ground" ;
    rdfs:comment "Related to the surface of the earth.  Used to indicate electrical\ncurrent being measured on an electrical ground conductor when applied to\na point entity that has the `elec` and `current` tags." ;
    ph:is ph:marker ;
    ph:lib phIoT:lib:phIoT .

phIoT:ground-floor a owl:Class ;
    rdfs:subClassOf phIoT:floor ;
    rdfs:label "ground-floor" ;
    ph:children _:0b2cb027-d4dd-e080-0e88-f23c91a70cca,
        _:0b2cb027-d4dd-e081-0e89-f23c91a70cca,
        _:0b2cb027-d4dd-e082-0e8a-f23c91a70cca ;
    rdfs:comment "Floor at ground level.  In North America this is typically called\nthe first floor, but in Europe its often labeled as floor zero.\nIf `floorNum` is defined, then it must be set to zero." ;
    ph:is phIoT:floor ;
    ph:lib phIoT:lib:phIoT ;
    ph:wikipedia "https://en.wikipedia.org/wiki/Storey"^^xsd:anyURI .

_:0b2cb027-d4dd-e080-0e88-f23c91a70cca a phIoT:equip ;
    ph:hasTag phIoT:equip ;
    rdfs:label "{equip}" .

_:0b2cb027-d4dd-e081-0e89-f23c91a70cca a phIoT:point ;
    ph:hasTag phIoT:point ;
    rdfs:label "{point}" .

_:0b2cb027-d4dd-e082-0e8a-f23c91a70cca a phIoT:space ;
    ph:hasTag phIoT:space ;
    rdfs:label "{space}" .

phIoT:ground-water a owl:Class ;
    rdfs:subClassOf phScience:water ;
    rdfs:label "ground-water" ;
    rdfs:comment "Water present under the ground or from a well" ;
    ph:is phScience:water ;
    ph:lib phIoT:lib:phIoT ;
    ph:wikipedia "https://en.wikipedia.org/wiki/Groundwater"^^xsd:anyURI .

phIct:haystack a owl:Class ;
    rdfs:subClassOf phIct:protocol ;
    rdfs:label "haystack" ;
    rdfs:comment "Haystack HTTP protocol for exchanging tagged data" ;
    ph:is phIct:protocol ;
    ph:lib phIct:lib:phIct ;
    ph:wikipedia "https://en.wikipedia.org/wiki/Communication_protocol"^^xsd:anyURI .

phIoT:header a owl:Class ;
    rdfs:subClassOf phIoT:pipeSection ;
    rdfs:label "header" ;
    rdfs:comment "Pipe used as central connection or manifold for other piping runs." ;
    ph:is phIoT:pipeSection ;
    ph:lib phIoT:lib:phIoT .

phIoT:heat a owl:Class ;
    rdfs:subClassOf ph:marker ;
    rdfs:label "heat" ;
    rdfs:comment "Associated with a heating process.  When used on a point,\nthis tag is associated with the control of heating." ;
    ph:is ph:marker ;
    ph:lib phIoT:lib:phIoT .

phIoT:heatExchanger a owl:Class ;
    rdfs:subClassOf phIoT:equip ;
    rdfs:label "heatExchanger" ;
    ph:children _:0b2cb027-d4dd-e083-0e8b-f23c91a70cca,
        _:0b2cb027-d4dd-e084-0e8c-f23c91a70cca ;
    rdfs:comment "Equipment to transfer heat between two working fluids." ;
    ph:is phIoT:equip ;
    ph:lib phIoT:lib:phIoT ;
    ph:wikipedia "https://en.wikipedia.org/wiki/Heat_exchanger"^^xsd:anyURI .

_:0b2cb027-d4dd-e083-0e8b-f23c91a70cca a phIoT:equip ;
    ph:hasTag phIoT:equip ;
    rdfs:label "{equip}" .

_:0b2cb027-d4dd-e084-0e8c-f23c91a70cca a phIoT:point ;
    ph:hasTag phIoT:point ;
    rdfs:label "{point}" .

phIoT:heatPump a owl:Class ;
    rdfs:subClassOf ph:marker ;
    rdfs:label "heatPump" ;
    rdfs:comment "Equipment that employs a vapor compression cycle with a reversing\nvalve to provide heating or cooling. For vapor compression heating\nwithout a reversing valve, such as for a heat pump water heater,\nsee `dxHeating` which should be used." ;
    ph:is ph:marker ;
    ph:lib phIoT:lib:phIoT ;
    ph:wikipedia "https://en.wikipedia.org/wiki/Heat_pump"^^xsd:anyURI .

phIoT:heatRecovery a owl:Class ;
    rdfs:subClassOf ph:marker ;
    rdfs:label "heatRecovery" ;
    rdfs:comment "Transfer of heat from one substance to another to reduce energy consumption." ;
    ph:is ph:marker ;
    ph:lib phIoT:lib:phIoT .

phIoT:heatWheel a owl:Class ;
    rdfs:subClassOf ph:marker ;
    rdfs:label "heatWheel" ;
    rdfs:comment "Boolean point indicating command state of AHU's heat wheel." ;
    ph:is ph:marker ;
    ph:lib phIoT:lib:phIoT ;
    ph:wikipedia "https://en.wikipedia.org/wiki/Thermal_wheel"^^xsd:anyURI .

phIoT:heating a owl:Class ;
    rdfs:subClassOf ph:marker ;
    rdfs:label "heating" ;
    rdfs:comment "Heating mode or process" ;
    ph:is ph:marker ;
    ph:lib phIoT:lib:phIoT .

phIoT:heatingCoil a owl:Class ;
    rdfs:subClassOf phIoT:coil ;
    rdfs:label "heatingCoil" ;
    ph:children _:0b2cb027-d50b-a740-0e8d-f23c91a70cca,
        _:0b2cb027-d50b-a741-0e8e-f23c91a70cca,
        _:0b2cb027-d50b-a742-0e8f-f23c91a70cca,
        _:0b2cb027-d50b-a743-0e90-f23c91a70cca,
        _:0b2cb027-d50b-a744-0e91-f23c91a70cca ;
    ph:childrenFlatten phIoT:ductDeck,
        phIoT:ductSection ;
    rdfs:comment "Coil used to heat air." ;
    ph:is phIoT:coil ;
    ph:lib phIoT:lib:phIoT ;
    ph:wikipedia "https://en.wikipedia.org/wiki/Heat_exchanger#HVAC_air_coils"^^xsd:anyURI .

_:0b2cb027-d50b-a740-0e8d-f23c91a70cca a phIoT:equip ;
    ph:hasTag phIoT:equip ;
    rdfs:label "{equip}" .

_:0b2cb027-d50b-a741-0e8e-f23c91a70cca a phIoT:point ;
    ph:hasTag phIoT:hot,
        phScience:water,
        phIoT:heat,
        phIoT:valve,
        phIoT:cmd,
        phIoT:point ;
    rdfs:label "{hot, water, heat, valve, cmd, point}" .

_:0b2cb027-d50b-a742-0e8f-f23c91a70cca a phIoT:point ;
    ph:hasTag phIoT:point ;
    rdfs:label "{point}" .

_:0b2cb027-d50b-a743-0e90-f23c91a70cca a phIoT:point ;
    ph:hasTag phIoT:heat,
        phIoT:run,
        phIoT:cmd,
        phIoT:point ;
    rdfs:label "{stage:1, heat, run, cmd, point}" ;
    phIoT:stage 1 .

_:0b2cb027-d50b-a744-0e91-f23c91a70cca a phIoT:point ;
    ph:hasTag phScience:steam,
        phIoT:heat,
        phIoT:valve,
        phIoT:cmd,
        phIoT:point ;
    rdfs:label "{steam, heat, valve, cmd, point}" .

phIoT:heatingOnly a owl:Class ;
    rdfs:subClassOf ph:marker ;
    rdfs:label "heatingOnly" ;
    rdfs:comment "Equipment without cooling" ;
    ph:is ph:marker ;
    ph:lib phIoT:lib:phIoT .

phIoT:heatingProcess a owl:Class ;
    rdfs:subClassOf ph:choice ;
    rdfs:label "heatingProcess" ;
    rdfs:comment "Processed used to heat a substance" ;
    ph:is ph:choice ;
    ph:lib phIoT:lib:phIoT ;
    ph:tagOn phIoT:airHandlingEquip,
        phIoT:boiler,
        phIoT:chilledBeam,
        phIoT:heatingCoil,
        phIoT:radiator,
        phIoT:radiantFloor,
        phIoT:vav .

phScience:hfc a owl:Class ;
    rdfs:subClassOf phScience:gas ;
    rdfs:label "hfc" ;
    rdfs:comment "Hydrofluorocarbons" ;
    ph:is phScience:gas ;
    ph:lib phScience:lib:phScience ;
    ph:wikipedia "https://en.wikipedia.org/wiki/Hydrofluorocarbon"^^xsd:anyURI .

phScience:hfc-emission a owl:Class ;
    rdfs:subClassOf phScience:emission ;
    rdfs:label "hfc-emission" ;
    rdfs:comment "Greenhouse gas emission of hydrofluorocarbons into the air." ;
    ph:is phScience:emission ;
    ph:lib phScience:lib:phScience ;
    phScience:prefUnit "kg",
        "ton",
        "lb" ;
    phScience:quantityOf phScience:air .

phIoT:his a owl:Class ;
    rdfs:subClassOf ph:marker ;
    rdfs:label "his" ;
    rdfs:comment "Supports historization of data" ;
    ph:is ph:marker ;
    ph:lib phIoT:lib:phIoT ;
    ph:tagOn phIoT:point .

phIoT:his-point a owl:Class ;
    rdfs:subClassOf phIoT:point ;
    rdfs:label "his-point" ;
    rdfs:comment "Historized point with a history log of timestamp/value pairs.  Points\nmarked as historized indicate the system can response to queries via\nthe 'hisRead' operation to return a trend log of timestamp/value pairs.\n\nThere are typically two mechanisms for historization:\n  - the local system performs the historization by logging the\n    point's `curVal` to local storage\n  - in overlay systems a downstream device performs the historization\n    and the local system synchronizes the history data in batch on\n    a periodic basis\n\nAlso see `docHaystack::Points#his` chapter." ;
    ph:is phIoT:point ;
    ph:lib phIoT:lib:phIoT .

phIoT:hisErr a owl:DatatypeProperty ;
    rdfs:domain phIoT:his-point ;
    rdfs:range ph:str ;
    rdfs:label "hisErr" ;
    rdfs:comment "Error description when `hisStatus` indicates error condition" ;
    ph:is ph:str ;
    ph:lib phIoT:lib:phIoT ;
    ph:tagOn phIoT:his-point ;
    ph:transient ph:marker .

phIoT:hisMode a owl:DatatypeProperty ;
    rdfs:domain phIoT:his-point ;
    rdfs:range ph:str ;
    rdfs:label "hisMode" ;
    rdfs:comment "Indicates the way that history data is collected for a point." ;
    ph:enum "- sampled: Data is sampled on a regular interval. The timestamp\n  indicates exactly when the sample was taken, and we assume linear\n  interpolation between samples.\n- cov: Data is logged when it changes. The means the timestamp\n  indicates exactly when it changed (inclusive) and it remains that\n  value until the next sample's timestamp (exclusive).\n- consumption: Integral data is sampled on a regular interval and\n  logged at the *end* of the interval. The timestamp indicates the\n  *end* of the interval. Therefore, the raw data is logged as\n  start *exclusive*, end *inclusive*.  This is mode is typical for\n  consumption meters." ;
    ph:is ph:str ;
    ph:lib phIoT:lib:phIoT ;
    ph:tagOn phIoT:his-point .

phIoT:hisStatus a owl:DatatypeProperty ;
    rdfs:domain phIoT:his-point ;
    rdfs:range ph:str ;
    rdfs:label "hisStatus" ;
    rdfs:comment "Status of point's history collection or synchronization" ;
    ph:enum "- ok: last sync attempt was successful\n- fault: a configuration problem - see `hisErr`\n- down: a communication or network problem - see `hisErr`\n- disabled: manual disable of the point or parent connector\n- unknown: we don't know anything (usually boot state)\n- pending: sync has been scheduled and is waiting to running\n- syncing: sync is currently running" ;
    ph:is ph:str ;
    ph:lib phIoT:lib:phIoT ;
    ph:tagOn phIoT:his-point ;
    ph:transient ph:marker .

phIoT:hisTotalized a owl:Class ;
    rdfs:subClassOf ph:marker ;
    rdfs:label "hisTotalized" ;
    rdfs:comment "Indicates values which are a continuous stream of totalization. History\ndata reads and should be normalized by computing the delta." ;
    ph:is ph:marker ;
    ph:lib phIoT:lib:phIoT ;
    ph:tagOn phIoT:his-point .

phIoT:hot a owl:Class ;
    rdfs:subClassOf ph:marker ;
    rdfs:label "hot" ;
    rdfs:comment "Having high degree of heat" ;
    ph:is ph:marker ;
    ph:lib phIoT:lib:phIoT .

phIoT:hot-water a owl:Class ;
    rdfs:subClassOf phScience:water ;
    rdfs:label "hot-water" ;
    rdfs:comment "Hot water used for HVAC heating or supplied to hot taps" ;
    ph:is phScience:water ;
    ph:lib phIoT:lib:phIoT ;
    ph:wikipedia "https://en.wikipedia.org/wiki/Water"^^xsd:anyURI .

phIoT:hot-water-boiler a owl:Class ;
    rdfs:subClassOf phIoT:boiler,
        phIoT:hot-water-output ;
    rdfs:label "hot-water-boiler" ;
    ph:children _:0b2cb027-d51a-e980-0e92-f23c91a70cca,
        _:0b2cb027-d51a-e981-0e93-f23c91a70cca,
        _:0b2cb027-d51a-e982-0e94-f23c91a70cca,
        _:0b2cb027-d51a-e983-0e95-f23c91a70cca,
        _:0b2cb027-d51a-e984-0e96-f23c91a70cca,
        _:0b2cb027-d51a-e985-0e97-f23c91a70cca,
        _:0b2cb027-d51a-e986-0e98-f23c91a70cca,
        _:0b2cb027-d51a-e987-0e99-f23c91a70cca,
        _:0b2cb027-d51a-e988-0e9a-f23c91a70cca ;
    rdfs:comment "Boiler which outputs hot water" ;
    ph:is phIoT:boiler,
        phIoT:hot-water-output ;
    ph:lib phIoT:lib:phIoT ;
    ph:wikipedia "https://en.wikipedia.org/wiki/Boiler"^^xsd:anyURI .

_:0b2cb027-d51a-e980-0e92-f23c91a70cca a phIoT:point ;
    ph:hasTag phIoT:alarm,
        phIoT:sensor,
        phIoT:point ;
    rdfs:label "{alarm, sensor, point}" .

_:0b2cb027-d51a-e981-0e93-f23c91a70cca a phIoT:pipe ;
    ph:hasTag phIoT:circ,
        phIoT:pipe,
        phIoT:equip ;
    rdfs:label "{circ, pipe, equip}" .

_:0b2cb027-d51a-e982-0e94-f23c91a70cca a phIoT:equip ;
    ph:hasTag phIoT:equip ;
    rdfs:label "{equip}" .

_:0b2cb027-d51a-e983-0e95-f23c91a70cca a phIoT:duct ;
    ph:hasTag phIoT:flue,
        phIoT:duct,
        phIoT:equip ;
    rdfs:label "{flue, duct, equip}" .

_:0b2cb027-d51a-e984-0e96-f23c91a70cca a phIoT:pipe ;
    ph:hasTag phIoT:hot,
        phScience:water,
        phIoT:entering,
        phIoT:pipe,
        phIoT:equip ;
    rdfs:label "{hot, water, entering, pipe, equip}" .

_:0b2cb027-d51a-e985-0e97-f23c91a70cca a phIoT:pipe ;
    ph:hasTag phIoT:hot,
        phScience:water,
        phIoT:leaving,
        phIoT:pipe,
        phIoT:equip ;
    rdfs:label "{hot, water, leaving, pipe, equip}" .

_:0b2cb027-d51a-e986-0e98-f23c91a70cca a phIoT:pipe ;
    ph:hasTag phIoT:makeup,
        phScience:water,
        phIoT:entering,
        phIoT:pipe,
        phIoT:equip ;
    rdfs:label "{makeup, water, entering, pipe, equip}" .

_:0b2cb027-d51a-e987-0e99-f23c91a70cca a phIoT:duct ;
    ph:hasTag phIoT:outside,
        phIoT:duct,
        phIoT:equip ;
    rdfs:label "{outside, duct, equip}" .

_:0b2cb027-d51a-e988-0e9a-f23c91a70cca a phIoT:point ;
    ph:hasTag phIoT:point ;
    rdfs:label "{point}" .

phIoT:hot-water-input a owl:Class ;
    rdfs:subClassOf ph:input ;
    rdfs:label "hot-water-input" ;
    rdfs:comment "Entity inputs hot water which flows from another entity" ;
    ph:is ph:input ;
    ph:lib phIoT:lib:phIoT .

phIoT:hot-water-output a owl:Class ;
    rdfs:subClassOf ph:output ;
    rdfs:label "hot-water-output" ;
    rdfs:comment "Entity outputs hot water to other entities" ;
    ph:is ph:output ;
    ph:lib phIoT:lib:phIoT .

phIoT:hot-water-plant a owl:Class ;
    rdfs:subClassOf phIoT:plant,
        phIoT:hot-water-output ;
    rdfs:label "hot-water-plant" ;
    ph:children _:0b2cb027-d52a-2bc0-0e9b-f23c91a70cca,
        _:0b2cb027-d52a-2bc1-0e9c-f23c91a70cca,
        _:0b2cb027-d52a-2bc2-0e9d-f23c91a70cca,
        _:0b2cb027-d52a-2bc3-0e9e-f23c91a70cca,
        _:0b2cb027-d52a-2bc4-0e9f-f23c91a70cca,
        _:0b2cb027-d52a-2bc5-0ea0-f23c91a70cca,
        _:0b2cb027-d52a-2bc6-0ea1-f23c91a70cca,
        _:0b2cb027-d52a-2bc7-0ea2-f23c91a70cca,
        _:0b2cb027-d52a-2bc8-0ea3-f23c91a70cca,
        _:0b2cb027-d52a-2bc9-0ea4-f23c91a70cca,
        _:0b2cb027-d52a-2bca-0ea5-f23c91a70cca,
        _:0b2cb027-d52a-2bcb-0ea6-f23c91a70cca,
        _:0b2cb027-d52a-2bcc-0ea7-f23c91a70cca,
        _:0b2cb027-d52a-2bcd-0ea8-f23c91a70cca,
        _:0b2cb027-d52a-2bce-0ea9-f23c91a70cca,
        _:0b2cb027-d52a-2bcf-0eaa-f23c91a70cca ;
    rdfs:comment "Plant used to generate hot water for heating.\nSee `docHaystack::Plants`." ;
    ph:is phIoT:plant,
        phIoT:hot-water-output ;
    ph:lib phIoT:lib:phIoT .

_:0b2cb027-d52a-2bc0-0e9b-f23c91a70cca a phIoT:point ;
    ph:hasTag phIoT:enable,
        phIoT:cmd,
        phIoT:point ;
    rdfs:label "{enable, cmd, point}" .

_:0b2cb027-d52a-2bc1-0e9c-f23c91a70cca a phIoT:equip ;
    ph:hasTag phIoT:equip ;
    rdfs:label "{equip}" .

_:0b2cb027-d52a-2bc2-0e9d-f23c91a70cca a phIoT:duct ;
    ph:hasTag phIoT:flue,
        phIoT:duct,
        phIoT:equip ;
    rdfs:label "{flue, duct, equip}" .

_:0b2cb027-d52a-2bc3-0e9e-f23c91a70cca a phIoT:hot-water-boiler ;
    ph:hasTag phIoT:hot,
        phScience:water,
        phIoT:boiler,
        phIoT:equip ;
    rdfs:label "{hot, water, boiler, equip}" .

_:0b2cb027-d52a-2bc4-0e9f-f23c91a70cca a phIoT:pipe ;
    ph:hasTag phIoT:hot,
        phScience:water,
        phIoT:bypass,
        phIoT:pipe,
        phIoT:equip ;
    rdfs:label "{hot, water, bypass, pipe, equip}" .

_:0b2cb027-d52a-2bc5-0ea0-f23c91a70cca a phIoT:point ;
    ph:hasTag phIoT:hot,
        phScience:water,
        phIoT:delta,
        phScience:flow,
        phIoT:sensor,
        phIoT:point ;
    rdfs:label "{hot, water, delta, flow, sensor, point}" .

_:0b2cb027-d52a-2bc6-0ea1-f23c91a70cca a phIoT:point ;
    ph:hasTag phIoT:hot,
        phScience:water,
        phIoT:delta,
        phScience:pressure,
        phIoT:sensor,
        phIoT:point ;
    rdfs:label "{hot, water, delta, pressure, sensor, point}" .

_:0b2cb027-d52a-2bc7-0ea2-f23c91a70cca a phIoT:point ;
    ph:hasTag phIoT:hot,
        phScience:water,
        phIoT:delta,
        phScience:temp,
        phIoT:sensor,
        phIoT:point ;
    rdfs:label "{hot, water, delta, temp, sensor, point}" .

_:0b2cb027-d52a-2bc8-0ea3-f23c91a70cca a phIoT:pipe ;
    ph:hasTag phIoT:hot,
        phScience:water,
        phIoT:entering,
        phIoT:pipe,
        phIoT:equip ;
    rdfs:label "{hot, water, entering, pipe, equip}" .

_:0b2cb027-d52a-2bc9-0ea4-f23c91a70cca a phIoT:pipe ;
    ph:hasTag phIoT:hot,
        phScience:water,
        phIoT:header,
        phIoT:pipe,
        phIoT:equip ;
    rdfs:label "{hot, water, header, pipe, equip}" .

_:0b2cb027-d52a-2bca-0ea5-f23c91a70cca a phIoT:heatExchanger ;
    ph:hasTag phIoT:hot,
        phScience:water,
        phIoT:heatExchanger,
        phIoT:equip ;
    rdfs:label "{hot, water, heatExchanger, equip}" .

_:0b2cb027-d52a-2bcb-0ea6-f23c91a70cca a phIoT:pipe ;
    ph:hasTag phIoT:hot,
        phScience:water,
        phIoT:leaving,
        phIoT:pipe,
        phIoT:equip ;
    rdfs:label "{hot, water, leaving, pipe, equip}" .

_:0b2cb027-d52a-2bcc-0ea7-f23c91a70cca a phIoT:point ;
    ph:hasTag phIoT:hot,
        phScience:water,
        phIoT:mixing,
        phIoT:valve,
        phIoT:cmd,
        phIoT:point ;
    rdfs:label "{hot, water, mixing, valve, cmd, point}" .

_:0b2cb027-d52a-2bcd-0ea8-f23c91a70cca a phIoT:pipe ;
    ph:hasTag phIoT:makeup,
        phScience:water,
        phIoT:entering,
        phIoT:pipe,
        phIoT:equip ;
    rdfs:label "{makeup, water, entering, pipe, equip}" .

_:0b2cb027-d52a-2bce-0ea9-f23c91a70cca a phIoT:duct ;
    ph:hasTag phIoT:outside,
        phIoT:duct,
        phIoT:equip ;
    rdfs:label "{outside, duct, equip}" .

_:0b2cb027-d52a-2bcf-0eaa-f23c91a70cca a phIoT:point ;
    ph:hasTag phIoT:point ;
    rdfs:label "{point}" .

phIoT:hot-water-system a owl:Class ;
    rdfs:subClassOf phIoT:water-system ;
    rdfs:label "hot-water-system" ;
    ph:children _:0b2cb027-d52a-2bd0-0eab-f23c91a70cca,
        _:0b2cb027-d52a-2bd1-0eac-f23c91a70cca ;
    rdfs:comment "System that circulates water in its liquid state for heating\na space or process." ;
    ph:is phIoT:water-system ;
    ph:lib phIoT:lib:phIoT .

_:0b2cb027-d52a-2bd0-0eab-f23c91a70cca a phIoT:equip ;
    ph:hasTag phIoT:equip ;
    rdfs:label "{equip}" .

_:0b2cb027-d52a-2bd1-0eac-f23c91a70cca a phIoT:point ;
    ph:hasTag phIoT:point ;
    rdfs:label "{point}" .

phIoT:hotDeck a owl:Class ;
    rdfs:subClassOf phIoT:ductDeck ;
    rdfs:label "hotDeck" ;
    rdfs:comment "Duct carries air for heating" ;
    ph:is phIoT:ductDeck ;
    ph:lib phIoT:lib:phIoT .

phIoT:hotWaterHeating a owl:Class ;
    rdfs:subClassOf phIoT:heatingProcess,
        phIoT:hot-water-input ;
    rdfs:label "hotWaterHeating" ;
    rdfs:comment "Heating using energy of hot water" ;
    ph:is phIoT:heatingProcess,
        phIoT:hot-water-input ;
    ph:lib phIoT:lib:phIoT .

phIoT:hotWaterRef a owl:ObjectProperty ;
    rdfs:domain phIoT:hot-water-input ;
    rdfs:range phIoT:hot-water-output ;
    rdfs:label "hotWaterRef" ;
    rdfs:comment "Hot water flows from the referent to this entity" ;
    ph:inputs phIoT:hot-water ;
    ph:is ph:ref ;
    ph:lib phIoT:lib:phIoT ;
    ph:of phIoT:hot-water-output ;
    ph:tagOn phIoT:hot-water-input .

phIct:http a owl:Class ;
    rdfs:subClassOf phIct:protocol ;
    rdfs:label "http" ;
    rdfs:comment "Hypertext Transfer Protocol which is foundation of the web" ;
    ph:is phIct:protocol ;
    ph:lib phIct:lib:phIct ;
    ph:wikipedia "https://en.wikipedia.org/wiki/Hypertext_Transfer_Protocol"^^xsd:anyURI .

phIoT:humidifier a owl:Class ;
    rdfs:subClassOf ph:marker ;
    rdfs:label "humidifier" ;
    rdfs:comment "Adding moisture to air" ;
    ph:is ph:marker ;
    ph:lib phIoT:lib:phIoT .

phIoT:humidifier-equip a owl:Class ;
    rdfs:subClassOf phIoT:equip ;
    rdfs:label "humidifier-equip" ;
    ph:children _:0b2cb027-d52a-2bd2-0ead-f23c91a70cca,
        _:0b2cb027-d52a-2bd3-0eae-f23c91a70cca,
        _:0b2cb027-d52a-2bd4-0eaf-f23c91a70cca,
        _:0b2cb027-d52a-2bd5-0eb0-f23c91a70cca ;
    rdfs:comment "Equipment which adds moisture to air to increase humidity" ;
    ph:is phIoT:equip ;
    ph:lib phIoT:lib:phIoT ;
    ph:wikipedia "https://en.wikipedia.org/wiki/Humidifier"^^xsd:anyURI .

_:0b2cb027-d52a-2bd2-0ead-f23c91a70cca a phIoT:equip ;
    ph:hasTag phIoT:equip ;
    rdfs:label "{equip}" .

_:0b2cb027-d52a-2bd3-0eae-f23c91a70cca a phIoT:point ;
    ph:hasTag phIoT:humidifier,
        phIoT:enable,
        phIoT:cmd,
        phIoT:point ;
    rdfs:label "{humidifier, enable, cmd, point}" .

_:0b2cb027-d52a-2bd4-0eaf-f23c91a70cca a phIoT:point ;
    ph:hasTag phIoT:humidifier,
        phIoT:run,
        phIoT:cmd,
        phIoT:point ;
    rdfs:label "{humidifier, run, cmd, point}" .

_:0b2cb027-d52a-2bd5-0eb0-f23c91a70cca a phIoT:point ;
    ph:hasTag phIoT:point ;
    rdfs:label "{point}" .

phScience:humidity a owl:Class ;
    rdfs:subClassOf phScience:quantity ;
    rdfs:label "humidity" ;
    rdfs:comment "Percent relative humidity; measure of moisture in the air" ;
    ph:is phScience:quantity ;
    ph:lib phScience:lib:phScience ;
    phScience:prefUnit "%RH" ;
    phScience:quantityOf phScience:air .

phIoT:hvac a owl:Class ;
    rdfs:subClassOf ph:marker ;
    rdfs:label "hvac" ;
    rdfs:comment "Heating, ventilation, and air conditioning" ;
    ph:is ph:marker ;
    ph:lib phIoT:lib:phIoT ;
    ph:wikipedia "https://en.wikipedia.org/wiki/HVAC"^^xsd:anyURI .

phIoT:hvac-zone-space a owl:Class ;
    rdfs:subClassOf phIoT:zone-space,
        phIoT:hvacZonePoints,
        phIoT:airQualityZonePoints,
        phIoT:air-input ;
    rdfs:label "hvac-zone-space" ;
    ph:children _:0b2cb027-d539-6e00-0eb1-f23c91a70cca,
        _:0b2cb027-d539-6e01-0eb2-f23c91a70cca,
        _:0b2cb027-d539-6e02-0eb3-f23c91a70cca,
        _:0b2cb027-d539-6e03-0eb4-f23c91a70cca,
        _:0b2cb027-d539-6e04-0eb5-f23c91a70cca,
        _:0b2cb027-d539-6e05-0eb6-f23c91a70cca,
        _:0b2cb027-d539-6e06-0eb7-f23c91a70cca,
        _:0b2cb027-d539-6e07-0eb8-f23c91a70cca,
        _:0b2cb027-d539-6e08-0eb9-f23c91a70cca,
        _:0b2cb027-d539-6e09-0eba-f23c91a70cca,
        _:0b2cb027-d539-6e0a-0ebb-f23c91a70cca,
        _:0b2cb027-d539-6e0b-0ebc-f23c91a70cca,
        _:0b2cb027-d539-6e0c-0ebd-f23c91a70cca,
        _:0b2cb027-d539-6e0d-0ebe-f23c91a70cca,
        _:0b2cb027-d539-6e0e-0ebf-f23c91a70cca,
        _:0b2cb027-d539-6e0f-0ec0-f23c91a70cca,
        _:0b2cb027-d539-6e10-0ec1-f23c91a70cca,
        _:0b2cb027-d539-6e11-0ec2-f23c91a70cca,
        _:0b2cb027-d539-6e12-0ec3-f23c91a70cca,
        _:0b2cb027-d539-6e13-0ec4-f23c91a70cca,
        _:0b2cb027-d539-6e14-0ec5-f23c91a70cca,
        _:0b2cb027-d539-6e15-0ec6-f23c91a70cca,
        _:0b2cb027-d539-6e16-0ec7-f23c91a70cca,
        _:0b2cb027-d539-6e17-0ec8-f23c91a70cca,
        _:0b2cb027-d539-6e18-0ec9-f23c91a70cca,
        _:0b2cb027-d539-6e19-0eca-f23c91a70cca,
        _:0b2cb027-d539-6e1a-0ecb-f23c91a70cca,
        _:0b2cb027-d539-6e1b-0ecc-f23c91a70cca,
        _:0b2cb027-d539-6e1c-0ecd-f23c91a70cca,
        _:0b2cb027-d539-6e1d-0ece-f23c91a70cca,
        _:0b2cb027-d539-6e1e-0ecf-f23c91a70cca,
        _:0b2cb027-d539-6e1f-0ed0-f23c91a70cca,
        _:0b2cb027-d539-6e20-0ed1-f23c91a70cca,
        _:0b2cb027-d539-6e21-0ed2-f23c91a70cca,
        _:0b2cb027-d539-6e22-0ed3-f23c91a70cca,
        _:0b2cb027-d539-6e23-0ed4-f23c91a70cca ;
    rdfs:comment "Zone related to conditioning of a space's air temperature and quality.\nSee `docHaystack::Spaces#zones` and `docHaystack::Zones#hvac` chapters." ;
    ph:is phIoT:zone-space,
        phIoT:hvacZonePoints,
        phIoT:airQualityZonePoints,
        phIoT:air-input ;
    ph:lib phIoT:lib:phIoT .

_:0b2cb027-d539-6e00-0eb1-f23c91a70cca a phIoT:equip ;
    ph:hasTag phIoT:equip ;
    rdfs:label "{equip}" .

_:0b2cb027-d539-6e01-0eb2-f23c91a70cca a phIoT:point ;
    ph:hasTag phIoT:occupancy,
        phIoT:sensor,
        phIoT:point ;
    rdfs:label "{occupancy, sensor, point}" .

_:0b2cb027-d539-6e02-0eb3-f23c91a70cca a phIoT:point ;
    ph:hasTag phIoT:occupied,
        phIoT:sensor,
        phIoT:point ;
    rdfs:label "{occupied, sensor, point}" .

_:0b2cb027-d539-6e03-0eb4-f23c91a70cca a phIoT:point ;
    ph:hasTag phIoT:occupied,
        phIoT:sp,
        phIoT:point ;
    rdfs:label "{occupied, sp, point}" .

_:0b2cb027-d539-6e04-0eb5-f23c91a70cca a phIoT:point ;
    ph:hasTag phIoT:point ;
    rdfs:label "{point}" .

_:0b2cb027-d539-6e05-0eb6-f23c91a70cca a phIoT:space ;
    ph:hasTag phIoT:space ;
    rdfs:label "{space}" .

_:0b2cb027-d539-6e06-0eb7-f23c91a70cca a phIoT:point ;
    ph:hasTag phIoT:zone,
        phScience:air,
        phScience:ch2o,
        phScience:concentration,
        phIoT:sensor,
        phIoT:point ;
    rdfs:label "{zone, air, ch2o, concentration, sensor, point}" .

_:0b2cb027-d539-6e07-0eb8-f23c91a70cca a phIoT:point ;
    ph:hasTag phIoT:zone,
        phScience:air,
        phScience:co,
        phScience:concentration,
        phIoT:sensor,
        phIoT:point ;
    rdfs:label "{zone, air, co, concentration, sensor, point}" .

_:0b2cb027-d539-6e08-0eb9-f23c91a70cca a phIoT:point ;
    ph:hasTag phIoT:zone,
        phScience:air,
        phScience:co2,
        phScience:concentration,
        phIoT:sensor,
        phIoT:point ;
    rdfs:label "{zone, air, co2, concentration, sensor, point}" .

_:0b2cb027-d539-6e09-0eba-f23c91a70cca a phIoT:point ;
    ph:hasTag phIoT:zone,
        phScience:air,
        phScience:co2,
        phScience:concentration,
        phIoT:sp,
        phIoT:point ;
    rdfs:label "{zone, air, co2, concentration, sp, point}" .

_:0b2cb027-d539-6e0a-0ebb-f23c91a70cca a phIoT:point ;
    ph:hasTag phIoT:zone,
        phScience:air,
        phScience:dewPoint,
        phIoT:sensor,
        phIoT:point ;
    rdfs:label "{zone, air, dewPoint, sensor, point}" .

_:0b2cb027-d539-6e0b-0ebc-f23c91a70cca a phIoT:point ;
    ph:hasTag phIoT:zone,
        phScience:air,
        phScience:dewPoint,
        phIoT:sp,
        phIoT:point ;
    rdfs:label "{zone, air, dewPoint, sp, point}" .

_:0b2cb027-d539-6e0c-0ebd-f23c91a70cca a phIoT:point ;
    ph:hasTag phIoT:zone,
        phScience:air,
        phScience:enthalpy,
        phIoT:sensor,
        phIoT:point ;
    rdfs:label "{zone, air, enthalpy, sensor, point}" .

_:0b2cb027-d539-6e0d-0ebe-f23c91a70cca a phIoT:point ;
    ph:hasTag phIoT:zone,
        phScience:air,
        phScience:enthalpy,
        phIoT:sp,
        phIoT:point ;
    rdfs:label "{zone, air, enthalpy, sp, point}" .

_:0b2cb027-d539-6e0e-0ebf-f23c91a70cca a phIoT:point ;
    ph:hasTag phIoT:zone,
        phScience:air,
        phScience:humidity,
        phIoT:sensor,
        phIoT:point ;
    rdfs:label "{zone, air, humidity, sensor, point}" .

_:0b2cb027-d539-6e0f-0ec0-f23c91a70cca a phIoT:point ;
    ph:hasTag phIoT:zone,
        phScience:air,
        phScience:humidity,
        phIoT:sp,
        phIoT:point ;
    rdfs:label "{zone, air, humidity, sp, point}" .

_:0b2cb027-d539-6e10-0ec1-f23c91a70cca a phIoT:point ;
    ph:hasTag phIoT:zone,
        phScience:air,
        phIoT:hvacMode,
        phIoT:sp,
        phIoT:point ;
    rdfs:label "{zone, air, hvacMode, sp, point}" .

_:0b2cb027-d539-6e11-0ec2-f23c91a70cca a phIoT:point ;
    ph:hasTag phIoT:zone,
        phScience:air,
        phScience:nh3,
        phScience:concentration,
        phIoT:sensor,
        phIoT:point ;
    rdfs:label "{zone, air, nh3, concentration, sensor, point}" .

_:0b2cb027-d539-6e12-0ec3-f23c91a70cca a phIoT:point ;
    ph:hasTag phIoT:zone,
        phScience:air,
        phScience:no2,
        phScience:concentration,
        phIoT:sensor,
        phIoT:point ;
    rdfs:label "{zone, air, no2, concentration, sensor, point}" .

_:0b2cb027-d539-6e13-0ec4-f23c91a70cca a phIoT:point ;
    ph:hasTag phIoT:zone,
        phScience:air,
        phScience:o3,
        phScience:concentration,
        phIoT:sensor,
        phIoT:point ;
    rdfs:label "{zone, air, o3, concentration, sensor, point}" .

_:0b2cb027-d539-6e14-0ec5-f23c91a70cca a phIoT:point ;
    ph:hasTag phIoT:zone,
        phScience:air,
        phScience:pm01,
        phScience:concentration,
        phIoT:sensor,
        phIoT:point ;
    rdfs:label "{zone, air, pm01, concentration, sensor, point}" .

_:0b2cb027-d539-6e15-0ec6-f23c91a70cca a phIoT:point ;
    ph:hasTag phIoT:zone,
        phScience:air,
        phScience:pm10,
        phScience:concentration,
        phIoT:sensor,
        phIoT:point ;
    rdfs:label "{zone, air, pm10, concentration, sensor, point}" .

_:0b2cb027-d539-6e16-0ec7-f23c91a70cca a phIoT:point ;
    ph:hasTag phIoT:zone,
        phScience:air,
        phScience:pm25,
        phScience:concentration,
        phIoT:sensor,
        phIoT:point ;
    rdfs:label "{zone, air, pm25, concentration, sensor, point}" .

_:0b2cb027-d539-6e17-0ec8-f23c91a70cca a phIoT:point ;
    ph:hasTag phIoT:zone,
        phScience:air,
        phScience:pressure,
        phIoT:sensor,
        phIoT:point ;
    rdfs:label "{zone, air, pressure, sensor, point}" .

_:0b2cb027-d539-6e18-0ec9-f23c91a70cca a phIoT:point ;
    ph:hasTag phIoT:zone,
        phScience:air,
        phScience:pressure,
        phIoT:sp,
        phIoT:point ;
    rdfs:label "{zone, air, pressure, sp, point}" .

_:0b2cb027-d539-6e19-0eca-f23c91a70cca a phIoT:point ;
    ph:hasTag phIoT:zone,
        phScience:air,
        phScience:temp,
        phIoT:effective,
        phIoT:cooling,
        phIoT:sp,
        phIoT:point ;
    rdfs:label "{zone, air, temp, effective, cooling, sp, point}" .

_:0b2cb027-d539-6e1a-0ecb-f23c91a70cca a phIoT:point ;
    ph:hasTag phIoT:zone,
        phScience:air,
        phScience:temp,
        phIoT:effective,
        phIoT:heating,
        phIoT:sp,
        phIoT:point ;
    rdfs:label "{zone, air, temp, effective, heating, sp, point}" .

_:0b2cb027-d539-6e1b-0ecc-f23c91a70cca a phIoT:point ;
    ph:hasTag phIoT:zone,
        phScience:air,
        phScience:temp,
        phIoT:effective,
        phIoT:sp,
        phIoT:point ;
    rdfs:label "{zone, air, temp, effective, sp, point}" .

_:0b2cb027-d539-6e1c-0ecd-f23c91a70cca a phIoT:point ;
    ph:hasTag phIoT:zone,
        phScience:air,
        phScience:temp,
        phIoT:occ,
        phIoT:cooling,
        phIoT:sp,
        phIoT:point ;
    rdfs:label "{zone, air, temp, occ, cooling, sp, point}" .

_:0b2cb027-d539-6e1d-0ece-f23c91a70cca a phIoT:point ;
    ph:hasTag phIoT:zone,
        phScience:air,
        phScience:temp,
        phIoT:occ,
        phIoT:heating,
        phIoT:sp,
        phIoT:point ;
    rdfs:label "{zone, air, temp, occ, heating, sp, point}" .

_:0b2cb027-d539-6e1e-0ecf-f23c91a70cca a phIoT:point ;
    ph:hasTag phIoT:zone,
        phScience:air,
        phScience:temp,
        phIoT:sensor,
        phIoT:point ;
    rdfs:label "{zone, air, temp, sensor, point}" .

_:0b2cb027-d539-6e1f-0ed0-f23c91a70cca a phIoT:point ;
    ph:hasTag phIoT:zone,
        phScience:air,
        phScience:temp,
        phIoT:standby,
        phIoT:cooling,
        phIoT:sp,
        phIoT:point ;
    rdfs:label "{zone, air, temp, standby, cooling, sp, point}" .

_:0b2cb027-d539-6e20-0ed1-f23c91a70cca a phIoT:point ;
    ph:hasTag phIoT:zone,
        phScience:air,
        phScience:temp,
        phIoT:standby,
        phIoT:heating,
        phIoT:sp,
        phIoT:point ;
    rdfs:label "{zone, air, temp, standby, heating, sp, point}" .

_:0b2cb027-d539-6e21-0ed2-f23c91a70cca a phIoT:point ;
    ph:hasTag phIoT:zone,
        phScience:air,
        phScience:temp,
        phIoT:unocc,
        phIoT:cooling,
        phIoT:sp,
        phIoT:point ;
    rdfs:label "{zone, air, temp, unocc, cooling, sp, point}" .

_:0b2cb027-d539-6e22-0ed3-f23c91a70cca a phIoT:point ;
    ph:hasTag phIoT:zone,
        phScience:air,
        phScience:temp,
        phIoT:unocc,
        phIoT:heating,
        phIoT:sp,
        phIoT:point ;
    rdfs:label "{zone, air, temp, unocc, heating, sp, point}" .

_:0b2cb027-d539-6e23-0ed4-f23c91a70cca a phIoT:point ;
    ph:hasTag phIoT:zone,
        phScience:air,
        phScience:tvoc,
        phScience:concentration,
        phIoT:sensor,
        phIoT:point ;
    rdfs:label "{zone, air, tvoc, concentration, sensor, point}" .

phIoT:hvacMode a owl:Class ;
    rdfs:subClassOf ph:marker ;
    rdfs:label "hvacMode" ;
    rdfs:comment "Operational mode for HVAC equipment" ;
    ph:enum "- cooling:\n- heating:\n- reheat:\n- warmup: morning warmup where AHU is supplying warm air\n- purge: night purge when AHU is supplying 100% fresh air\n- pressurize:\n- depressurize:\n- manual:" ;
    ph:is ph:marker ;
    ph:lib phIoT:lib:phIoT .

phIoT:hvacZonePoints a owl:Class ;
    rdfs:subClassOf phIoT:pointGroup ;
    rdfs:label "hvacZonePoints" ;
    ph:children _:0b2cb027-d585-b940-0ed5-f23c91a70cca,
        _:0b2cb027-d585-b941-0ed6-f23c91a70cca,
        _:0b2cb027-d585-b942-0ed7-f23c91a70cca,
        _:0b2cb027-d585-b943-0ed8-f23c91a70cca,
        _:0b2cb027-d585-b944-0ed9-f23c91a70cca,
        _:0b2cb027-d585-b945-0eda-f23c91a70cca,
        _:0b2cb027-d585-b946-0edb-f23c91a70cca,
        _:0b2cb027-d585-b947-0edc-f23c91a70cca,
        _:0b2cb027-d585-b948-0edd-f23c91a70cca,
        _:0b2cb027-d585-b949-0ede-f23c91a70cca,
        _:0b2cb027-d585-b94a-0edf-f23c91a70cca,
        _:0b2cb027-d585-b94b-0ee0-f23c91a70cca,
        _:0b2cb027-d585-b94c-0ee1-f23c91a70cca,
        _:0b2cb027-d585-b94d-0ee2-f23c91a70cca,
        _:0b2cb027-d585-b94e-0ee3-f23c91a70cca,
        _:0b2cb027-d585-b94f-0ee4-f23c91a70cca,
        _:0b2cb027-d585-b950-0ee5-f23c91a70cca,
        _:0b2cb027-d585-b951-0ee6-f23c91a70cca,
        _:0b2cb027-d585-b952-0ee7-f23c91a70cca ;
    rdfs:comment "Entity with logical grouping of zone HVAC air points.\nSee `docHaystack::Zones#hvac` chapter." ;
    ph:is phIoT:pointGroup ;
    ph:lib phIoT:lib:phIoT .

_:0b2cb027-d585-b940-0ed5-f23c91a70cca a phIoT:point ;
    ph:hasTag phIoT:zone,
        phScience:air,
        phIoT:hvacMode,
        phIoT:sp,
        phIoT:point ;
    rdfs:label "{zone, air, hvacMode, sp, point}" .

_:0b2cb027-d585-b941-0ed6-f23c91a70cca a phIoT:point ;
    ph:hasTag phIoT:zone,
        phScience:air,
        phScience:temp,
        phIoT:sensor,
        phIoT:point ;
    rdfs:label "{zone, air, temp, sensor, point}" .

_:0b2cb027-d585-b942-0ed7-f23c91a70cca a phIoT:point ;
    ph:hasTag phIoT:zone,
        phScience:air,
        phScience:temp,
        phIoT:effective,
        phIoT:sp,
        phIoT:point ;
    rdfs:label "{zone, air, temp, effective, sp, point}" .

_:0b2cb027-d585-b943-0ed8-f23c91a70cca a phIoT:point ;
    ph:hasTag phIoT:zone,
        phScience:air,
        phScience:temp,
        phIoT:effective,
        phIoT:cooling,
        phIoT:sp,
        phIoT:point ;
    rdfs:label "{zone, air, temp, effective, cooling, sp, point}" .

_:0b2cb027-d585-b944-0ed9-f23c91a70cca a phIoT:point ;
    ph:hasTag phIoT:zone,
        phScience:air,
        phScience:temp,
        phIoT:effective,
        phIoT:heating,
        phIoT:sp,
        phIoT:point ;
    rdfs:label "{zone, air, temp, effective, heating, sp, point}" .

_:0b2cb027-d585-b945-0eda-f23c91a70cca a phIoT:point ;
    ph:hasTag phIoT:zone,
        phScience:air,
        phScience:temp,
        phIoT:occ,
        phIoT:cooling,
        phIoT:sp,
        phIoT:point ;
    rdfs:label "{zone, air, temp, occ, cooling, sp, point}" .

_:0b2cb027-d585-b946-0edb-f23c91a70cca a phIoT:point ;
    ph:hasTag phIoT:zone,
        phScience:air,
        phScience:temp,
        phIoT:occ,
        phIoT:heating,
        phIoT:sp,
        phIoT:point ;
    rdfs:label "{zone, air, temp, occ, heating, sp, point}" .

_:0b2cb027-d585-b947-0edc-f23c91a70cca a phIoT:point ;
    ph:hasTag phIoT:zone,
        phScience:air,
        phScience:temp,
        phIoT:unocc,
        phIoT:cooling,
        phIoT:sp,
        phIoT:point ;
    rdfs:label "{zone, air, temp, unocc, cooling, sp, point}" .

_:0b2cb027-d585-b948-0edd-f23c91a70cca a phIoT:point ;
    ph:hasTag phIoT:zone,
        phScience:air,
        phScience:temp,
        phIoT:unocc,
        phIoT:heating,
        phIoT:sp,
        phIoT:point ;
    rdfs:label "{zone, air, temp, unocc, heating, sp, point}" .

_:0b2cb027-d585-b949-0ede-f23c91a70cca a phIoT:point ;
    ph:hasTag phIoT:zone,
        phScience:air,
        phScience:temp,
        phIoT:standby,
        phIoT:cooling,
        phIoT:sp,
        phIoT:point ;
    rdfs:label "{zone, air, temp, standby, cooling, sp, point}" .

_:0b2cb027-d585-b94a-0edf-f23c91a70cca a phIoT:point ;
    ph:hasTag phIoT:zone,
        phScience:air,
        phScience:temp,
        phIoT:standby,
        phIoT:heating,
        phIoT:sp,
        phIoT:point ;
    rdfs:label "{zone, air, temp, standby, heating, sp, point}" .

_:0b2cb027-d585-b94b-0ee0-f23c91a70cca a phIoT:point ;
    ph:hasTag phIoT:zone,
        phScience:air,
        phScience:pressure,
        phIoT:sensor,
        phIoT:point ;
    rdfs:label "{zone, air, pressure, sensor, point}" .

_:0b2cb027-d585-b94c-0ee1-f23c91a70cca a phIoT:point ;
    ph:hasTag phIoT:zone,
        phScience:air,
        phScience:pressure,
        phIoT:sp,
        phIoT:point ;
    rdfs:label "{zone, air, pressure, sp, point}" .

_:0b2cb027-d585-b94d-0ee2-f23c91a70cca a phIoT:point ;
    ph:hasTag phIoT:zone,
        phScience:air,
        phScience:humidity,
        phIoT:sensor,
        phIoT:point ;
    rdfs:label "{zone, air, humidity, sensor, point}" .

_:0b2cb027-d585-b94e-0ee3-f23c91a70cca a phIoT:point ;
    ph:hasTag phIoT:zone,
        phScience:air,
        phScience:humidity,
        phIoT:sp,
        phIoT:point ;
    rdfs:label "{zone, air, humidity, sp, point}" .

_:0b2cb027-d585-b94f-0ee4-f23c91a70cca a phIoT:point ;
    ph:hasTag phIoT:zone,
        phScience:air,
        phScience:dewPoint,
        phIoT:sensor,
        phIoT:point ;
    rdfs:label "{zone, air, dewPoint, sensor, point}" .

_:0b2cb027-d585-b950-0ee5-f23c91a70cca a phIoT:point ;
    ph:hasTag phIoT:zone,
        phScience:air,
        phScience:dewPoint,
        phIoT:sp,
        phIoT:point ;
    rdfs:label "{zone, air, dewPoint, sp, point}" .

_:0b2cb027-d585-b951-0ee6-f23c91a70cca a phIoT:point ;
    ph:hasTag phIoT:zone,
        phScience:air,
        phScience:enthalpy,
        phIoT:sensor,
        phIoT:point ;
    rdfs:label "{zone, air, enthalpy, sensor, point}" .

_:0b2cb027-d585-b952-0ee7-f23c91a70cca a phIoT:point ;
    ph:hasTag phIoT:zone,
        phScience:air,
        phScience:enthalpy,
        phIoT:sp,
        phIoT:point ;
    rdfs:label "{zone, air, enthalpy, sp, point}" .

phScience:ice a owl:Class ;
    rdfs:subClassOf phScience:solid ;
    rdfs:label "ice" ;
    rdfs:comment "Water in its solid form" ;
    ph:is phScience:solid ;
    ph:lib phScience:lib:phScience ;
    ph:wikipedia "https://en.wikipedia.org/wiki/Ice"^^xsd:anyURI .

ph:id a owl:ObjectProperty ;
    rdfs:domain ph:entity ;
    rdfs:range ph:entity ;
    rdfs:label "id" ;
    rdfs:comment "Defines the unique identifier of an entity in system using a `ref` value\ntype. The scope of an entity is undefined, but must be unique with a\ngiven system or project. This identifier may be used by other entities\nfor cross-referencing.  See `docHaystack::Ontology#entities` chapter." ;
    ph:is ph:ref ;
    ph:lib ph:lib:ph ;
    ph:tagOn ph:entity .

phScience:illuminance a owl:Class ;
    rdfs:subClassOf phScience:quantity ;
    rdfs:label "illuminance" ;
    rdfs:comment "Luminous flux hitting the inside of the sphere at a specific point.\n\nAlso see [ies.org]`https://www.ies.org/definitions/illuminance/`" ;
    ph:is phScience:quantity ;
    ph:lib phScience:lib:phScience ;
    phScience:prefUnit "lux",
        "footcandle",
        "phot" ;
    phScience:quantityOf phScience:light ;
    ph:wikipedia "https://en.wikipedia.org/wiki/Illuminance"^^xsd:anyURI .

phIct:imap a owl:Class ;
    rdfs:subClassOf phIct:protocol ;
    rdfs:label "imap" ;
    rdfs:comment "Internet Message Access Protocol for retrieving email" ;
    ph:is phIct:protocol ;
    ph:lib phIct:lib:phIct ;
    ph:wikipedia "https://en.wikipedia.org/wiki/Internet_Message_Access_Protocol"^^xsd:anyURI .

phIoT:imbalance a owl:Class ;
    rdfs:subClassOf ph:marker ;
    rdfs:label "imbalance" ;
    rdfs:comment "Lacking balance" ;
    ph:is ph:marker ;
    ph:lib phIoT:lib:phIoT .

phIoT:import a owl:Class ;
    rdfs:subClassOf ph:marker ;
    rdfs:label "import" ;
    rdfs:comment "Received into a system" ;
    ph:is ph:marker ;
    ph:lib phIoT:lib:phIoT .

phIoT:indoorUnit a owl:Class ;
    rdfs:subClassOf ph:marker ;
    rdfs:label "indoorUnit" ;
    rdfs:comment "Operates inside the conditioned space" ;
    ph:is ph:marker ;
    ph:lib phIoT:lib:phIoT .

phIoT:infiltration a owl:Class ;
    rdfs:subClassOf ph:marker ;
    rdfs:label "infiltration" ;
    rdfs:comment "Permeation of a substance into another substance" ;
    ph:is ph:marker ;
    ph:lib phIoT:lib:phIoT .

phIoT:inlet a owl:Class ;
    rdfs:subClassOf phIoT:ductSection ;
    rdfs:label "inlet" ;
    rdfs:comment "Duct with air entering an equipment" ;
    ph:is phIoT:ductSection ;
    ph:lib phIoT:lib:phIoT .

ph:input a owl:Class ;
    rdfs:subClassOf ph:marker ;
    rdfs:label "input" ;
    rdfs:comment "Entity inputs a substance which flows from another entity" ;
    ph:is ph:marker ;
    ph:lib ph:lib:ph .

ph:inputs a owl:DatatypeProperty ;
    rdfs:range ph:symbol ;
    rdfs:label "inputs" ;
    rdfs:comment "The entity inputs a substance from the referent.\nThe value of this tag is what is received." ;
    ph:is ph:relationship ;
    ph:lib ph:lib:ph ;
    ph:reciprocalOf ph:outputs ;
    ph:transitive ph:marker .

ph:int a owl:DatatypeProperty ;
    rdfs:range ph:number ;
    rdfs:label "int" ;
    rdfs:comment "Unitless integer number" ;
    ph:is ph:number ;
    ph:lib ph:lib:ph .

phScience:intensity a owl:Class ;
    rdfs:subClassOf ph:marker ;
    rdfs:label "intensity" ;
    rdfs:comment "Measure of an electromagnetic field" ;
    ph:is ph:marker ;
    ph:lib phScience:lib:phScience .

phScience:irradiance a owl:Class ;
    rdfs:subClassOf phScience:quantity ;
    rdfs:label "irradiance" ;
    rdfs:comment "Energy received at a surface by area" ;
    ph:is phScience:quantity ;
    ph:lib phScience:lib:phScience .

ph:is a owl:DatatypeProperty ;
    rdfs:domain ph:def ;
    rdfs:range ph:list ;
    rdfs:label "is" ;
    rdfs:comment "Defines one or more supertypes of a subtyping relationship.\nSee [Subtyping]`docHaystack::Subtyping` chapter." ;
    ph:is ph:association ;
    ph:lib ph:lib:ph ;
    ph:of ph:symbol ;
    ph:tagOn ph:def .

phIoT:isolation a owl:Class ;
    rdfs:subClassOf ph:marker ;
    rdfs:label "isolation" ;
    rdfs:comment "Actuator used to isolate an equipment from a pipe or ductwork system" ;
    ph:is ph:marker ;
    ph:lib phIoT:lib:phIoT .

ph:kind a owl:DatatypeProperty ;
    rdfs:domain phIoT:point ;
    rdfs:range ph:str ;
    rdfs:label "kind" ;
    rdfs:comment "Kind name used to identity a value data type" ;
    ph:enum "- Marker: is-a label\n- Bool: true or false\n- NA: not available\n- Number: floating point with optional unit\n- Str: Unicode string\n- Uri: Universal resource identifier\n- Ref: reference to an entity\n- Date: an ISO 8601 date as year, month, day: 2011-06-07\n- Time: an ISO 8601 time as hour, minute, seconds: 09:51:27.354\n- DateTime: an ISO 8601 timestamp followed by timezone name\n- Coord: geographic coordinate in latitude/longitude formatted as C(lat,lng)\n- XStr: extended string with type name\n- List: ordered sequence\n- Dict: key/value map\n- Grid: two dimensional tabular data collection" ;
    ph:is ph:str ;
    ph:lib ph:lib:ph ;
    ph:tagOn phIoT:point .

phIct:knx a owl:Class ;
    rdfs:subClassOf phIct:protocol ;
    rdfs:label "knx" ;
    rdfs:comment "KNX protocol commonly used for lighting systems" ;
    ph:is phIct:protocol ;
    ph:lib phIct:lib:phIct ;
    ph:wikipedia "https://en.wikipedia.org/wiki/KNX_(standard)"^^xsd:anyURI .

phIct:laptop a owl:Class ;
    rdfs:subClassOf phIct:computer ;
    rdfs:label "laptop" ;
    rdfs:comment "Portable laptop computer." ;
    ph:is phIct:computer ;
    ph:lib phIct:lib:phIct ;
    ph:wikipedia "https://en.wikipedia.org/wiki/Laptop"^^xsd:anyURI .

phIoT:leaving a owl:Class ;
    rdfs:subClassOf phIoT:pipeSection ;
    rdfs:label "leaving" ;
    rdfs:comment "Pipe conveys fluid out of an equipment" ;
    ph:is phIoT:pipeSection ;
    ph:lib phIoT:lib:phIoT .

phScience:level a owl:Class ;
    rdfs:subClassOf phScience:quantity ;
    rdfs:label "level" ;
    rdfs:comment "Range from 0% to 100%.  When paired with a fluid this implies a fill\nlevel where 0% is empty and 100% is full." ;
    ph:is phScience:quantity ;
    ph:lib phScience:lib:phScience ;
    phScience:prefUnit "%" ;
    phScience:quantityOf phScience:fluid .

ph:lib rdfs:label "lib" ;
    rdfs:comment "Library module of symbolic definitions.\nSee `docHaystack::Namespaces#libs` chapter." ;
    ph:is ph:feature ;
    ph:lib ph:lib:ph .

ph:lib:ph rdfs:label "lib:ph" ;
    ph:baseUri "https://project-haystack.org/def/ph/"^^xsd:anyURI ;
    rdfs:comment "Project Haystack core definitions" ;
    ph:is ph:lib ;
    ph:lib ph:lib:ph ;
    ph:version "4.0.0" .

phIct:lib:phIct rdfs:label "lib:phIct" ;
    ph:baseUri "https://project-haystack.org/def/phIct/"^^xsd:anyURI ;
    ph:depends ph:lib:ph,
        phIoT:lib:phIoT ;
    rdfs:comment "Project Haystack definitions for Information and Communications Technology.\nThis includes microprocessor based hardware, software, and networking\ntechnologies." ;
    ph:is ph:lib ;
    ph:lib phIct:lib:phIct ;
    ph:version "4.0.0" ;
    ph:wikipedia "https://en.wikipedia.org/wiki/Information_and_communications_technology"^^xsd:anyURI .

phIoT:lib:phIoT rdfs:label "lib:phIoT" ;
    ph:baseUri "https://project-haystack.org/def/phIoT/"^^xsd:anyURI ;
    ph:depends ph:lib:ph,
        phScience:lib:phScience ;
    rdfs:comment "Project Haystack definitions for Internet of Things" ;
    ph:is ph:lib ;
    ph:lib phIoT:lib:phIoT ;
    ph:version "4.0.0" ;
    ph:wikipedia "https://en.wikipedia.org/wiki/Internet_of_things"^^xsd:anyURI .

phScience:lib:phScience rdfs:label "lib:phScience" ;
    ph:baseUri "https://project-haystack.org/def/phScience/"^^xsd:anyURI ;
    ph:depends ph:lib:ph ;
    rdfs:comment "Project Haystack scientific definitions" ;
    ph:is ph:lib ;
    ph:lib phScience:lib:phScience ;
    ph:version "4.0.0" .

phScience:light a owl:Class ;
    rdfs:subClassOf phScience:phenomenon ;
    rdfs:label "light" ;
    rdfs:comment "Electromagnetic radiation in the visible spectrum" ;
    ph:is phScience:phenomenon ;
    ph:lib phScience:lib:phScience ;
    ph:wikipedia "https://en.wikipedia.org/wiki/Light"^^xsd:anyURI .

phScience:light-level a owl:Class ;
    rdfs:subClassOf phScience:level ;
    rdfs:label "light-level" ;
    rdfs:comment "Sensed or controlled dimming level of electrical lighting.\nLevel is measured as a percentage where 0% is off and 100%\nis full brightness." ;
    ph:is phScience:level ;
    ph:lib phScience:lib:phScience ;
    phScience:prefUnit "%" ;
    phScience:quantityOf phScience:light .

phIoT:lighting a owl:Class ;
    rdfs:subClassOf ph:marker ;
    rdfs:label "lighting" ;
    rdfs:comment "Systems associated with illumination in the built environment" ;
    ph:is ph:marker ;
    ph:lib phIoT:lib:phIoT ;
    ph:wikipedia "https://en.wikipedia.org/wiki/Lighting"^^xsd:anyURI .

phIoT:lighting-system a owl:Class ;
    rdfs:subClassOf phIoT:elec-system ;
    rdfs:label "lighting-system" ;
    ph:children _:0b2cb027-d5a4-3dc0-0ee8-f23c91a70cca,
        _:0b2cb027-d5a4-3dc1-0ee9-f23c91a70cca ;
    rdfs:comment "System designed to provide lighting." ;
    ph:is phIoT:elec-system ;
    ph:lib phIoT:lib:phIoT .

_:0b2cb027-d5a4-3dc0-0ee8-f23c91a70cca a phIoT:equip ;
    ph:hasTag phIoT:equip ;
    rdfs:label "{equip}" .

_:0b2cb027-d5a4-3dc1-0ee9-f23c91a70cca a phIoT:point ;
    ph:hasTag phIoT:point ;
    rdfs:label "{point}" .

phIoT:lighting-zone-space a owl:Class ;
    rdfs:subClassOf phIoT:zone-space,
        phIoT:lightingZonePoints ;
    rdfs:label "lighting-zone-space" ;
    ph:children _:0b2cb027-d5a4-3dc2-0eea-f23c91a70cca,
        _:0b2cb027-d5a4-3dc3-0eeb-f23c91a70cca,
        _:0b2cb027-d5a4-3dc4-0eec-f23c91a70cca,
        _:0b2cb027-d5a4-3dc5-0eed-f23c91a70cca,
        _:0b2cb027-d5a4-3dc6-0eee-f23c91a70cca,
        _:0b2cb027-d5a4-3dc7-0eef-f23c91a70cca,
        _:0b2cb027-d5a4-3dc8-0ef0-f23c91a70cca,
        _:0b2cb027-d5a4-3dc9-0ef1-f23c91a70cca,
        _:0b2cb027-d5a4-3dca-0ef2-f23c91a70cca,
        _:0b2cb027-d5a4-3dcb-0ef3-f23c91a70cca ;
    rdfs:comment "Zone related to lighting system.\nSee `docHaystack::Spaces#zones` and `docHaystack::Zones#lighting` chapters." ;
    ph:is phIoT:zone-space,
        phIoT:lightingZonePoints ;
    ph:lib phIoT:lib:phIoT .

_:0b2cb027-d5a4-3dc2-0eea-f23c91a70cca a phIoT:equip ;
    ph:hasTag phIoT:equip ;
    rdfs:label "{equip}" .

_:0b2cb027-d5a4-3dc3-0eeb-f23c91a70cca a phIoT:point ;
    ph:hasTag phScience:light,
        phScience:illuminance,
        phIoT:sensor,
        phIoT:point ;
    rdfs:label "{light, illuminance, sensor, point}" .

_:0b2cb027-d5a4-3dc4-0eec-f23c91a70cca a phIoT:point ;
    ph:hasTag phScience:light,
        phScience:level,
        phIoT:sensor,
        phIoT:point ;
    rdfs:label "{light, level, sensor, point}" .

_:0b2cb027-d5a4-3dc5-0eed-f23c91a70cca a phIoT:point ;
    ph:hasTag phScience:light,
        phScience:level,
        phIoT:sp,
        phIoT:point ;
    rdfs:label "{light, level, sp, point}" .

_:0b2cb027-d5a4-3dc6-0eee-f23c91a70cca a phIoT:point ;
    ph:hasTag phScience:light,
        phScience:luminous,
        phScience:flux,
        phIoT:sensor,
        phIoT:point ;
    rdfs:label "{light, luminous, flux, sensor, point}" .

_:0b2cb027-d5a4-3dc7-0eef-f23c91a70cca a phIoT:point ;
    ph:hasTag phIoT:occupancy,
        phIoT:sensor,
        phIoT:point ;
    rdfs:label "{occupancy, sensor, point}" .

_:0b2cb027-d5a4-3dc8-0ef0-f23c91a70cca a phIoT:point ;
    ph:hasTag phIoT:occupied,
        phIoT:sensor,
        phIoT:point ;
    rdfs:label "{occupied, sensor, point}" .

_:0b2cb027-d5a4-3dc9-0ef1-f23c91a70cca a phIoT:point ;
    ph:hasTag phIoT:occupied,
        phIoT:sp,
        phIoT:point ;
    rdfs:label "{occupied, sp, point}" .

_:0b2cb027-d5a4-3dca-0ef2-f23c91a70cca a phIoT:point ;
    ph:hasTag phIoT:point ;
    rdfs:label "{point}" .

_:0b2cb027-d5a4-3dcb-0ef3-f23c91a70cca a phIoT:space ;
    ph:hasTag phIoT:space ;
    rdfs:label "{space}" .

phIoT:lightingZonePoints a owl:Class ;
    rdfs:subClassOf phIoT:pointGroup ;
    rdfs:label "lightingZonePoints" ;
    ph:children _:0b2cb027-d5e1-46c0-0ef4-f23c91a70cca,
        _:0b2cb027-d5e1-46c1-0ef5-f23c91a70cca,
        _:0b2cb027-d5e1-46c2-0ef6-f23c91a70cca,
        _:0b2cb027-d5e1-46c3-0ef7-f23c91a70cca ;
    rdfs:comment "Entity with logical grouping of lighting points.\nSee `docHaystack::Zones#lighting` chapter." ;
    ph:is phIoT:pointGroup ;
    ph:lib phIoT:lib:phIoT .

_:0b2cb027-d5e1-46c0-0ef4-f23c91a70cca a phIoT:point ;
    ph:hasTag phScience:light,
        phScience:level,
        phIoT:sensor,
        phIoT:point ;
    rdfs:label "{light, level, sensor, point}" .

_:0b2cb027-d5e1-46c1-0ef5-f23c91a70cca a phIoT:point ;
    ph:hasTag phScience:light,
        phScience:level,
        phIoT:sp,
        phIoT:point ;
    rdfs:label "{light, level, sp, point}" .

_:0b2cb027-d5e1-46c2-0ef6-f23c91a70cca a phIoT:point ;
    ph:hasTag phScience:light,
        phScience:illuminance,
        phIoT:sensor,
        phIoT:point ;
    rdfs:label "{light, illuminance, sensor, point}" .

_:0b2cb027-d5e1-46c3-0ef7-f23c91a70cca a phIoT:point ;
    ph:hasTag phScience:light,
        phScience:luminous,
        phScience:flux,
        phIoT:sensor,
        phIoT:point ;
    rdfs:label "{light, luminous, flux, sensor, point}" .

phIoT:lineAvg a owl:Class ;
    rdfs:subClassOf ph:marker ;
    rdfs:label "lineAvg" ;
    rdfs:comment "Line average of single-phase electrical quantity measurements in an AC\nelectric power system.\n\nWhen applied to a point entity that has the `elec` and `volt` tags,\nindicates the average of all available `lineVolt` measurements.\n\nWhen applied to a point entity that has the `elec` and `current` tags,\nindicates the average of all available `lineCurrent` measurements.\n\nWhen applied to a point entity that has the `elec` and `power` tags,\nindicates the average of all available `linePower` measurements.\n\nWhen applied to a point entity that has the `elec` and `pf` tags,\nindicates the average of all available `linePf` measurements.\n\nWhen applied to a point entity that has the `elec` and `energy` tags,\nindicates the average of all available `lineEnergy` measurements.\n" ;
    ph:is ph:marker ;
    ph:lib phIoT:lib:phIoT .

phIoT:lineCurrent a owl:DatatypeProperty ;
    rdfs:range ph:str ;
    rdfs:label "lineCurrent" ;
    rdfs:comment "Single-phase line current measured in an AC electric power system." ;
    ph:enum "- L1: line 1 measurement\n- L2: line 2 measurement\n- L3: line 3 measurement" ;
    ph:is phIoT:elecLine ;
    ph:lib phIoT:lib:phIoT .

phIoT:lineEnergy a owl:DatatypeProperty ;
    rdfs:range ph:str ;
    rdfs:label "lineEnergy" ;
    rdfs:comment "Single-phase energy measured line-to-line in an AC electric power\nsystem." ;
    ph:enum "- L1-L2: line 1 to line 2 measurement\n- L2-L3: line 2 to line 3 measurement\n- L3-L1: line 3 to line 1 measurement" ;
    ph:is phIoT:elecLineToLine ;
    ph:lib phIoT:lib:phIoT .

phIoT:linePf a owl:DatatypeProperty ;
    rdfs:range ph:str ;
    rdfs:label "linePf" ;
    rdfs:comment "Single-phase power factor measured line-to-line in an AC electric power\nsystem." ;
    ph:enum "- L1-L2: line 1 to line 2 measurement\n- L2-L3: line 2 to line 3 measurement\n- L3-L1: line 3 to line 1 measurement" ;
    ph:is phIoT:elecLineToLine ;
    ph:lib phIoT:lib:phIoT .

phIoT:linePower a owl:DatatypeProperty ;
    rdfs:range ph:str ;
    rdfs:label "linePower" ;
    rdfs:comment "Single-phase power measured line-to-line in an AC electric power system.\nMay also be referred to as a line power measurement." ;
    ph:enum "- L1-L2: line 1 to line 2 measurement\n- L2-L3: line 2 to line 3 measurement\n- L3-L1: line 3 to line 1 measurement" ;
    ph:is phIoT:elecLineToLine ;
    ph:lib phIoT:lib:phIoT .

phIoT:lineVolt a owl:DatatypeProperty ;
    rdfs:range ph:str ;
    rdfs:label "lineVolt" ;
    rdfs:comment "Single-phase voltage measured line-to-line in an AC electric power\nsystem.  May also be referred to as a line voltage measurement." ;
    ph:enum "- L1-L2: line 1 to line 2 measurement\n- L2-L3: line 2 to line 3 measurement\n- L3-L1: line 3 to line 1 measurement" ;
    ph:is phIoT:elecLineToLine ;
    ph:lib phIoT:lib:phIoT .

phScience:liquid a owl:Class ;
    rdfs:subClassOf phScience:fluid ;
    rdfs:label "liquid" ;
    rdfs:comment "Substance with definite volume but takes the shape of its container" ;
    ph:is phScience:fluid ;
    ph:lib phScience:lib:phScience ;
    ph:wikipedia "https://en.wikipedia.org/wiki/Liquid"^^xsd:anyURI .

ph:list a owl:DatatypeProperty ;
    rdfs:range ph:list ;
    rdfs:label "list" ;
    rdfs:comment "Ordered list of zero or more values.\nSee [Kinds chapter]`docHaystack::Kinds#list`." ;
    ph:is ph:val ;
    ph:lib ph:lib:ph .

phIoT:load a owl:Class ;
    rdfs:subClassOf ph:marker ;
    rdfs:label "load" ;
    rdfs:comment "Chiller point to command or measure the chiller's load as a percentage\nfrom \"0%\" to \"100%\". When paired with cmd this models the chiller's\nload limit. When paired with sensor this models the chiller's current\nload factor." ;
    ph:is ph:marker ;
    ph:lib phIoT:lib:phIoT .

phIoT:luminaire a owl:Class ;
    rdfs:subClassOf phIoT:equip,
        phIoT:lightingZonePoints,
        phIoT:elec-input ;
    rdfs:label "luminaire" ;
    ph:children _:0b2cb027-d5e1-46c4-0ef8-f23c91a70cca,
        _:0b2cb027-d5e1-46c5-0ef9-f23c91a70cca,
        _:0b2cb027-d5e1-46c6-0efa-f23c91a70cca,
        _:0b2cb027-d5e1-46c7-0efb-f23c91a70cca,
        _:0b2cb027-d5e1-46c8-0efc-f23c91a70cca,
        _:0b2cb027-d5e1-46c9-0efd-f23c91a70cca ;
    rdfs:comment "Light fixture using electricity to provide illumination" ;
    ph:is phIoT:equip,
        phIoT:lightingZonePoints,
        phIoT:elec-input ;
    ph:lib phIoT:lib:phIoT ;
    ph:wikipedia "https://en.wikipedia.org/wiki/Light_fixture"^^xsd:anyURI .

_:0b2cb027-d5e1-46c4-0ef8-f23c91a70cca a phIoT:equip ;
    ph:hasTag phIoT:equip ;
    rdfs:label "{equip}" .

_:0b2cb027-d5e1-46c5-0ef9-f23c91a70cca a phIoT:point ;
    ph:hasTag phScience:light,
        phScience:illuminance,
        phIoT:sensor,
        phIoT:point ;
    rdfs:label "{light, illuminance, sensor, point}" .

_:0b2cb027-d5e1-46c6-0efa-f23c91a70cca a phIoT:point ;
    ph:hasTag phScience:light,
        phScience:level,
        phIoT:sensor,
        phIoT:point ;
    rdfs:label "{light, level, sensor, point}" .

_:0b2cb027-d5e1-46c7-0efb-f23c91a70cca a phIoT:point ;
    ph:hasTag phScience:light,
        phScience:level,
        phIoT:sp,
        phIoT:point ;
    rdfs:label "{light, level, sp, point}" .

_:0b2cb027-d5e1-46c8-0efc-f23c91a70cca a phIoT:point ;
    ph:hasTag phScience:light,
        phScience:luminous,
        phScience:flux,
        phIoT:sensor,
        phIoT:point ;
    rdfs:label "{light, luminous, flux, sensor, point}" .

_:0b2cb027-d5e1-46c9-0efd-f23c91a70cca a phIoT:point ;
    ph:hasTag phIoT:point ;
    rdfs:label "{point}" .

phScience:luminance a owl:Class ;
    rdfs:subClassOf phScience:quantity ;
    rdfs:label "luminance" ;
    rdfs:comment "Energy of light in a given direction.\n\nAlso see [ies.org]`https://www.ies.org/definitions/luminance/`" ;
    ph:is phScience:quantity ;
    ph:lib phScience:lib:phScience ;
    phScience:prefUnit "candelas_per_square_meter",
        "candelas_per_square_foot" ;
    phScience:quantityOf phScience:light ;
    ph:wikipedia "https://en.wikipedia.org/wiki/Luminance"^^xsd:anyURI .

phScience:luminous a owl:Class ;
    rdfs:subClassOf ph:marker ;
    rdfs:label "luminous" ;
    rdfs:comment "Relating to light as perceived by the eye" ;
    ph:is ph:marker ;
    ph:lib phScience:lib:phScience .

phScience:luminous-flux a owl:Class ;
    rdfs:subClassOf phScience:quantity ;
    rdfs:label "luminous-flux" ;
    rdfs:comment "Total perceived light in all directions.\n\nAlso see [ies.org]`https://www.ies.org/definitions/luminous-flux/`" ;
    ph:is phScience:quantity ;
    ph:lib phScience:lib:phScience ;
    phScience:prefUnit "lumen" ;
    phScience:quantityOf phScience:light ;
    ph:wikipedia "https://en.wikipedia.org/wiki/Luminous_flux"^^xsd:anyURI .

phScience:luminous-intensity a owl:Class ;
    rdfs:subClassOf phScience:quantity ;
    rdfs:label "luminous-intensity" ;
    rdfs:comment "Perceived light in a particular direction per unit solid angle.\n\nAlso see [ies.org]`https://www.ies.org/definitions/luminous-intensity/`" ;
    ph:is phScience:quantity ;
    ph:lib phScience:lib:phScience ;
    phScience:prefUnit "candela" ;
    phScience:quantityOf phScience:light ;
    ph:wikipedia "https://en.wikipedia.org/wiki/Luminous_intensity"^^xsd:anyURI .

phScience:magnitude a owl:Class ;
    rdfs:subClassOf ph:marker ;
    rdfs:label "magnitude" ;
    rdfs:comment "Size or extent" ;
    ph:is ph:marker ;
    ph:lib phScience:lib:phScience .

phIoT:makeup a owl:Class ;
    rdfs:subClassOf ph:marker ;
    rdfs:label "makeup" ;
    rdfs:comment "Restore something missed or lost" ;
    ph:is ph:marker ;
    ph:lib phIoT:lib:phIoT .

phIoT:makeup-water a owl:Class ;
    rdfs:subClassOf phScience:water ;
    rdfs:label "makeup-water" ;
    rdfs:comment "Water used used to makeup water loss through leaks, evaporation, or blowdown" ;
    ph:is phScience:water ;
    ph:lib phIoT:lib:phIoT ;
    ph:wikipedia "https://en.wikipedia.org/wiki/Water"^^xsd:anyURI .

phIoT:makeup-water-input a owl:Class ;
    rdfs:subClassOf ph:input ;
    rdfs:label "makeup-water-input" ;
    rdfs:comment "Entity inputs makeup water which flows from another entity" ;
    ph:is ph:input ;
    ph:lib phIoT:lib:phIoT .

phIoT:makeup-water-output a owl:Class ;
    rdfs:subClassOf ph:output ;
    rdfs:label "makeup-water-output" ;
    rdfs:comment "Entity outputs makeup water to other entities" ;
    ph:is ph:output ;
    ph:lib phIoT:lib:phIoT .

phIoT:makeupWaterRef a owl:ObjectProperty ;
    rdfs:domain phIoT:makeup-water-input ;
    rdfs:range phIoT:makeup-water-output ;
    rdfs:label "makeupWaterRef" ;
    rdfs:comment "Makeup water flows from the referent to this entity" ;
    ph:inputs phIoT:makeup-water ;
    ph:is ph:ref ;
    ph:lib phIoT:lib:phIoT ;
    ph:of phIoT:makeup-water-output ;
    ph:tagOn phIoT:makeup-water-input .

ph:mandatory a owl:Class ;
    rdfs:subClassOf ph:marker ;
    rdfs:label "mandatory" ;
    rdfs:comment "Requires that the marker be applied to dicts which use the marker's subtypes.\nThis tag is typically applied to top-level entity tags such as 'equip'.\nFor example if an instance is tagged with a subtype of 'equip' such\nas 'tank', then the instance must also include the 'equip' tag as a\nmandatory marker." ;
    ph:is ph:marker ;
    ph:lib ph:lib:ph ;
    ph:notInherited ph:marker ;
    ph:tagOn ph:def .

ph:marker a owl:Class ;
    rdfs:label "marker" ;
    rdfs:comment "Marker labels a dict with typing information.\nSee [Kinds chapter]`docHaystack::Kinds#marker`." ;
    ph:docTaxonomy ph:marker ;
    ph:lib ph:lib:ph .

phIoT:mau a owl:Class ;
    rdfs:subClassOf phIoT:doas ;
    rdfs:label "mau" ;
    ph:children _:0b2cb027-d60f-0d80-0efe-f23c91a70cca,
        _:0b2cb027-d60f-0d81-0eff-f23c91a70cca,
        _:0b2cb027-d60f-0d82-0f00-f23c91a70cca,
        _:0b2cb027-d60f-0d83-0f01-f23c91a70cca,
        _:0b2cb027-d60f-0d84-0f02-f23c91a70cca,
        _:0b2cb027-d60f-0d85-0f03-f23c91a70cca,
        _:0b2cb027-d60f-0d86-0f04-f23c91a70cca,
        _:0b2cb027-d60f-0d87-0f05-f23c91a70cca,
        _:0b2cb027-d60f-0d88-0f06-f23c91a70cca,
        _:0b2cb027-d60f-0d89-0f07-f23c91a70cca,
        _:0b2cb027-d60f-0d8a-0f08-f23c91a70cca,
        _:0b2cb027-d60f-0d8b-0f09-f23c91a70cca,
        _:0b2cb027-d60f-0d8c-0f0a-f23c91a70cca,
        _:0b2cb027-d60f-0d8d-0f0b-f23c91a70cca,
        _:0b2cb027-d60f-0d8e-0f0c-f23c91a70cca,
        _:0b2cb027-d60f-0d8f-0f0d-f23c91a70cca,
        _:0b2cb027-d60f-0d90-0f0e-f23c91a70cca,
        _:0b2cb027-d60f-0d91-0f0f-f23c91a70cca,
        _:0b2cb027-d60f-0d92-0f10-f23c91a70cca,
        _:0b2cb027-d60f-0d93-0f11-f23c91a70cca,
        _:0b2cb027-d60f-0d94-0f12-f23c91a70cca ;
    rdfs:comment "Makeup Air Unit: A DOAS that provides make-up air for a separate, dedicated\nexhaust system. That is, this equip does not contain an exhaust air section.\nSee `docHaystack::AHUs` chapter." ;
    ph:is phIoT:doas ;
    ph:lib phIoT:lib:phIoT ;
    ph:wikipedia "https://en.wikipedia.org/wiki/Air_handler"^^xsd:anyURI .

_:0b2cb027-d60f-0d80-0efe-f23c91a70cca a phIoT:point ;
    ph:hasTag phIoT:bypass,
        phIoT:damper,
        phIoT:cmd,
        phIoT:point ;
    rdfs:label "{bypass, damper, cmd, point}" .

_:0b2cb027-d60f-0d81-0eff-f23c91a70cca a phIoT:point ;
    ph:hasTag phIoT:cool,
        phIoT:cmd,
        phIoT:point ;
    rdfs:label "{cool, cmd, point}" .

_:0b2cb027-d60f-0d82-0f00-f23c91a70cca a phIoT:point ;
    ph:hasTag phIoT:dessicantDehumidifier,
        phIoT:cmd,
        phIoT:point ;
    rdfs:label "{dessicantDehumidifier, cmd, point}" .

_:0b2cb027-d60f-0d83-0f01-f23c91a70cca a phIoT:duct ;
    ph:hasTag phIoT:discharge,
        phIoT:duct,
        phIoT:equip ;
    rdfs:label "{discharge, duct, equip}" .

_:0b2cb027-d60f-0d84-0f02-f23c91a70cca a phIoT:duct ;
    ph:hasTag phIoT:economizer,
        phIoT:duct,
        phIoT:equip ;
    rdfs:label "{economizer, duct, equip}" .

_:0b2cb027-d60f-0d85-0f03-f23c91a70cca a phIoT:point ;
    ph:hasTag phIoT:economizing,
        phIoT:cmd,
        phIoT:point ;
    rdfs:label "{economizing, cmd, point}" .

_:0b2cb027-d60f-0d86-0f04-f23c91a70cca a phIoT:equip ;
    ph:hasTag phIoT:equip ;
    rdfs:label "{equip}" .

_:0b2cb027-d60f-0d87-0f05-f23c91a70cca a phIoT:duct ;
    ph:hasTag phIoT:exhaust,
        phIoT:duct,
        phIoT:equip ;
    rdfs:label "{exhaust, duct, equip}" .

_:0b2cb027-d60f-0d88-0f06-f23c91a70cca a phIoT:point ;
    ph:hasTag phIoT:faceBypass,
        phIoT:cmd,
        phIoT:point ;
    rdfs:label "{faceBypass, cmd, point}" .

_:0b2cb027-d60f-0d89-0f07-f23c91a70cca a phIoT:point ;
    ph:hasTag phIoT:filter,
        phIoT:sensor,
        phIoT:point ;
    rdfs:label "{filter, sensor, point}" .

_:0b2cb027-d60f-0d8a-0f08-f23c91a70cca a phIoT:point ;
    ph:hasTag phIoT:freezeStat,
        phIoT:sensor,
        phIoT:point ;
    rdfs:label "{freezeStat, sensor, point}" .

_:0b2cb027-d60f-0d8b-0f09-f23c91a70cca a phIoT:point ;
    ph:hasTag phIoT:heat,
        phIoT:cmd,
        phIoT:point ;
    rdfs:label "{heat, cmd, point}" .

_:0b2cb027-d60f-0d8c-0f0a-f23c91a70cca a phIoT:point ;
    ph:hasTag phIoT:heatWheel,
        phIoT:cmd,
        phIoT:point ;
    rdfs:label "{heatWheel, cmd, point}" .

_:0b2cb027-d60f-0d8d-0f0b-f23c91a70cca a phIoT:humidifier-equip ;
    ph:hasTag phIoT:humidifier,
        phIoT:equip ;
    rdfs:label "{humidifier, equip}" .

_:0b2cb027-d60f-0d8e-0f0c-f23c91a70cca a phIoT:point ;
    ph:hasTag phIoT:hvacMode,
        phIoT:sp,
        phIoT:point ;
    rdfs:label "{hvacMode, sp, point}" .

_:0b2cb027-d60f-0d8f-0f0d-f23c91a70cca a phIoT:duct ;
    ph:hasTag phIoT:mixed,
        phIoT:duct,
        phIoT:equip ;
    rdfs:label "{mixed, duct, equip}" .

_:0b2cb027-d60f-0d90-0f0e-f23c91a70cca a phIoT:duct ;
    ph:hasTag phIoT:outside,
        phIoT:duct,
        phIoT:equip ;
    rdfs:label "{outside, duct, equip}" .

_:0b2cb027-d60f-0d91-0f0f-f23c91a70cca a phIoT:point ;
    ph:hasTag phIoT:point ;
    rdfs:label "{point}" .

_:0b2cb027-d60f-0d92-0f10-f23c91a70cca a phIoT:duct ;
    ph:hasTag phIoT:return,
        phIoT:duct,
        phIoT:equip ;
    rdfs:label "{return, duct, equip}" .

_:0b2cb027-d60f-0d93-0f11-f23c91a70cca a phIoT:thermostat ;
    ph:hasTag phIoT:thermostat,
        phIoT:equip ;
    rdfs:label "{thermostat, equip}" .

_:0b2cb027-d60f-0d94-0f12-f23c91a70cca a phIoT:duct ;
    ph:hasTag phIoT:ventilation,
        phIoT:duct,
        phIoT:equip ;
    rdfs:label "{ventilation, duct, equip}" .

ph:max a owl:Class ;
    rdfs:subClassOf ph:marker ;
    rdfs:label "max" ;
    rdfs:comment "Maximum" ;
    ph:is ph:marker ;
    ph:lib ph:lib:ph .

ph:maxVal a owl:DatatypeProperty ;
    rdfs:domain ph:def,
        phIoT:point ;
    rdfs:range ph:number ;
    rdfs:label "maxVal" ;
    rdfs:comment "Inclusive maximum for a numeric value." ;
    ph:is ph:number ;
    ph:lib ph:lib:ph ;
    ph:tagOn ph:def,
        phIoT:point .

phIoT:mech a owl:Class ;
    rdfs:subClassOf ph:marker ;
    rdfs:label "mech" ;
    rdfs:comment "Associated with a machine or its mechanical force, torque, power, or energy.\nThis is often opposed to `elec` electrical energy." ;
    ph:is ph:marker ;
    ph:lib phIoT:lib:phIoT .

phIoT:meter a owl:Class ;
    rdfs:subClassOf phIoT:equip ;
    rdfs:label "meter" ;
    ph:children _:0b2cb027-d61e-4fc0-0f13-f23c91a70cca,
        _:0b2cb027-d61e-4fc1-0f14-f23c91a70cca ;
    rdfs:comment "Equipment to meter a substance or phenomenon.\nSee `docHaystack::Meters` chapter." ;
    ph:is phIoT:equip ;
    ph:lib phIoT:lib:phIoT .

_:0b2cb027-d61e-4fc0-0f13-f23c91a70cca a phIoT:equip ;
    ph:hasTag phIoT:equip ;
    rdfs:label "{equip}" .

_:0b2cb027-d61e-4fc1-0f14-f23c91a70cca a phIoT:point ;
    ph:hasTag phIoT:point ;
    rdfs:label "{point}" .

phIoT:meterScope a owl:Class ;
    rdfs:subClassOf ph:choice ;
    rdfs:label "meterScope" ;
    rdfs:comment "Classifies a meter as a main site meter or submeter" ;
    ph:is ph:choice ;
    ph:lib phIoT:lib:phIoT ;
    ph:tagOn phIoT:meter .

ph:mime a owl:DatatypeProperty ;
    rdfs:domain ph:filetype ;
    rdfs:range ph:str ;
    rdfs:label "mime" ;
    rdfs:comment "Mime type formatted as type/subtype" ;
    ph:is ph:str ;
    ph:lib ph:lib:ph ;
    ph:tagOn ph:filetype .

ph:min a owl:Class ;
    rdfs:subClassOf ph:marker ;
    rdfs:label "min" ;
    rdfs:comment "Minimum" ;
    ph:is ph:marker ;
    ph:lib ph:lib:ph .

ph:minVal a owl:DatatypeProperty ;
    rdfs:domain ph:def,
        phIoT:point ;
    rdfs:range ph:number ;
    rdfs:label "minVal" ;
    rdfs:comment "Inclusive minimum for a numeric value." ;
    ph:is ph:number ;
    ph:lib ph:lib:ph ;
    ph:tagOn ph:def,
        phIoT:point .

phIoT:mixed a owl:Class ;
    rdfs:subClassOf phIoT:ductSection ;
    rdfs:label "mixed" ;
    rdfs:comment "Duct where fresh outside air and return air is mixed together" ;
    ph:is phIoT:ductSection ;
    ph:lib phIoT:lib:phIoT .

phIoT:mixing a owl:Class ;
    rdfs:subClassOf ph:marker ;
    rdfs:label "mixing" ;
    rdfs:comment "Three way valve which inputs two pipes and outputs a mixture\nbetween the two to a single output pipe." ;
    ph:is ph:marker ;
    ph:lib phIoT:lib:phIoT .

phIoT:ml a owl:Class ;
    rdfs:subClassOf phIoT:synthetic ;
    rdfs:label "ml" ;
    rdfs:comment "Machine learning point. See `docHaystack::Synthetics` chapter." ;
    ph:is phIoT:synthetic ;
    ph:lib phIoT:lib:phIoT .

phIoT:ml-point a owl:Class ;
    rdfs:subClassOf phIoT:synthetic-point ;
    rdfs:label "ml-point" ;
    rdfs:comment "See `docHaystack::Synthetics` chapter." ;
    ph:is phIoT:synthetic-point ;
    ph:lib phIoT:lib:phIoT .

phIoT:mlIdentificationPeriod a owl:DatatypeProperty ;
    rdfs:domain phIoT:mlModel ;
    rdfs:range ph:xstr ;
    rdfs:label "mlIdentificationPeriod" ;
    rdfs:comment "Training period description, known as the identification period\nor baseline, utilized during the model training process." ;
    ph:is ph:span ;
    ph:lib phIoT:lib:phIoT ;
    ph:tagOn phIoT:mlModel .

phIoT:mlInputVarRefs a owl:DatatypeProperty ;
    rdfs:domain phIoT:mlModel ;
    rdfs:range ph:list ;
    rdfs:label "mlInputVarRefs" ;
    rdfs:comment "List of independent variables, also known as model inputs or features,\nassociated with a machine learning model." ;
    ph:is ph:list ;
    ph:lib phIoT:lib:phIoT ;
    ph:of phIoT:mlVarRef ;
    ph:tagOn phIoT:mlModel .

phIoT:mlModel a owl:Class ;
    rdfs:subClassOf phIoT:syntheticModel ;
    rdfs:label "mlModel" ;
    rdfs:comment "See `docHaystack::Synthetics` chapter." ;
    ph:is phIoT:syntheticModel ;
    ph:lib phIoT:lib:phIoT .

phIoT:mlModelMetrics a owl:DatatypeProperty ;
    rdfs:domain phIoT:mlModel ;
    rdfs:range ph:dict ;
    rdfs:label "mlModelMetrics" ;
    rdfs:comment "Goodness-of-fit metrics provided in the form of a simple dictionary.\nFor example: {r2:0.7889, cvrmse:58}." ;
    ph:is ph:dict ;
    ph:lib phIoT:lib:phIoT ;
    ph:tagOn phIoT:mlModel .

phIoT:mlModelParameters a owl:DatatypeProperty ;
    rdfs:domain phIoT:mlModel ;
    rdfs:range ph:dict ;
    rdfs:label "mlModelParameters" ;
    rdfs:comment "Result of model identification, which may appear as a list of\nmodel parameters for simpler models or as a reference to a stored model,\nin the form of a file uri. The structure of the dict is user-specific." ;
    ph:is ph:dict ;
    ph:lib phIoT:lib:phIoT ;
    ph:tagOn phIoT:mlModel .

phIoT:mlOutputVarRef a owl:ObjectProperty ;
    rdfs:domain phIoT:mlModel ;
    rdfs:range phIoT:mlVar ;
    rdfs:label "mlOutputVarRef" ;
    rdfs:comment "Dependent variable, also known as the model output or target,\nassociated, with a machine learning model.\nRepresents the predicted outcome generated by the model." ;
    ph:is ph:ref ;
    ph:lib phIoT:lib:phIoT ;
    ph:of phIoT:mlVar ;
    ph:tagOn phIoT:mlModel .

phIoT:mlVar a owl:Class ;
    rdfs:subClassOf ph:entity ;
    rdfs:label "mlVar" ;
    rdfs:comment "Machine learning variable representing both model inputs and outputs." ;
    ph:is ph:entity ;
    ph:lib phIoT:lib:phIoT ;
    ph:mandatory ph:marker .

phIoT:mlVarFilter a owl:DatatypeProperty ;
    rdfs:domain phIoT:mlVar ;
    rdfs:range ph:str ;
    rdfs:label "mlVarFilter" ;
    rdfs:comment "Filter used for querying points by tags, providing more flexibility\nthan mlVarPoint, although it is not mandatory." ;
    ph:is ph:filterStr ;
    ph:lib phIoT:lib:phIoT ;
    ph:tagOn phIoT:mlVar .

phIoT:mlVarPoint a owl:ObjectProperty ;
    rdfs:domain phIoT:mlVar ;
    rdfs:range phIoT:point ;
    rdfs:label "mlVarPoint" ;
    rdfs:comment "Reference to a point associated with a machine learning variable,\nknown as a machine learning variable point." ;
    ph:is ph:ref ;
    ph:lib phIoT:lib:phIoT ;
    ph:of phIoT:point ;
    ph:tagOn phIoT:mlVar .

phIoT:mlVarRef a owl:ObjectProperty ;
    rdfs:range phIoT:mlVar ;
    rdfs:label "mlVarRef" ;
    rdfs:comment "Reference to a machine learning variable." ;
    ph:is ph:ref ;
    ph:lib phIoT:lib:phIoT ;
    ph:of phIoT:mlVar .

phIct:mobile a owl:Class ;
    rdfs:subClassOf ph:marker ;
    rdfs:label "mobile" ;
    rdfs:comment "Relating to mobile phones, hand-held computers, and similar technology" ;
    ph:is ph:marker ;
    ph:lib phIct:lib:phIct .

phIct:mobile-phone a owl:Class ;
    rdfs:subClassOf phIct:phone ;
    rdfs:label "mobile-phone" ;
    rdfs:comment "Cellular phone providing telecommunication over radio links." ;
    ph:is phIct:phone ;
    ph:lib phIct:lib:phIct ;
    ph:wikipedia "https://en.wikipedia.org/wiki/Mobile_phone"^^xsd:anyURI .

phIct:modbus a owl:Class ;
    rdfs:subClassOf phIct:protocol ;
    rdfs:label "modbus" ;
    rdfs:comment "Register based communication protocol used with industrial devices." ;
    ph:is phIct:protocol ;
    ph:lib phIct:lib:phIct ;
    ph:wikipedia "https://en.wikipedia.org/wiki/Modbus"^^xsd:anyURI .

phIoT:motor a owl:Class ;
    rdfs:subClassOf phIoT:equip,
        phIoT:elec-input ;
    rdfs:label "motor" ;
    ph:children _:0b2cb027-d62d-9200-0f15-f23c91a70cca,
        _:0b2cb027-d62d-9201-0f16-f23c91a70cca,
        _:0b2cb027-d62d-9202-0f17-f23c91a70cca,
        _:0b2cb027-d62d-9203-0f18-f23c91a70cca,
        _:0b2cb027-d62d-9204-0f19-f23c91a70cca,
        _:0b2cb027-d62d-9205-0f1a-f23c91a70cca,
        _:0b2cb027-d62d-9206-0f1b-f23c91a70cca,
        _:0b2cb027-d62d-9207-0f1c-f23c91a70cca,
        _:0b2cb027-d62d-9208-0f1d-f23c91a70cca,
        _:0b2cb027-d62d-9209-0f1e-f23c91a70cca,
        _:0b2cb027-d62d-920a-0f1f-f23c91a70cca ;
    rdfs:comment "Equipment that converts electrical energy into mechanical energy.\nSee `docHaystack::Motors` chapter." ;
    ph:is phIoT:equip,
        phIoT:elec-input ;
    ph:lib phIoT:lib:phIoT ;
    ph:wikipedia "https://en.wikipedia.org/wiki/Electric_motor"^^xsd:anyURI .

_:0b2cb027-d62d-9200-0f15-f23c91a70cca a phIoT:point ;
    ph:hasTag phIoT:alarm,
        phIoT:sensor,
        phIoT:point ;
    rdfs:label "{alarm, sensor, point}" .

_:0b2cb027-d62d-9201-0f16-f23c91a70cca a phIoT:point ;
    ph:hasTag phIoT:enable,
        phIoT:cmd,
        phIoT:point ;
    rdfs:label "{enable, cmd, point}" .

_:0b2cb027-d62d-9202-0f17-f23c91a70cca a phIoT:point ;
    ph:hasTag phIoT:enable,
        phIoT:sensor,
        phIoT:point ;
    rdfs:label "{enable, sensor, point}" .

_:0b2cb027-d62d-9203-0f18-f23c91a70cca a phIoT:equip ;
    ph:hasTag phIoT:equip ;
    rdfs:label "{equip}" .

_:0b2cb027-d62d-9204-0f19-f23c91a70cca a phIoT:point ;
    ph:hasTag phIoT:point ;
    rdfs:label "{point}" .

_:0b2cb027-d62d-9205-0f1a-f23c91a70cca a phIoT:point ;
    ph:hasTag phIoT:run,
        phIoT:cmd,
        phIoT:point ;
    rdfs:label "{run, cmd, point}" .

_:0b2cb027-d62d-9206-0f1b-f23c91a70cca a phIoT:point ;
    ph:hasTag phIoT:run,
        phIoT:sensor,
        phIoT:point ;
    rdfs:label "{run, sensor, point}" .

_:0b2cb027-d62d-9207-0f1c-f23c91a70cca a phIoT:point ;
    ph:hasTag phIoT:vfd,
        phScience:freq,
        phIoT:cmd,
        phIoT:point ;
    rdfs:label "{vfd, freq, cmd, point}" .

_:0b2cb027-d62d-9208-0f1d-f23c91a70cca a phIoT:point ;
    ph:hasTag phIoT:vfd,
        phScience:freq,
        phIoT:sensor,
        phIoT:point ;
    rdfs:label "{vfd, freq, sensor, point}" .

_:0b2cb027-d62d-9209-0f1e-f23c91a70cca a phIoT:point ;
    ph:hasTag phIoT:vfd,
        phScience:speed,
        phIoT:cmd,
        phIoT:point ;
    rdfs:label "{vfd, speed, cmd, point}" .

_:0b2cb027-d62d-920a-0f1f-f23c91a70cca a phIoT:point ;
    ph:hasTag phIoT:vfd,
        phScience:speed,
        phIoT:sensor,
        phIoT:point ;
    rdfs:label "{vfd, speed, sensor, point}" .

phIoT:movingWalkway a owl:Class ;
    rdfs:subClassOf phIoT:verticalTransport,
        phIoT:elec-input ;
    rdfs:label "movingWalkway" ;
    ph:children _:0b2cb027-d62d-920b-0f20-f23c91a70cca,
        _:0b2cb027-d62d-920c-0f21-f23c91a70cca ;
    rdfs:comment "Conveyor to move people across a horizontal or inclined plane." ;
    ph:is phIoT:verticalTransport,
        phIoT:elec-input ;
    ph:lib phIoT:lib:phIoT ;
    ph:wikipedia "https://en.wikipedia.org/wiki/Moving_walkway"^^xsd:anyURI .

_:0b2cb027-d62d-920b-0f20-f23c91a70cca a phIoT:equip ;
    ph:hasTag phIoT:equip ;
    rdfs:label "{equip}" .

_:0b2cb027-d62d-920c-0f21-f23c91a70cca a phIoT:point ;
    ph:hasTag phIoT:point ;
    rdfs:label "{point}" .

phIct:mqtt a owl:Class ;
    rdfs:subClassOf phIct:protocol ;
    rdfs:label "mqtt" ;
    rdfs:comment "Message Queuing Telemetry Transport publish/subscribe protocol" ;
    ph:is phIct:protocol ;
    ph:lib phIct:lib:phIct ;
    ph:wikipedia "https://en.wikipedia.org/wiki/MQTT"^^xsd:anyURI .

phIoT:multiZone a owl:Class ;
    rdfs:subClassOf phIoT:ahuZoneDelivery ;
    rdfs:label "multiZone" ;
    rdfs:comment "AHU discharge air is split into a duct per zone" ;
    ph:is phIoT:ahuZoneDelivery ;
    ph:lib phIoT:lib:phIoT .

phScience:n2o a owl:Class ;
    rdfs:subClassOf phScience:gas ;
    rdfs:label "n2o" ;
    rdfs:comment "Nitrous oxide (N\u2082O)" ;
    ph:is phScience:gas ;
    ph:lib phScience:lib:phScience ;
    ph:wikipedia "https://en.wikipedia.org/wiki/Nitrous_oxide"^^xsd:anyURI .

phScience:n2o-emission a owl:Class ;
    rdfs:subClassOf phScience:emission ;
    rdfs:label "n2o-emission" ;
    rdfs:comment "Greenhouse gas emission of nitrous oxide (N\u2082O) into the air." ;
    ph:is phScience:emission ;
    ph:lib phScience:lib:phScience ;
    phScience:prefUnit "kg",
        "ton",
        "lb" ;
    phScience:quantityOf phScience:air .

ph:na a owl:DatatypeProperty ;
    rdfs:subClassOf xsd:string ;
    rdfs:label "na" ;
    rdfs:comment "Not available used to indicate invalid or missing data.\nSee [Kinds chapter]`docHaystack::Kinds#na`." ;
    ph:is ph:scalar ;
    ph:lib ph:lib:ph .

phIoT:naturalGas a owl:Class ;
    rdfs:subClassOf phScience:gas ;
    rdfs:label "naturalGas" ;
    rdfs:comment "Fossil fuel energy source consisting largely of methane and other hydrocarbons.\n\nThe energy content of natural gas varies by region within a range determined\non impurities in the gas.  You can find a table of these conversions\n[here]`https://en.wikipedia.org/wiki/Heat_of_combustion#Higher_heating_values_of_natural_gases_from_various_sources`" ;
    ph:is phScience:gas ;
    ph:lib phIoT:lib:phIoT ;
    ph:wikipedia "https://en.wikipedia.org/wiki/Natural_gas"^^xsd:anyURI .

phIoT:naturalGas-input a owl:Class ;
    rdfs:subClassOf ph:input ;
    rdfs:label "naturalGas-input" ;
    rdfs:comment "Entity inputs natural gas which flows from another entity" ;
    ph:is ph:input ;
    ph:lib phIoT:lib:phIoT .

phIoT:naturalGas-output a owl:Class ;
    rdfs:subClassOf ph:output ;
    rdfs:label "naturalGas-output" ;
    rdfs:comment "Entity outputs natural gas to other entities" ;
    ph:is ph:output ;
    ph:lib phIoT:lib:phIoT .

phIoT:naturalGasHeating a owl:Class ;
    rdfs:subClassOf phIoT:heatingProcess,
        phIoT:naturalGas-input ;
    rdfs:label "naturalGasHeating" ;
    rdfs:comment "Heating by the combustion of natural gas" ;
    ph:is phIoT:heatingProcess,
        phIoT:naturalGas-input ;
    ph:lib phIoT:lib:phIoT .

phIoT:naturalGasRef a owl:ObjectProperty ;
    rdfs:domain phIoT:naturalGas-input ;
    rdfs:range phIoT:naturalGas-output ;
    rdfs:label "naturalGasRef" ;
    rdfs:comment "Natural gas flows from the referent to this entity" ;
    ph:inputs phIoT:naturalGas ;
    ph:is ph:ref ;
    ph:lib phIoT:lib:phIoT ;
    ph:of phIoT:naturalGas-output ;
    ph:tagOn phIoT:naturalGas-input .

phIoT:net a owl:Class ;
    rdfs:subClassOf ph:marker ;
    rdfs:label "net" ;
    rdfs:comment "Difference between import and export" ;
    ph:is ph:marker ;
    ph:lib phIoT:lib:phIoT .

phIct:network a owl:Class ;
    rdfs:subClassOf ph:entity ;
    rdfs:label "network" ;
    rdfs:comment "Logical communications network between two or more devices.\nSee `docHaystack::Devices#networks` chapter." ;
    ph:is ph:entity ;
    ph:lib phIct:lib:phIct .

phIct:networkRef a owl:ObjectProperty ;
    rdfs:range phIct:network ;
    rdfs:label "networkRef" ;
    rdfs:comment "Associates a device which communicates on specific a network." ;
    ph:is ph:ref ;
    ph:lib phIct:lib:phIct ;
    ph:of phIct:network .

phIct:networking a owl:Class ;
    rdfs:subClassOf ph:marker ;
    rdfs:label "networking" ;
    rdfs:comment "Related to data communication networks" ;
    ph:is ph:marker ;
    ph:lib phIct:lib:phIct .

phIct:networking-device a owl:Class ;
    rdfs:subClassOf phIct:device ;
    rdfs:label "networking-device" ;
    rdfs:comment "Microprocessor device used to establish networks." ;
    ph:is phIct:device ;
    ph:lib phIct:lib:phIct ;
    ph:wikipedia "https://en.wikipedia.org/wiki/Networking_hardware"^^xsd:anyURI .

phIct:networking-router a owl:Class ;
    rdfs:subClassOf phIct:networking-device ;
    rdfs:label "networking-router" ;
    rdfs:comment "Networking device used to route data between different networks." ;
    ph:is phIct:networking-device ;
    ph:lib phIct:lib:phIct ;
    ph:wikipedia "https://en.wikipedia.org/wiki/Router_(computing)"^^xsd:anyURI .

phIct:networking-switch a owl:Class ;
    rdfs:subClassOf phIct:networking-device ;
    rdfs:label "networking-switch" ;
    rdfs:comment "Networking device used to connect devices on the same network." ;
    ph:is phIct:networking-device ;
    ph:lib phIct:lib:phIct ;
    ph:wikipedia "https://en.wikipedia.org/wiki/Network_switch"^^xsd:anyURI .

phIoT:neutral a owl:Class ;
    rdfs:subClassOf ph:marker ;
    rdfs:label "neutral" ;
    rdfs:comment "when applied to a point entity that has the `elec` and `current` tags,\nindicates electrical current being measured on an electrical neutral\nconductor." ;
    ph:is ph:marker ;
    ph:lib phIoT:lib:phIoT .

phIoT:neutralDeck a owl:Class ;
    rdfs:subClassOf phIoT:ductDeck ;
    rdfs:label "neutralDeck" ;
    rdfs:comment "Duct carries air which by-passes both heating and cooling coils" ;
    ph:is phIoT:ductDeck ;
    ph:lib phIoT:lib:phIoT .

phScience:nf3 a owl:Class ;
    rdfs:subClassOf phScience:gas ;
    rdfs:label "nf3" ;
    rdfs:comment "Nitrogen trifluoride (NF\u2083)" ;
    ph:is phScience:gas ;
    ph:lib phScience:lib:phScience ;
    ph:wikipedia "https://en.wikipedia.org/wiki/Nitrogen_trifluoride"^^xsd:anyURI .

phScience:nf3-emission a owl:Class ;
    rdfs:subClassOf phScience:emission ;
    rdfs:label "nf3-emission" ;
    rdfs:comment "Greenhouse gas emission of nitrogen trifluoride (NF\u2083) into the air." ;
    ph:is phScience:emission ;
    ph:lib phScience:lib:phScience ;
    phScience:prefUnit "kg",
        "ton",
        "lb" ;
    phScience:quantityOf phScience:air .

phScience:nh3 a owl:Class ;
    rdfs:subClassOf phScience:gas ;
    rdfs:label "nh3" ;
    rdfs:comment "Ammonia (NH\u2083)" ;
    ph:is phScience:gas ;
    ph:lib phScience:lib:phScience ;
    ph:wikipedia "https://en.wikipedia.org/wiki/Ammonia"^^xsd:anyURI .

phScience:nh3-concentration a owl:Class ;
    rdfs:subClassOf phScience:airQuality ;
    rdfs:label "nh3-concentration" ;
    rdfs:comment "Concentration of ammonia (NH\u2083) in the air" ;
    ph:is phScience:airQuality ;
    ph:lib phScience:lib:phScience ;
    phScience:prefUnit "\u00b5g/m\u00b3",
        "ppb" ;
    phScience:quantityOf phScience:air ;
    ph:wikipedia "https://en.wikipedia.org/wiki/Concentration"^^xsd:anyURI .

phScience:no2 a owl:Class ;
    rdfs:subClassOf phScience:gas ;
    rdfs:label "no2" ;
    rdfs:comment "Nitrogen dioxide (NO\u2082)" ;
    ph:is phScience:gas ;
    ph:lib phScience:lib:phScience ;
    ph:wikipedia "https://en.wikipedia.org/wiki/Nitrogen_dioxide"^^xsd:anyURI .

phScience:no2-concentration a owl:Class ;
    rdfs:subClassOf phScience:airQuality ;
    rdfs:label "no2-concentration" ;
    rdfs:comment "Concentration of nitrogen dioxide (NO\u2082) in the air" ;
    ph:is phScience:airQuality ;
    ph:lib phScience:lib:phScience ;
    phScience:prefUnit "\u00b5g/m\u00b3",
        "ppb" ;
    phScience:quantityOf phScience:air ;
    ph:wikipedia "https://en.wikipedia.org/wiki/Concentration"^^xsd:anyURI .

ph:noSideEffects a owl:Class ;
    rdfs:subClassOf ph:marker ;
    rdfs:label "noSideEffects" ;
    rdfs:comment "Marks a function or operation as having no side effects.  The function\nmay or may not be *pure* in that calling it multiple times with the\nsame arguments always evaluates to the same result." ;
    ph:is ph:marker ;
    ph:lib ph:lib:ph ;
    ph:wikipedia "https://en.wikipedia.org/wiki/Side_effect_(computer_science)"^^xsd:anyURI .

ph:nodoc a owl:Class ;
    rdfs:subClassOf ph:marker ;
    rdfs:label "nodoc" ;
    rdfs:comment "Undocumented and not officially supported" ;
    ph:is ph:marker ;
    ph:lib ph:lib:ph .

ph:nosrc a owl:Class ;
    rdfs:subClassOf ph:marker ;
    rdfs:label "nosrc" ;
    rdfs:comment "Do not include source code in documentation" ;
    ph:is ph:marker ;
    ph:lib ph:lib:ph .

ph:notInherited a owl:Class ;
    rdfs:subClassOf ph:marker ;
    rdfs:label "notInherited" ;
    rdfs:comment "Marker applied to a def to indicate that is not inherited into\nsubtype definitions." ;
    ph:is ph:marker ;
    ph:lib ph:lib:ph ;
    ph:tagOn ph:def .

ph:number a owl:DatatypeProperty ;
    rdfs:subClassOf xsd:double ;
    rdfs:label "number" ;
    rdfs:comment "Integer or floating point numbers annotated with an optional unit.\nSee [Kinds chapter]`docHaystack::Kinds#number`." ;
    ph:is ph:scalar ;
    ph:lib ph:lib:ph .

phScience:o2 a owl:Class ;
    rdfs:subClassOf phScience:gas ;
    rdfs:label "o2" ;
    rdfs:comment "Oxygen (O\u2082) - the common dioxygen allotrope in the air" ;
    ph:is phScience:gas ;
    ph:lib phScience:lib:phScience ;
    ph:wikipedia "https://en.wikipedia.org/wiki/Oxygen"^^xsd:anyURI .

phScience:o3 a owl:Class ;
    rdfs:subClassOf phScience:gas ;
    rdfs:label "o3" ;
    rdfs:comment "Ozone (O\u2083)" ;
    ph:is phScience:gas ;
    ph:lib phScience:lib:phScience ;
    ph:wikipedia "https://en.wikipedia.org/wiki/Ozone"^^xsd:anyURI .

phScience:o3-concentration a owl:Class ;
    rdfs:subClassOf phScience:airQuality ;
    rdfs:label "o3-concentration" ;
    rdfs:comment "Concentration of ozone (O\u2083) in the air" ;
    ph:is phScience:airQuality ;
    ph:lib phScience:lib:phScience ;
    phScience:prefUnit "ppm" ;
    phScience:quantityOf phScience:air ;
    ph:wikipedia "https://en.wikipedia.org/wiki/Concentration"^^xsd:anyURI .

phIct:obix a owl:Class ;
    rdfs:subClassOf phIct:protocol ;
    rdfs:label "obix" ;
    rdfs:comment "XML based Open Building Information eXchange protocol." ;
    ph:is phIct:protocol ;
    ph:lib phIct:lib:phIct ;
    ph:wikipedia "https://en.wikipedia.org/wiki/OBIX"^^xsd:anyURI .

phIoT:occ a owl:Class ;
    rdfs:subClassOf ph:marker ;
    rdfs:label "occ" ;
    rdfs:comment "Occupied mode of a space.\nSee `docHaystack::Zones#occupancy` chapter." ;
    ph:is ph:marker ;
    ph:lib phIoT:lib:phIoT .

phIoT:occupancy a owl:Class ;
    rdfs:subClassOf ph:marker ;
    rdfs:label "occupancy" ;
    rdfs:comment "Number of occupants in a space.\nSee `docHaystack::Zones#occupancy` chapter." ;
    ph:is ph:marker ;
    ph:lib phIoT:lib:phIoT .

phIoT:occupants a owl:Class ;
    rdfs:subClassOf ph:marker ;
    rdfs:label "occupants" ;
    rdfs:comment "People who use the built environment.\nSee `docHaystack::Zones#occupancy` chapter." ;
    ph:is ph:marker ;
    ph:lib phIoT:lib:phIoT .

phIoT:occupied a owl:Class ;
    rdfs:subClassOf ph:marker ;
    rdfs:label "occupied" ;
    rdfs:comment "Setpoint or sensor indicating occupancy of a space.\nSee `docHaystack::Zones#occupancy` chapter." ;
    ph:is ph:marker ;
    ph:lib phIoT:lib:phIoT .

ph:of a owl:DatatypeProperty ;
    rdfs:domain ph:def ;
    rdfs:range ph:symbol ;
    rdfs:label "of" ;
    rdfs:comment "Expected value type of a collection, reference, or choice" ;
    ph:is ph:symbol ;
    ph:lib ph:lib:ph ;
    ph:tagOn ph:def .

ph:op rdfs:label "op" ;
    rdfs:comment "Operation for HTTP API.\nSee `docHaystack::Ops` chapter." ;
    ph:is ph:feature ;
    ph:lib ph:lib:ph .

ph:op:about rdfs:label "op:about" ;
    rdfs:comment "Query basic information about the server.\nSee `docHaystack::Ops#about` chapter." ;
    ph:is ph:op ;
    ph:lib ph:lib:ph ;
    ph:noSideEffects ph:marker .

ph:op:close rdfs:label "op:close" ;
    rdfs:comment "Close the current session and cancel the auth bearer token.\nSee `docHaystack::Ops#close` chapter." ;
    ph:is ph:op ;
    ph:lib ph:lib:ph .

ph:op:defs rdfs:label "op:defs" ;
    rdfs:comment "Query the definitions in the current namespace.\nSee `docHaystack::Ops#defs` chapter." ;
    ph:is ph:op ;
    ph:lib ph:lib:ph ;
    ph:noSideEffects ph:marker .

ph:op:filetypes rdfs:label "op:filetypes" ;
    rdfs:comment "Query the filetype defs in the current namespace.\nSee `docHaystack::Ops#filetypes` chapter." ;
    ph:is ph:op ;
    ph:lib ph:lib:ph ;
    ph:noSideEffects ph:marker .

phIoT:op:hisRead rdfs:label "op:hisRead" ;
    rdfs:comment "Read historized time series data from a `his-point`.\nSee `docHaystack::Ops#hisRead` chapter." ;
    ph:is ph:op ;
    ph:lib phIoT:lib:phIoT ;
    ph:noSideEffects ph:marker .

phIoT:op:hisWrite rdfs:label "op:hisWrite" ;
    rdfs:comment "Write historized time series data from a `his-point`.\nSee `docHaystack::Ops#hisWrite` chapter." ;
    ph:is ph:op ;
    ph:lib phIoT:lib:phIoT .

phIoT:op:invokeAction rdfs:label "op:invokeAction" ;
    rdfs:comment "Invoke a user action on a target entity.\nSee `docHaystack::Ops#invokeAction` chapter." ;
    ph:is ph:op ;
    ph:lib phIoT:lib:phIoT .

ph:op:libs rdfs:label "op:libs" ;
    rdfs:comment "Query the lib defs in the current namespace.\nSee `docHaystack::Ops#libs` chapter." ;
    ph:is ph:op ;
    ph:lib ph:lib:ph ;
    ph:noSideEffects ph:marker .

ph:op:nav rdfs:label "op:nav" ;
    rdfs:comment "Query the navigation tree for discovery.\nSee `docHaystack::Ops#nav` chapter." ;
    ph:is ph:op ;
    ph:lib ph:lib:ph ;
    ph:noSideEffects ph:marker .

ph:op:ops rdfs:label "op:ops" ;
    rdfs:comment "Query the op defs in the current namespace.\nSee `docHaystack::Ops#ops` chapter." ;
    ph:is ph:op ;
    ph:lib ph:lib:ph ;
    ph:noSideEffects ph:marker .

phIoT:op:pointWrite rdfs:label "op:pointWrite" ;
    rdfs:comment "Read or command a `writable-point`.\nSee `docHaystack::Ops#pointWrite` chapter." ;
    ph:is ph:op ;
    ph:lib phIoT:lib:phIoT .

ph:op:read rdfs:label "op:read" ;
    rdfs:comment "Query the a set of entity records by id or by filter.\nSee `docHaystack::Ops#read` chapter." ;
    ph:is ph:op ;
    ph:lib ph:lib:ph ;
    ph:noSideEffects ph:marker .

ph:op:watchPoll rdfs:label "op:watchPoll" ;
    rdfs:comment "Poll a watch subscription.\nSee `docHaystack::Ops#watchPoll` chapter." ;
    ph:is ph:op ;
    ph:lib ph:lib:ph .

ph:op:watchSub rdfs:label "op:watchSub" ;
    rdfs:comment "Subscribe to entity data.\nSee `docHaystack::Ops#watchSub` chapter." ;
    ph:is ph:op ;
    ph:lib ph:lib:ph .

ph:op:watchUnsub rdfs:label "op:watchUnsub" ;
    rdfs:comment "Unsubscribe to entity data.\nSee `docHaystack::Ops#watchUnsub` chapter." ;
    ph:is ph:op ;
    ph:lib ph:lib:ph .

ph:openEnum a owl:Class ;
    rdfs:subClassOf ph:marker ;
    rdfs:label "openEnum" ;
    rdfs:comment "Apply to str enum tags where the enumeration range is open ended.\nUser interfaces should support data entry for arbitrary strings, but\nalso provide a dropdown for the predefined enumeration." ;
    ph:is ph:marker ;
    ph:lib ph:lib:ph .

phIoT:outdoorUnit a owl:Class ;
    rdfs:subClassOf ph:marker ;
    rdfs:label "outdoorUnit" ;
    rdfs:comment "operates outside the conditioned space" ;
    ph:is ph:marker ;
    ph:lib phIoT:lib:phIoT .

ph:output a owl:Class ;
    rdfs:subClassOf ph:marker ;
    rdfs:label "output" ;
    rdfs:comment "Entity outputs a substance with flows to other entities" ;
    ph:is ph:marker ;
    ph:lib ph:lib:ph .

ph:outputs a owl:DatatypeProperty ;
    rdfs:range ph:symbol ;
    rdfs:label "outputs" ;
    rdfs:comment "The entity outputs a substance to the referent.\nThe value of this tag is what is supplied." ;
    ph:is ph:relationship ;
    ph:lib ph:lib:ph ;
    ph:reciprocalOf ph:inputs ;
    ph:transitive ph:marker .

phIoT:outside a owl:Class ;
    rdfs:subClassOf phIoT:ductSection ;
    rdfs:label "outside" ;
    rdfs:comment "Duct to access fresh outside air for both ventilation and economizer." ;
    ph:is phIoT:ductSection ;
    ph:lib phIoT:lib:phIoT .

phIoT:panel a owl:Class ;
    rdfs:subClassOf phIoT:equip ;
    rdfs:label "panel" ;
    ph:children _:0b2cb027-d6c6-2880-0f22-f23c91a70cca,
        _:0b2cb027-d6c6-2881-0f23-f23c91a70cca ;
    rdfs:comment "Enclosure for electrical and control equipment.  Panels may be\nused to isolate electrical connections and provide environmental\nprotection." ;
    ph:is phIoT:equip ;
    ph:lib phIoT:lib:phIoT .

_:0b2cb027-d6c6-2880-0f22-f23c91a70cca a phIoT:equip ;
    ph:hasTag phIoT:equip ;
    rdfs:label "{equip}" .

_:0b2cb027-d6c6-2881-0f23-f23c91a70cca a phIoT:point ;
    ph:hasTag phIoT:point ;
    rdfs:label "{point}" .

phIoT:parallel a owl:Class ;
    rdfs:subClassOf ph:marker ;
    rdfs:label "parallel" ;
    rdfs:comment "Circuit with multiple paths of flow" ;
    ph:is ph:marker ;
    ph:lib phIoT:lib:phIoT .

phIoT:perimeterHeat a owl:Class ;
    rdfs:subClassOf ph:marker ;
    rdfs:label "perimeterHeat" ;
    rdfs:comment "Auxiliary heating points associated with a `vav`" ;
    ph:is ph:marker ;
    ph:lib phIoT:lib:phIoT .

phIoT:pf a owl:Class ;
    rdfs:subClassOf phScience:quantity ;
    rdfs:label "pf" ;
    rdfs:comment "Electric power factor; which is the ratio of active power to apparent\npower in an AC electric power system.  Measured with values in the range\nof -1.0 to 1.0 or 0.0 to 1.0 without a unit.  When the range of -1.0 to\n1.0 is applied, a negative value for power factor indicates the\nelectrical current leads the electrical voltage and a positive value\nindicates the electrical current lags the electrical voltage." ;
    ph:is phScience:quantity ;
    ph:lib phIoT:lib:phIoT ;
    phScience:prefUnit "pf" ;
    phScience:quantityOf phIoT:ac-elec ;
    ph:wikipedia "https://en.wikipedia.org/wiki/Power_factor"^^xsd:anyURI .

phIoT:pfDisplacement a owl:Class ;
    rdfs:subClassOf phIoT:pfScope ;
    rdfs:label "pfDisplacement" ;
    rdfs:comment "Displacement power factor, which accounts for the phase angle between\nvoltage and current but excludes effects of nonlinear waveforms (\nharmonic distortion)." ;
    ph:is phIoT:pfScope ;
    ph:lib phIoT:lib:phIoT .

phIoT:pfDistortion a owl:Class ;
    rdfs:subClassOf phIoT:pfScope ;
    rdfs:label "pfDistortion" ;
    rdfs:comment "Distortion power factor, which measures the component of power factor\nattributable to harmonic distortion in voltage and current waveforms." ;
    ph:is phIoT:pfScope ;
    ph:lib phIoT:lib:phIoT ;
    ph:wikipedia "https://en.wikipedia.org/wiki/Power_factor#Distortion_power_factor"^^xsd:anyURI .

phIoT:pfIec a owl:Class ;
    rdfs:subClassOf phIoT:pfStandard ;
    rdfs:label "pfIec" ;
    rdfs:comment "Power factor according to the IEC convention defines a positive or\nnegative sign based on the direction of active power flow.  Power factor\nis positive when active power flows into a load.  Power factor is negative\nwhen active power flows out of a load." ;
    ph:is phIoT:pfStandard ;
    ph:lib phIoT:lib:phIoT .

phIoT:pfIeee a owl:Class ;
    rdfs:subClassOf phIoT:pfStandard ;
    rdfs:label "pfIeee" ;
    rdfs:comment "Power factor according to the IEEE convention defines a positive or\nnegative sign based on whether the load is capacitive or inductive.  Power\nfactor is positive when the load is capacitive, or when voltage lags behind\ncurrent.  Power factor is negative when the load is inductive, or when\ncurrent lags behind voltage." ;
    ph:is phIoT:pfStandard ;
    ph:lib phIoT:lib:phIoT .

phIoT:pfScope a owl:Class ;
    rdfs:subClassOf ph:choice ;
    rdfs:label "pfScope" ;
    rdfs:comment "Power factor scope" ;
    ph:is ph:choice ;
    ph:lib phIoT:lib:phIoT .

phIoT:pfStandard a owl:Class ;
    rdfs:subClassOf ph:choice ;
    rdfs:label "pfStandard" ;
    rdfs:comment "Standard for interpreting power factor's positive or negative sign" ;
    ph:is ph:choice ;
    ph:lib phIoT:lib:phIoT .

phIoT:pfTrue a owl:Class ;
    rdfs:subClassOf phIoT:pfScope ;
    rdfs:label "pfTrue" ;
    rdfs:comment "True power factor, which includes effects of harmonic distortion.\nPower factor is assumed to be true power factor when `pfScope` is not\ndefined.  However, it is recommended to specify a scope for power\nfactor to help avoid misinterpretation of data." ;
    ph:is phIoT:pfScope ;
    ph:lib phIoT:lib:phIoT .

phScience:pfc a owl:Class ;
    rdfs:subClassOf phScience:gas ;
    rdfs:label "pfc" ;
    rdfs:comment "Perfluorocarbons" ;
    ph:is phScience:gas ;
    ph:lib phScience:lib:phScience ;
    ph:wikipedia "https://en.wikipedia.org/wiki/Fluorocarbon"^^xsd:anyURI .

phScience:pfc-emission a owl:Class ;
    rdfs:subClassOf phScience:emission ;
    rdfs:label "pfc-emission" ;
    rdfs:comment "Greenhouse gas emission of perfluorocarbons into the air." ;
    ph:is phScience:emission ;
    ph:lib phScience:lib:phScience ;
    phScience:prefUnit "kg",
        "ton",
        "lb" ;
    phScience:quantityOf phScience:air .

phIoT:phase a owl:DatatypeProperty ;
    rdfs:range ph:str ;
    rdfs:label "phase" ;
    rdfs:comment "Phase measurement in a three-phase electrical system. This tag is\ndeprecated in favor of more precise tags:\n- `lineVolt`\n- `phaseVolt`\n- `lineCurrent`\n- `phaseCurrent`\n- `linePower`\n- `phasePower`\n- `linePf`\n- `phasePf`\n- `lineEnergy`\n- `phaseEnergy`\n- `lineAvg`\n- `phaseAvg`\n- `neutral`\n- `ground`" ;
    ph:enum "- A: line-to-neutral measurement\n- B: line-to-neutral measurement\n- C: line-to-neutral measurement\n- AB: line-to-line measurement\n- BC: line-to-line measurement\n- CA: line-to-line measurement\n- N: neutral current" ;
    ph:is ph:str ;
    ph:lib phIoT:lib:phIoT ;
    ph:wikipedia "https://en.wikipedia.org/wiki/Three-phase_electric_power"^^xsd:anyURI .

phIoT:phaseAvg a owl:Class ;
    rdfs:subClassOf ph:marker ;
    rdfs:label "phaseAvg" ;
    rdfs:comment "Phase average of single-phase electrical quantity measurements in an AC\nelectric power system.\n\nWhen applied to a point entity that has the `elec` and `volt` tags,\nindicates the average of all available `phaseVolt` measurements.\n\nWhen applied to a point entity that has the `elec` and `current` tags,\nindicates the average of all available `phaseCurrent` measurements.\n\nWhen applied to a point entity that has the `elec` and `power` tags,\nindicates the average of all available `phasePower` measurements.\n\nWhen applied to a point entity that has the `elec` and `pf` tags,\nindicates the average of all available `phasePf` measurements.\n\nWhen applied to a point entity that has the `elec` and `energy` tags,\nindicates the average of all available `phaseEnergy` measurements." ;
    ph:is ph:marker ;
    ph:lib phIoT:lib:phIoT .

phIoT:phaseCount a owl:Class ;
    rdfs:subClassOf ph:choice ;
    rdfs:label "phaseCount" ;
    rdfs:comment "Number of phases for an AC electrical power system or\nconnected equipment: single-phase, split-phase, two-phase, or\nthree-phase." ;
    ph:is ph:choice ;
    ph:lib phIoT:lib:phIoT ;
    ph:tagOn phIoT:ac-elec-meter,
        phIoT:motor .

phIoT:phaseCurrent a owl:DatatypeProperty ;
    rdfs:range ph:str ;
    rdfs:label "phaseCurrent" ;
    rdfs:comment "Single-phase current measured line-to-line in an AC electric power\nsystem.  May also be referred to as a phase current measurement." ;
    ph:enum "- L1-L2: line 1 to line 2 measurement\n- L2-L3: line 2 to line 3 measurement\n- L3-L1: line 3 to line 1 measurement" ;
    ph:is phIoT:elecLineToLine ;
    ph:lib phIoT:lib:phIoT .

phIoT:phaseEnergy a owl:DatatypeProperty ;
    rdfs:range ph:str ;
    rdfs:label "phaseEnergy" ;
    rdfs:comment "Single-phase energy measured line-to-neutral in an AC electric power\nsystem.  Neutral might not be referenced, but implied." ;
    ph:enum "- L1: line 1 measurement\n- L2: line 2 measurement\n- L3: line 3 measurement" ;
    ph:is phIoT:elecLine ;
    ph:lib phIoT:lib:phIoT .

phIoT:phasePf a owl:DatatypeProperty ;
    rdfs:range ph:str ;
    rdfs:label "phasePf" ;
    rdfs:comment "Single-phase power factor measured line-to-neutral in an AC electric\npower system.  Neutral might not be referenced, but implied." ;
    ph:enum "- L1: line 1 measurement\n- L2: line 2 measurement\n- L3: line 3 measurement" ;
    ph:is phIoT:elecLine ;
    ph:lib phIoT:lib:phIoT .

phIoT:phasePower a owl:DatatypeProperty ;
    rdfs:range ph:str ;
    rdfs:label "phasePower" ;
    rdfs:comment "Single-phase power measured line-to-neutral in an AC electric power\nsystem.  May also be referred to as a phase power measurement.  Neutral\nmight not be referenced, but implied." ;
    ph:enum "- L1: line 1 measurement\n- L2: line 2 measurement\n- L3: line 3 measurement" ;
    ph:is phIoT:elecLine ;
    ph:lib phIoT:lib:phIoT .

phIoT:phaseVolt a owl:DatatypeProperty ;
    rdfs:range ph:str ;
    rdfs:label "phaseVolt" ;
    rdfs:comment "Single-phase voltage measured line-to-neutral in an AC electric power\nsystem.  May also be referred to as a phase voltage measurement." ;
    ph:enum "- L1-N: line 1 to neutral measurement\n- L2-N: line 2 to neutral measurement\n- L3-N: line 3 to neutral measurement" ;
    ph:is phIoT:elecLineToNeutral ;
    ph:lib phIoT:lib:phIoT .

phScience:phenomenon a owl:Class ;
    rdfs:subClassOf ph:marker ;
    rdfs:label "phenomenon" ;
    rdfs:comment "Aspect of scientific interest with measurable quantities" ;
    ph:docTaxonomy ph:marker ;
    ph:is ph:marker ;
    ph:lib phScience:lib:phScience .

phIct:phone a owl:Class ;
    rdfs:subClassOf phIct:device ;
    rdfs:label "phone" ;
    rdfs:comment "Telephone used for voice telecommunication." ;
    ph:is phIct:device ;
    ph:lib phIct:lib:phIct ;
    ph:wikipedia "https://en.wikipedia.org/wiki/Telephone"^^xsd:anyURI .

phIoT:pipe a owl:Class ;
    rdfs:subClassOf phIoT:conduit ;
    rdfs:label "pipe" ;
    ph:children _:0b2cb027-d6d5-6ac0-0f24-f23c91a70cca,
        _:0b2cb027-d712-73c0-0f25-f23c91a70cca,
        _:0b2cb027-d712-73c1-0f26-f23c91a70cca,
        _:0b2cb027-d712-73c2-0f27-f23c91a70cca,
        _:0b2cb027-d712-73c3-0f28-f23c91a70cca,
        _:0b2cb027-d712-73c4-0f29-f23c91a70cca,
        _:0b2cb027-d712-73c5-0f2a-f23c91a70cca,
        _:0b2cb027-d712-73c6-0f2b-f23c91a70cca,
        _:0b2cb027-d712-73c7-0f2c-f23c91a70cca,
        _:0b2cb027-d712-73c8-0f2d-f23c91a70cca ;
    ph:childrenFlatten phScience:fluid,
        phIoT:pipeSection,
        phIoT:plantLoop ;
    rdfs:comment "Conduit used to convey a fluid" ;
    ph:is phIoT:conduit ;
    ph:lib phIoT:lib:phIoT ;
    ph:wikipedia "https://en.wikipedia.org/wiki/Pipe_(fluid_conveyance)"^^xsd:anyURI .

_:0b2cb027-d6d5-6ac0-0f24-f23c91a70cca a phIoT:equip ;
    ph:hasTag phIoT:equip ;
    rdfs:label "{equip}" .

_:0b2cb027-d712-73c0-0f25-f23c91a70cca a phIoT:point ;
    ph:hasTag phScience:flow,
        phIoT:sensor,
        phIoT:point ;
    rdfs:label "{flow, sensor, point}" .

_:0b2cb027-d712-73c1-0f26-f23c91a70cca a phIoT:point ;
    ph:hasTag phScience:flow,
        phIoT:sp,
        phIoT:point ;
    rdfs:label "{flow, sp, point}" .

_:0b2cb027-d712-73c2-0f27-f23c91a70cca a phIoT:point ;
    ph:hasTag phIoT:point ;
    rdfs:label "{point}" .

_:0b2cb027-d712-73c3-0f28-f23c91a70cca a phIoT:point ;
    ph:hasTag phScience:pressure,
        phIoT:sensor,
        phIoT:point ;
    rdfs:label "{pressure, sensor, point}" .

_:0b2cb027-d712-73c4-0f29-f23c91a70cca a phIoT:point ;
    ph:hasTag phScience:pressure,
        phIoT:sp,
        phIoT:point ;
    rdfs:label "{pressure, sp, point}" .

_:0b2cb027-d712-73c5-0f2a-f23c91a70cca a phIoT:pump-motor ;
    ph:hasTag phIoT:pump,
        phIoT:motor,
        phIoT:equip ;
    rdfs:label "{pump, motor, equip}" .

_:0b2cb027-d712-73c6-0f2b-f23c91a70cca a phIoT:point ;
    ph:hasTag phScience:temp,
        phIoT:sensor,
        phIoT:point ;
    rdfs:label "{temp, sensor, point}" .

_:0b2cb027-d712-73c7-0f2c-f23c91a70cca a phIoT:point ;
    ph:hasTag phScience:temp,
        phIoT:sp,
        phIoT:point ;
    rdfs:label "{temp, sp, point}" .

_:0b2cb027-d712-73c8-0f2d-f23c91a70cca a phIoT:valve-actuator ;
    ph:hasTag phIoT:valve,
        phIoT:actuator,
        phIoT:equip ;
    rdfs:label "{valve, actuator, equip}" .

phIoT:pipeFluid a owl:Class ;
    rdfs:subClassOf ph:choice ;
    rdfs:label "pipeFluid" ;
    rdfs:comment "Type of fluid conveyed by piping" ;
    ph:is ph:choice ;
    ph:lib phIoT:lib:phIoT ;
    ph:of phScience:fluid ;
    ph:tagOn phIoT:pipe,
        phIoT:valve-actuator,
        phIoT:pump-motor .

phIoT:pipeSection a owl:Class ;
    rdfs:subClassOf ph:choice ;
    rdfs:label "pipeSection" ;
    rdfs:comment "Equipment section of piping" ;
    ph:is ph:choice ;
    ph:lib phIoT:lib:phIoT ;
    ph:tagOn phIoT:pipe,
        phIoT:valve-actuator,
        phIoT:pump-motor .

phIoT:plant a owl:Class ;
    rdfs:subClassOf phIoT:equip ;
    rdfs:label "plant" ;
    ph:children _:0b2cb027-d712-73c9-0f2e-f23c91a70cca,
        _:0b2cb027-d712-73ca-0f2f-f23c91a70cca,
        _:0b2cb027-d712-73cb-0f30-f23c91a70cca ;
    rdfs:comment "Central plant used to generate a substance for a process.\nSee `docHaystack::Plants`." ;
    ph:is phIoT:equip ;
    ph:lib phIoT:lib:phIoT .

_:0b2cb027-d712-73c9-0f2e-f23c91a70cca a phIoT:point ;
    ph:hasTag phIoT:enable,
        phIoT:cmd,
        phIoT:point ;
    rdfs:label "{enable, cmd, point}" .

_:0b2cb027-d712-73ca-0f2f-f23c91a70cca a phIoT:equip ;
    ph:hasTag phIoT:equip ;
    rdfs:label "{equip}" .

_:0b2cb027-d712-73cb-0f30-f23c91a70cca a phIoT:point ;
    ph:hasTag phIoT:point ;
    rdfs:label "{point}" .

phIoT:plantLoop a owl:Class ;
    rdfs:subClassOf ph:choice ;
    rdfs:label "plantLoop" ;
    rdfs:comment "Plant piping loop: primary, secondary, or tertiary" ;
    ph:is ph:choice ;
    ph:lib phIoT:lib:phIoT ;
    ph:tagOn phIoT:pipe .

phScience:pm01 a owl:Class ;
    rdfs:subClassOf phScience:solid ;
    rdfs:label "pm01" ;
    rdfs:comment "Particulate matter 0.1; atmospheric pollutant of fine particles with an aerodynamic diameter of 0.1 micrometers or less" ;
    ph:is phScience:solid ;
    ph:lib phScience:lib:phScience ;
    ph:wikipedia "https://en.wikipedia.org/wiki/Particulates"^^xsd:anyURI .

phScience:pm01-concentration a owl:Class ;
    rdfs:subClassOf phScience:airQuality ;
    rdfs:label "pm01-concentration" ;
    rdfs:comment "Concentration of particulate matter 0.1 in the air." ;
    ph:is phScience:airQuality ;
    ph:lib phScience:lib:phScience ;
    phScience:prefUnit "\u00b5g/m\u00b3",
        "ppb" ;
    phScience:quantityOf phScience:air ;
    ph:wikipedia "https://en.wikipedia.org/wiki/Concentration"^^xsd:anyURI .

phScience:pm10 a owl:Class ;
    rdfs:subClassOf phScience:solid ;
    rdfs:label "pm10" ;
    rdfs:comment "Particulate matter 10; atmospheric pollutant of fine particles with an aerodynamic diameter of 10 micrometers or less" ;
    ph:is phScience:solid ;
    ph:lib phScience:lib:phScience ;
    ph:wikipedia "https://en.wikipedia.org/wiki/Particulates"^^xsd:anyURI .

phScience:pm10-concentration a owl:Class ;
    rdfs:subClassOf phScience:airQuality ;
    rdfs:label "pm10-concentration" ;
    rdfs:comment "Concentration of particulate matter 10 in the air" ;
    ph:is phScience:airQuality ;
    ph:lib phScience:lib:phScience ;
    phScience:prefUnit "\u00b5g/m\u00b3",
        "ppb" ;
    phScience:quantityOf phScience:air ;
    ph:wikipedia "https://en.wikipedia.org/wiki/Concentration"^^xsd:anyURI .

phScience:pm25 a owl:Class ;
    rdfs:subClassOf phScience:solid ;
    rdfs:label "pm25" ;
    rdfs:comment "Particulate matter 2.5; atmospheric pollutant of fine particles with an aerodynamic diameter of 2.5 micrometers or less" ;
    ph:is phScience:solid ;
    ph:lib phScience:lib:phScience ;
    ph:wikipedia "https://en.wikipedia.org/wiki/Particulates"^^xsd:anyURI .

phScience:pm25-concentration a owl:Class ;
    rdfs:subClassOf phScience:airQuality ;
    rdfs:label "pm25-concentration" ;
    rdfs:comment "Concentration of particulate matter 2.5 in the air." ;
    ph:is phScience:airQuality ;
    ph:lib phScience:lib:phScience ;
    phScience:prefUnit "\u00b5g/m\u00b3",
        "ppb" ;
    phScience:quantityOf phScience:air ;
    ph:wikipedia "https://en.wikipedia.org/wiki/Concentration"^^xsd:anyURI .

phIoT:point a owl:Class ;
    rdfs:subClassOf ph:entity ;
    rdfs:label "point" ;
    rdfs:comment "Data point such as a sensor or actuator.\nSee `docHaystack::Points` chapter." ;
    ph:docTaxonomy ph:marker ;
    ph:is ph:entity ;
    ph:lib phIoT:lib:phIoT ;
    ph:mandatory ph:marker .

phIoT:pointFunction a owl:Class ;
    rdfs:subClassOf ph:choice ;
    rdfs:label "pointFunction" ;
    rdfs:comment "Classifies the point as a sensor, command, or setpoint.\nSee `docHaystack::Points#function` chapter." ;
    ph:is ph:choice ;
    ph:lib phIoT:lib:phIoT ;
    ph:tagOn phIoT:point .

phIoT:pointGroup a owl:Class ;
    rdfs:subClassOf ph:entity ;
    rdfs:label "pointGroup" ;
    rdfs:comment "Grouping of children points used by spaces and equipment" ;
    ph:is ph:entity ;
    ph:lib phIoT:lib:phIoT .

phIoT:pointQuantity a owl:Class ;
    rdfs:subClassOf ph:choice ;
    rdfs:label "pointQuantity" ;
    rdfs:comment "Quantity the point senses or controls" ;
    ph:is ph:choice ;
    ph:lib phIoT:lib:phIoT ;
    ph:of phScience:quantity ;
    ph:tagOn phIoT:point .

phIoT:pointRef a owl:ObjectProperty ;
    rdfs:domain phIoT:sim-point ;
    rdfs:range phIoT:point ;
    rdfs:label "pointRef" ;
    rdfs:comment "See `docHaystack::Synthetics#structure` chapter." ;
    ph:is ph:ref ;
    ph:lib phIoT:lib:phIoT ;
    ph:of phIoT:point ;
    ph:tagOn phIoT:sim-point .

phIoT:pointSubject a owl:Class ;
    rdfs:subClassOf ph:choice ;
    rdfs:label "pointSubject" ;
    rdfs:comment "What the point senses or controls" ;
    ph:is ph:choice ;
    ph:lib phIoT:lib:phIoT ;
    ph:of phScience:phenomenon ;
    ph:tagOn phIoT:point .

phIct:pop3 a owl:Class ;
    rdfs:subClassOf phIct:protocol ;
    rdfs:label "pop3" ;
    rdfs:comment "Post Office Protocol version 3 for retrieving email" ;
    ph:is phIct:protocol ;
    ph:lib phIct:lib:phIct ;
    ph:wikipedia "https://en.wikipedia.org/wiki/Post_Office_Protocol"^^xsd:anyURI .

phIoT:port a owl:Class ;
    rdfs:subClassOf ph:marker ;
    rdfs:label "port" ;
    rdfs:comment "A gateway or opening used to transfer a substance." ;
    ph:is ph:marker ;
    ph:lib phIoT:lib:phIoT .

phScience:power a owl:Class ;
    rdfs:subClassOf phScience:quantity ;
    rdfs:label "power" ;
    rdfs:comment "Energy consumed per unit time" ;
    ph:is phScience:quantity ;
    ph:lib phScience:lib:phScience .

phIoT:powerConverter a owl:Class ;
    rdfs:subClassOf ph:marker ;
    rdfs:label "powerConverter" ;
    rdfs:comment "Converts one electrical waveform to another using power electronic\ncircuitry.  Involves the use of one or more power modules.\n\nMay convert:\n - `ac` to `dc`\n - `ac` to `ac`\n - `dc` to `dc`\n - `dc` to `ac`\n\nNote:  An AC/AC power converter performs the same task as a power\ntransformer but using power electronics.  Similarly, a DC/DC power\nconverter transforms an input DC voltage to an output DC voltage at\nanother level." ;
    ph:is ph:marker ;
    ph:lib phIoT:lib:phIoT .

phScience:precipitation a owl:Class ;
    rdfs:subClassOf phScience:quantity ;
    rdfs:label "precipitation" ;
    rdfs:comment "Amount of atmospheric water vapor fallen including rain, sleet, snow, and hail" ;
    ph:is phScience:quantity ;
    ph:lib phScience:lib:phScience ;
    phScience:prefUnit "mm",
        "in" ;
    phScience:quantityOf phScience:weather .

phScience:prefUnit a owl:DatatypeProperty ;
    rdfs:range ph:list ;
    rdfs:label "prefUnit" ;
    rdfs:comment "Defines a preferred unit to be used with a quantity" ;
    ph:is ph:list ;
    ph:lib phScience:lib:phScience ;
    ph:of ph:unit .

phScience:pressure a owl:Class ;
    rdfs:subClassOf phScience:quantity ;
    rdfs:label "pressure" ;
    rdfs:comment "Measure of force applied" ;
    ph:is phScience:quantity ;
    ph:lib phScience:lib:phScience ;
    phScience:prefUnit "kPa",
        "psi" ;
    phScience:quantityOf phScience:fluid ;
    ph:wikipedia "https://en.wikipedia.org/wiki/Pressure"^^xsd:anyURI .

phIoT:pressureDependent a owl:Class ;
    rdfs:subClassOf phIoT:vavModulation ;
    rdfs:label "pressureDependent" ;
    rdfs:comment "VAV damper modulates to control space temp; dependent on duct pressure\nbeing maintained" ;
    ph:is phIoT:vavModulation ;
    ph:lib phIoT:lib:phIoT .

phIoT:pressureIndependent a owl:Class ;
    rdfs:subClassOf phIoT:vavModulation ;
    rdfs:label "pressureIndependent" ;
    rdfs:comment "VAV damper or a control valve that modulates to maintain desired flow\nsetpoint; independent of the duct pressure" ;
    ph:is phIoT:vavModulation ;
    ph:lib phIoT:lib:phIoT .

phIoT:primaryFunction a owl:DatatypeProperty ;
    rdfs:domain phIoT:site ;
    rdfs:range ph:str ;
    rdfs:label "primaryFunction" ;
    rdfs:comment "Primary function of building as US Energy Star key" ;
    ph:enum "Adult Education\nAmbulatory Surgical Center\nAquarium\nAutomobile Dealership\nBank Branch\nBar/Nightclub\nBarracks\nBowling Alley\nCasino\nCollege/University\nConvenience Store with Gas Station\nConvenience Store without Gas Station\nConvention Center\nCourthouse\nData Center\nDistribution Center\nDrinking Water Treatment & Distribution\nEnclosed Mall\nEnergy/Power Station\nFast Food Restaurant\nFinancial Office\nFire Station\nFitness Center/Health Club/Gym\nFood Sales\nFood Service\nHospital (General Medical & Surgical)\nHotel\nIce/Curling Rink\nIndoor Arena\nK-12 School\nLaboratory\nLibrary\nLifestyle Center\nMailing Center/Post Office\nManufacturing/Industrial Plant\nMedical Office\nMixed Use Property\nMovie Theater\nMultifamily Housing\nMuseum\nNon-Refrigerated Warehouse\nOffice\nOther - Education\nOther - Entertainment/Public Assembly\nOther - Lodging/Residential\nOther - Mall\nOther - Public Services\nOther - Recreation\nOther - Restaurant/Bar\nOther - Services\nOther - Stadium\nOther - Technology/Science\nOther - Utility\nOther\nOther/Specialty Hospital\nOutpatient Rehabilitation/Physical Therapy\nParking\nPerforming Arts\nPersonal Services (Health/Beauty, Dry Cleaning, etc)\nPolice Station\nPre-school/Daycare\nPrison/Incarceration\nRace Track\nRefrigerated Warehouse\nRepair Services (Vehicle, Shoe, Locksmith, etc)\nResidence Hall/Dormitory\nRestaurant\nRetail Store\nRoller Rink\nSelf-Storage Facility\nSenior Care Community\nSingle Family Home\nSocial/Meeting Hall\nStadium (Closed)\nStadium (Open)\nStrip Mall\nSupermarket/Grocery Store\nSwimming Pool\nTransportation Terminal/Station\nUrgent Care/Clinic/Other Outpatient\nVeterinary Office\nVocational School\nWastewater Treatment Plant\nWholesale Club/Supercenter\nWorship Facility\nZoo" ;
    ph:is ph:str ;
    ph:lib phIoT:lib:phIoT ;
    ph:tagOn phIoT:site .

phIoT:primaryLoop a owl:Class ;
    rdfs:subClassOf phIoT:plantLoop ;
    rdfs:label "primaryLoop" ;
    rdfs:comment "Pipework which circulates closest to the energy source.  In a central\nplant, the primary loop indicates the pipes and equipment within the\ncentral plant.  In context of heat exchangers between the primary\nand secondary loops, this tag indicates the side closest to the plant." ;
    ph:is phIoT:plantLoop ;
    ph:lib phIoT:lib:phIoT .

phIoT:process a owl:Class ;
    rdfs:subClassOf ph:marker ;
    rdfs:label "process" ;
    rdfs:comment "Industrial or HVAC process" ;
    ph:docTaxonomy ph:marker ;
    ph:is ph:marker ;
    ph:lib phIoT:lib:phIoT .

phIoT:propane a owl:Class ;
    rdfs:subClassOf phScience:gas ;
    rdfs:label "propane" ;
    rdfs:comment "By-product of natural gas processing and petroleum refining (C\u2083H\u2088)" ;
    ph:is phScience:gas ;
    ph:lib phIoT:lib:phIoT ;
    ph:wikipedia "https://en.wikipedia.org/wiki/Propane"^^xsd:anyURI .

phIoT:propaneHeating a owl:Class ;
    rdfs:subClassOf phIoT:heatingProcess ;
    rdfs:label "propaneHeating" ;
    rdfs:comment "Heating by the combustion of propane" ;
    ph:is phIoT:heatingProcess ;
    ph:lib phIoT:lib:phIoT .

phIct:protocol a owl:Class ;
    rdfs:subClassOf ph:marker ;
    rdfs:label "protocol" ;
    rdfs:comment "Communication protocol used for devices on a network." ;
    ph:docTaxonomy ph:marker ;
    ph:is ph:marker ;
    ph:lib phIct:lib:phIct ;
    ph:wikipedia "https://en.wikipedia.org/wiki/Communication_protocol"^^xsd:anyURI .

phIoT:pump a owl:Class ;
    rdfs:subClassOf ph:marker ;
    rdfs:label "pump" ;
    rdfs:comment "Pump equipment or control point" ;
    ph:is ph:marker ;
    ph:lib phIoT:lib:phIoT ;
    ph:wikipedia "https://en.wikipedia.org/wiki/Pump"^^xsd:anyURI .

phIoT:pump-motor a owl:Class ;
    rdfs:subClassOf phIoT:motor ;
    rdfs:label "pump-motor" ;
    ph:children _:0b2cb027-d721-b600-0f31-f23c91a70cca,
        _:0b2cb027-d721-b601-0f32-f23c91a70cca,
        _:0b2cb027-d721-b602-0f33-f23c91a70cca,
        _:0b2cb027-d721-b603-0f34-f23c91a70cca,
        _:0b2cb027-d721-b604-0f35-f23c91a70cca,
        _:0b2cb027-d721-b605-0f36-f23c91a70cca,
        _:0b2cb027-d721-b606-0f37-f23c91a70cca,
        _:0b2cb027-d721-b607-0f38-f23c91a70cca,
        _:0b2cb027-d721-b608-0f39-f23c91a70cca,
        _:0b2cb027-d721-b609-0f3a-f23c91a70cca,
        _:0b2cb027-d721-b60a-0f3b-f23c91a70cca ;
    ph:childrenFlatten phScience:fluid,
        phIoT:pipeSection,
        phIoT:pump ;
    rdfs:comment "Motor used with a pump to move fluid.\nSee `docHaystack::Motors` chapter." ;
    ph:is phIoT:motor ;
    ph:lib phIoT:lib:phIoT ;
    ph:wikipedia "https://en.wikipedia.org/wiki/Pump"^^xsd:anyURI .

_:0b2cb027-d721-b600-0f31-f23c91a70cca a phIoT:point ;
    ph:hasTag phIoT:alarm,
        phIoT:sensor,
        phIoT:point ;
    rdfs:label "{alarm, sensor, point}" .

_:0b2cb027-d721-b601-0f32-f23c91a70cca a phIoT:point ;
    ph:hasTag phIoT:enable,
        phIoT:cmd,
        phIoT:point ;
    rdfs:label "{enable, cmd, point}" .

_:0b2cb027-d721-b602-0f33-f23c91a70cca a phIoT:point ;
    ph:hasTag phIoT:enable,
        phIoT:sensor,
        phIoT:point ;
    rdfs:label "{enable, sensor, point}" .

_:0b2cb027-d721-b603-0f34-f23c91a70cca a phIoT:equip ;
    ph:hasTag phIoT:equip ;
    rdfs:label "{equip}" .

_:0b2cb027-d721-b604-0f35-f23c91a70cca a phIoT:point ;
    ph:hasTag phIoT:point ;
    rdfs:label "{point}" .

_:0b2cb027-d721-b605-0f36-f23c91a70cca a phIoT:point ;
    ph:hasTag phIoT:run,
        phIoT:cmd,
        phIoT:point ;
    rdfs:label "{run, cmd, point}" .

_:0b2cb027-d721-b606-0f37-f23c91a70cca a phIoT:point ;
    ph:hasTag phIoT:run,
        phIoT:sensor,
        phIoT:point ;
    rdfs:label "{run, sensor, point}" .

_:0b2cb027-d721-b607-0f38-f23c91a70cca a phIoT:point ;
    ph:hasTag phIoT:vfd,
        phScience:freq,
        phIoT:cmd,
        phIoT:point ;
    rdfs:label "{vfd, freq, cmd, point}" .

_:0b2cb027-d721-b608-0f39-f23c91a70cca a phIoT:point ;
    ph:hasTag phIoT:vfd,
        phScience:freq,
        phIoT:sensor,
        phIoT:point ;
    rdfs:label "{vfd, freq, sensor, point}" .

_:0b2cb027-d721-b609-0f3a-f23c91a70cca a phIoT:point ;
    ph:hasTag phIoT:vfd,
        phScience:speed,
        phIoT:cmd,
        phIoT:point ;
    rdfs:label "{vfd, speed, cmd, point}" .

_:0b2cb027-d721-b60a-0f3b-f23c91a70cca a phIoT:point ;
    ph:hasTag phIoT:vfd,
        phScience:speed,
        phIoT:sensor,
        phIoT:point ;
    rdfs:label "{vfd, speed, sensor, point}" .

phIoT:purge a owl:Class ;
    rdfs:subClassOf ph:marker ;
    rdfs:label "purge" ;
    rdfs:comment "Associated with a cleaning process to remove contaminants.\nMost commonly it indicates purging water or air by using a filter or by\nletting out a certain amount of the substance at a high flow rate." ;
    ph:is ph:marker ;
    ph:lib phIoT:lib:phIoT .

phIoT:purge-water a owl:Class ;
    rdfs:subClassOf phScience:water ;
    rdfs:label "purge-water" ;
    rdfs:comment "Water expelled from a system to remove contaminants." ;
    ph:is phScience:water ;
    ph:lib phIoT:lib:phIoT ;
    ph:wikipedia "https://en.wikipedia.org/wiki/Water"^^xsd:anyURI .

phScience:quality a owl:Class ;
    rdfs:subClassOf ph:marker ;
    rdfs:label "quality" ;
    rdfs:comment "Quantity measured against standard metric" ;
    ph:is ph:marker ;
    ph:lib phScience:lib:phScience .

phScience:quantities a owl:DatatypeProperty ;
    rdfs:range ph:list ;
    rdfs:label "quantities" ;
    ph:computedFromReciprocal ph:marker ;
    rdfs:comment "Quantities used to measure this phenomenon" ;
    ph:docAssociations ph:marker ;
    ph:is ph:association ;
    ph:lib phScience:lib:phScience ;
    ph:of ph:symbol ;
    ph:reciprocalOf phScience:quantityOf .

phScience:quantity a owl:Class ;
    rdfs:subClassOf ph:marker ;
    rdfs:label "quantity" ;
    rdfs:comment "Measurable property of a substance or phenomenon" ;
    ph:docTaxonomy ph:marker ;
    ph:is ph:marker ;
    ph:lib phScience:lib:phScience .

phScience:quantityOf a owl:DatatypeProperty ;
    rdfs:range ph:list ;
    rdfs:label "quantityOf" ;
    rdfs:comment "Associates quantity as measurement of a phenomenon" ;
    ph:is ph:association ;
    ph:lib phScience:lib:phScience ;
    ph:of phScience:phenomenon ;
    ph:reciprocalOf phScience:quantities .

phIct:rack a owl:Class ;
    rdfs:subClassOf phIoT:equip ;
    rdfs:label "rack" ;
    ph:children _:0b2cb027-d730-f840-0f3c-f23c91a70cca,
        _:0b2cb027-d730-f841-0f3d-f23c91a70cca,
        _:0b2cb027-d730-f842-0f3e-f23c91a70cca,
        _:0b2cb027-d730-f843-0f3f-f23c91a70cca ;
    rdfs:comment "Enclosure or chassis used to mount computer and networking gear.\nDevices are mounted to rails of a standard width, typically 19 or 23\ninches.  Height is measured in *rack units* where one 1U is 1.75 inches.\nA full rack has a height of 42U.\nSee `docHaystack::DataCenters#racks` chapter." ;
    ph:is phIoT:equip ;
    ph:lib phIct:lib:phIct ;
    ph:wikipedia "https://en.wikipedia.org/wiki/19-inch_rack"^^xsd:anyURI .

_:0b2cb027-d730-f840-0f3c-f23c91a70cca a phIoT:equip ;
    ph:hasTag phIoT:equip ;
    rdfs:label "{equip}" .

_:0b2cb027-d730-f841-0f3d-f23c91a70cca a phIct:networking-device ;
    ph:hasTag phIct:networking,
        phIct:device ;
    rdfs:label "{networking, device}" .

_:0b2cb027-d730-f842-0f3e-f23c91a70cca a phIoT:point ;
    ph:hasTag phIoT:point ;
    rdfs:label "{point}" .

_:0b2cb027-d730-f843-0f3f-f23c91a70cca a phIct:device ;
    ph:hasTag phIct:server,
        phIct:device ;
    rdfs:label "{server, device}" .

phIoT:radiantEquip a owl:Class ;
    rdfs:subClassOf phIoT:equip ;
    rdfs:label "radiantEquip" ;
    ph:children _:0b2cb027-d730-f844-0f40-f23c91a70cca,
        _:0b2cb027-d730-f845-0f41-f23c91a70cca ;
    rdfs:comment "HVAC equipment that conditions a space without forced air." ;
    ph:is phIoT:equip ;
    ph:lib phIoT:lib:phIoT .

_:0b2cb027-d730-f844-0f40-f23c91a70cca a phIoT:equip ;
    ph:hasTag phIoT:equip ;
    rdfs:label "{equip}" .

_:0b2cb027-d730-f845-0f41-f23c91a70cca a phIoT:point ;
    ph:hasTag phIoT:point ;
    rdfs:label "{point}" .

phIoT:radiantFloor a owl:Class ;
    rdfs:subClassOf phIoT:radiantEquip ;
    rdfs:label "radiantFloor" ;
    ph:children _:0b2cb027-d730-f846-0f42-f23c91a70cca,
        _:0b2cb027-d730-f847-0f43-f23c91a70cca ;
    rdfs:comment "Heats a space using pipes or cables embedded beneath floor." ;
    ph:is phIoT:radiantEquip ;
    ph:lib phIoT:lib:phIoT ;
    ph:wikipedia "https://en.wikipedia.org/wiki/Underfloor_heating"^^xsd:anyURI .

_:0b2cb027-d730-f846-0f42-f23c91a70cca a phIoT:equip ;
    ph:hasTag phIoT:equip ;
    rdfs:label "{equip}" .

_:0b2cb027-d730-f847-0f43-f23c91a70cca a phIoT:point ;
    ph:hasTag phIoT:point ;
    rdfs:label "{point}" .

phIoT:radiator a owl:Class ;
    rdfs:subClassOf phIoT:radiantEquip ;
    rdfs:label "radiator" ;
    ph:children _:0b2cb027-d730-f848-0f44-f23c91a70cca,
        _:0b2cb027-d730-f849-0f45-f23c91a70cca ;
    rdfs:comment "Heats a space using exposed pipes or coils.  Hot water and steam\nradiators are often cast iron and installed directly in the space\nor along the baseboard.  Electric radiators are typically installed\non the baseboard." ;
    ph:is phIoT:radiantEquip ;
    ph:lib phIoT:lib:phIoT ;
    ph:wikipedia "https://en.wikipedia.org/wiki/Radiator_(heating)"^^xsd:anyURI .

_:0b2cb027-d730-f848-0f44-f23c91a70cca a phIoT:equip ;
    ph:hasTag phIoT:equip ;
    rdfs:label "{equip}" .

_:0b2cb027-d730-f849-0f45-f23c91a70cca a phIoT:point ;
    ph:hasTag phIoT:point ;
    rdfs:label "{point}" .

phIoT:rated a owl:Class ;
    rdfs:subClassOf ph:marker ;
    rdfs:label "rated" ;
    rdfs:comment "Data specified by a manufacturer or rating organization.  Typically this\ninformation is from the equipment data plate or cut sheet.  Also see `design`." ;
    ph:is ph:marker ;
    ph:lib phIoT:lib:phIoT .

phIoT:reactive a owl:Class ;
    rdfs:subClassOf ph:marker ;
    rdfs:label "reactive" ;
    rdfs:comment "Relating to reactance" ;
    ph:is ph:marker ;
    ph:lib phIoT:lib:phIoT .

phIoT:reactive-energy a owl:Class ;
    rdfs:subClassOf phScience:quantity ;
    rdfs:label "reactive-energy" ;
    rdfs:comment "Reactive energy in an AC eletrical power system. Integral of\n`reactive-power` over time." ;
    ph:is phScience:quantity ;
    ph:lib phIoT:lib:phIoT ;
    phScience:quantityOf phIoT:ac-elec .

phIoT:reactive-power a owl:Class ;
    rdfs:subClassOf phScience:quantity ;
    rdfs:label "reactive-power" ;
    rdfs:comment "Reactive power or imaginary power; represents energy that recirculates\nwithin an AC power system but does not contribute useful work." ;
    ph:is phScience:quantity ;
    ph:lib phIoT:lib:phIoT ;
    phScience:prefUnit "kVAR" ;
    phScience:quantityOf phIoT:ac-elec .

phIoT:reciprocal a owl:Class ;
    rdfs:subClassOf ph:marker ;
    rdfs:label "reciprocal" ;
    rdfs:comment "Piston compressor driven by a crankshaft" ;
    ph:is ph:marker ;
    ph:lib phIoT:lib:phIoT ;
    ph:wikipedia "https://en.wikipedia.org/wiki/Reciprocating_compressor"^^xsd:anyURI .

ph:reciprocalOf a owl:DatatypeProperty ;
    rdfs:range ph:symbol ;
    rdfs:label "reciprocalOf" ;
    rdfs:comment "Specifies the inverse of an association or relationships.\nSee [Associations]`docHaystack::Associations#reciprocalOf` and\n[Relationships]`docHaystack::Relationships#reciprocalOf` chapter." ;
    ph:is ph:symbol ;
    ph:lib ph:lib:ph .

ph:ref a owl:DatatypeProperty ;
    rdfs:subClassOf xsd:anyURI ;
    rdfs:label "ref" ;
    rdfs:comment "Reference to an entity. Ref values are ASCII strings limited to the\nfollowing chars: a-z, A-Z, 0-9, underbar, colon, dash, dot, or tilde.\nSee [Kinds chapter]`docHaystack::Kinds#ref`." ;
    ph:is ph:scalar ;
    ph:lib ph:lib:ph .

phIoT:refrig a owl:Class ;
    rdfs:subClassOf phScience:fluid ;
    rdfs:label "refrig" ;
    rdfs:comment "Fluid used in refrigeration and heat exchange.  Refrigerants typically\nalternate between liquid and gas state." ;
    ph:is phScience:fluid ;
    ph:lib phIoT:lib:phIoT ;
    ph:wikipedia "https://en.wikipedia.org/wiki/Refrigerant"^^xsd:anyURI .

phIoT:refrig-input a owl:Class ;
    rdfs:subClassOf ph:input ;
    rdfs:label "refrig-input" ;
    rdfs:comment "Entity inputs refrigerant which flows from another entity" ;
    ph:is ph:input ;
    ph:lib phIoT:lib:phIoT .

phIoT:refrig-output a owl:Class ;
    rdfs:subClassOf ph:output ;
    rdfs:label "refrig-output" ;
    rdfs:comment "Entity outputs refrigerant to other entities" ;
    ph:is ph:output ;
    ph:lib phIoT:lib:phIoT .

phIoT:refrig-system a owl:Class ;
    rdfs:subClassOf phIoT:system ;
    rdfs:label "refrig-system" ;
    ph:children _:0b2cb027-d740-3a80-0f46-f23c91a70cca,
        _:0b2cb027-d740-3a81-0f47-f23c91a70cca ;
    rdfs:comment "Refrigerant distribution to fulfill all or parts of a refrigeration cycle." ;
    ph:is phIoT:system ;
    ph:lib phIoT:lib:phIoT .

_:0b2cb027-d740-3a80-0f46-f23c91a70cca a phIoT:equip ;
    ph:hasTag phIoT:equip ;
    rdfs:label "{equip}" .

_:0b2cb027-d740-3a81-0f47-f23c91a70cca a phIoT:point ;
    ph:hasTag phIoT:point ;
    rdfs:label "{point}" .

phIoT:refrigRef a owl:ObjectProperty ;
    rdfs:domain phIoT:refrig-input ;
    rdfs:range phIoT:refrig-output ;
    rdfs:label "refrigRef" ;
    rdfs:comment "Refrigerant flows from the referent to this entity" ;
    ph:inputs phIoT:refrig ;
    ph:is ph:ref ;
    ph:lib phIoT:lib:phIoT ;
    ph:of phIoT:refrig-output ;
    ph:tagOn phIoT:refrig-input .

phIoT:reheat a owl:Class ;
    rdfs:subClassOf ph:marker ;
    rdfs:label "reheat" ;
    rdfs:comment "Command point for reheating process" ;
    ph:is ph:marker ;
    ph:lib phIoT:lib:phIoT .

ph:relationship a owl:DatatypeProperty ;
    rdfs:range ph:symbol ;
    rdfs:label "relationship" ;
    rdfs:comment "Ref tags used to model entity-to-entity relationships.\nSee [Relationships]`docHaystack::Relationships` chapter." ;
    ph:docTaxonomy ph:marker ;
    ph:is ph:symbol ;
    ph:lib ph:lib:ph .

ph:remove a owl:DatatypeProperty ;
    rdfs:subClassOf xsd:string ;
    rdfs:label "remove" ;
    rdfs:comment "Singleton for remove operation.\nSee [Kinds chapter]`docHaystack::Kinds#remove`." ;
    ph:is ph:scalar ;
    ph:lib ph:lib:ph .

phIoT:return a owl:Class ;
    rdfs:subClassOf phIoT:ductSection ;
    rdfs:label "return" ;
    rdfs:comment "Duct returning air back to equipment" ;
    ph:is phIoT:ductSection ;
    ph:lib phIoT:lib:phIoT .

phIoT:roof a owl:Class ;
    rdfs:subClassOf ph:marker ;
    rdfs:label "roof" ;
    rdfs:comment "Envelope covering the top of a building" ;
    ph:is ph:marker ;
    ph:lib phIoT:lib:phIoT .

phIoT:roof-floor a owl:Class ;
    rdfs:subClassOf phIoT:floor ;
    rdfs:label "roof-floor" ;
    ph:children _:0b2cb027-d76e-0140-0f48-f23c91a70cca,
        _:0b2cb027-d76e-0141-0f49-f23c91a70cca,
        _:0b2cb027-d76e-0142-0f4a-f23c91a70cca ;
    rdfs:comment "The roof floor is the topmost level of a building.  It is often\nwhere HVAC equipment is located such as rooftop AHUs." ;
    ph:is phIoT:floor ;
    ph:lib phIoT:lib:phIoT ;
    ph:wikipedia "https://en.wikipedia.org/wiki/Storey"^^xsd:anyURI .

_:0b2cb027-d76e-0140-0f48-f23c91a70cca a phIoT:equip ;
    ph:hasTag phIoT:equip ;
    rdfs:label "{equip}" .

_:0b2cb027-d76e-0141-0f49-f23c91a70cca a phIoT:point ;
    ph:hasTag phIoT:point ;
    rdfs:label "{point}" .

_:0b2cb027-d76e-0142-0f4a-f23c91a70cca a phIoT:space ;
    ph:hasTag phIoT:space ;
    rdfs:label "{space}" .

phIoT:room a owl:Class ;
    rdfs:subClassOf phIoT:space ;
    rdfs:label "room" ;
    ph:children _:0b2cb027-d76e-0143-0f4b-f23c91a70cca,
        _:0b2cb027-d76e-0144-0f4c-f23c91a70cca,
        _:0b2cb027-d76e-0145-0f4d-f23c91a70cca ;
    rdfs:comment "Enclosed room of a building" ;
    ph:is phIoT:space ;
    ph:lib phIoT:lib:phIoT ;
    ph:wikipedia "https://en.wikipedia.org/wiki/Room"^^xsd:anyURI .

_:0b2cb027-d76e-0143-0f4b-f23c91a70cca a phIoT:space ;
    ph:hasTag phIoT:space ;
    rdfs:label "{space}" .

_:0b2cb027-d76e-0144-0f4c-f23c91a70cca a phIoT:equip ;
    ph:hasTag phIoT:equip ;
    rdfs:label "{equip}" .

_:0b2cb027-d76e-0145-0f4d-f23c91a70cca a phIoT:point ;
    ph:hasTag phIoT:point ;
    rdfs:label "{point}" .

phIoT:rotaryScrew a owl:Class ;
    rdfs:subClassOf ph:marker ;
    rdfs:label "rotaryScrew" ;
    rdfs:comment "Rotary screw compression" ;
    ph:is ph:marker ;
    ph:lib phIoT:lib:phIoT ;
    ph:wikipedia "https://en.wikipedia.org/wiki/Rotary-screw_compressor"^^xsd:anyURI .

phIct:router a owl:Class ;
    rdfs:subClassOf ph:marker ;
    rdfs:label "router" ;
    rdfs:comment "Device used to route data packets" ;
    ph:is ph:marker ;
    ph:lib phIct:lib:phIct .

phIoT:rtu a owl:Class ;
    rdfs:subClassOf phIoT:ahu ;
    rdfs:label "rtu" ;
    ph:children _:0b2cb027-d77d-4380-0f4e-f23c91a70cca,
        _:0b2cb027-d77d-4381-0f4f-f23c91a70cca,
        _:0b2cb027-d77d-4382-0f50-f23c91a70cca,
        _:0b2cb027-d77d-4383-0f51-f23c91a70cca,
        _:0b2cb027-d77d-4384-0f52-f23c91a70cca,
        _:0b2cb027-d77d-4385-0f53-f23c91a70cca,
        _:0b2cb027-d77d-4386-0f54-f23c91a70cca,
        _:0b2cb027-d77d-4387-0f55-f23c91a70cca,
        _:0b2cb027-d77d-4388-0f56-f23c91a70cca,
        _:0b2cb027-d77d-4389-0f57-f23c91a70cca,
        _:0b2cb027-d77d-438a-0f58-f23c91a70cca,
        _:0b2cb027-d77d-438b-0f59-f23c91a70cca,
        _:0b2cb027-d77d-438c-0f5a-f23c91a70cca,
        _:0b2cb027-d77d-438d-0f5b-f23c91a70cca,
        _:0b2cb027-d77d-438e-0f5c-f23c91a70cca,
        _:0b2cb027-d77d-438f-0f5d-f23c91a70cca,
        _:0b2cb027-d77d-4390-0f5e-f23c91a70cca,
        _:0b2cb027-d77d-4391-0f5f-f23c91a70cca,
        _:0b2cb027-d77d-4392-0f60-f23c91a70cca,
        _:0b2cb027-d77d-4393-0f61-f23c91a70cca,
        _:0b2cb027-d77d-4394-0f62-f23c91a70cca ;
    rdfs:comment "Roof Top Unit: A unitary AHU that is weatherized for outdoor use.\nSee `docHaystack::AHUs` chapter." ;
    ph:is phIoT:ahu ;
    ph:lib phIoT:lib:phIoT ;
    ph:wikipedia "https://en.wikipedia.org/wiki/Air_handler"^^xsd:anyURI .

_:0b2cb027-d77d-4380-0f4e-f23c91a70cca a phIoT:point ;
    ph:hasTag phIoT:bypass,
        phIoT:damper,
        phIoT:cmd,
        phIoT:point ;
    rdfs:label "{bypass, damper, cmd, point}" .

_:0b2cb027-d77d-4381-0f4f-f23c91a70cca a phIoT:point ;
    ph:hasTag phIoT:cool,
        phIoT:cmd,
        phIoT:point ;
    rdfs:label "{cool, cmd, point}" .

_:0b2cb027-d77d-4382-0f50-f23c91a70cca a phIoT:point ;
    ph:hasTag phIoT:dessicantDehumidifier,
        phIoT:cmd,
        phIoT:point ;
    rdfs:label "{dessicantDehumidifier, cmd, point}" .

_:0b2cb027-d77d-4383-0f51-f23c91a70cca a phIoT:duct ;
    ph:hasTag phIoT:discharge,
        phIoT:duct,
        phIoT:equip ;
    rdfs:label "{discharge, duct, equip}" .

_:0b2cb027-d77d-4384-0f52-f23c91a70cca a phIoT:duct ;
    ph:hasTag phIoT:economizer,
        phIoT:duct,
        phIoT:equip ;
    rdfs:label "{economizer, duct, equip}" .

_:0b2cb027-d77d-4385-0f53-f23c91a70cca a phIoT:point ;
    ph:hasTag phIoT:economizing,
        phIoT:cmd,
        phIoT:point ;
    rdfs:label "{economizing, cmd, point}" .

_:0b2cb027-d77d-4386-0f54-f23c91a70cca a phIoT:equip ;
    ph:hasTag phIoT:equip ;
    rdfs:label "{equip}" .

_:0b2cb027-d77d-4387-0f55-f23c91a70cca a phIoT:duct ;
    ph:hasTag phIoT:exhaust,
        phIoT:duct,
        phIoT:equip ;
    rdfs:label "{exhaust, duct, equip}" .

_:0b2cb027-d77d-4388-0f56-f23c91a70cca a phIoT:point ;
    ph:hasTag phIoT:faceBypass,
        phIoT:cmd,
        phIoT:point ;
    rdfs:label "{faceBypass, cmd, point}" .

_:0b2cb027-d77d-4389-0f57-f23c91a70cca a phIoT:point ;
    ph:hasTag phIoT:filter,
        phIoT:sensor,
        phIoT:point ;
    rdfs:label "{filter, sensor, point}" .

_:0b2cb027-d77d-438a-0f58-f23c91a70cca a phIoT:point ;
    ph:hasTag phIoT:freezeStat,
        phIoT:sensor,
        phIoT:point ;
    rdfs:label "{freezeStat, sensor, point}" .

_:0b2cb027-d77d-438b-0f59-f23c91a70cca a phIoT:point ;
    ph:hasTag phIoT:heat,
        phIoT:cmd,
        phIoT:point ;
    rdfs:label "{heat, cmd, point}" .

_:0b2cb027-d77d-438c-0f5a-f23c91a70cca a phIoT:point ;
    ph:hasTag phIoT:heatWheel,
        phIoT:cmd,
        phIoT:point ;
    rdfs:label "{heatWheel, cmd, point}" .

_:0b2cb027-d77d-438d-0f5b-f23c91a70cca a phIoT:humidifier-equip ;
    ph:hasTag phIoT:humidifier,
        phIoT:equip ;
    rdfs:label "{humidifier, equip}" .

_:0b2cb027-d77d-438e-0f5c-f23c91a70cca a phIoT:point ;
    ph:hasTag phIoT:hvacMode,
        phIoT:sp,
        phIoT:point ;
    rdfs:label "{hvacMode, sp, point}" .

_:0b2cb027-d77d-438f-0f5d-f23c91a70cca a phIoT:duct ;
    ph:hasTag phIoT:mixed,
        phIoT:duct,
        phIoT:equip ;
    rdfs:label "{mixed, duct, equip}" .

_:0b2cb027-d77d-4390-0f5e-f23c91a70cca a phIoT:duct ;
    ph:hasTag phIoT:outside,
        phIoT:duct,
        phIoT:equip ;
    rdfs:label "{outside, duct, equip}" .

_:0b2cb027-d77d-4391-0f5f-f23c91a70cca a phIoT:point ;
    ph:hasTag phIoT:point ;
    rdfs:label "{point}" .

_:0b2cb027-d77d-4392-0f60-f23c91a70cca a phIoT:duct ;
    ph:hasTag phIoT:return,
        phIoT:duct,
        phIoT:equip ;
    rdfs:label "{return, duct, equip}" .

_:0b2cb027-d77d-4393-0f61-f23c91a70cca a phIoT:thermostat ;
    ph:hasTag phIoT:thermostat,
        phIoT:equip ;
    rdfs:label "{thermostat, equip}" .

_:0b2cb027-d77d-4394-0f62-f23c91a70cca a phIoT:duct ;
    ph:hasTag phIoT:ventilation,
        phIoT:duct,
        phIoT:equip ;
    rdfs:label "{ventilation, duct, equip}" .

phIoT:run a owl:Class ;
    rdfs:subClassOf ph:marker ;
    rdfs:label "run" ;
    rdfs:comment "Primary on/off `point` of an `equip` especially used with a `vfd`.\nRun is used with Bool points where true indicates on and false indicates\noff. When paired with `cmd` this is the commanded state of the equipment.\nWhen paired with `sensor` this is the actual status of the equip.  If\nthe equipment also defines an `enable` point then both must be commanded\non in order to run the equipment." ;
    ph:is ph:marker ;
    ph:lib phIoT:lib:phIoT .

ph:scalar a owl:DatatypeProperty ;
    rdfs:range ph:scalar ;
    rdfs:label "scalar" ;
    rdfs:comment "Scalar is an atomic value kind" ;
    ph:is ph:val ;
    ph:lib ph:lib:ph .

phIoT:secondaryLoop a owl:Class ;
    rdfs:subClassOf phIoT:plantLoop ;
    rdfs:label "secondaryLoop" ;
    rdfs:comment "Pipework which circulates closest to the building or end use. In a\ncentral plant, the secondary loop indicates the pipes and equipment between\nthe central plant and the building.  In context of heat exchangers between\nthe primary and secondary loops, this tag indicates the side closest to\nthe building." ;
    ph:is phIoT:plantLoop ;
    ph:lib phIoT:lib:phIoT .

phIoT:sensor a owl:Class ;
    rdfs:subClassOf phIoT:pointFunction ;
    rdfs:label "sensor" ;
    rdfs:comment "Point is a sensor, input, AI/BI.\nSee `docHaystack::Points#function` chapter." ;
    ph:is phIoT:pointFunction ;
    ph:lib phIoT:lib:phIoT .

phIoT:series a owl:Class ;
    rdfs:subClassOf ph:marker ;
    rdfs:label "series" ;
    rdfs:comment "Circuit with single path of flow" ;
    ph:is ph:marker ;
    ph:lib phIoT:lib:phIoT .

phIct:server a owl:Class ;
    rdfs:subClassOf ph:marker ;
    rdfs:label "server" ;
    rdfs:comment "Hardware or software which provides services for other programs or devices." ;
    ph:is ph:marker ;
    ph:lib phIct:lib:phIct ;
    ph:wikipedia "https://en.wikipedia.org/wiki/Server_(computing)"^^xsd:anyURI .

phIct:server-computer a owl:Class ;
    rdfs:subClassOf phIct:computer ;
    rdfs:label "server-computer" ;
    rdfs:comment "General purpose computer used as a server.  Typically servers are rack mounted." ;
    ph:is phIct:computer ;
    ph:lib phIct:lib:phIct ;
    ph:wikipedia "https://en.wikipedia.org/wiki/Server_(computing)"^^xsd:anyURI .

phIoT:serviceFactor a owl:Class ;
    rdfs:subClassOf ph:marker ;
    rdfs:label "serviceFactor" ;
    rdfs:comment "Ratio of the maximum continuous output capacity at which a machine or\nsystem may operate without damage to the machine or system\u2019s nominal\noutput capacity." ;
    ph:is ph:marker ;
    ph:lib phIoT:lib:phIoT .

phScience:sf6 a owl:Class ;
    rdfs:subClassOf phScience:gas ;
    rdfs:label "sf6" ;
    rdfs:comment "Sulphur hexafluoride (SF\u2086)" ;
    ph:is phScience:gas ;
    ph:lib phScience:lib:phScience ;
    ph:wikipedia "https://en.wikipedia.org/wiki/Sulfur_hexafluoride"^^xsd:anyURI .

phScience:sf6-emission a owl:Class ;
    rdfs:subClassOf phScience:emission ;
    rdfs:label "sf6-emission" ;
    rdfs:comment "Greenhouse gas emission of sulphur hexafluoride (SF\u2086) into the air." ;
    ph:is phScience:emission ;
    ph:lib phScience:lib:phScience ;
    phScience:prefUnit "kg",
        "ton",
        "lb" ;
    phScience:quantityOf phScience:air .

phIoT:sim a owl:Class ;
    rdfs:subClassOf phIoT:synthetic ;
    rdfs:label "sim" ;
    rdfs:comment "Simulation point. See `docHaystack::Synthetics` chapter." ;
    ph:is phIoT:synthetic ;
    ph:lib phIoT:lib:phIoT .

phIoT:sim-point a owl:Class ;
    rdfs:subClassOf phIoT:synthetic-point ;
    rdfs:label "sim-point" ;
    rdfs:comment "See `docHaystack::Synthetics` chapter." ;
    ph:is phIoT:synthetic-point ;
    ph:lib phIoT:lib:phIoT .

phIoT:simBaseline a owl:Class ;
    rdfs:subClassOf phIoT:simScenario ;
    rdfs:label "Baseline" ;
    ph:dis "Baseline" ;
    rdfs:comment "See `docHaystack::Synthetics#sims` chapter." ;
    ph:is phIoT:simScenario ;
    ph:lib phIoT:lib:phIoT .

phIoT:simModel a owl:Class ;
    rdfs:subClassOf phIoT:syntheticModel ;
    rdfs:label "simModel" ;
    rdfs:comment "See `docHaystack::Synthetics` chapter." ;
    ph:is phIoT:syntheticModel ;
    ph:lib phIoT:lib:phIoT .

phIoT:simOperation a owl:Class ;
    rdfs:subClassOf phIoT:simScenario ;
    rdfs:label "Operation" ;
    ph:dis "Operation" ;
    rdfs:comment "See `docHaystack::Synthetics#sims` chapter." ;
    ph:is phIoT:simScenario ;
    ph:lib phIoT:lib:phIoT .

phIoT:simOptimum a owl:Class ;
    rdfs:subClassOf phIoT:simScenario ;
    rdfs:label "Optimum" ;
    ph:dis "Optimum" ;
    rdfs:comment "See `docHaystack::Synthetics#sims` chapter." ;
    ph:is phIoT:simScenario ;
    ph:lib phIoT:lib:phIoT .

phIoT:simScenario a owl:Class ;
    rdfs:subClassOf ph:choice ;
    rdfs:label "simScenario" ;
    rdfs:comment "See `docHaystack::Synthetics#sims` chapter." ;
    ph:is ph:choice ;
    ph:lib phIoT:lib:phIoT ;
    ph:tagOn phIoT:sim-point .

phIoT:singleDuct a owl:Class ;
    rdfs:subClassOf phIoT:ductConfig ;
    rdfs:label "singleDuct" ;
    rdfs:comment "One single duct" ;
    ph:is phIoT:ductConfig ;
    ph:lib phIoT:lib:phIoT .

phIoT:singlePhase a owl:Class ;
    rdfs:subClassOf phIoT:phaseCount ;
    rdfs:label "singlePhase" ;
    rdfs:comment "Single-phase AC electricity. Power is provided by a\nsingle AC voltage source with a 2-wire connection." ;
    ph:is phIoT:phaseCount ;
    ph:lib phIoT:lib:phIoT ;
    ph:wikipedia "https://en.wikipedia.org/wiki/Single-phase_electric_power"^^xsd:anyURI .

phIoT:site a owl:Class ;
    rdfs:subClassOf ph:entity,
        ph:geoPlace ;
    rdfs:label "site" ;
    ph:children _:0b2cb027-d79b-c800-0f63-f23c91a70cca,
        _:0b2cb027-d79b-c801-0f64-f23c91a70cca ;
    rdfs:comment "Site is a geographic location of the built environment.\nTypically site maps to one building with its own unique\nstreet address.  See `docHaystack::Sites` chapter." ;
    ph:docTaxonomy ph:marker ;
    ph:is ph:entity,
        ph:geoPlace ;
    ph:lib phIoT:lib:phIoT ;
    ph:mandatory ph:marker .

_:0b2cb027-d79b-c800-0f63-f23c91a70cca a phIoT:space ;
    ph:hasTag phIoT:space ;
    rdfs:label "{space}" .

_:0b2cb027-d79b-c801-0f64-f23c91a70cca a phIoT:equip ;
    ph:hasTag phIoT:equip ;
    rdfs:label "{equip}" .

phIoT:siteMeter a owl:Class ;
    rdfs:subClassOf phIoT:meterScope ;
    rdfs:label "siteMeter" ;
    rdfs:comment "Main meter for the associated site" ;
    ph:is phIoT:meterScope ;
    ph:lib phIoT:lib:phIoT .

phIoT:siteRef a owl:ObjectProperty ;
    rdfs:domain phIoT:system,
        phIoT:space,
        phIoT:equip,
        phIoT:point ;
    rdfs:range phIoT:site ;
    rdfs:label "siteRef" ;
    ph:containedBy phIoT:site ;
    rdfs:comment "Reference to site which contains the entity" ;
    ph:is ph:ref ;
    ph:lib phIoT:lib:phIoT ;
    ph:of phIoT:site ;
    ph:tagOn phIoT:system,
        phIoT:space,
        phIoT:equip,
        phIoT:point .

phIct:smtp a owl:Class ;
    rdfs:subClassOf phIct:protocol ;
    rdfs:label "smtp" ;
    rdfs:comment "Simple Mail Transfer Protocol for sending email" ;
    ph:is phIct:protocol ;
    ph:lib phIct:lib:phIct ;
    ph:wikipedia "https://en.wikipedia.org/wiki/Simple_Mail_Transfer_Protocol"^^xsd:anyURI .

phIct:snmp a owl:Class ;
    rdfs:subClassOf phIct:protocol ;
    rdfs:label "snmp" ;
    rdfs:comment "Simple Network Management Protocol for managing IP devices" ;
    ph:is phIct:protocol ;
    ph:lib phIct:lib:phIct ;
    ph:wikipedia "https://en.wikipedia.org/wiki/Simple_Network_Management_Protocol"^^xsd:anyURI .

phScience:solar a owl:Class ;
    rdfs:subClassOf phScience:phenomenon ;
    rdfs:label "solar" ;
    rdfs:comment "Relating to energy from the sun" ;
    ph:is phScience:phenomenon ;
    ph:lib phScience:lib:phScience .

phScience:solar-irradiance a owl:Class ;
    rdfs:subClassOf phScience:irradiance ;
    rdfs:label "solar-irradiance" ;
    rdfs:comment "Energy received on surface of the earth from the sun" ;
    ph:is phScience:irradiance ;
    ph:lib phScience:lib:phScience ;
    phScience:prefUnit "W/m\u00b2" ;
    phScience:quantityOf phScience:solar .

phScience:solid a owl:Class ;
    rdfs:subClassOf phScience:substance ;
    rdfs:label "solid" ;
    rdfs:comment "Substance with definite shape and volume" ;
    ph:is phScience:substance ;
    ph:lib phScience:lib:phScience ;
    ph:wikipedia "https://en.wikipedia.org/wiki/Solid"^^xsd:anyURI .

phIct:sox a owl:Class ;
    rdfs:subClassOf phIct:protocol ;
    rdfs:label "sox" ;
    rdfs:comment "Sedona Framework UDP based communication protocol" ;
    ph:is phIct:protocol ;
    ph:lib phIct:lib:phIct ;
    ph:wikipedia "https://en.wikipedia.org/wiki/Communication_protocol"^^xsd:anyURI .

phIoT:sp a owl:Class ;
    rdfs:subClassOf phIoT:pointFunction ;
    rdfs:label "sp" ;
    rdfs:comment "Point is a setpoint, soft point, internal control variable, schedule.\nSee `docHaystack::Points#function` chapter." ;
    ph:is phIoT:pointFunction ;
    ph:lib phIoT:lib:phIoT .

phIoT:space a owl:Class ;
    rdfs:subClassOf ph:entity ;
    rdfs:label "space" ;
    ph:children _:0b2cb027-d79b-c802-0f65-f23c91a70cca,
        _:0b2cb027-d79b-c803-0f66-f23c91a70cca,
        _:0b2cb027-d79b-c804-0f67-f23c91a70cca ;
    rdfs:comment "Space is a three-dimensional volume in the built environment.\nSee `docHaystack::Spaces` chapter." ;
    ph:docTaxonomy ph:marker ;
    ph:is ph:entity ;
    ph:lib phIoT:lib:phIoT ;
    ph:mandatory ph:marker .

_:0b2cb027-d79b-c802-0f65-f23c91a70cca a phIoT:space ;
    ph:hasTag phIoT:space ;
    rdfs:label "{space}" .

_:0b2cb027-d79b-c803-0f66-f23c91a70cca a phIoT:equip ;
    ph:hasTag phIoT:equip ;
    rdfs:label "{equip}" .

_:0b2cb027-d79b-c804-0f67-f23c91a70cca a phIoT:point ;
    ph:hasTag phIoT:point ;
    rdfs:label "{point}" .

phIoT:spaceRef a owl:ObjectProperty ;
    rdfs:domain phIoT:space,
        phIoT:equip,
        phIoT:point ;
    rdfs:range phIoT:space ;
    rdfs:label "spaceRef" ;
    ph:containedBy phIoT:space ;
    rdfs:comment "Reference to space which contains this entity" ;
    ph:is ph:ref ;
    ph:lib phIoT:lib:phIoT ;
    ph:of phIoT:space ;
    ph:tagOn phIoT:space,
        phIoT:equip,
        phIoT:point .

ph:span a owl:DatatypeProperty ;
    rdfs:range ph:xstr ;
    rdfs:label "span" ;
    rdfs:comment "Time span as modeled encoded as XStr.  This is a placeholder\nto eventually formalize the time range used by hisRead op." ;
    ph:is ph:xstr ;
    ph:lib ph:lib:ph .

phScience:speed a owl:Class ;
    rdfs:subClassOf phScience:quantity ;
    rdfs:label "speed" ;
    rdfs:comment "Distance per unit time" ;
    ph:is phScience:quantity ;
    ph:lib phScience:lib:phScience ;
    phScience:prefUnit "km/h",
        "mph" .

phIoT:splitPhase a owl:Class ;
    rdfs:subClassOf phIoT:phaseCount ;
    rdfs:label "splitPhase" ;
    rdfs:comment "Split-phase AC electricity. Power is provided by a\nsingle AC voltage source with a 3-wire connection, consisting of two hot\nwires (phases), separated from each other by a 180-degree phase angle,\nand one neutral wire.  Despite having two labeled phases, split-phase AC\nelectricity is not a true two-phase system." ;
    ph:is phIoT:phaseCount ;
    ph:lib phIoT:lib:phIoT ;
    ph:wikipedia "https://en.wikipedia.org/wiki/Split-phase_electric_power"^^xsd:anyURI .

phIoT:stage a owl:DatatypeProperty ;
    rdfs:range ph:number ;
    rdfs:label "stage" ;
    rdfs:comment "Stage number of staged equipment operation such as coil or pump.\nThe first stage is 1, second stage 2, etc." ;
    ph:is ph:int ;
    ph:lib phIoT:lib:phIoT ;
    ph:minVal 1 .

phIoT:standby a owl:Class ;
    rdfs:subClassOf ph:marker ;
    rdfs:label "standby" ;
    rdfs:comment "Readiness mode of a space" ;
    ph:is ph:marker ;
    ph:lib phIoT:lib:phIoT .

phIoT:stateOfCharge a owl:Class ;
    rdfs:subClassOf phScience:quantity ;
    rdfs:label "stateOfCharge" ;
    rdfs:comment "State of charge (SoC) of an electric `battery`.  Uses a percentage in\nthe range of 0% to 100%, where no charge is indicated as 0% and full\ncharge is indicated as 100%." ;
    ph:is phScience:quantity ;
    ph:lib phIoT:lib:phIoT ;
    phScience:prefUnit "%" ;
    phScience:quantityOf phIoT:dc-elec ;
    ph:wikipedia "https://en.wikipedia.org/wiki/State_of_charge"^^xsd:anyURI .

phScience:steam a owl:Class ;
    rdfs:subClassOf phScience:gas ;
    rdfs:label "steam" ;
    rdfs:comment "Water in its gas form" ;
    ph:is phScience:gas ;
    ph:lib phScience:lib:phScience ;
    ph:wikipedia "https://en.wikipedia.org/wiki/Steam"^^xsd:anyURI .

phIoT:steam-boiler a owl:Class ;
    rdfs:subClassOf phIoT:boiler,
        phIoT:steam-output ;
    rdfs:label "steam-boiler" ;
    ph:children _:0b2cb027-d7d8-d100-0f68-f23c91a70cca,
        _:0b2cb027-d7d8-d101-0f69-f23c91a70cca,
        _:0b2cb027-d7d8-d102-0f6a-f23c91a70cca,
        _:0b2cb027-d7d8-d103-0f6b-f23c91a70cca,
        _:0b2cb027-d7d8-d104-0f6c-f23c91a70cca,
        _:0b2cb027-d7d8-d105-0f6d-f23c91a70cca,
        _:0b2cb027-d7d8-d106-0f6e-f23c91a70cca,
        _:0b2cb027-d7d8-d107-0f6f-f23c91a70cca,
        _:0b2cb027-d7d8-d108-0f70-f23c91a70cca ;
    rdfs:comment "Boiler which outputs steam" ;
    ph:is phIoT:boiler,
        phIoT:steam-output ;
    ph:lib phIoT:lib:phIoT ;
    ph:wikipedia "https://en.wikipedia.org/wiki/Boiler"^^xsd:anyURI .

_:0b2cb027-d7d8-d100-0f68-f23c91a70cca a phIoT:point ;
    ph:hasTag phIoT:alarm,
        phIoT:sensor,
        phIoT:point ;
    rdfs:label "{alarm, sensor, point}" .

_:0b2cb027-d7d8-d101-0f69-f23c91a70cca a phIoT:pipe ;
    ph:hasTag phIoT:circ,
        phIoT:pipe,
        phIoT:equip ;
    rdfs:label "{circ, pipe, equip}" .

_:0b2cb027-d7d8-d102-0f6a-f23c91a70cca a phIoT:pipe ;
    ph:hasTag phIoT:condensate,
        phIoT:entering,
        phIoT:pipe,
        phIoT:equip ;
    rdfs:label "{condensate, entering, pipe, equip}" .

_:0b2cb027-d7d8-d103-0f6b-f23c91a70cca a phIoT:equip ;
    ph:hasTag phIoT:equip ;
    rdfs:label "{equip}" .

_:0b2cb027-d7d8-d104-0f6c-f23c91a70cca a phIoT:duct ;
    ph:hasTag phIoT:flue,
        phIoT:duct,
        phIoT:equip ;
    rdfs:label "{flue, duct, equip}" .

_:0b2cb027-d7d8-d105-0f6d-f23c91a70cca a phIoT:pipe ;
    ph:hasTag phIoT:makeup,
        phScience:water,
        phIoT:entering,
        phIoT:pipe,
        phIoT:equip ;
    rdfs:label "{makeup, water, entering, pipe, equip}" .

_:0b2cb027-d7d8-d106-0f6e-f23c91a70cca a phIoT:duct ;
    ph:hasTag phIoT:outside,
        phIoT:duct,
        phIoT:equip ;
    rdfs:label "{outside, duct, equip}" .

_:0b2cb027-d7d8-d107-0f6f-f23c91a70cca a phIoT:point ;
    ph:hasTag phIoT:point ;
    rdfs:label "{point}" .

_:0b2cb027-d7d8-d108-0f70-f23c91a70cca a phIoT:pipe ;
    ph:hasTag phScience:steam,
        phIoT:leaving,
        phIoT:pipe,
        phIoT:equip ;
    rdfs:label "{steam, leaving, pipe, equip}" .

phIoT:steam-input a owl:Class ;
    rdfs:subClassOf ph:input ;
    rdfs:label "steam-input" ;
    rdfs:comment "Entity inputs steam which flows from another entity" ;
    ph:is ph:input ;
    ph:lib phIoT:lib:phIoT .

phIoT:steam-output a owl:Class ;
    rdfs:subClassOf ph:output ;
    rdfs:label "steam-output" ;
    rdfs:comment "Entity outputs steam to other entities" ;
    ph:is ph:output ;
    ph:lib phIoT:lib:phIoT .

phIoT:steam-plant a owl:Class ;
    rdfs:subClassOf phIoT:plant,
        phIoT:steam-output ;
    rdfs:label "steam-plant" ;
    ph:children _:0b2cb027-d843-a0c0-0f71-f23c91a70cca,
        _:0b2cb027-d843-a0c1-0f72-f23c91a70cca,
        _:0b2cb027-d843-a0c2-0f73-f23c91a70cca,
        _:0b2cb027-d843-a0c3-0f74-f23c91a70cca,
        _:0b2cb027-d843-a0c4-0f75-f23c91a70cca,
        _:0b2cb027-d843-a0c5-0f76-f23c91a70cca,
        _:0b2cb027-d843-a0c6-0f77-f23c91a70cca,
        _:0b2cb027-d843-a0c7-0f78-f23c91a70cca,
        _:0b2cb027-d843-a0c8-0f79-f23c91a70cca,
        _:0b2cb027-d843-a0c9-0f7a-f23c91a70cca,
        _:0b2cb027-d843-a0ca-0f7b-f23c91a70cca,
        _:0b2cb027-d843-a0cb-0f7c-f23c91a70cca,
        _:0b2cb027-d843-a0cc-0f7d-f23c91a70cca,
        _:0b2cb027-d843-a0cd-0f7e-f23c91a70cca,
        _:0b2cb027-d843-a0ce-0f7f-f23c91a70cca,
        _:0b2cb027-d843-a0cf-0f80-f23c91a70cca ;
    rdfs:comment "Plant used to generate steam for heating.\nSee `docHaystack::Plants`." ;
    ph:is phIoT:plant,
        phIoT:steam-output ;
    ph:lib phIoT:lib:phIoT .

_:0b2cb027-d843-a0c0-0f71-f23c91a70cca a phIoT:pipe ;
    ph:hasTag phIoT:condensate,
        phIoT:entering,
        phIoT:pipe,
        phIoT:equip ;
    rdfs:label "{condensate, entering, pipe, equip}" .

_:0b2cb027-d843-a0c1-0f72-f23c91a70cca a phIoT:point ;
    ph:hasTag phIoT:enable,
        phIoT:cmd,
        phIoT:point ;
    rdfs:label "{enable, cmd, point}" .

_:0b2cb027-d843-a0c2-0f73-f23c91a70cca a phIoT:equip ;
    ph:hasTag phIoT:equip ;
    rdfs:label "{equip}" .

_:0b2cb027-d843-a0c3-0f74-f23c91a70cca a phIoT:duct ;
    ph:hasTag phIoT:flue,
        phIoT:duct,
        phIoT:equip ;
    rdfs:label "{flue, duct, equip}" .

_:0b2cb027-d843-a0c4-0f75-f23c91a70cca a phIoT:pipe ;
    ph:hasTag phIoT:makeup,
        phScience:water,
        phIoT:entering,
        phIoT:pipe,
        phIoT:equip ;
    rdfs:label "{makeup, water, entering, pipe, equip}" .

_:0b2cb027-d843-a0c5-0f76-f23c91a70cca a phIoT:duct ;
    ph:hasTag phIoT:outside,
        phIoT:duct,
        phIoT:equip ;
    rdfs:label "{outside, duct, equip}" .

_:0b2cb027-d843-a0c6-0f77-f23c91a70cca a phIoT:point ;
    ph:hasTag phIoT:point ;
    rdfs:label "{point}" .

_:0b2cb027-d843-a0c7-0f78-f23c91a70cca a phIoT:steam-boiler ;
    ph:hasTag phScience:steam,
        phIoT:boiler,
        phIoT:equip ;
    rdfs:label "{steam, boiler, equip}" .

_:0b2cb027-d843-a0c8-0f79-f23c91a70cca a phIoT:pipe ;
    ph:hasTag phScience:steam,
        phIoT:bypass,
        phIoT:pipe,
        phIoT:equip ;
    rdfs:label "{steam, bypass, pipe, equip}" .

_:0b2cb027-d843-a0c9-0f7a-f23c91a70cca a phIoT:point ;
    ph:hasTag phScience:steam,
        phIoT:delta,
        phScience:flow,
        phIoT:sensor,
        phIoT:point ;
    rdfs:label "{steam, delta, flow, sensor, point}" .

_:0b2cb027-d843-a0ca-0f7b-f23c91a70cca a phIoT:point ;
    ph:hasTag phScience:steam,
        phIoT:delta,
        phScience:pressure,
        phIoT:sensor,
        phIoT:point ;
    rdfs:label "{steam, delta, pressure, sensor, point}" .

_:0b2cb027-d843-a0cb-0f7c-f23c91a70cca a phIoT:point ;
    ph:hasTag phScience:steam,
        phIoT:delta,
        phScience:temp,
        phIoT:sensor,
        phIoT:point ;
    rdfs:label "{steam, delta, temp, sensor, point}" .

_:0b2cb027-d843-a0cc-0f7d-f23c91a70cca a phIoT:pipe ;
    ph:hasTag phScience:steam,
        phIoT:header,
        phIoT:pipe,
        phIoT:equip ;
    rdfs:label "{steam, header, pipe, equip}" .

_:0b2cb027-d843-a0cd-0f7e-f23c91a70cca a phIoT:heatExchanger ;
    ph:hasTag phScience:steam,
        phIoT:heatExchanger,
        phIoT:equip ;
    rdfs:label "{steam, heatExchanger, equip}" .

_:0b2cb027-d843-a0ce-0f7f-f23c91a70cca a phIoT:pipe ;
    ph:hasTag phScience:steam,
        phIoT:leaving,
        phIoT:pipe,
        phIoT:equip ;
    rdfs:label "{steam, leaving, pipe, equip}" .

_:0b2cb027-d843-a0cf-0f80-f23c91a70cca a phIoT:point ;
    ph:hasTag phScience:steam,
        phIoT:mixing,
        phIoT:valve,
        phIoT:cmd,
        phIoT:point ;
    rdfs:label "{steam, mixing, valve, cmd, point}" .

phIoT:steam-system a owl:Class ;
    rdfs:subClassOf phIoT:water-system ;
    rdfs:label "steam-system" ;
    ph:children _:0b2cb027-d852-e300-0f81-f23c91a70cca,
        _:0b2cb027-d852-e301-0f82-f23c91a70cca ;
    rdfs:comment "System that circulates water in its vapor state for heating\na space or process." ;
    ph:is phIoT:water-system ;
    ph:lib phIoT:lib:phIoT .

_:0b2cb027-d852-e300-0f81-f23c91a70cca a phIoT:equip ;
    ph:hasTag phIoT:equip ;
    rdfs:label "{equip}" .

_:0b2cb027-d852-e301-0f82-f23c91a70cca a phIoT:point ;
    ph:hasTag phIoT:point ;
    rdfs:label "{point}" .

phIoT:steamHeating a owl:Class ;
    rdfs:subClassOf phIoT:heatingProcess,
        phIoT:steam-input ;
    rdfs:label "steamHeating" ;
    rdfs:comment "Heating using energy of steam" ;
    ph:is phIoT:heatingProcess,
        phIoT:steam-input ;
    ph:lib phIoT:lib:phIoT .

phIoT:steamRef a owl:ObjectProperty ;
    rdfs:domain phIoT:steam-input ;
    rdfs:range phIoT:steam-output ;
    rdfs:label "steamRef" ;
    rdfs:comment "Steam flows from the referent to this entity" ;
    ph:inputs phScience:steam ;
    ph:is ph:ref ;
    ph:lib phIoT:lib:phIoT ;
    ph:of phIoT:steam-output ;
    ph:tagOn phIoT:steam-input .

ph:str a owl:DatatypeProperty ;
    rdfs:subClassOf xsd:string ;
    rdfs:label "str" ;
    rdfs:comment "Unicode string of characters.\nSee [Kinds chapter]`docHaystack::Kinds#str`." ;
    ph:is ph:scalar ;
    ph:lib ph:lib:ph .

phIoT:submeter a owl:Class ;
    rdfs:subClassOf phIoT:meterScope ;
    rdfs:label "submeter" ;
    rdfs:comment "Submeters measure usage of a sub-system or equipment within a site" ;
    ph:is phIoT:meterScope ;
    ph:lib phIoT:lib:phIoT .

phIoT:submeterOf a owl:ObjectProperty ;
    rdfs:domain phIoT:meter ;
    rdfs:range phIoT:meter ;
    rdfs:label "submeterOf" ;
    rdfs:comment "Reference to parent meter which is immediately upstream of this meter" ;
    ph:is ph:ref ;
    ph:lib phIoT:lib:phIoT ;
    ph:of phIoT:meter ;
    ph:tagOn phIoT:meter .

phScience:substance a owl:Class ;
    rdfs:subClassOf phScience:phenomenon ;
    rdfs:label "substance" ;
    rdfs:comment "Matter in one the three states solid, liquid, or gas" ;
    ph:is phScience:phenomenon ;
    ph:lib phScience:lib:phScience ;
    ph:wikipedia "https://en.wikipedia.org/wiki/Matter"^^xsd:anyURI .

phIoT:subterranean a owl:Class ;
    rdfs:subClassOf ph:marker ;
    rdfs:label "subterranean" ;
    rdfs:comment "Below the surface of the earth" ;
    ph:is ph:marker ;
    ph:lib phIoT:lib:phIoT .

phIoT:subterranean-floor a owl:Class ;
    rdfs:subClassOf phIoT:floor ;
    rdfs:label "subterranean-floor" ;
    ph:children _:0b2cb027-d852-e302-0f83-f23c91a70cca,
        _:0b2cb027-d852-e303-0f84-f23c91a70cca,
        _:0b2cb027-d852-e304-0f85-f23c91a70cca ;
    rdfs:comment "Floor below ground level.  Subterranean floors are also known as\nbasements, lower levels, or cellars." ;
    ph:is phIoT:floor ;
    ph:lib phIoT:lib:phIoT ;
    ph:wikipedia "https://en.wikipedia.org/wiki/Storey"^^xsd:anyURI .

_:0b2cb027-d852-e302-0f83-f23c91a70cca a phIoT:equip ;
    ph:hasTag phIoT:equip ;
    rdfs:label "{equip}" .

_:0b2cb027-d852-e303-0f84-f23c91a70cca a phIoT:point ;
    ph:hasTag phIoT:point ;
    rdfs:label "{point}" .

_:0b2cb027-d852-e304-0f85-f23c91a70cca a phIoT:space ;
    ph:hasTag phIoT:space ;
    rdfs:label "{space}" .

phIoT:switch a owl:Class ;
    rdfs:subClassOf ph:marker ;
    rdfs:label "switch" ;
    rdfs:comment "Device for toggling state or routing data" ;
    ph:is ph:marker ;
    ph:lib phIoT:lib:phIoT .

ph:symbol a owl:DatatypeProperty ;
    rdfs:subClassOf xsd:anyURI ;
    rdfs:label "symbol" ;
    rdfs:comment "Symbol to a def. Symbol values are ASCII strings limited to the\nfollowing chars: a-z, A-Z, 0-9, underbar, colon, dash, dot.\nSee [Kinds chapter]`docHaystack::Kinds#symbol`." ;
    ph:is ph:scalar ;
    ph:lib ph:lib:ph .

phIoT:synthetic a owl:Class ;
    rdfs:subClassOf phIoT:pointFunction ;
    rdfs:label "synthetic" ;
    rdfs:comment "Synthetic point with computed operational data. The computed data\nif classified as:\n  - `ml` for machine learning\n  - `sim` for simulation\n  - `computed` as catch all for other computations\n\nSee `docHaystack::Synthetics` chapter." ;
    ph:is phIoT:pointFunction ;
    ph:lib phIoT:lib:phIoT ;
    ph:mandatory ph:marker ;
    ph:tagOn phIoT:point .

phIoT:synthetic-point a owl:Class ;
    rdfs:subClassOf phIoT:point ;
    rdfs:label "synthetic-point" ;
    rdfs:comment "See `docHaystack::Synthetics` chapter." ;
    ph:is phIoT:point ;
    ph:lib phIoT:lib:phIoT .

phIoT:syntheticModel a owl:Class ;
    rdfs:subClassOf ph:entity ;
    rdfs:label "syntheticModel" ;
    rdfs:comment "See `docHaystack::Synthetics` chapter." ;
    ph:is ph:entity ;
    ph:lib phIoT:lib:phIoT ;
    ph:mandatory ph:marker .

phIoT:syntheticModelRef a owl:ObjectProperty ;
    rdfs:domain phIoT:synthetic-point ;
    rdfs:range phIoT:syntheticModel ;
    rdfs:label "syntheticModelRef" ;
    rdfs:comment "See `docHaystack::Synthetics` chapter." ;
    ph:is ph:ref ;
    ph:lib phIoT:lib:phIoT ;
    ph:of phIoT:syntheticModel ;
    ph:tagOn phIoT:synthetic-point .

phIoT:system a owl:Class ;
    rdfs:subClassOf ph:entity ;
    rdfs:label "system" ;
    ph:children _:0b2cb027-d852-e305-0f86-f23c91a70cca,
        _:0b2cb027-d852-e306-0f87-f23c91a70cca ;
    rdfs:comment "Grouping of related equipment dedicated to a single application.\nSee `docHaystack::Systems` chapter." ;
    ph:docTaxonomy ph:marker ;
    ph:is ph:entity ;
    ph:lib phIoT:lib:phIoT ;
    ph:mandatory ph:marker .

_:0b2cb027-d852-e305-0f86-f23c91a70cca a phIoT:equip ;
    ph:hasTag phIoT:equip ;
    rdfs:label "{equip}" .

_:0b2cb027-d852-e306-0f87-f23c91a70cca a phIoT:point ;
    ph:hasTag phIoT:point ;
    rdfs:label "{point}" .

phIoT:systemRef a owl:ObjectProperty ;
    rdfs:domain phIoT:equip,
        phIoT:point,
        phIoT:system ;
    rdfs:range phIoT:system ;
    rdfs:label "systemRef" ;
    rdfs:comment "Reference to system" ;
    ph:is ph:ref ;
    ph:lib phIoT:lib:phIoT ;
    ph:of phIoT:system ;
    ph:tagOn phIoT:equip,
        phIoT:point,
        phIoT:system .

phIct:tablet a owl:Class ;
    rdfs:subClassOf phIct:device ;
    rdfs:label "tablet" ;
    rdfs:comment "Mobile device with touch screen for user input." ;
    ph:is phIct:device ;
    ph:lib phIct:lib:phIct ;
    ph:wikipedia "https://en.wikipedia.org/wiki/Tablet_computer"^^xsd:anyURI .

ph:tagOn a owl:DatatypeProperty ;
    rdfs:domain ph:def ;
    rdfs:range ph:list ;
    rdfs:label "tagOn" ;
    ph:accumulate ph:marker ;
    rdfs:comment "This tag is used on the given entity" ;
    ph:is ph:association ;
    ph:lib ph:lib:ph ;
    ph:notInherited ph:marker ;
    ph:of ph:symbol ;
    ph:reciprocalOf ph:tags ;
    ph:tagOn ph:def .

ph:tags a owl:DatatypeProperty ;
    rdfs:range ph:list ;
    rdfs:label "tags" ;
    ph:computedFromReciprocal ph:marker ;
    rdfs:comment "Tags used with this entity" ;
    ph:docAssociations ph:marker ;
    ph:is ph:association ;
    ph:lib ph:lib:ph ;
    ph:of ph:symbol ;
    ph:reciprocalOf ph:tagOn .

phIoT:tank a owl:Class ;
    rdfs:subClassOf phIoT:equip ;
    rdfs:label "tank" ;
    ph:children _:0b2cb027-d862-2540-0f88-f23c91a70cca,
        _:0b2cb027-d862-2541-0f89-f23c91a70cca,
        _:0b2cb027-d862-2542-0f8a-f23c91a70cca,
        _:0b2cb027-d862-2543-0f8b-f23c91a70cca,
        _:0b2cb027-d862-2544-0f8c-f23c91a70cca ;
    ph:childrenFlatten phScience:substance ;
    rdfs:comment "Tank used to store a substance for temporary holding" ;
    ph:is phIoT:equip ;
    ph:lib phIoT:lib:phIoT ;
    ph:wikipedia "https://en.wikipedia.org/wiki/Storage_tank"^^xsd:anyURI .

_:0b2cb027-d862-2540-0f88-f23c91a70cca a phIoT:equip ;
    ph:hasTag phIoT:equip ;
    rdfs:label "{equip}" .

_:0b2cb027-d862-2541-0f89-f23c91a70cca a phIoT:point ;
    ph:hasTag phScience:level,
        phIoT:sensor,
        phIoT:point ;
    rdfs:label "{level, sensor, point}" .

_:0b2cb027-d862-2542-0f8a-f23c91a70cca a phIoT:point ;
    ph:hasTag phIoT:point ;
    rdfs:label "{point}" .

_:0b2cb027-d862-2543-0f8b-f23c91a70cca a phIoT:point ;
    ph:hasTag phScience:pressure,
        phIoT:sensor,
        phIoT:point ;
    rdfs:label "{pressure, sensor, point}" .

_:0b2cb027-d862-2544-0f8c-f23c91a70cca a phIoT:point ;
    ph:hasTag phScience:temp,
        phIoT:sensor,
        phIoT:point ;
    rdfs:label "{temp, sensor, point}" .

phIoT:tankSubstance a owl:Class ;
    rdfs:subClassOf ph:choice ;
    rdfs:label "tankSubstance" ;
    rdfs:comment "Substance stored by a tank" ;
    ph:is ph:choice ;
    ph:lib phIoT:lib:phIoT ;
    ph:of phScience:substance ;
    ph:tagOn phIoT:tank .

phScience:temp a owl:Class ;
    rdfs:subClassOf phScience:quantity ;
    rdfs:label "temp" ;
    rdfs:comment "Temperature - measure of hot and cold" ;
    ph:is phScience:quantity ;
    ph:lib phScience:lib:phScience ;
    phScience:prefUnit "\u00b0C",
        "\u00b0F" ;
    phScience:quantityOf phScience:substance ;
    ph:wikipedia "https://en.wikipedia.org/wiki/Temperature"^^xsd:anyURI .

phIoT:tertiaryLoop a owl:Class ;
    rdfs:subClassOf phIoT:plantLoop ;
    rdfs:label "tertiaryLoop" ;
    rdfs:comment "Pipework which circulates within the building." ;
    ph:is phIoT:plantLoop ;
    ph:lib phIoT:lib:phIoT .

phIoT:thd a owl:Class ;
    rdfs:subClassOf ph:marker ;
    rdfs:label "thd" ;
    rdfs:comment "Total harmonic distortion" ;
    ph:is ph:marker ;
    ph:lib phIoT:lib:phIoT .

phIoT:thermal a owl:Class ;
    rdfs:subClassOf ph:marker ;
    rdfs:label "thermal" ;
    rdfs:comment "Related to energy of heat" ;
    ph:is ph:marker ;
    ph:lib phIoT:lib:phIoT .

phIoT:thermostat a owl:Class ;
    rdfs:subClassOf phIoT:equip,
        phIoT:hvacZonePoints ;
    rdfs:label "thermostat" ;
    ph:children _:0b2cb027-d862-2545-0f8d-f23c91a70cca,
        _:0b2cb027-d862-2546-0f8e-f23c91a70cca,
        _:0b2cb027-d862-2547-0f8f-f23c91a70cca,
        _:0b2cb027-d862-2548-0f90-f23c91a70cca,
        _:0b2cb027-d862-2549-0f91-f23c91a70cca,
        _:0b2cb027-d862-254a-0f92-f23c91a70cca,
        _:0b2cb027-d862-254b-0f93-f23c91a70cca,
        _:0b2cb027-d862-254c-0f94-f23c91a70cca,
        _:0b2cb027-d862-254d-0f95-f23c91a70cca,
        _:0b2cb027-d862-254e-0f96-f23c91a70cca,
        _:0b2cb027-d862-254f-0f97-f23c91a70cca,
        _:0b2cb027-d862-2550-0f98-f23c91a70cca,
        _:0b2cb027-d862-2551-0f99-f23c91a70cca,
        _:0b2cb027-d862-2552-0f9a-f23c91a70cca,
        _:0b2cb027-d862-2553-0f9b-f23c91a70cca,
        _:0b2cb027-d862-2554-0f9c-f23c91a70cca,
        _:0b2cb027-d862-2555-0f9d-f23c91a70cca,
        _:0b2cb027-d862-2556-0f9e-f23c91a70cca,
        _:0b2cb027-d862-2557-0f9f-f23c91a70cca,
        _:0b2cb027-d862-2558-0fa0-f23c91a70cca,
        _:0b2cb027-d862-2559-0fa1-f23c91a70cca ;
    rdfs:comment "Senses and controls temperature of space in HVAC system.  Thermostats\nmay provide an interface for setpoint control." ;
    ph:is phIoT:equip,
        phIoT:hvacZonePoints ;
    ph:lib phIoT:lib:phIoT ;
    ph:wikipedia "https://en.wikipedia.org/wiki/Thermostat"^^xsd:anyURI .

_:0b2cb027-d862-2545-0f8d-f23c91a70cca a phIoT:equip ;
    ph:hasTag phIoT:equip ;
    rdfs:label "{equip}" .

_:0b2cb027-d862-2546-0f8e-f23c91a70cca a phIoT:point ;
    ph:hasTag phIoT:point ;
    rdfs:label "{point}" .

_:0b2cb027-d862-2547-0f8f-f23c91a70cca a phIoT:point ;
    ph:hasTag phIoT:zone,
        phScience:air,
        phScience:dewPoint,
        phIoT:sensor,
        phIoT:point ;
    rdfs:label "{zone, air, dewPoint, sensor, point}" .

_:0b2cb027-d862-2548-0f90-f23c91a70cca a phIoT:point ;
    ph:hasTag phIoT:zone,
        phScience:air,
        phScience:dewPoint,
        phIoT:sp,
        phIoT:point ;
    rdfs:label "{zone, air, dewPoint, sp, point}" .

_:0b2cb027-d862-2549-0f91-f23c91a70cca a phIoT:point ;
    ph:hasTag phIoT:zone,
        phScience:air,
        phScience:enthalpy,
        phIoT:sensor,
        phIoT:point ;
    rdfs:label "{zone, air, enthalpy, sensor, point}" .

_:0b2cb027-d862-254a-0f92-f23c91a70cca a phIoT:point ;
    ph:hasTag phIoT:zone,
        phScience:air,
        phScience:enthalpy,
        phIoT:sp,
        phIoT:point ;
    rdfs:label "{zone, air, enthalpy, sp, point}" .

_:0b2cb027-d862-254b-0f93-f23c91a70cca a phIoT:point ;
    ph:hasTag phIoT:zone,
        phScience:air,
        phScience:humidity,
        phIoT:sensor,
        phIoT:point ;
    rdfs:label "{zone, air, humidity, sensor, point}" .

_:0b2cb027-d862-254c-0f94-f23c91a70cca a phIoT:point ;
    ph:hasTag phIoT:zone,
        phScience:air,
        phScience:humidity,
        phIoT:sp,
        phIoT:point ;
    rdfs:label "{zone, air, humidity, sp, point}" .

_:0b2cb027-d862-254d-0f95-f23c91a70cca a phIoT:point ;
    ph:hasTag phIoT:zone,
        phScience:air,
        phIoT:hvacMode,
        phIoT:sp,
        phIoT:point ;
    rdfs:label "{zone, air, hvacMode, sp, point}" .

_:0b2cb027-d862-254e-0f96-f23c91a70cca a phIoT:point ;
    ph:hasTag phIoT:zone,
        phScience:air,
        phScience:pressure,
        phIoT:sensor,
        phIoT:point ;
    rdfs:label "{zone, air, pressure, sensor, point}" .

_:0b2cb027-d862-254f-0f97-f23c91a70cca a phIoT:point ;
    ph:hasTag phIoT:zone,
        phScience:air,
        phScience:pressure,
        phIoT:sp,
        phIoT:point ;
    rdfs:label "{zone, air, pressure, sp, point}" .

_:0b2cb027-d862-2550-0f98-f23c91a70cca a phIoT:point ;
    ph:hasTag phIoT:zone,
        phScience:air,
        phScience:temp,
        phIoT:effective,
        phIoT:cooling,
        phIoT:sp,
        phIoT:point ;
    rdfs:label "{zone, air, temp, effective, cooling, sp, point}" .

_:0b2cb027-d862-2551-0f99-f23c91a70cca a phIoT:point ;
    ph:hasTag phIoT:zone,
        phScience:air,
        phScience:temp,
        phIoT:effective,
        phIoT:heating,
        phIoT:sp,
        phIoT:point ;
    rdfs:label "{zone, air, temp, effective, heating, sp, point}" .

_:0b2cb027-d862-2552-0f9a-f23c91a70cca a phIoT:point ;
    ph:hasTag phIoT:zone,
        phScience:air,
        phScience:temp,
        phIoT:effective,
        phIoT:sp,
        phIoT:point ;
    rdfs:label "{zone, air, temp, effective, sp, point}" .

_:0b2cb027-d862-2553-0f9b-f23c91a70cca a phIoT:point ;
    ph:hasTag phIoT:zone,
        phScience:air,
        phScience:temp,
        phIoT:occ,
        phIoT:cooling,
        phIoT:sp,
        phIoT:point ;
    rdfs:label "{zone, air, temp, occ, cooling, sp, point}" .

_:0b2cb027-d862-2554-0f9c-f23c91a70cca a phIoT:point ;
    ph:hasTag phIoT:zone,
        phScience:air,
        phScience:temp,
        phIoT:occ,
        phIoT:heating,
        phIoT:sp,
        phIoT:point ;
    rdfs:label "{zone, air, temp, occ, heating, sp, point}" .

_:0b2cb027-d862-2555-0f9d-f23c91a70cca a phIoT:point ;
    ph:hasTag phIoT:zone,
        phScience:air,
        phScience:temp,
        phIoT:sensor,
        phIoT:point ;
    rdfs:label "{zone, air, temp, sensor, point}" .

_:0b2cb027-d862-2556-0f9e-f23c91a70cca a phIoT:point ;
    ph:hasTag phIoT:zone,
        phScience:air,
        phScience:temp,
        phIoT:standby,
        phIoT:cooling,
        phIoT:sp,
        phIoT:point ;
    rdfs:label "{zone, air, temp, standby, cooling, sp, point}" .

_:0b2cb027-d862-2557-0f9f-f23c91a70cca a phIoT:point ;
    ph:hasTag phIoT:zone,
        phScience:air,
        phScience:temp,
        phIoT:standby,
        phIoT:heating,
        phIoT:sp,
        phIoT:point ;
    rdfs:label "{zone, air, temp, standby, heating, sp, point}" .

_:0b2cb027-d862-2558-0fa0-f23c91a70cca a phIoT:point ;
    ph:hasTag phIoT:zone,
        phScience:air,
        phScience:temp,
        phIoT:unocc,
        phIoT:cooling,
        phIoT:sp,
        phIoT:point ;
    rdfs:label "{zone, air, temp, unocc, cooling, sp, point}" .

_:0b2cb027-d862-2559-0fa1-f23c91a70cca a phIoT:point ;
    ph:hasTag phIoT:zone,
        phScience:air,
        phScience:temp,
        phIoT:unocc,
        phIoT:heating,
        phIoT:sp,
        phIoT:point ;
    rdfs:label "{zone, air, temp, unocc, heating, sp, point}" .

phIoT:threePhase a owl:Class ;
    rdfs:subClassOf phIoT:phaseCount ;
    rdfs:label "threePhase" ;
    rdfs:comment "Three-phase AC electricity. Power is provided by three AC voltage\nsources, each separated from the others by a 120-degree phase angle.\nMay have a 4-wire connection with a neutral (Wye) or a 3-wire connection\nwithout a neutral (Delta)." ;
    ph:is phIoT:phaseCount ;
    ph:lib phIoT:lib:phIoT ;
    ph:wikipedia "https://en.wikipedia.org/wiki/Three-phase_electric_power"^^xsd:anyURI .

ph:time a owl:DatatypeProperty ;
    rdfs:subClassOf xsd:time ;
    rdfs:label "time" ;
    rdfs:comment "ISO 8601 time as hour, minute, seconds: '09:51:27.354'.\nSee [Kinds chapter]`docHaystack::Kinds#time`." ;
    ph:is ph:scalar ;
    ph:lib ph:lib:ph .

phScience:total a owl:Class ;
    rdfs:subClassOf ph:marker ;
    rdfs:label "total" ;
    rdfs:comment "Complete or absolute" ;
    ph:is ph:marker ;
    ph:lib phScience:lib:phScience .

ph:transient a owl:Class ;
    rdfs:subClassOf ph:marker ;
    rdfs:label "transient" ;
    rdfs:comment "Indicates a value tag which should not be persisted.  Transient\nvalues often change frequently and do not provide long term informational\nvalue. Typyically they are stored only in RAM and should not be stored\nto durable storage." ;
    ph:is ph:marker ;
    ph:lib ph:lib:ph ;
    ph:tagOn ph:def .

ph:transitive a owl:Class ;
    rdfs:subClassOf ph:marker ;
    rdfs:label "transitive" ;
    rdfs:comment "This marker is applied to a `relationship` to indicate it is transitive.\nTransitivity requires that if the relationship applies to A,B and B,C\nthen it also applies to A,C." ;
    ph:is ph:marker ;
    ph:lib ph:lib:ph .

phIoT:tripleDuct a owl:Class ;
    rdfs:subClassOf phIoT:ductConfig ;
    rdfs:label "tripleDuct" ;
    rdfs:comment "Three ducts: hotDeck, coldDeck, or neutralDeck" ;
    ph:is phIoT:ductConfig ;
    ph:lib phIoT:lib:phIoT .

phScience:tvoc a owl:Class ;
    rdfs:subClassOf phScience:gas ;
    rdfs:label "tvoc" ;
    rdfs:comment "Total volatile organic compound (TVOC)." ;
    ph:is phScience:gas ;
    ph:lib phScience:lib:phScience ;
    ph:wikipedia "https://en.wikipedia.org/wiki/Volatile_organic_compound"^^xsd:anyURI .

phScience:tvoc-concentration a owl:Class ;
    rdfs:subClassOf phScience:airQuality ;
    rdfs:label "tvoc-concentration" ;
    rdfs:comment "Concentration of total volatile organic compounds (TVOC) in the air" ;
    ph:is phScience:airQuality ;
    ph:lib phScience:lib:phScience ;
    phScience:prefUnit "\u00b5g/m\u00b3",
        "ppb" ;
    phScience:quantityOf phScience:air ;
    ph:wikipedia "https://en.wikipedia.org/wiki/Concentration"^^xsd:anyURI .

phIoT:twoPhase a owl:Class ;
    rdfs:subClassOf phIoT:phaseCount ;
    rdfs:label "twoPhase" ;
    rdfs:comment "Two-phase AC electricity. Power is provided by two AC voltage sources,\nseparated from each other by a 90-degree phase angle. Two-phase systems\nare extremely rare in modern buildings; they have been replaced by\nmodern `threePhase` systems." ;
    ph:is phIoT:phaseCount ;
    ph:lib phIoT:lib:phIoT ;
    ph:wikipedia "https://en.wikipedia.org/wiki/Two-phase_electric_power"^^xsd:anyURI .

ph:tz a owl:DatatypeProperty ;
    rdfs:domain phIoT:point,
        phIoT:site,
        phIoT:weatherStation ;
    rdfs:range ph:str ;
    rdfs:label "tz" ;
    rdfs:comment "Timezone identifier from standard [timezone database]`docHaystack::TimeZones`" ;
    ph:enum "Abidjan\nAccra\nAdak\nAdelaide\nAlgiers\nAlmaty\nAmman\nAmsterdam\nAnadyr\nAnchorage\nAndorra\nApia\nAqtau\nAqtobe\nAraguaina\nAshgabat\nAstrakhan\nAsuncion\nAthens\nAtikokan\nAtyrau\nAuckland\nAzores\nBaghdad\nBahia\nBahia_Banderas\nBaku\nBangkok\nBarbados\nBarnaul\nBeirut\nBelem\nBelgrade\nBelize\nBerlin\nBermuda\nBeulah\nBishkek\nBissau\nBlanc-Sablon\nBoa_Vista\nBogota\nBoise\nBougainville\nBrisbane\nBroken_Hill\nBrunei\nBrussels\nBucharest\nBudapest\nBuenos_Aires\nCET\nCST6CDT\nCairo\nCambridge_Bay\nCampo_Grande\nCanary\nCancun\nCape_Verde\nCaracas\nCasablanca\nCasey\nCatamarca\nCayenne\nCenter\nCeuta\nChagos\nChatham\nChicago\nChihuahua\nChisinau\nChita\nChoibalsan\nChristmas\nChuuk\nCocos\nColombo\nCopenhagen\nCordoba\nCosta_Rica\nCreston\nCuiaba\nCuracao\nCurrie\nDamascus\nDanmarkshavn\nDarwin\nDavis\nDawson\nDawson_Creek\nDenver\nDetroit\nDhaka\nDili\nDubai\nDublin\nDumontDUrville\nDushanbe\nEET\nEST\nEST5EDT\nEaster\nEdmonton\nEfate\nEirunepe\nEl_Aaiun\nEl_Salvador\nEnderbury\nEucla\nFakaofo\nFamagusta\nFaroe\nFiji\nFort_Nelson\nFortaleza\nFunafuti\nGMT\nGMT+1\nGMT+10\nGMT+11\nGMT+12\nGMT+2\nGMT+3\nGMT+4\nGMT+5\nGMT+6\nGMT+7\nGMT+8\nGMT+9\nGMT-1\nGMT-10\nGMT-11\nGMT-12\nGMT-13\nGMT-14\nGMT-2\nGMT-3\nGMT-4\nGMT-5\nGMT-6\nGMT-7\nGMT-8\nGMT-9\nGalapagos\nGambier\nGaza\nGibraltar\nGlace_Bay\nGodthab\nGoose_Bay\nGrand_Turk\nGuadalcanal\nGuam\nGuatemala\nGuayaquil\nGuyana\nHST\nHalifax\nHavana\nHebron\nHelsinki\nHermosillo\nHo_Chi_Minh\nHobart\nHong_Kong\nHonolulu\nHovd\nIndianapolis\nInuvik\nIqaluit\nIrkutsk\nIstanbul\nJakarta\nJamaica\nJayapura\nJerusalem\nJohannesburg\nJuba\nJujuy\nJuneau\nKabul\nKaliningrad\nKamchatka\nKarachi\nKathmandu\nKerguelen\nKhandyga\nKhartoum\nKiev\nKiritimati\nKirov\nKnox\nKolkata\nKosrae\nKrasnoyarsk\nKuala_Lumpur\nKuching\nKwajalein\nLa_Paz\nLa_Rioja\nLagos\nLima\nLindeman\nLisbon\nLondon\nLord_Howe\nLos_Angeles\nLouisville\nLuxembourg\nMET\nMST\nMST7MDT\nMacau\nMaceio\nMacquarie\nMadeira\nMadrid\nMagadan\nMahe\nMajuro\nMakassar\nMaldives\nMalta\nManagua\nManaus\nManila\nMaputo\nMarengo\nMarquesas\nMartinique\nMatamoros\nMauritius\nMawson\nMazatlan\nMelbourne\nMendoza\nMenominee\nMerida\nMetlakatla\nMexico_City\nMinsk\nMiquelon\nMonaco\nMoncton\nMonrovia\nMonterrey\nMontevideo\nMonticello\nMoscow\nNairobi\nNassau\nNauru\nNdjamena\nNew_Salem\nNew_York\nNicosia\nNipigon\nNiue\nNome\nNorfolk\nNoronha\nNoumea\nNovokuznetsk\nNovosibirsk\nOjinaga\nOmsk\nOral\nOslo\nPST8PDT\nPago_Pago\nPalau\nPalmer\nPanama\nPangnirtung\nParamaribo\nParis\nPerth\nPetersburg\nPhoenix\nPitcairn\nPohnpei\nPontianak\nPort-au-Prince\nPort_Moresby\nPort_of_Spain\nPorto_Velho\nPrague\nPuerto_Rico\nPunta_Arenas\nPyongyang\nQatar\nQostanay\nQyzylorda\nRainy_River\nRankin_Inlet\nRarotonga\nRecife\nRegina\nRel\nResolute\nReunion\nReykjavik\nRiga\nRio_Branco\nRio_Gallegos\nRiyadh\nRome\nRothera\nSakhalin\nSalta\nSamara\nSamarkand\nSan_Juan\nSan_Luis\nSantarem\nSantiago\nSanto_Domingo\nSao_Paulo\nSao_Tome\nSaratov\nScoresbysund\nSeoul\nShanghai\nSimferopol\nSingapore\nSitka\nSofia\nSouth_Georgia\nSrednekolymsk\nSt_Johns\nStanley\nStockholm\nSwift_Current\nSydney\nSyowa\nTahiti\nTaipei\nTallinn\nTarawa\nTashkent\nTbilisi\nTegucigalpa\nTehran\nTell_City\nThimphu\nThule\nThunder_Bay\nTijuana\nTirane\nTokyo\nTomsk\nTongatapu\nToronto\nTripoli\nTroll\nTucuman\nTunis\nUTC\nUlaanbaatar\nUlyanovsk\nUrumqi\nUshuaia\nUst-Nera\nUzhgorod\nVancouver\nVevay\nVienna\nVilnius\nVincennes\nVladivostok\nVolgograd\nVostok\nWET\nWake\nWallis\nWarsaw\nWhitehorse\nWinamac\nWindhoek\nWinnipeg\nYakutat\nYakutsk\nYangon\nYekaterinburg\nYellowknife\nYerevan\nZaporozhye\nZurich" ;
    ph:is ph:str ;
    ph:lib ph:lib:ph ;
    ph:tagOn phIoT:point,
        phIoT:site,
        phIoT:weatherStation .

ph:unit a owl:DatatypeProperty ;
    rdfs:domain phIoT:point ;
    rdfs:range ph:str ;
    rdfs:label "unit" ;
    rdfs:comment "Unit identifier from standard unit database" ;
    ph:enum "- %: percent (dimensionless)\n- %RH: percent_relative_humidity (dimensionless)\n- px: pixel (dimensionless)\n- db: decibel (dimensionless)\n- pf: power_factor (dimensionless)\n- pH: ph (dimensionless)\n- gH\u2082O/kgAir: grams_of_water_per_kilogram_dry_air (dimensionless)\n- V/K: volts_per_degree_kelvin (dimensionless)\n- \u00b0daysC: degree_days_celsius (dimensionless)\n- \u00b0daysF: degree_days_fahrenheit (dimensionless)\n- %obsc/ft: percent_obscuration_per_foot (dimensionless)\n- %obsc/m: percent_obscuration_per_meter (dimensionless)\n- psi/\u00b0F: psi_per_degree_fahrenheit (dimensionless)\n- m\u00b2/N: square_meters_per_newton (dimensionless)\n- W/m\u00b2K: watts_per_square_meter_degree_kelvin (dimensionless)\n- dBmV: db_millivolt (dimensionless)\n- dB\u00b5V: db_microvolt (dimensionless)\n- ppu: parts_per_unit (dimensionless)\n- ppm: parts_per_million (dimensionless)\n- ppb: parts_per_billion (dimensionless)\n- g/kg: grams_per_kilogram (dimensionless)\n- rad: radian (dimensionless)\n- deg: degrees_angular (dimensionless)\n- degPh: degrees_phase (dimensionless)\n- sr: steradian (dimensionless)\n- ntu: nephelometric_turbidity_units (dimensionless)\n- fnu: formazin_nephelometric_unit (dimensionless)\n- PUE: power_usage_effectiveness (dimensionless)\n- DCIE: data_center_infrastructure_efficiency (dimensionless)\n- Af: afghani (currency)\n- DZD: algerian_dinar (currency)\n- ARS: argentine_peso (currency)\n- \u0534: armenian_dram (currency)\n- \u0192: aruban_guilder_florin (currency)\n- AUD: australian_dollar (currency)\n- \u043c\u0430\u043d: azerbaijanian_manat (currency)\n- BSD: bahamian_dollar (currency)\n- BHD: bahraini_dinar (currency)\n- \u0e3f: baht (currency)\n- PAB: balboa (currency)\n- BBD: barbados_dollar (currency)\n- Br: belarussian_ruble (currency)\n- BZD: belize_dollar (currency)\n- BMD: bermudian_dollar (currency)\n- VEF: bolivar_fuerte (currency)\n- BOB: boliviano (currency)\n- R$: brazilian_real (currency)\n- BND: brunei_dollar (currency)\n- \u043b\u0432: bulgarian_lev (currency)\n- BIF: burundi_franc (currency)\n- CAD: canadian_dollar (currency)\n- CVE: cape_verde_escudo (currency)\n- KYD: cayman_islands_dollar (currency)\n- \u20b5: cedi (currency)\n- XAF: cfa_franc_bceao (currency)\n- XPF: cfp_franc (currency)\n- CLP: chilean_peso (currency)\n- \u5143: chinese_yuan (currency)\n- CDF: congolese_franc (currency)\n- C$: cordoba_oro (currency)\n- \u20a1: costa_rican_colon (currency)\n- Kn: croatian_kuna (currency)\n- CUP: cuban_peso (currency)\n- K\u010d: czech_koruna (currency)\n- GMD: dalasi (currency)\n- kr: danish_krone (currency)\n- \u0434\u0435\u043d: denar (currency)\n- DJF: djibouti_franc (currency)\n- Db: dobra (currency)\n- DOP: dominican_peso (currency)\n- \u20ab: dong (currency)\n- XCD: east_caribbean_dollar (currency)\n- EGP: egyptian_pound (currency)\n- ETB: ethiopian_birr (currency)\n- \u20ac: euro (currency)\n- FKP: falkland_islands_pound (currency)\n- FJD: fiji_dollar (currency)\n- HUF: forint (currency)\n- GIP: gibraltar_pound (currency)\n- HTG: gourde (currency)\n- \u20b2: guarani (currency)\n- GNF: guinea_franc (currency)\n- GYD: guyana_dollar (currency)\n- HKD: hong_kong_dollar (currency)\n- \u20b4: hryvnia (currency)\n- Kr: iceland_krona (currency)\n- \u20b9: indian_rupee (currency)\n- IRR: iranian_rial (currency)\n- IQD: iraqi_dinar (currency)\n- JMD: jamaican_dollar (currency)\n- JOD: jordanian_dinar (currency)\n- Sh: kenyan_shilling (currency)\n- PGK: kina (currency)\n- \u20ad: kip (currency)\n- \u041a\u041c: konvertibilna_marka (currency)\n- KWD: kuwaiti_dinar (currency)\n- MK: kwacha (currency)\n- Kz: kwanza (currency)\n- MMK: kyat (currency)\n- \u10da: lari (currency)\n- LBP: lebanese_pound (currency)\n- ALL: lek (currency)\n- HNL: lempira (currency)\n- Le: leone (currency)\n- RON: leu (currency)\n- LRD: liberian_dollar (currency)\n- LYD: libyan_dinar (currency)\n- SZL: lilangeni (currency)\n- LSL: loti (currency)\n- MGA: malagasy_ariary (currency)\n- RM: malaysian_ringgit (currency)\n- TMT: manat (currency)\n- MUR: mauritius_rupee (currency)\n- MTn: metical (currency)\n- MXN: mexican_peso (currency)\n- MDL: moldavian_leu (currency)\n- MAD: moroccan_dirham (currency)\n- \u20a6: naira (currency)\n- Nfk: nakfa (currency)\n- NAD: namibia_dollar (currency)\n- NPR: nepalese_rupee (currency)\n- \u20aa: new_israeli_shekel (currency)\n- NZD: new_zealand_dollar (currency)\n- BTN: ngultrum (currency)\n- KPW: north_korean_won (currency)\n- NOK: norwegian_krone (currency)\n- PEN: nuevo_sol (currency)\n- UM: ouguiya (currency)\n- \u20a8: pakistan_rupee (currency)\n- MOP: pataca (currency)\n- UYU: peso_uruguayo (currency)\n- \u20b1: philippine_peso (currency)\n- \u00a3: pound_sterling (currency)\n- BWP: pula (currency)\n- z\u0142: pzloty (currency)\n- QAR: qatari_rial (currency)\n- GTQ: quetzal (currency)\n- ZAR: rand (currency)\n- OMR: rial_omani (currency)\n- KHR: riel (currency)\n- MVR: rufiyaa (currency)\n- Rp: rupiah (currency)\n- RUB: russian_ruble (currency)\n- RWF: rwanda_franc (currency)\n- SHP: saint_helena_pound (currency)\n- SAR: saudi_riyal (currency)\n- din: serbian_dinar (currency)\n- SCR: seychelles_rupee (currency)\n- SGD: singapore_dollar (currency)\n- SBD: solomon_islands_dollar (currency)\n- KGS: som (currency)\n- SOS: somali_shilling (currency)\n- \u0405\u041c: somoni (currency)\n- \u20a9: south_korean_won (currency)\n- Rs: sri_lanka_rupee (currency)\n- SDG: sudanese_pound (currency)\n- SRD: suriname_dollar (currency)\n- SEK: swedish_krona (currency)\n- SFr: swiss_franc (currency)\n- SYP: syrian_pound (currency)\n- TWD: taiwan_dollar (currency)\n- \u09f3: taka (currency)\n- WST: tala (currency)\n- TZS: tanzanian_shilling (currency)\n- \u3012: tenge (currency)\n- TTD: trinidad_and_tobago_dollar (currency)\n- \u20ae: tugrik (currency)\n- TND: tunisian_dinar (currency)\n- \u20a4: turkish_lira (currency)\n- AED: uae_dirham (currency)\n- UGX: uganda_shilling (currency)\n- $: us_dollar (currency)\n- UZS: uzbekistan_sum (currency)\n- Vt: vatu (currency)\n- YER: yemeni_rial (currency)\n- \u00a5: yen (currency)\n- ZK: zambian_kwacha (currency)\n- ZWL: zimbabwe_dollar (currency)\n- m/s\u00b2: meters_per_second_squared (acceleration)\n- rad/s\u00b2: radians_per_second_squared (angular acceleration)\n- Js: joule_second (angular momentum)\n- rad/s: radians_per_second (angular velocity)\n- rpm: revolutions_per_minute (angular velocity)\n- m\u00b2: square_meter (area)\n- mm\u00b2: square_millimeter (area)\n- cm\u00b2: square_centimeter (area)\n- km\u00b2: square_kilometer (area)\n- in\u00b2: square_inch (area)\n- ft\u00b2: square_foot (area)\n- yd\u00b2: square_yard (area)\n- mile\u00b2: square_mile (area)\n- acre: acre (area)\n- F: farad (capacitance)\n- COP: coefficient_of_performance (cooling efficiency)\n- EER: energy_efficiency_ratio (cooling efficiency)\n- kW/ton: kilowatt_per_ton (cooling efficiency)\n- kg/m\u00b3: kilograms_per_cubic_meter (density)\n- g/m\u00b3: grams_per_cubic_meter (density)\n- mg/m\u00b3: milligrams_per_cubic_meter (density)\n- \u00b5g/m\u00b3: micrograms_per_cubic_meter (density)\n- kg/L: kilograms_per_liter (density)\n- mg/L: milligrams_per_liter (density)\n- C: coulomb (electric charge)\n- Ah: ampere_hour (electric charge)\n- S: siemens (electric conductance)\n- A: ampere (electric current)\n- mA: milliampere (electric current)\n- Am\u00b2: ampere_square_meter (electromagnetic moment)\n- A/m\u00b2: amperes_per_square_meter (electric current density)\n- V/m: volts_per_meter (electric field strength)\n- V: volt (electric potential)\n- mV: millivolt (electric potential)\n- kV: kilovolt (electric potential)\n- MV: megavolt (electric potential)\n- \u2126: ohm (electric resistance)\n- k\u2126: kilohm (electric resistance)\n- M\u2126: megohm (electric resistance)\n- m\u2126: milliohm (electric resistance)\n- S/m: siemens_per_meter (electrical conductivity)\n- \u2126m: ohm_meter (electrical resistivity)\n- J: joule (energy)\n- kJ: kilojoule (energy)\n- Wh: watt_hour (energy)\n- kWh: kilowatt_hour (energy)\n- MWh: megawatt_hour (energy)\n- GWh: gigawatt_hour (energy)\n- BTU: btu (energy)\n- kBTU: kilobtu (energy)\n- MMBTU: megabtu (energy)\n- hph: horsepower_hour (energy)\n- cal: calorie (energy)\n- therm: therm (energy)\n- tonrefh: tons_refrigeration_hour (energy)\n- MJ: megajoule (energy)\n- GJ: gigajoule (energy)\n- Nm: newton_meter (energy)\n- m\u00b3_gas: cubic_meters_natural_gas (energy)\n- ft\u00b3_gas: cubic_feet_natural_gas (energy)\n- Hcf_natural_gas: hundred_cubic_feet_natural_gas (energy)\n- Ccf_natural_gas: centum_cubic_feet_natural_gas (energy)\n- Mcf_natural_gas: thousand_cubic_feet_natural_gas (energy)\n- MMcf_natural_gas: million_cubic_feet_natural_gas (energy)\n- VAh: volt_ampere_hour (apparent energy)\n- kVAh: kilovolt_ampere_hour (apparent energy)\n- MVAh: megavolt_ampere_hour (apparent energy)\n- VARh: volt_ampere_reactive_hour (reactive energy)\n- kVARh: kilovolt_ampere_reactive_hour (reactive energy)\n- MVARh: megavolt_ampere_reactive_hour (reactive energy)\n- J/m\u00b2: joules_per_square_meter (energy by area)\n- Wh/m\u00b2: watt_hours_per_square_meter (energy by area)\n- Wh/ft\u00b2: watt_hours_per_square_foot (energy by area)\n- kWh/m\u00b2: kilowatt_hours_per_square_meter (energy by area)\n- kWh/ft\u00b2: kilowatt_hours_per_square_foot (energy by area)\n- MWh/m\u00b2: megawatt_hours_per_square_meter (energy by area)\n- MWh/ft\u00b2: megawatt_hours_per_square_foot (energy by area)\n- MJ/m\u00b2: megajoules_per_square_meter (energy by area)\n- MJ/ft\u00b2: megajoules_per_square_foot (energy by area)\n- BTU/ft\u00b2: btu_per_square_foot (energy by area)\n- kBTU/ft\u00b2: kilobtu_per_square_foot (energy by area)\n- MBTU/ft\u00b2: megabtu_per_square_foot (energy by area)\n- J/m\u00b3: joules_per_cubic_meter (energy by volume)\n- GJ/m\u00b3: gigajoules_per_cubic_meter (energy by volume)\n- kWh/m\u00b3: kilowatt_hours_per_cubic_meter (energy by volume)\n- J/g: joules_per_gram (enthalpy)\n- J/kg: joules_per_kilogram (enthalpy)\n- J/kg_dry: joules_per_kilogram_dry_air (enthalpy)\n- BTU/lb: btu_per_pound (enthalpy)\n- btu/lb_dry: btus_per_pound_dry_air (enthalpy)\n- kJ/kg: kilojoules_per_kilogram (enthalpy)\n- kJ/kg_dry: kilojoules_per_kilogram_dry_air (enthalpy)\n- MJ/kg_dry: megajoules_per_kilogram_dry_air (enthalpy)\n- cal/g: calorie_per_gram (enthalpy)\n- J/\u00b0K: joules_per_degree_kelvin (entropy)\n- kJ/\u00b0K: kilojoules_per_degree_kelvin (entropy)\n- MJ/\u00b0K: megajoules_per_degree_kelvin (entropy)\n- N: newton (force)\n- lbf: pound_force (force)\n- Hz: hertz (frequency)\n- kHz: kilohertz (frequency)\n- cph: cycles_per_hour (frequency)\n- cpm: cycles_per_minute (frequency)\n- MHz: megahertz (frequency)\n- /min: per_minute (frequency)\n- /s: per_second (frequency)\n- /h: per_hour (frequency)\n- %/s: percent_per_second (frequency)\n- ACH: air_changes_per_hour (frequency)\n- kg/m\u00b2: kilograms_per_square_meter (grammage)\n- g/m\u00b2: grams_per_square_meter (grammage)\n- K/s: degrees_kelvin_per_second (heating rate)\n- \u00b0C/h: degrees_celsius_per_hour (heating rate)\n- \u00b0C/min: degrees_celsius_per_minute (heating rate)\n- \u00b0F/h: degrees_fahrenheit_per_hour (heating rate)\n- \u00b0F/min: degrees_fahrenheit_per_minute (heating rate)\n- K/h: degrees_kelvin_per_hour (heating rate)\n- K/min: degrees_kelvin_per_minute (heating rate)\n- lx: lux (illuminance)\n- fc: footcandle (illuminance)\n- phot: phot (illuminance)\n- H: henry (inductance)\n- W/m\u00b2_irr: watts_per_square_meter_irradiance (irradiance)\n- W/ft\u00b2_irr: watts_per_square_foot_irradiance (irradiance)\n- m: meter (length)\n- \u00b5m: micrometer (length)\n- mm: millimeter (length)\n- cm: centimeter (length)\n- km: kilometer (length)\n- in: inch (length)\n- ft: foot (length)\n- yd: yard (length)\n- mile: mile (length)\n- cd/m\u00b2: candelas_per_square_meter (luminance)\n- cd/ft\u00b2: candels_per_square_foot (luminance)\n- lm: lumen (luminous flux)\n- cd: candela (luminous intensity)\n- A/m: amperes_per_meter (magnetic field strength)\n- Wb: weber (magnetic flux)\n- T: tesla (magnetic flux density)\n- kg: kilogram (mass)\n- mg: milligram (mass)\n- g: gram (mass)\n- oz: ounce (mass)\n- lb: pound (mass)\n- klb: kilopound (mass)\n- ton: metric_ton (mass)\n- t: short_ton (mass)\n- kg/s: kilograms_per_second (mass flow)\n- kg/min: kilograms_per_minute (mass flow)\n- kg/h: kilograms_per_hour (mass flow)\n- lb/min: pounds_per_minute (mass flow)\n- lb/h: pounds_per_hour (mass flow)\n- lb/s: pounds_per_second (mass flow)\n- klb/h: kilopounds_per_hour (mass flow)\n- g/s: grams_per_second (mass flow)\n- g/min: grams_per_minute (mass flow)\n- ton/h: metric_tons_per_hour (mass flow)\n- Ns: newton_second (momentum)\n- W: watt (power)\n- mW: milliwatt (power)\n- kW: kilowatt (power)\n- MW: megawatt (power)\n- GW: gigawatt (power)\n- BTU/h: btus_per_hour (power)\n- therm/h: therms_per_hour (power)\n- hp: horsepower (power)\n- ftlbs/sec: foot_pounds_per_second (power)\n- tonref: tons_refrigeration (power)\n- kBTU/h: kilobtus_per_hour (power)\n- MMBTU/h: megabtus_per_hour (power)\n- J/h: joules_per_hour (power)\n- kJ/h: kilojoules_per_hour (power)\n- MJ/h: megajoules_per_hour (power)\n- GJ/h: gigajoules_per_hour (power)\n- W/m\u00b2: watts_per_square_meter (power by area)\n- W/ft\u00b2: watts_per_square_foot (power by area)\n- kW/m\u00b2: kilowatts_per_square_meter (power by area)\n- kW/ft\u00b2: kilowatts_per_square_foot (power by area)\n- kBTU/h/ft\u00b2: kilobtus_per_hour_per_square_foot (power by area)\n- W/m\u00b3/s: watts_per_cubic_meters_per_second (power by volumetric flow)\n- W/cfm: watts_per_cubic_feet_per_minute (power by volumetric flow)\n- kW/kcfm: kilowatts_per_kilocubic_feet_per_minute (power by volumetric flow)\n- kW/gal/min: kilowatts_per_gallons_per_minute (power by volumetric flow)\n- VA: volt_ampere (apparent power)\n- kVA: kilovolt_ampere (apparent power)\n- mVA: megavolt_ampere (apparent power)\n- VAR: volt_ampere_reactive (reactive power)\n- kVAR: kilovolt_ampere_reactive (reactive power)\n- MVAR: megavolt_ampere_reactive (reactive power)\n- Pa: pascal (pressure)\n- kPa: kilopascal (pressure)\n- bar: bar (pressure)\n- atm: atmosphere (pressure)\n- psi: pounds_per_square_inch (pressure)\n- cmH\u2082O: centimeters_of_water (pressure)\n- inH\u2082O: inches_of_water (pressure)\n- mmHg: millimeters_of_mercury (pressure)\n- cmHg: centimeters_of_mercury (pressure)\n- inHg: inches_of_mercury (pressure)\n- hPa: hectopascal (pressure)\n- mbar: millibar (pressure)\n- J/kg\u00b0K: joules_per_kilogram_degree_kelvin (specific entropy)\n- N/m: newtons_per_meter (surface tension)\n- \u00b0F: fahrenheit (temperature)\n- \u00b0C: celsius (temperature)\n- K: kelvin (temperature)\n- \u0394\u00b0F: fahrenheit_degrees (temperature differential)\n- \u0394\u00b0C: celsius_degrees (temperature differential)\n- \u0394K: kelvin_degrees (temperature differential)\n- W/m\u00b0K: watts_per_meter_degree_kelvin (thermal conductivity)\n- ns: nanosecond (time)\n- \u00b5s: microsecond (time)\n- ms: millisecond (time)\n- cs: hundredths_second (time)\n- ds: tenths_second (time)\n- sec: second (time)\n- min: minute (time)\n- hr: hour (time)\n- day: day (time)\n- wk: week (time)\n- mo: julian_month (time)\n- yr: year (time)\n- m/s: meters_per_second (velocity)\n- km/s: kilometers_per_second (velocity)\n- km/h: kilometers_per_hour (velocity)\n- mph: miles_per_hour (velocity)\n- ft/s: feet_per_second (velocity)\n- ft/min: feet_per_minute (velocity)\n- in/h: inches_per_hour (velocity)\n- mm/s: millimeters_per_second (velocity)\n- mm/min: millimeters_per_minute (velocity)\n- mm/h: millimeters_per_hour (velocity)\n- m/min: meters_per_minute (velocity)\n- m/h: meters_per_hour (velocity)\n- knot: knot (velocity)\n- cfm/ft\u00b2: cubic_feet_per_minute_per_square_foot (velocity)\n- m\u00b3: cubic_meter (volume)\n- mm\u00b3: cubic_millimeter (volume)\n- cm\u00b3: cubic_centimeter (volume)\n- mL: milliliter (volume)\n- hL: hectoliter (volume)\n- L: liter (volume)\n- kL: kiloliter (volume)\n- in\u00b3: cubic_inch (volume)\n- ft\u00b3: cubic_foot (volume)\n- yd\u00b3: cubic_yard (volume)\n- gal: gallon (volume)\n- kgal: kilogallon (volume)\n- qt: quart (volume)\n- pt: pint (volume)\n- fl_oz: fluid_ounce (volume)\n- galUK: imperial_gallon (volume)\n- hft\u00b3: hecto_cubic_foot (volume)\n- Hcf: hundred_cubic_feet (volume)\n- Ccf: centum_cubic_feet (volume)\n- Mcf: thousand_cubic_feet (volume)\n- MMcf: million_cubic_feet (volume)\n- m\u00b3/s: cubic_meters_per_second (volumetric flow)\n- mL/s: milliliters_per_second (volumetric flow)\n- hL/s: hectoliters_per_second (volumetric flow)\n- L/s: liters_per_second (volumetric flow)\n- cfs: cubic_feet_per_second (volumetric flow)\n- cfm: cubic_feet_per_minute (volumetric flow)\n- cfh: cubic_feet_per_hour (volumetric flow)\n- kcfm: kilocubic_feet_per_minute (volumetric flow)\n- galUK/min: imperial_gallons_per_minute (volumetric flow)\n- L/min: liters_per_minute (volumetric flow)\n- gal/min: gallons_per_minute (volumetric flow)\n- gph: gallons_per_hour (volumetric flow)\n- L/h: liters_per_hour (volumetric flow)\n- m\u00b3/min: cubic_meters_per_minute (volumetric flow)\n- m\u00b3/h: cubic_meters_per_hour (volumetric flow)\n- byte: byte (bytes)\n- kB: kilobyte (bytes)\n- MB: megabyte (bytes)\n- GB: gigabyte (bytes)\n- TB: terabyte (bytes)\n- PB: petabyte (bytes)\n" ;
    ph:is ph:str ;
    ph:lib ph:lib:ph ;
    ph:tagOn phIoT:point .

phIoT:unitVent a owl:Class ;
    rdfs:subClassOf phIoT:fcu ;
    rdfs:label "unitVent" ;
    ph:children _:0b2cb027-d8ae-7080-0fa2-f23c91a70cca,
        _:0b2cb027-d8ae-7081-0fa3-f23c91a70cca,
        _:0b2cb027-d8ae-7082-0fa4-f23c91a70cca,
        _:0b2cb027-d8ae-7083-0fa5-f23c91a70cca,
        _:0b2cb027-d8ae-7084-0fa6-f23c91a70cca,
        _:0b2cb027-d8ae-7085-0fa7-f23c91a70cca,
        _:0b2cb027-d8ae-7086-0fa8-f23c91a70cca,
        _:0b2cb027-d8ae-7087-0fa9-f23c91a70cca,
        _:0b2cb027-d8ae-7088-0faa-f23c91a70cca,
        _:0b2cb027-d8ae-7089-0fab-f23c91a70cca,
        _:0b2cb027-d8ae-708a-0fac-f23c91a70cca,
        _:0b2cb027-d8ae-708b-0fad-f23c91a70cca,
        _:0b2cb027-d8ae-708c-0fae-f23c91a70cca,
        _:0b2cb027-d8ae-708d-0faf-f23c91a70cca,
        _:0b2cb027-d8ae-708e-0fb0-f23c91a70cca,
        _:0b2cb027-d8ae-708f-0fb1-f23c91a70cca,
        _:0b2cb027-d8ae-7090-0fb2-f23c91a70cca,
        _:0b2cb027-d8ae-7091-0fb3-f23c91a70cca,
        _:0b2cb027-d8ae-7092-0fb4-f23c91a70cca,
        _:0b2cb027-d8ae-7093-0fb5-f23c91a70cca,
        _:0b2cb027-d8ae-7094-0fb6-f23c91a70cca ;
    rdfs:comment "Unit Ventilator: An FCU that has direct access to outside air to provide\nthe space with ventilation.  See `docHaystack::AHUs` chapter." ;
    ph:is phIoT:fcu ;
    ph:lib phIoT:lib:phIoT ;
    ph:wikipedia "https://en.wikipedia.org/wiki/Fan_coil_unit"^^xsd:anyURI .

_:0b2cb027-d8ae-7080-0fa2-f23c91a70cca a phIoT:point ;
    ph:hasTag phIoT:bypass,
        phIoT:damper,
        phIoT:cmd,
        phIoT:point ;
    rdfs:label "{bypass, damper, cmd, point}" .

_:0b2cb027-d8ae-7081-0fa3-f23c91a70cca a phIoT:point ;
    ph:hasTag phIoT:cool,
        phIoT:cmd,
        phIoT:point ;
    rdfs:label "{cool, cmd, point}" .

_:0b2cb027-d8ae-7082-0fa4-f23c91a70cca a phIoT:point ;
    ph:hasTag phIoT:dessicantDehumidifier,
        phIoT:cmd,
        phIoT:point ;
    rdfs:label "{dessicantDehumidifier, cmd, point}" .

_:0b2cb027-d8ae-7083-0fa5-f23c91a70cca a phIoT:duct ;
    ph:hasTag phIoT:discharge,
        phIoT:duct,
        phIoT:equip ;
    rdfs:label "{discharge, duct, equip}" .

_:0b2cb027-d8ae-7084-0fa6-f23c91a70cca a phIoT:duct ;
    ph:hasTag phIoT:economizer,
        phIoT:duct,
        phIoT:equip ;
    rdfs:label "{economizer, duct, equip}" .

_:0b2cb027-d8ae-7085-0fa7-f23c91a70cca a phIoT:point ;
    ph:hasTag phIoT:economizing,
        phIoT:cmd,
        phIoT:point ;
    rdfs:label "{economizing, cmd, point}" .

_:0b2cb027-d8ae-7086-0fa8-f23c91a70cca a phIoT:equip ;
    ph:hasTag phIoT:equip ;
    rdfs:label "{equip}" .

_:0b2cb027-d8ae-7087-0fa9-f23c91a70cca a phIoT:duct ;
    ph:hasTag phIoT:exhaust,
        phIoT:duct,
        phIoT:equip ;
    rdfs:label "{exhaust, duct, equip}" .

_:0b2cb027-d8ae-7088-0faa-f23c91a70cca a phIoT:point ;
    ph:hasTag phIoT:faceBypass,
        phIoT:cmd,
        phIoT:point ;
    rdfs:label "{faceBypass, cmd, point}" .

_:0b2cb027-d8ae-7089-0fab-f23c91a70cca a phIoT:point ;
    ph:hasTag phIoT:filter,
        phIoT:sensor,
        phIoT:point ;
    rdfs:label "{filter, sensor, point}" .

_:0b2cb027-d8ae-708a-0fac-f23c91a70cca a phIoT:point ;
    ph:hasTag phIoT:freezeStat,
        phIoT:sensor,
        phIoT:point ;
    rdfs:label "{freezeStat, sensor, point}" .

_:0b2cb027-d8ae-708b-0fad-f23c91a70cca a phIoT:point ;
    ph:hasTag phIoT:heat,
        phIoT:cmd,
        phIoT:point ;
    rdfs:label "{heat, cmd, point}" .

_:0b2cb027-d8ae-708c-0fae-f23c91a70cca a phIoT:point ;
    ph:hasTag phIoT:heatWheel,
        phIoT:cmd,
        phIoT:point ;
    rdfs:label "{heatWheel, cmd, point}" .

_:0b2cb027-d8ae-708d-0faf-f23c91a70cca a phIoT:humidifier-equip ;
    ph:hasTag phIoT:humidifier,
        phIoT:equip ;
    rdfs:label "{humidifier, equip}" .

_:0b2cb027-d8ae-708e-0fb0-f23c91a70cca a phIoT:point ;
    ph:hasTag phIoT:hvacMode,
        phIoT:sp,
        phIoT:point ;
    rdfs:label "{hvacMode, sp, point}" .

_:0b2cb027-d8ae-708f-0fb1-f23c91a70cca a phIoT:duct ;
    ph:hasTag phIoT:mixed,
        phIoT:duct,
        phIoT:equip ;
    rdfs:label "{mixed, duct, equip}" .

_:0b2cb027-d8ae-7090-0fb2-f23c91a70cca a phIoT:duct ;
    ph:hasTag phIoT:outside,
        phIoT:duct,
        phIoT:equip ;
    rdfs:label "{outside, duct, equip}" .

_:0b2cb027-d8ae-7091-0fb3-f23c91a70cca a phIoT:point ;
    ph:hasTag phIoT:point ;
    rdfs:label "{point}" .

_:0b2cb027-d8ae-7092-0fb4-f23c91a70cca a phIoT:duct ;
    ph:hasTag phIoT:return,
        phIoT:duct,
        phIoT:equip ;
    rdfs:label "{return, duct, equip}" .

_:0b2cb027-d8ae-7093-0fb5-f23c91a70cca a phIoT:thermostat ;
    ph:hasTag phIoT:thermostat,
        phIoT:equip ;
    rdfs:label "{thermostat, equip}" .

_:0b2cb027-d8ae-7094-0fb6-f23c91a70cca a phIoT:duct ;
    ph:hasTag phIoT:ventilation,
        phIoT:duct,
        phIoT:equip ;
    rdfs:label "{ventilation, duct, equip}" .

phIoT:unocc a owl:Class ;
    rdfs:subClassOf ph:marker ;
    rdfs:label "unocc" ;
    rdfs:comment "Unoccupied mode of a space.\nSee `docHaystack::Zones#occupancy` chapter." ;
    ph:is ph:marker ;
    ph:lib phIoT:lib:phIoT .

phIct:ups a owl:Class ;
    rdfs:subClassOf phIoT:equip ;
    rdfs:label "ups" ;
    ph:children _:0b2cb027-d8ae-7095-0fb7-f23c91a70cca,
        _:0b2cb027-d8ae-7096-0fb8-f23c91a70cca ;
    rdfs:comment "Uninterruptible power supply" ;
    ph:is phIoT:equip ;
    ph:lib phIct:lib:phIct ;
    ph:wikipedia "https://en.wikipedia.org/wiki/Uninterruptible_power_supply"^^xsd:anyURI .

_:0b2cb027-d8ae-7095-0fb7-f23c91a70cca a phIoT:equip ;
    ph:hasTag phIoT:equip ;
    rdfs:label "{equip}" .

_:0b2cb027-d8ae-7096-0fb8-f23c91a70cca a phIoT:point ;
    ph:hasTag phIoT:point ;
    rdfs:label "{point}" .

ph:uri a owl:DatatypeProperty ;
    rdfs:subClassOf xsd:anyURI ;
    rdfs:label "uri" ;
    rdfs:comment "Universal resource identifier.\nSee [Kinds chapter]`docHaystack::Kinds#uri`." ;
    ph:is ph:scalar ;
    ph:lib ph:lib:ph .

ph:val rdfs:label "val" ;
    rdfs:comment "Data value type" ;
    ph:docTaxonomy ph:marker ;
    ph:lib ph:lib:ph .

phIoT:valve a owl:Class ;
    rdfs:subClassOf ph:marker ;
    rdfs:label "valve" ;
    rdfs:comment "Valve equipment or control point" ;
    ph:is ph:marker ;
    ph:lib phIoT:lib:phIoT ;
    ph:wikipedia "https://en.wikipedia.org/wiki/Valve"^^xsd:anyURI .

phIoT:valve-actuator a owl:Class ;
    rdfs:subClassOf phIoT:actuator ;
    rdfs:label "valve-actuator" ;
    ph:children _:0b2cb027-d8ae-7097-0fb9-f23c91a70cca,
        _:0b2cb027-d8ae-7098-0fba-f23c91a70cca,
        _:0b2cb027-d8ae-7099-0fbb-f23c91a70cca,
        _:0b2cb027-d8ae-709a-0fbc-f23c91a70cca ;
    ph:childrenFlatten phScience:fluid,
        phIoT:pipeSection ;
    rdfs:comment "Actuator to regulate the flow of fluid." ;
    ph:is phIoT:actuator ;
    ph:lib phIoT:lib:phIoT ;
    ph:wikipedia "https://en.wikipedia.org/wiki/Valve"^^xsd:anyURI .

_:0b2cb027-d8ae-7097-0fb9-f23c91a70cca a phIoT:equip ;
    ph:hasTag phIoT:equip ;
    rdfs:label "{equip}" .

_:0b2cb027-d8ae-7098-0fba-f23c91a70cca a phIoT:point ;
    ph:hasTag phIoT:point ;
    rdfs:label "{point}" .

_:0b2cb027-d8ae-7099-0fbb-f23c91a70cca a phIoT:point ;
    ph:hasTag phIoT:valve,
        phIoT:cmd,
        phIoT:point ;
    rdfs:label "{valve, cmd, point}" .

_:0b2cb027-d8ae-709a-0fbc-f23c91a70cca a phIoT:point ;
    ph:hasTag phIoT:valve,
        phIoT:sensor,
        phIoT:point ;
    rdfs:label "{valve, sensor, point}" .

phIoT:variableAirVolume a owl:Class ;
    rdfs:subClassOf phIoT:airVolumeAdjustability ;
    rdfs:label "variableAirVolume" ;
    rdfs:comment "Delivers a variable volume of air flow.   Most variable volume systems\nare powered by a VFD fan. However other techniques such as inlet vanes\nmay be used in older systems." ;
    ph:is phIoT:airVolumeAdjustability ;
    ph:lib phIoT:lib:phIoT .

phIoT:vav a owl:Class ;
    rdfs:subClassOf phIoT:airTerminalUnit ;
    rdfs:label "vav" ;
    ph:children _:0b2cb027-d8bd-b2c0-0fbd-f23c91a70cca,
        _:0b2cb027-d8bd-b2c1-0fbe-f23c91a70cca,
        _:0b2cb027-d8bd-b2c2-0fbf-f23c91a70cca,
        _:0b2cb027-d8bd-b2c3-0fc0-f23c91a70cca,
        _:0b2cb027-d8bd-b2c4-0fc1-f23c91a70cca,
        _:0b2cb027-d8bd-b2c5-0fc2-f23c91a70cca,
        _:0b2cb027-d8bd-b2c6-0fc3-f23c91a70cca,
        _:0b2cb027-d8bd-b2c7-0fc4-f23c91a70cca,
        _:0b2cb027-d8bd-b2c8-0fc5-f23c91a70cca ;
    rdfs:comment "Variable air volume terminal unit.  VAV systems use a constant air\ntemperature with a variable air flow rate.  See `docHaystack::VAVs` chapter." ;
    ph:is phIoT:airTerminalUnit ;
    ph:lib phIoT:lib:phIoT ;
    ph:wikipedia "https://en.wikipedia.org/wiki/Variable_air_volume"^^xsd:anyURI .

_:0b2cb027-d8bd-b2c0-0fbd-f23c91a70cca a phIoT:duct ;
    ph:hasTag phIoT:discharge,
        phIoT:duct,
        phIoT:equip ;
    rdfs:label "{discharge, duct, equip}" .

_:0b2cb027-d8bd-b2c1-0fbe-f23c91a70cca a phIoT:point ;
    ph:hasTag phIoT:ductArea,
        phIoT:sp,
        phIoT:point ;
    rdfs:label "{ductArea, sp, point}" .

_:0b2cb027-d8bd-b2c2-0fbf-f23c91a70cca a phIoT:equip ;
    ph:hasTag phIoT:equip ;
    rdfs:label "{equip}" .

_:0b2cb027-d8bd-b2c3-0fc0-f23c91a70cca a phIoT:point ;
    ph:hasTag phIoT:hvacMode,
        phIoT:sp,
        phIoT:point ;
    rdfs:label "{hvacMode, sp, point}" .

_:0b2cb027-d8bd-b2c4-0fc1-f23c91a70cca a phIoT:duct ;
    ph:hasTag phIoT:inlet,
        phIoT:duct,
        phIoT:equip ;
    rdfs:label "{inlet, duct, equip}" .

_:0b2cb027-d8bd-b2c5-0fc2-f23c91a70cca a phIoT:point ;
    ph:hasTag phIoT:perimeterHeat,
        phIoT:cmd,
        phIoT:point ;
    rdfs:label "{perimeterHeat, cmd, point}" .

_:0b2cb027-d8bd-b2c6-0fc3-f23c91a70cca a phIoT:point ;
    ph:hasTag phIoT:point ;
    rdfs:label "{point}" .

_:0b2cb027-d8bd-b2c7-0fc4-f23c91a70cca a phIoT:point ;
    ph:hasTag phIoT:reheat,
        phIoT:cmd,
        phIoT:point ;
    rdfs:label "{reheat, cmd, point}" .

_:0b2cb027-d8bd-b2c8-0fc5-f23c91a70cca a phIoT:thermostat ;
    ph:hasTag phIoT:thermostat,
        phIoT:equip ;
    rdfs:label "{thermostat, equip}" .

phIoT:vav-parallel a owl:Class ;
    rdfs:subClassOf phIoT:vavAirCircuit ;
    rdfs:label "vav-parallel" ;
    rdfs:comment "VAV pulls air from outside the primary air flow" ;
    ph:is phIoT:vavAirCircuit ;
    ph:lib phIoT:lib:phIoT .

phIoT:vav-series a owl:Class ;
    rdfs:subClassOf phIoT:vavAirCircuit ;
    rdfs:label "vav-series" ;
    rdfs:comment "VAV pulls air from the primary air flow" ;
    ph:is phIoT:vavAirCircuit ;
    ph:lib phIoT:lib:phIoT .

phIoT:vavAirCircuit a owl:Class ;
    rdfs:subClassOf ph:choice ;
    rdfs:label "vavAirCircuit" ;
    rdfs:comment "How does the VAV pull in air" ;
    ph:is ph:choice ;
    ph:lib phIoT:lib:phIoT ;
    ph:tagOn phIoT:vav .

phIoT:vavModulation a owl:Class ;
    rdfs:subClassOf ph:choice ;
    rdfs:label "vavModulation" ;
    rdfs:comment "How does VAV modulate the temp based on duct pressure" ;
    ph:is ph:choice ;
    ph:lib phIoT:lib:phIoT ;
    ph:tagOn phIoT:vav .

phIoT:vavZone a owl:Class ;
    rdfs:subClassOf phIoT:ahuZoneDelivery ;
    rdfs:label "vavZone" ;
    rdfs:comment "AHU supplies air to VAV terminal units" ;
    ph:is phIoT:ahuZoneDelivery ;
    ph:lib phIoT:lib:phIoT .

phScience:velocity a owl:Class ;
    rdfs:subClassOf ph:marker ;
    rdfs:label "velocity" ;
    rdfs:comment "Speed in a given direction" ;
    ph:is ph:marker ;
    ph:lib phScience:lib:phScience .

phIoT:ventilation a owl:Class ;
    rdfs:subClassOf phIoT:ductSection ;
    rdfs:label "ventilation" ;
    rdfs:comment "Duct to access fresh outside air only for ventilation, not economizing" ;
    ph:is phIoT:ductSection ;
    ph:lib phIoT:lib:phIoT .

ph:version a owl:DatatypeProperty ;
    rdfs:domain ph:lib ;
    rdfs:range ph:str ;
    rdfs:label "version" ;
    rdfs:comment "Version string formatted as decimal integers separated by a dot" ;
    ph:is ph:str ;
    ph:lib ph:lib:ph ;
    ph:tagOn ph:lib .

phIoT:verticalTransport a owl:Class ;
    rdfs:subClassOf phIoT:equip ;
    rdfs:label "verticalTransport" ;
    ph:children _:0b2cb027-d8bd-b2c9-0fc6-f23c91a70cca,
        _:0b2cb027-d8bd-b2ca-0fc7-f23c91a70cca ;
    rdfs:comment "Equipment to move humans and materials" ;
    ph:is phIoT:equip ;
    ph:lib phIoT:lib:phIoT .

_:0b2cb027-d8bd-b2c9-0fc6-f23c91a70cca a phIoT:equip ;
    ph:hasTag phIoT:equip ;
    rdfs:label "{equip}" .

_:0b2cb027-d8bd-b2ca-0fc7-f23c91a70cca a phIoT:point ;
    ph:hasTag phIoT:point ;
    rdfs:label "{point}" .

phIoT:vfd a owl:Class ;
    rdfs:subClassOf ph:marker ;
    rdfs:label "vfd" ;
    rdfs:comment "Variable-frequency drive.\nSee `docHaystack::Motors` chapter." ;
    ph:is ph:marker ;
    ph:lib phIoT:lib:phIoT ;
    ph:tagOn phIoT:motor ;
    ph:wikipedia "https://en.wikipedia.org/wiki/Variable-frequency_drive"^^xsd:anyURI .

phIoT:vfd-freq a owl:Class ;
    rdfs:subClassOf phScience:quantity ;
    rdfs:label "vfd-freq" ;
    rdfs:comment "VFD frequency measured in \"Hz\"." ;
    ph:is phScience:quantity ;
    ph:lib phIoT:lib:phIoT ;
    phScience:prefUnit "Hz" .

phIoT:vfd-speed a owl:Class ;
    rdfs:subClassOf phScience:quantity ;
    rdfs:label "vfd-speed" ;
    rdfs:comment "VFD speed measured in \"%\"; 0% is off and 100% is the fastest speed." ;
    ph:is phScience:quantity ;
    ph:lib phIoT:lib:phIoT ;
    phScience:prefUnit "%" .

phScience:visibility a owl:Class ;
    rdfs:subClassOf phScience:quantity ;
    rdfs:label "visibility" ;
    rdfs:comment "Distance at which light can be clearly discerned" ;
    ph:is phScience:quantity ;
    ph:lib phScience:lib:phScience ;
    phScience:prefUnit "km",
        "mile" ;
    phScience:quantityOf phScience:weather .

phScience:volt a owl:Class ;
    rdfs:subClassOf ph:marker ;
    rdfs:label "volt" ;
    rdfs:comment "Electrical potential difference or electromotive force." ;
    ph:is ph:marker ;
    ph:lib phScience:lib:phScience .

phIoT:volt-angle a owl:Class ;
    rdfs:subClassOf phScience:quantity ;
    rdfs:label "volt-angle" ;
    rdfs:comment "AC voltage phase angle" ;
    ph:is phScience:quantity ;
    ph:lib phIoT:lib:phIoT ;
    phScience:prefUnit "deg" ;
    phScience:quantityOf phIoT:ac-elec .

phIoT:volt-imbalance a owl:Class ;
    rdfs:subClassOf phScience:quantity ;
    rdfs:label "volt-imbalance" ;
    rdfs:comment "AC voltage phase imbalance. Also referred to as voltage unbalance." ;
    ph:is phScience:quantity ;
    ph:lib phIoT:lib:phIoT ;
    phScience:prefUnit "%" ;
    phScience:quantityOf phIoT:ac-elec .

phIoT:volt-magnitude a owl:Class ;
    rdfs:subClassOf phScience:elec-volt ;
    rdfs:label "volt-magnitude" ;
    rdfs:comment "Root-mean-square (RMS) magnitude of AC electrical voltage" ;
    ph:is phScience:elec-volt ;
    ph:lib phIoT:lib:phIoT ;
    phScience:prefUnit "A" ;
    phScience:quantityOf phIoT:ac-elec .

phIoT:volt-thd a owl:Class ;
    rdfs:subClassOf phScience:quantity ;
    rdfs:label "volt-thd" ;
    rdfs:comment "Total harmonic distortion (THD) of AC voltage" ;
    ph:is phScience:quantity ;
    ph:lib phIoT:lib:phIoT ;
    phScience:prefUnit "%" ;
    phScience:quantityOf phIoT:ac-elec .

phScience:volume a owl:Class ;
    rdfs:subClassOf phScience:quantity ;
    rdfs:label "volume" ;
    rdfs:comment "Three dimensional space occupied by a substance" ;
    ph:is phScience:quantity ;
    ph:lib phScience:lib:phScience ;
    phScience:prefUnit "m\u00b3",
        "ft\u00b3",
        "L",
        "gal" ;
    phScience:quantityOf phScience:substance ;
    ph:wikipedia "https://en.wikipedia.org/wiki/Volume"^^xsd:anyURI .

phIoT:vrf a owl:Class ;
    rdfs:subClassOf ph:marker ;
    rdfs:label "vrf" ;
    rdfs:comment "Variable refigerant flow.  See `docHaystack::VRF` chapter." ;
    ph:is ph:marker ;
    ph:lib phIoT:lib:phIoT ;
    ph:wikipedia "https://en.wikipedia.org/wiki/Variable_refrigerant_flow"^^xsd:anyURI .

phIoT:vrf-coolingOnly-system a owl:Class ;
    rdfs:subClassOf phIoT:vrf-system ;
    rdfs:label "vrf-coolingOnly-system" ;
    ph:children _:0b2cb027-d8dc-3740-0fc8-f23c91a70cca,
        _:0b2cb027-d8dc-3741-0fc9-f23c91a70cca,
        _:0b2cb027-d8dc-3742-0fca-f23c91a70cca,
        _:0b2cb027-d8dc-3743-0fcb-f23c91a70cca,
        _:0b2cb027-d8dc-3744-0fcc-f23c91a70cca ;
    rdfs:comment "Cooling only VRF system can only cool; heating is not available.\nSee `docHaystack::VRF#types` chapter." ;
    ph:is phIoT:vrf-system ;
    ph:lib phIoT:lib:phIoT .

_:0b2cb027-d8dc-3740-0fc8-f23c91a70cca a phIoT:equip ;
    ph:hasTag phIoT:equip ;
    rdfs:label "{equip}" .

_:0b2cb027-d8dc-3741-0fc9-f23c91a70cca a phIoT:point ;
    ph:hasTag phIoT:point ;
    rdfs:label "{point}" .

_:0b2cb027-d8dc-3742-0fca-f23c91a70cca a phIoT:vrf-indoorUnit ;
    ph:hasTag phIoT:vrf,
        phIoT:indoorUnit,
        phIoT:equip ;
    rdfs:label "{vrf, indoorUnit, equip}" .

_:0b2cb027-d8dc-3743-0fcb-f23c91a70cca a phIoT:vrf-outdoorUnit ;
    ph:hasTag phIoT:vrf,
        phIoT:outdoorUnit,
        phIoT:equip ;
    rdfs:label "{vrf, outdoorUnit, equip}" .

_:0b2cb027-d8dc-3744-0fcc-f23c91a70cca a phIoT:vrf-equip,
        phIoT:vrf-refrig-plant ;
    ph:hasTag phIoT:vrf,
        phIoT:refrig,
        phIoT:plant,
        phIoT:equip ;
    rdfs:label "{vrf, refrig, plant, equip}" .

phIoT:vrf-equip a owl:Class ;
    rdfs:subClassOf phIoT:equip ;
    rdfs:label "vrf-equip" ;
    ph:children _:0b2cb027-d8dc-3745-0fcd-f23c91a70cca,
        _:0b2cb027-d8dc-3746-0fce-f23c91a70cca ;
    rdfs:comment "Equipment used in VRF systems.  See `docHaystack::VRF#equip` chapter." ;
    ph:is phIoT:equip ;
    ph:lib phIoT:lib:phIoT .

_:0b2cb027-d8dc-3745-0fcd-f23c91a70cca a phIoT:equip ;
    ph:hasTag phIoT:equip ;
    rdfs:label "{equip}" .

_:0b2cb027-d8dc-3746-0fce-f23c91a70cca a phIoT:point ;
    ph:hasTag phIoT:point ;
    rdfs:label "{point}" .

phIoT:vrf-heatPump-system a owl:Class ;
    rdfs:subClassOf phIoT:vrf-system ;
    rdfs:label "vrf-heatPump-system" ;
    ph:children _:0b2cb027-d8dc-3747-0fcf-f23c91a70cca,
        _:0b2cb027-d8dc-3748-0fd0-f23c91a70cca,
        _:0b2cb027-d8dc-3749-0fd1-f23c91a70cca,
        _:0b2cb027-d8dc-374a-0fd2-f23c91a70cca,
        _:0b2cb027-d8dc-374b-0fd3-f23c91a70cca ;
    rdfs:comment "Heat pump VRF system can either heat, or cool, but not at the same time.\nSee `docHaystack::VRF#types` chapter." ;
    ph:is phIoT:vrf-system ;
    ph:lib phIoT:lib:phIoT .

_:0b2cb027-d8dc-3747-0fcf-f23c91a70cca a phIoT:equip ;
    ph:hasTag phIoT:equip ;
    rdfs:label "{equip}" .

_:0b2cb027-d8dc-3748-0fd0-f23c91a70cca a phIoT:point ;
    ph:hasTag phIoT:point ;
    rdfs:label "{point}" .

_:0b2cb027-d8dc-3749-0fd1-f23c91a70cca a phIoT:vrf-indoorUnit ;
    ph:hasTag phIoT:vrf,
        phIoT:indoorUnit,
        phIoT:equip ;
    rdfs:label "{vrf, indoorUnit, equip}" .

_:0b2cb027-d8dc-374a-0fd2-f23c91a70cca a phIoT:vrf-outdoorUnit ;
    ph:hasTag phIoT:vrf,
        phIoT:outdoorUnit,
        phIoT:equip ;
    rdfs:label "{vrf, outdoorUnit, equip}" .

_:0b2cb027-d8dc-374b-0fd3-f23c91a70cca a phIoT:vrf-equip,
        phIoT:vrf-refrig-plant ;
    ph:hasTag phIoT:vrf,
        phIoT:refrig,
        phIoT:plant,
        phIoT:equip ;
    rdfs:label "{vrf, refrig, plant, equip}" .

phIoT:vrf-heatRecovery-system a owl:Class ;
    rdfs:subClassOf phIoT:vrf-system ;
    rdfs:label "vrf-heatRecovery-system" ;
    ph:children _:0b2cb027-d8dc-374c-0fd4-f23c91a70cca,
        _:0b2cb027-d8dc-374d-0fd5-f23c91a70cca,
        _:0b2cb027-d8dc-374e-0fd6-f23c91a70cca,
        _:0b2cb027-d8dc-374f-0fd7-f23c91a70cca,
        _:0b2cb027-d8dc-3750-0fd8-f23c91a70cca,
        _:0b2cb027-d8dc-3751-0fd9-f23c91a70cca ;
    rdfs:comment "Heat recovery VRF system can operate cooling and heating by each indoor unit\nindependently, at the same time. Heat recovery VRF systems have branch selectors\nto control how much, and which (hot gas or subcooled liquid) refrigerant\ngoes to each indoor unit.  See `docHaystack::VRF#types` chapter." ;
    ph:is phIoT:vrf-system ;
    ph:lib phIoT:lib:phIoT .

_:0b2cb027-d8dc-374c-0fd4-f23c91a70cca a phIoT:equip ;
    ph:hasTag phIoT:equip ;
    rdfs:label "{equip}" .

_:0b2cb027-d8dc-374d-0fd5-f23c91a70cca a phIoT:point ;
    ph:hasTag phIoT:point ;
    rdfs:label "{point}" .

_:0b2cb027-d8dc-374e-0fd6-f23c91a70cca a phIoT:branchSelector ;
    ph:hasTag phIoT:vrf,
        phIoT:branchSelector,
        phIoT:equip ;
    rdfs:label "{vrf, branchSelector, equip}" .

_:0b2cb027-d8dc-374f-0fd7-f23c91a70cca a phIoT:vrf-indoorUnit ;
    ph:hasTag phIoT:vrf,
        phIoT:indoorUnit,
        phIoT:equip ;
    rdfs:label "{vrf, indoorUnit, equip}" .

_:0b2cb027-d8dc-3750-0fd8-f23c91a70cca a phIoT:vrf-outdoorUnit ;
    ph:hasTag phIoT:vrf,
        phIoT:outdoorUnit,
        phIoT:equip ;
    rdfs:label "{vrf, outdoorUnit, equip}" .

_:0b2cb027-d8dc-3751-0fd9-f23c91a70cca a phIoT:vrf-equip,
        phIoT:vrf-refrig-plant ;
    ph:hasTag phIoT:vrf,
        phIoT:refrig,
        phIoT:plant,
        phIoT:equip ;
    rdfs:label "{vrf, refrig, plant, equip}" .

phIoT:vrf-indoorUnit a owl:Class ;
    rdfs:subClassOf phIoT:vrf-equip,
        phIoT:refrig-input ;
    rdfs:label "vrf-indoorUnit" ;
    ph:children _:0b2cb027-d8dc-3752-0fda-f23c91a70cca,
        _:0b2cb027-d8dc-3753-0fdb-f23c91a70cca ;
    rdfs:comment "Indoor unit in a VRF system.  Indoor units operate to satisfy a heating\nor cooling load. See `docHaystack::VRF#indoorUnits` chapter." ;
    ph:is phIoT:vrf-equip,
        phIoT:refrig-input ;
    ph:lib phIoT:lib:phIoT .

_:0b2cb027-d8dc-3752-0fda-f23c91a70cca a phIoT:equip ;
    ph:hasTag phIoT:equip ;
    rdfs:label "{equip}" .

_:0b2cb027-d8dc-3753-0fdb-f23c91a70cca a phIoT:point ;
    ph:hasTag phIoT:point ;
    rdfs:label "{point}" .

phIoT:vrf-indoorUnit-fcu a owl:Class ;
    rdfs:subClassOf phIoT:vrf-indoorUnit,
        phIoT:fcu ;
    rdfs:label "vrf-indoorUnit-fcu" ;
    ph:children _:0b2cb027-d8dc-3754-0fdc-f23c91a70cca,
        _:0b2cb027-d8dc-3755-0fdd-f23c91a70cca,
        _:0b2cb027-d8dc-3756-0fde-f23c91a70cca,
        _:0b2cb027-d8dc-3757-0fdf-f23c91a70cca,
        _:0b2cb027-d8dc-3758-0fe0-f23c91a70cca,
        _:0b2cb027-d8dc-3759-0fe1-f23c91a70cca,
        _:0b2cb027-d8dc-375a-0fe2-f23c91a70cca,
        _:0b2cb027-d8dc-375b-0fe3-f23c91a70cca,
        _:0b2cb027-d8dc-375c-0fe4-f23c91a70cca,
        _:0b2cb027-d8dc-375d-0fe5-f23c91a70cca,
        _:0b2cb027-d8dc-375e-0fe6-f23c91a70cca,
        _:0b2cb027-d8dc-375f-0fe7-f23c91a70cca,
        _:0b2cb027-d8dc-3760-0fe8-f23c91a70cca,
        _:0b2cb027-d8dc-3761-0fe9-f23c91a70cca,
        _:0b2cb027-d8dc-3762-0fea-f23c91a70cca,
        _:0b2cb027-d8dc-3763-0feb-f23c91a70cca,
        _:0b2cb027-d8dc-3764-0fec-f23c91a70cca,
        _:0b2cb027-d8dc-3765-0fed-f23c91a70cca,
        _:0b2cb027-d8dc-3766-0fee-f23c91a70cca,
        _:0b2cb027-d8dc-3767-0fef-f23c91a70cca,
        _:0b2cb027-d8dc-3768-0ff0-f23c91a70cca ;
    rdfs:comment "Indoor unit fan coil unit in a VRF system.  This includes but is not\nlimited to: ducted-type and non-ducted types such as wall-mount,\nfloor-mount, ceiling-mount and cassettes.  Indoor unit fan coils operate\nto satisfy a heating  or cooling load in a zone based on a zone thermostat\ntemperature set point." ;
    ph:is phIoT:vrf-indoorUnit,
        phIoT:fcu ;
    ph:lib phIoT:lib:phIoT ;
    ph:wikipedia "https://en.wikipedia.org/wiki/Fan_coil_unit"^^xsd:anyURI .

_:0b2cb027-d8dc-3754-0fdc-f23c91a70cca a phIoT:point ;
    ph:hasTag phIoT:bypass,
        phIoT:damper,
        phIoT:cmd,
        phIoT:point ;
    rdfs:label "{bypass, damper, cmd, point}" .

_:0b2cb027-d8dc-3755-0fdd-f23c91a70cca a phIoT:point ;
    ph:hasTag phIoT:cool,
        phIoT:cmd,
        phIoT:point ;
    rdfs:label "{cool, cmd, point}" .

_:0b2cb027-d8dc-3756-0fde-f23c91a70cca a phIoT:point ;
    ph:hasTag phIoT:dessicantDehumidifier,
        phIoT:cmd,
        phIoT:point ;
    rdfs:label "{dessicantDehumidifier, cmd, point}" .

_:0b2cb027-d8dc-3757-0fdf-f23c91a70cca a phIoT:duct ;
    ph:hasTag phIoT:discharge,
        phIoT:duct,
        phIoT:equip ;
    rdfs:label "{discharge, duct, equip}" .

_:0b2cb027-d8dc-3758-0fe0-f23c91a70cca a phIoT:duct ;
    ph:hasTag phIoT:economizer,
        phIoT:duct,
        phIoT:equip ;
    rdfs:label "{economizer, duct, equip}" .

_:0b2cb027-d8dc-3759-0fe1-f23c91a70cca a phIoT:point ;
    ph:hasTag phIoT:economizing,
        phIoT:cmd,
        phIoT:point ;
    rdfs:label "{economizing, cmd, point}" .

_:0b2cb027-d8dc-375a-0fe2-f23c91a70cca a phIoT:equip ;
    ph:hasTag phIoT:equip ;
    rdfs:label "{equip}" .

_:0b2cb027-d8dc-375b-0fe3-f23c91a70cca a phIoT:duct ;
    ph:hasTag phIoT:exhaust,
        phIoT:duct,
        phIoT:equip ;
    rdfs:label "{exhaust, duct, equip}" .

_:0b2cb027-d8dc-375c-0fe4-f23c91a70cca a phIoT:point ;
    ph:hasTag phIoT:faceBypass,
        phIoT:cmd,
        phIoT:point ;
    rdfs:label "{faceBypass, cmd, point}" .

_:0b2cb027-d8dc-375d-0fe5-f23c91a70cca a phIoT:point ;
    ph:hasTag phIoT:filter,
        phIoT:sensor,
        phIoT:point ;
    rdfs:label "{filter, sensor, point}" .

_:0b2cb027-d8dc-375e-0fe6-f23c91a70cca a phIoT:point ;
    ph:hasTag phIoT:freezeStat,
        phIoT:sensor,
        phIoT:point ;
    rdfs:label "{freezeStat, sensor, point}" .

_:0b2cb027-d8dc-375f-0fe7-f23c91a70cca a phIoT:point ;
    ph:hasTag phIoT:heat,
        phIoT:cmd,
        phIoT:point ;
    rdfs:label "{heat, cmd, point}" .

_:0b2cb027-d8dc-3760-0fe8-f23c91a70cca a phIoT:point ;
    ph:hasTag phIoT:heatWheel,
        phIoT:cmd,
        phIoT:point ;
    rdfs:label "{heatWheel, cmd, point}" .

_:0b2cb027-d8dc-3761-0fe9-f23c91a70cca a phIoT:humidifier-equip ;
    ph:hasTag phIoT:humidifier,
        phIoT:equip ;
    rdfs:label "{humidifier, equip}" .

_:0b2cb027-d8dc-3762-0fea-f23c91a70cca a phIoT:point ;
    ph:hasTag phIoT:hvacMode,
        phIoT:sp,
        phIoT:point ;
    rdfs:label "{hvacMode, sp, point}" .

_:0b2cb027-d8dc-3763-0feb-f23c91a70cca a phIoT:duct ;
    ph:hasTag phIoT:mixed,
        phIoT:duct,
        phIoT:equip ;
    rdfs:label "{mixed, duct, equip}" .

_:0b2cb027-d8dc-3764-0fec-f23c91a70cca a phIoT:duct ;
    ph:hasTag phIoT:outside,
        phIoT:duct,
        phIoT:equip ;
    rdfs:label "{outside, duct, equip}" .

_:0b2cb027-d8dc-3765-0fed-f23c91a70cca a phIoT:point ;
    ph:hasTag phIoT:point ;
    rdfs:label "{point}" .

_:0b2cb027-d8dc-3766-0fee-f23c91a70cca a phIoT:duct ;
    ph:hasTag phIoT:return,
        phIoT:duct,
        phIoT:equip ;
    rdfs:label "{return, duct, equip}" .

_:0b2cb027-d8dc-3767-0fef-f23c91a70cca a phIoT:thermostat ;
    ph:hasTag phIoT:thermostat,
        phIoT:equip ;
    rdfs:label "{thermostat, equip}" .

_:0b2cb027-d8dc-3768-0ff0-f23c91a70cca a phIoT:duct ;
    ph:hasTag phIoT:ventilation,
        phIoT:duct,
        phIoT:equip ;
    rdfs:label "{ventilation, duct, equip}" .

phIoT:vrf-outdoorUnit a owl:Class ;
    rdfs:subClassOf phIoT:vrf-equip,
        phIoT:refrig-output ;
    rdfs:label "vrf-outdoorUnit" ;
    ph:children _:0b2cb027-d8eb-7980-0ff1-f23c91a70cca,
        _:0b2cb027-d8eb-7981-0ff2-f23c91a70cca ;
    rdfs:comment "Outdoor unit with one or more compressors in a VRF system. As each indoor\nunit sends a demand to the outdoor unit, outdoor unit delivers the amount\nof refrigerant needed to meet the individual requirements of each indoor\nunit.  See `docHaystack::VRF#outdoorUnits` chapter." ;
    ph:is phIoT:vrf-equip,
        phIoT:refrig-output ;
    ph:lib phIoT:lib:phIoT .

_:0b2cb027-d8eb-7980-0ff1-f23c91a70cca a phIoT:equip ;
    ph:hasTag phIoT:equip ;
    rdfs:label "{equip}" .

_:0b2cb027-d8eb-7981-0ff2-f23c91a70cca a phIoT:point ;
    ph:hasTag phIoT:point ;
    rdfs:label "{point}" .

phIoT:vrf-refrig-plant a owl:Class ;
    rdfs:subClassOf phIoT:plant,
        phIoT:refrig-output ;
    rdfs:label "vrf-refrig-plant" ;
    ph:children _:0b2cb027-d8eb-7982-0ff3-f23c91a70cca,
        _:0b2cb027-d8eb-7983-0ff4-f23c91a70cca,
        _:0b2cb027-d8eb-7984-0ff5-f23c91a70cca,
        _:0b2cb027-d8eb-7985-0ff6-f23c91a70cca ;
    rdfs:comment "Group of outdoor units in a VRF system.  See `docHaystack::VRF#refrigPlant`." ;
    ph:is phIoT:plant,
        phIoT:refrig-output ;
    ph:lib phIoT:lib:phIoT .

_:0b2cb027-d8eb-7982-0ff3-f23c91a70cca a phIoT:point ;
    ph:hasTag phIoT:enable,
        phIoT:cmd,
        phIoT:point ;
    rdfs:label "{enable, cmd, point}" .

_:0b2cb027-d8eb-7983-0ff4-f23c91a70cca a phIoT:equip ;
    ph:hasTag phIoT:equip ;
    rdfs:label "{equip}" .

_:0b2cb027-d8eb-7984-0ff5-f23c91a70cca a phIoT:point ;
    ph:hasTag phIoT:point ;
    rdfs:label "{point}" .

_:0b2cb027-d8eb-7985-0ff6-f23c91a70cca a phIoT:vrf-outdoorUnit ;
    ph:hasTag phIoT:vrf,
        phIoT:outdoorUnit,
        phIoT:equip ;
    rdfs:label "{vrf, outdoorUnit, equip}" .

phIoT:vrf-system a owl:Class ;
    rdfs:subClassOf phIoT:refrig-system ;
    rdfs:label "vrf-system" ;
    ph:children _:0b2cb027-d8eb-7986-0ff7-f23c91a70cca,
        _:0b2cb027-d8eb-7987-0ff8-f23c91a70cca,
        _:0b2cb027-d8eb-7988-0ff9-f23c91a70cca,
        _:0b2cb027-d8eb-7989-0ffa-f23c91a70cca,
        _:0b2cb027-d8eb-798a-0ffb-f23c91a70cca ;
    rdfs:comment "Variable refigerant flow system.  The system contains the indoor\nunits, outdoor units, and branch selectors.  See `docHaystack::VRF#types`\nchapter." ;
    ph:is phIoT:refrig-system ;
    ph:lib phIoT:lib:phIoT .

_:0b2cb027-d8eb-7986-0ff7-f23c91a70cca a phIoT:equip ;
    ph:hasTag phIoT:equip ;
    rdfs:label "{equip}" .

_:0b2cb027-d8eb-7987-0ff8-f23c91a70cca a phIoT:point ;
    ph:hasTag phIoT:point ;
    rdfs:label "{point}" .

_:0b2cb027-d8eb-7988-0ff9-f23c91a70cca a phIoT:vrf-indoorUnit ;
    ph:hasTag phIoT:vrf,
        phIoT:indoorUnit,
        phIoT:equip ;
    rdfs:label "{vrf, indoorUnit, equip}" .

_:0b2cb027-d8eb-7989-0ffa-f23c91a70cca a phIoT:vrf-outdoorUnit ;
    ph:hasTag phIoT:vrf,
        phIoT:outdoorUnit,
        phIoT:equip ;
    rdfs:label "{vrf, outdoorUnit, equip}" .

_:0b2cb027-d8eb-798a-0ffb-f23c91a70cca a phIoT:vrf-equip,
        phIoT:vrf-refrig-plant ;
    ph:hasTag phIoT:vrf,
        phIoT:refrig,
        phIoT:plant,
        phIoT:equip ;
    rdfs:label "{vrf, refrig, plant, equip}" .

phIoT:warm a owl:Class ;
    rdfs:subClassOf ph:marker ;
    rdfs:label "warm" ;
    rdfs:comment "Relatively warm in comparison to another substance, without being\nactively heated. The substance can be used as a source of energy for\na heating process, for example a warm water well in an `ates` system." ;
    ph:is ph:marker ;
    ph:lib phIoT:lib:phIoT .

phIoT:warm-water a owl:Class ;
    rdfs:subClassOf phScience:water ;
    rdfs:label "warm-water" ;
    rdfs:comment "Relatively warm water without active heating" ;
    ph:is phScience:water ;
    ph:lib phIoT:lib:phIoT ;
    ph:wikipedia "https://en.wikipedia.org/wiki/Water"^^xsd:anyURI .

phScience:water a owl:Class ;
    rdfs:subClassOf phScience:liquid ;
    rdfs:label "water" ;
    rdfs:comment "Water in its liquid form" ;
    ph:is phScience:liquid ;
    ph:lib phScience:lib:phScience ;
    ph:wikipedia "https://en.wikipedia.org/wiki/Water"^^xsd:anyURI .

phIoT:water-system a owl:Class ;
    rdfs:subClassOf phIoT:system ;
    rdfs:label "water-system" ;
    ph:children _:0b2cb027-d8eb-798b-0ffc-f23c91a70cca,
        _:0b2cb027-d8eb-798c-0ffd-f23c91a70cca ;
    rdfs:comment "System that supplies or collects potable or non-potable water in any state." ;
    ph:is phIoT:system ;
    ph:lib phIoT:lib:phIoT .

_:0b2cb027-d8eb-798b-0ffc-f23c91a70cca a phIoT:equip ;
    ph:hasTag phIoT:equip ;
    rdfs:label "{equip}" .

_:0b2cb027-d8eb-798c-0ffd-f23c91a70cca a phIoT:point ;
    ph:hasTag phIoT:point ;
    rdfs:label "{point}" .

phIoT:waterCooling a owl:Class ;
    rdfs:subClassOf phIoT:coolingProcess ;
    rdfs:label "waterCooling" ;
    rdfs:comment "Cooling using transfer of heat to water which is not explicitly chilled" ;
    ph:is phIoT:coolingProcess ;
    ph:lib phIoT:lib:phIoT ;
    ph:wikipedia "https://en.wikipedia.org/wiki/Water_cooling"^^xsd:anyURI .

phScience:weather a owl:Class ;
    rdfs:subClassOf phScience:phenomenon ;
    rdfs:label "weather" ;
    rdfs:comment "Associated with atmospheric air or phenomenon.\nSee `docHaystack::Weather` chapter." ;
    ph:is phScience:phenomenon ;
    ph:lib phScience:lib:phScience ;
    ph:wikipedia "https://en.wikipedia.org/wiki/Weather"^^xsd:anyURI .

phIoT:weather-point a owl:Class ;
    rdfs:subClassOf phIoT:point ;
    rdfs:label "weather-point" ;
    rdfs:comment "Weather station observation point.\nSee `docHaystack::Weather#points` chapter." ;
    ph:is phIoT:point ;
    ph:lib phIoT:lib:phIoT .

phScience:weatherCond a owl:Class ;
    rdfs:subClassOf phScience:quantity ;
    rdfs:label "weatherCond" ;
    rdfs:comment "Enumeration of weather conditions" ;
    ph:enum "unknown\nclear\npartlyCloudy\ncloudy\nshowers\nrain\nthunderstorms\nice\nflurries\nsnow" ;
    ph:is phScience:quantity ;
    ph:lib phScience:lib:phScience ;
    phScience:quantityOf phScience:weather .

phIoT:weatherStation a owl:Class ;
    rdfs:subClassOf ph:entity,
        ph:geoPlace ;
    rdfs:label "weatherStation" ;
    ph:children _:0b2cb027-d8fa-bbc0-0ffe-f23c91a70cca,
        _:0b2cb027-d8fa-bbc1-0fff-f23c91a70cca,
        _:0b2cb027-d8fa-bbc2-1000-f23c91a70cca,
        _:0b2cb027-d8fa-bbc3-1001-f23c91a70cca,
        _:0b2cb027-d8fa-bbc4-1002-f23c91a70cca,
        _:0b2cb027-d8fa-bbc5-1003-f23c91a70cca,
        _:0b2cb027-d8fa-bbc6-1004-f23c91a70cca,
        _:0b2cb027-d8fa-bbc7-1005-f23c91a70cca,
        _:0b2cb027-d8fa-bbc8-1006-f23c91a70cca,
        _:0b2cb027-d8fa-bbc9-1007-f23c91a70cca,
        _:0b2cb027-d8fa-bbca-1008-f23c91a70cca,
        _:0b2cb027-d8fa-bbcb-1009-f23c91a70cca,
        _:0b2cb027-d8fa-bbcc-100a-f23c91a70cca,
        _:0b2cb027-d8fa-bbcd-100b-f23c91a70cca,
        _:0b2cb027-d8fa-bbce-100c-f23c91a70cca ;
    rdfs:comment "Logical weather station and its measurement points.\nSee `docHaystack::Weather#stations` chapter." ;
    ph:is ph:entity,
        ph:geoPlace ;
    ph:lib phIoT:lib:phIoT ;
    ph:mandatory ph:marker ;
    ph:wikipedia "https://en.wikipedia.org/wiki/Weather_station"^^xsd:anyURI .

_:0b2cb027-d8fa-bbc0-0ffe-f23c91a70cca a phIoT:weather-point ;
    ph:hasTag phScience:weather,
        phScience:air,
        phScience:temp,
        phIoT:sensor,
        phIoT:point ;
    rdfs:label "{weather, air, temp, sensor, point}" .

_:0b2cb027-d8fa-bbc1-0fff-f23c91a70cca a phIoT:weather-point ;
    ph:hasTag phScience:weather,
        phScience:air,
        phScience:wetBulb,
        phIoT:sensor,
        phIoT:point ;
    rdfs:label "{weather, air, wetBulb, sensor, point}" .

_:0b2cb027-d8fa-bbc2-1000-f23c91a70cca a phIoT:weather-point ;
    ph:hasTag phScience:weather,
        phScience:air,
        phScience:feelsLike,
        phIoT:sensor,
        phIoT:point ;
    rdfs:label "{weather, air, feelsLike, sensor, point}" .

_:0b2cb027-d8fa-bbc3-1001-f23c91a70cca a phIoT:weather-point ;
    ph:hasTag phScience:weather,
        phScience:air,
        phScience:dewPoint,
        phIoT:sensor,
        phIoT:point ;
    rdfs:label "{weather, air, dewPoint, sensor, point}" .

_:0b2cb027-d8fa-bbc4-1002-f23c91a70cca a phIoT:weather-point ;
    ph:hasTag phScience:weather,
        phScience:air,
        phScience:humidity,
        phIoT:sensor,
        phIoT:point ;
    rdfs:label "{weather, air, humidity, sensor, point}" .

_:0b2cb027-d8fa-bbc5-1003-f23c91a70cca a phIoT:weather-point ;
    ph:hasTag phScience:weather,
        phScience:air,
        phScience:enthalpy,
        phIoT:sensor,
        phIoT:point ;
    rdfs:label "{weather, air, enthalpy, sensor, point}" .

_:0b2cb027-d8fa-bbc6-1004-f23c91a70cca a phIoT:weather-point ;
    ph:hasTag phScience:weather,
        phScience:atmospheric,
        phScience:pressure,
        phIoT:sensor,
        phIoT:point ;
    rdfs:label "{weather, atmospheric, pressure, sensor, point}" .

_:0b2cb027-d8fa-bbc7-1005-f23c91a70cca a phIoT:weather-point ;
    ph:hasTag phScience:weather,
        phScience:cloudage,
        phIoT:sensor,
        phIoT:point ;
    rdfs:label "{weather, cloudage, sensor, point}" .

_:0b2cb027-d8fa-bbc8-1006-f23c91a70cca a phIoT:weather-point ;
    ph:hasTag phScience:weather,
        phScience:daytime,
        phIoT:sensor,
        phIoT:point ;
    rdfs:label "{weather, daytime, sensor, point}" .

_:0b2cb027-d8fa-bbc9-1007-f23c91a70cca a phIoT:weather-point ;
    ph:hasTag phScience:weather,
        phScience:precipitation,
        phIoT:sensor,
        phIoT:point ;
    rdfs:label "{weather, precipitation, sensor, point}" .

_:0b2cb027-d8fa-bbca-1008-f23c91a70cca a phIoT:weather-point ;
    ph:hasTag phScience:weather,
        phScience:solar,
        phScience:irradiance,
        phIoT:sensor,
        phIoT:point ;
    rdfs:label "{weather, solar, irradiance, sensor, point}" .

_:0b2cb027-d8fa-bbcb-1009-f23c91a70cca a phIoT:weather-point ;
    ph:hasTag phScience:weather,
        phScience:weatherCond,
        phIoT:sensor,
        phIoT:point ;
    rdfs:label "{weather, weatherCond, sensor, point}" .

_:0b2cb027-d8fa-bbcc-100a-f23c91a70cca a phIoT:weather-point ;
    ph:hasTag phScience:weather,
        phScience:wind,
        phScience:speed,
        phIoT:sensor,
        phIoT:point ;
    rdfs:label "{weather, wind, speed, sensor, point}" .

_:0b2cb027-d8fa-bbcd-100b-f23c91a70cca a phIoT:weather-point ;
    ph:hasTag phScience:weather,
        phScience:wind,
        phScience:direction,
        phIoT:sensor,
        phIoT:point ;
    rdfs:label "{weather, wind, direction, sensor, point}" .

_:0b2cb027-d8fa-bbce-100c-f23c91a70cca a phIoT:weather-point ;
    ph:hasTag phScience:weather,
        phScience:visibility,
        phIoT:sensor,
        phIoT:point ;
    rdfs:label "{weather, visibility, sensor, point}" .

phIoT:weatherStationRef a owl:ObjectProperty ;
    rdfs:domain phIoT:site,
        phIoT:weather-point ;
    rdfs:range phIoT:weatherStation ;
    rdfs:label "weatherStationRef" ;
    rdfs:comment "Reference to weather station for to use this entity" ;
    ph:is ph:ref ;
    ph:lib phIoT:lib:phIoT ;
    ph:of phIoT:weatherStation ;
    ph:tagOn phIoT:site,
        phIoT:weather-point .

phIoT:well a owl:Class ;
    rdfs:subClassOf phIoT:equip ;
    rdfs:label "well" ;
    ph:children _:0b2cb027-d8fa-bbcf-100d-f23c91a70cca,
        _:0b2cb027-d8fa-bbd0-100e-f23c91a70cca,
        _:0b2cb027-d8fa-bbd1-100f-f23c91a70cca,
        _:0b2cb027-d8fa-bbd2-1010-f23c91a70cca,
        _:0b2cb027-d8fa-bbd3-1011-f23c91a70cca,
        _:0b2cb027-d8fa-bbd4-1012-f23c91a70cca,
        _:0b2cb027-d8fa-bbd5-1013-f23c91a70cca,
        _:0b2cb027-d8fa-bbd6-1014-f23c91a70cca ;
    rdfs:comment "A well is a source of groundwater and potentially thermal energy.  When\nused within an [ATES]`docHaystack::ATES` system, the well facilitates thermal\nenergy exchange with the ground warm and cool water sources. In this case, a\nwell can be either a closed system that transports water through pipes in the\nground, or an open system that pumps up and returns ground water." ;
    ph:is phIoT:equip ;
    ph:lib phIoT:lib:phIoT .

_:0b2cb027-d8fa-bbcf-100d-f23c91a70cca a phIoT:equip ;
    ph:hasTag phIoT:equip ;
    rdfs:label "{equip}" .

_:0b2cb027-d8fa-bbd0-100e-f23c91a70cca a phIoT:point ;
    ph:hasTag phIoT:point ;
    rdfs:label "{point}" .

_:0b2cb027-d8fa-bbd1-100f-f23c91a70cca a phIoT:point ;
    ph:hasTag phScience:water,
        phScience:flow,
        phIoT:sensor,
        phIoT:point ;
    rdfs:label "{water, flow, sensor, point}" .

_:0b2cb027-d8fa-bbd2-1010-f23c91a70cca a phIoT:point ;
    ph:hasTag phScience:water,
        phScience:level,
        phIoT:sensor,
        phIoT:point ;
    rdfs:label "{water, level, sensor, point}" .

_:0b2cb027-d8fa-bbd3-1011-f23c91a70cca a phIoT:point ;
    ph:hasTag phScience:water,
        phScience:pressure,
        phIoT:sensor,
        phIoT:point ;
    rdfs:label "{water, pressure, sensor, point}" .

_:0b2cb027-d8fa-bbd4-1012-f23c91a70cca a phIoT:pump-motor ;
    ph:hasTag phScience:water,
        phIoT:pump,
        phIoT:motor,
        phIoT:equip ;
    rdfs:label "{water, pump, motor, equip}" .

_:0b2cb027-d8fa-bbd5-1013-f23c91a70cca a phIoT:point ;
    ph:hasTag phScience:water,
        phScience:temp,
        phIoT:sensor,
        phIoT:point ;
    rdfs:label "{water, temp, sensor, point}" .

_:0b2cb027-d8fa-bbd6-1014-f23c91a70cca a phIoT:point ;
    ph:hasTag phScience:water,
        phScience:volume,
        phIoT:sensor,
        phIoT:point ;
    rdfs:label "{water, volume, sensor, point}" .

phScience:wetBulb a owl:Class ;
    rdfs:subClassOf phScience:quantity ;
    rdfs:label "wetBulb" ;
    rdfs:comment "Wet bulb air temperature.  Temperature which the air would have if cooled to saturation by the evaporation of water into it." ;
    ph:is phScience:quantity ;
    ph:lib phScience:lib:phScience ;
    phScience:prefUnit "\u00b0C",
        "\u00b0F" ;
    phScience:quantityOf phScience:air .

ph:wikipedia a owl:DatatypeProperty ;
    rdfs:domain ph:def ;
    rdfs:range ph:uri ;
    rdfs:label "wikipedia" ;
    rdfs:comment "Hyperlink to the subject's page on Wikipedia" ;
    ph:is ph:uri ;
    ph:lib ph:lib:ph ;
    ph:tagOn ph:def .

phScience:wind a owl:Class ;
    rdfs:subClassOf phScience:phenomenon ;
    rdfs:label "wind" ;
    rdfs:comment "Flow of air on surface of the Earth" ;
    ph:is phScience:phenomenon ;
    ph:lib phScience:lib:phScience ;
    ph:wikipedia "https://en.wikipedia.org/wiki/Wind"^^xsd:anyURI .

phScience:wind-direction a owl:Class ;
    rdfs:subClassOf phScience:direction ;
    rdfs:label "wind-direction" ;
    rdfs:comment "Compass direction from which wind originates" ;
    ph:is phScience:direction ;
    ph:lib phScience:lib:phScience ;
    phScience:prefUnit "deg" ;
    phScience:quantityOf phScience:wind .

phScience:wind-speed a owl:Class ;
    rdfs:subClassOf phScience:speed ;
    rdfs:label "wind-speed" ;
    rdfs:comment "Wind flow speed" ;
    ph:is phScience:speed ;
    ph:lib phScience:lib:phScience ;
    phScience:prefUnit "km/h",
        "mph" ;
    phScience:quantityOf phScience:wind .

phIoT:wire a owl:Class ;
    rdfs:subClassOf phIoT:conduit ;
    rdfs:label "wire" ;
    ph:children _:0b2cb027-d909-fe00-1015-f23c91a70cca,
        _:0b2cb027-d909-fe01-1016-f23c91a70cca ;
    rdfs:comment "Cabling used to convey electricity or data" ;
    ph:is phIoT:conduit ;
    ph:lib phIoT:lib:phIoT .

_:0b2cb027-d909-fe00-1015-f23c91a70cca a phIoT:equip ;
    ph:hasTag phIoT:equip ;
    rdfs:label "{equip}" .

_:0b2cb027-d909-fe01-1016-f23c91a70cca a phIoT:point ;
    ph:hasTag phIoT:point ;
    rdfs:label "{point}" .

phIoT:writable a owl:Class ;
    rdfs:subClassOf ph:marker ;
    rdfs:label "writable" ;
    rdfs:comment "Supports writing data" ;
    ph:is ph:marker ;
    ph:lib phIoT:lib:phIoT ;
    ph:tagOn phIoT:point .

phIoT:writable-point a owl:Class ;
    rdfs:subClassOf phIoT:point ;
    rdfs:label "writable-point" ;
    rdfs:comment "Point with writable output using 16-level priority array.  Writable\npoints typically are a setpoint or actuator command.  Haystack writable\npoints are modeled on the BACnet 16-level priority array with a\nrelinquish default which effectively acts as level 17.\n\nThe following levels have special behavior:\n - **Level 1**: highest priority reserved for emergency overrides\n - **Level 8**: manual override with ability to set timer to expire back to auto\n - **Default**: implicitly acts as level 17 for relinquish default\n\nThe priority array provides for contention resolution when many different\ncontrol applications may be vying for control of a given point. Low level\napplications like scheduling typically control levels 14, 15, or 16. Then\nusers can override at level 8. But a higher levels like 2 to 7 can be used\nto trump a user override (for example a demand response energy routine\nthat requires higher priority).\n\nThe actual value to write is resolved by starting at level 1 and working down\nto relinquish default to find the first non-null value. It is possible for\nall levels to be null, in which case the overall write output is null (which\nin turn may be auto/null to another system). Anytime a null value is written\nto a priority level, we say that level has been set to auto or released (this\nallows the next highest level to take command of the output).\n\nAlso see `docHaystack::Points#writable` chapter." ;
    ph:is phIoT:point ;
    ph:lib phIoT:lib:phIoT .

phIoT:writeErr a owl:DatatypeProperty ;
    rdfs:domain phIoT:writable-point ;
    rdfs:range ph:str ;
    rdfs:label "writeErr" ;
    rdfs:comment "Error description when `writeStatus` indicates error condition" ;
    ph:is ph:str ;
    ph:lib phIoT:lib:phIoT ;
    ph:tagOn phIoT:writable-point ;
    ph:transient ph:marker .

phIoT:writeLevel a owl:DatatypeProperty ;
    rdfs:domain phIoT:writable-point ;
    rdfs:range ph:number ;
    rdfs:label "writeLevel" ;
    rdfs:comment "Current priority level for `writeVal` as number between 1 and 17.\nThe value 17 indicates the relinquish default value." ;
    ph:is ph:int ;
    ph:lib phIoT:lib:phIoT ;
    ph:maxVal 17 ;
    ph:minVal 1 ;
    ph:tagOn phIoT:writable-point ;
    ph:transient ph:marker .

phIoT:writeStatus a owl:DatatypeProperty ;
    rdfs:domain phIoT:writable-point ;
    rdfs:range ph:str ;
    rdfs:label "writeStatus" ;
    rdfs:comment "Current status of a writable point output" ;
    ph:enum "- unbound: writable point is not bound to any output\n- ok: last write was successful\n- down: connectivity/networking problem - see `writeErr`\n- fault: configuration or hardware error  - see `writeErr`\n- disabled: manual disable of the point or connector\n- unknown: we don't know anything (typically boot state)" ;
    ph:is ph:str ;
    ph:lib phIoT:lib:phIoT ;
    ph:tagOn phIoT:writable-point ;
    ph:transient ph:marker .

phIoT:writeVal a owl:DatatypeProperty ;
    rdfs:subClassOf rdfs:Literal ;
    rdfs:label "writeVal" ;
    rdfs:comment "Current desired value to write to output.  This is the current \"winning\"\nvalue of the priority array indicated by `writeLevel`.  If this tag\nis missing then the winning value is null/auto." ;
    ph:is ph:scalar ;
    ph:lib phIoT:lib:phIoT ;
    ph:tagOn phIoT:writable-point ;
    ph:transient ph:marker .

ph:xstr a owl:DatatypeProperty ;
    rdfs:subClassOf xsd:string ;
    rdfs:label "xstr" ;
    rdfs:comment "Extended string - type name and string value encoding.\nSee [Kinds chapter]`docHaystack::Kinds#xstr`." ;
    ph:is ph:scalar ;
    ph:lib ph:lib:ph .

phIoT:yearBuilt a owl:DatatypeProperty ;
    rdfs:domain phIoT:site ;
    rdfs:range ph:number ;
    rdfs:label "yearBuilt" ;
    rdfs:comment "Original year of construction as four digit year such as 1980" ;
    ph:is ph:int ;
    ph:lib phIoT:lib:phIoT ;
    ph:tagOn phIoT:site .

phIct:zigbee a owl:Class ;
    rdfs:subClassOf phIct:protocol ;
    rdfs:label "zigbee" ;
    rdfs:comment "Low power wireless communication protocol for home automation" ;
    ph:is phIct:protocol ;
    ph:lib phIct:lib:phIct ;
    ph:wikipedia "https://en.wikipedia.org/wiki/Zigbee"^^xsd:anyURI .

phIoT:zone a owl:Class ;
    rdfs:subClassOf ph:marker ;
    rdfs:label "zone" ;
    rdfs:comment "Related to spaces from a system perspective" ;
    ph:is ph:marker ;
    ph:lib phIoT:lib:phIoT .

phIoT:zone-space a owl:Class ;
    rdfs:subClassOf phIoT:space ;
    rdfs:label "zone-space" ;
    ph:children _:0b2cb027-d947-0700-1017-f23c91a70cca,
        _:0b2cb027-d947-0701-1018-f23c91a70cca,
        _:0b2cb027-d947-0702-1019-f23c91a70cca,
        _:0b2cb027-d947-0703-101a-f23c91a70cca,
        _:0b2cb027-d947-0704-101b-f23c91a70cca,
        _:0b2cb027-d947-0705-101c-f23c91a70cca ;
    rdfs:comment "Space associated with a specific system.\nSee `docHaystack::Spaces#zones` and `docHaystack::Zones` chapters." ;
    ph:is phIoT:space ;
    ph:lib phIoT:lib:phIoT .

_:0b2cb027-d947-0700-1017-f23c91a70cca a phIoT:equip ;
    ph:hasTag phIoT:equip ;
    rdfs:label "{equip}" .

_:0b2cb027-d947-0701-1018-f23c91a70cca a phIoT:point ;
    ph:hasTag phIoT:occupancy,
        phIoT:sensor,
        phIoT:point ;
    rdfs:label "{occupancy, sensor, point}" .

_:0b2cb027-d947-0702-1019-f23c91a70cca a phIoT:point ;
    ph:hasTag phIoT:occupied,
        phIoT:sensor,
        phIoT:point ;
    rdfs:label "{occupied, sensor, point}" .

_:0b2cb027-d947-0703-101a-f23c91a70cca a phIoT:point ;
    ph:hasTag phIoT:occupied,
        phIoT:sp,
        phIoT:point ;
    rdfs:label "{occupied, sp, point}" .

_:0b2cb027-d947-0704-101b-f23c91a70cca a phIoT:point ;
    ph:hasTag phIoT:point ;
    rdfs:label "{point}" .

_:0b2cb027-d947-0705-101c-f23c91a70cca a phIoT:space ;
    ph:hasTag phIoT:space ;
    rdfs:label "{space}" .

phIct:zwave a owl:Class ;
    rdfs:subClassOf phIct:protocol ;
    rdfs:label "zwave" ;
    rdfs:comment "Low power wireless communication protocol for home automation" ;
    ph:is phIct:protocol ;
    ph:lib phIct:lib:phIct ;
    ph:wikipedia "https://en.wikipedia.org/wiki/Z-Wave"^^xsd:anyURI .
